<?xml version="1.0"?>


<!DOCTYPE rdf:RDF [
    <!ENTITY owl "http://www.w3.org/2002/07/owl#" >
    <!ENTITY dc "http://purl.org/dc/elements/1.1/" >
    <!ENTITY xsd "http://www.w3.org/2001/XMLSchema#" >
    <!ENTITY skos "http://www.w3.org/2004/02/skos/core#" >
    <!ENTITY rdfs "http://www.w3.org/2000/01/rdf-schema#" >
    <!ENTITY rdf "http://www.w3.org/1999/02/22-rdf-syntax-ns#" >
    <!ENTITY OBO_annotation_properties "http://ontology.neuinfo.org/NIF/Backend/OBO_annotation_properties.owl#" >
]>


<rdf:RDF xmlns="http://ontology.neuinfo.org/NIF/Backend/OBO_annotation_properties.owl#"
     xml:base="http://ontology.neuinfo.org/NIF/Backend/OBO_annotation_properties.owl"
     xmlns:dc="http://purl.org/dc/elements/1.1/"
     xmlns:rdfs="http://www.w3.org/2000/01/rdf-schema#"
     xmlns:owl="http://www.w3.org/2002/07/owl#"
     xmlns:xsd="http://www.w3.org/2001/XMLSchema#"
     xmlns:rdf="http://www.w3.org/1999/02/22-rdf-syntax-ns#"
     xmlns:skos="http://www.w3.org/2004/02/skos/core#"
     xmlns:OBO_annotation_properties="http://ontology.neuinfo.org/NIF/Backend/OBO_annotation_properties.owl#">
    <owl:Ontology rdf:about="http://ontology.neuinfo.org/NIF/Backend/OBO_annotation_properties.owl">
        <owl:versionInfo rdf:datatype="&xsd;string">1.3.0</owl:versionInfo>
        <dc:date rdf:datatype="&xsd;string">2006-10-07 (createdDate)</dc:date>
        <dc:date rdf:datatype="&xsd;string">2008-03-13 (modifiedDate)</dc:date>
        <dc:creator rdf:datatype="&xsd;string">The BIRN Ontology Task Force</dc:creator>
        <skos:changeNote xml:lang="en"> (2008-01-28) - fixed and annotationType that was missing the namespace prefix obo_annot.</skos:changeNote>
        <skos:changeNote xml:lang="en"> (2008-03-13) - finally added annotation prop for GO ID.</skos:changeNote>
        <skos:changeNote xml:lang="en">Explicitly removed ALL rdfs:type=DatatypeProperty declarations automatigically added to these AnnotationProperties by Protege-OWL v3.3beta</skos:changeNote>
        <skos:changeNote xml:lang="en">Have &#39;cleansed&#39; the file to be OWL-DL.</skos:changeNote>
        <skos:changeNote xml:lang="en">Now using a specific set of AnnotationProperties that link to specific Enumeration classes to specify annotations from a fixed list of values - e.g., ExternalSource, DefinitionSource.  This is the second iteration of this mechanism (first was put in v1.2.2).  This second version follows a patter recommended by Alan Ruttenberg which avoids using ObjectProperties as the Manchester design pattern for Value Partitions recommends, and instead sticks to AnnotationProperties only.  Note this version of OBO_annotation_properties uses the same EnumerationClasses from v1.2.2, and still includes the related ObjectProperties, so as to be able to support XSLT-based translation of the BIRNLex files that used the v1.2.2 pattern.  The next version of this file will eliminate the ObjectProperties and will rename the equivalent AnnotationProperties to remove the trailing &#39;2&#39; put in there to provide a unique name.</skos:changeNote>
        <dc:title xml:lang="en">OBO Annotation Properties (BIRN derived)</dc:title>
        <rdfs:comment xml:lang="en">These are annotation properties the BIRN OTF expects will be shared by the community, not limited to the specific ontology development needs of BIRN.  This current ontology is a proposal to be reviewed by the OBO Foundry participants and developers of other OBO Foundry ontologies - e.g., OBI, PaTO, GO, etc..</rdfs:comment>
        <skos:changeNote xml:lang="en">v1.3.0 (2007-08-03) - Changed many things, but primarily: (1) removed rdf:datatype xsd:string specs for all AnnotationProperties, since they are now all untyped and should assume STRING as a the default; (2) added the typing of AnnotationProperties using annotationType which should aid in algorithmically processing.</skos:changeNote>
        <owl:imports rdf:resource="http://www.w3.org/2004/02/skos/core/owl-dl/skos-core-owl-dl.owl"/>
    </owl:Ontology>
    


    <!-- 
    ///////////////////////////////////////////////////////////////////////////////////////
    //
    // Annotation properties
    //
    ///////////////////////////////////////////////////////////////////////////////////////
     -->

    <owl:AnnotationProperty rdf:about="&OBO_annotation_properties;hasExternalSource">
        <annotationPropertyRange rdf:datatype="&xsd;string">http://ontology.neuinfo.org/NIF/Backend/OBO_annotation_properties.owl#EnumerationClass</annotationPropertyRange>
        <annotationPropertyDomain rdf:datatype="&xsd;string">owl:Class</annotationPropertyDomain>
        <hasValidationMethod rdf:datatype="&xsd;string">sparql_verify_annotation_domain_and_range</hasValidationMethod>
    </owl:AnnotationProperty>
    <owl:AnnotationProperty rdf:about="&OBO_annotation_properties;tempDefinition">
        <annotationType rdf:datatype="&xsd;string">http://www.w3.org/2004/02/skos/core#definition</annotationType>
        <skos:definition xml:lang="en">a definition specifically declared to be temporary and in the midst of more detailed curation efforts.</skos:definition>
    </owl:AnnotationProperty>
    <owl:AnnotationProperty rdf:about="&OBO_annotation_properties;externalSourceURI">
        <annotationType rdf:datatype="&xsd;string">http://purl.org/dc/elements/1.1/relation</annotationType>
        <skos:definition xml:lang="en">A publically accessible URI other than a standard bibliographic citation to the specific external source from which the content of an ontology Class was derived.</skos:definition>
    </owl:AnnotationProperty>
    <owl:AnnotationProperty rdf:about="&OBO_annotation_properties;definingCitation">
        <skos:definition xml:lang="en">A literature a citation providing information fundamental to the definition of an ontology class.</skos:definition>
        <usageNote xml:lang="en">This AnnotationProperty should only be used whether there is neither a publicly accessible URI nor a namespace-qualified ID which can be used to algorithmically construct a complete citation for use in a user interface or search system (e.g., the way one can use PMID and the NCBI PublMed webservices or HTTP services to automatically access citation information).</usageNote>
    </owl:AnnotationProperty>
    <owl:AnnotationProperty rdf:about="&OBO_annotation_properties;GOid">
        <annotationType rdf:datatype="&xsd;string">http://ontology.neuinfo.org/NIF/Backend/OBO_annotation_properties.owl#externalSourceId</annotationType>
        <skos:editorialNote xml:lang="en">Is a type of obo_annot:obo_external_source_ID.</skos:editorialNote>
        <skos:definition xml:lang="en">This is the Gene Ontology ID for the concept associated with this class.</skos:definition>
    </owl:AnnotationProperty>
    <owl:AnnotationProperty rdf:about="&OBO_annotation_properties;acronym">
        <annotationType rdf:datatype="&xsd;string">http://www.w3.org/2004/02/skos/core#altLabel</annotationType>
        <skos:definition xml:lang="en">A synonym consisting of a sequence of letters typically taken from the beginning of words of which either the preferred label or another synonym are composed.</skos:definition>
    </owl:AnnotationProperty>
    <owl:AnnotationProperty rdf:about="&OBO_annotation_properties;externalSourceId">
        <annotationType rdf:datatype="&xsd;string">http://purl.org/dc/elements/1.1/identifier</annotationType>
        <skos:definition xml:lang="en">This field is to maintain the link back to an external source (see the externalSource property).</skos:definition>
    </owl:AnnotationProperty>
    <owl:AnnotationProperty rdf:about="&OBO_annotation_properties;pendingObjectRelationNote">
        <annotationType rdf:datatype="&xsd;string">http://ontology.neuinfo.org/NIF/Backend/OBO_annotation_properties.owl#pendingActionNote</annotationType>
        <skos:definition xml:lang="en">A note describing a known relation in which this class participates that is beyond pure subsumptive is_a relations.</skos:definition>
    </owl:AnnotationProperty>
    <owl:AnnotationProperty rdf:about="&OBO_annotation_properties;pendingFunctionalRelationNote">
        <annotationType rdf:datatype="&xsd;string">http://ontology.neuinfo.org/NIF/Backend/OBO_annotation_properties.owl#pendingActionNote</annotationType>
        <skos:definition xml:lang="en">A note describing a known functional/process/occurant relation in which this class participates that is beyond pure subsumptive is_a relation.  Is a type of pending_object_relation_note.</skos:definition>
    </owl:AnnotationProperty>
    <owl:AnnotationProperty rdf:about="&OBO_annotation_properties;annotationType">
        <skos:definition xml:lang="en">A category designed to help data processing systems automatically determine how to process a given annotation.</skos:definition>
        <skos:editorialNote xml:lang="en">The current use of this meta-property is to identify types of definitions (core:definition) and types of external source ID (dc:identifier) (BB: 2007-08-03.</skos:editorialNote>
        <usageNote xml:lang="en">The legal cardinality range for annotationType applied to AnnotationProperties = 0...n - i.e., it is neither required, nor is it limited to a cardinality of 1, though it is recommend there be at least one annotationType for each AnnotationProperty, whenever there is an appropriate super-class available..</usageNote>
        <skos:scopeNote xml:lang="en">The only valid values for this property are DC, SKOS, or BIRN AnnotationProperty URIs.</skos:scopeNote>
        <skos:editorialNote xml:lang="en">This is required, since sub-classing AnnotationProperties is not allowed in OWL-DL.  Using this descriptive metadata AnnotationProperties, we can construct a chained code representation of a classification graph for AnnotationProperities very likely to be useful for information systems built to parse and process OWL content.</skos:editorialNote>
    </owl:AnnotationProperty>
    <owl:AnnotationProperty rdf:about="&OBO_annotation_properties;externallySourcedDefinition">
        <annotationType rdf:datatype="&xsd;string">http://www.w3.org/2004/02/skos/core#definition</annotationType>
        <skos:definition xml:lang="en">This is a class definition derived AS IS from an external, community knowledge resource.</skos:definition>
    </owl:AnnotationProperty>
    <owl:AnnotationProperty rdf:about="&OBO_annotation_properties;hasAbbrevSource">
        <annotationPropertyRange rdf:datatype="&xsd;string">http://ontology.neuinfo.org/NIF/Backend/OBO_annotation_properties.owl#EnumerationClass</annotationPropertyRange>
        <annotationType rdf:datatype="&xsd;string">http://purl.org/dc/elements/1.1/relation</annotationType>
        <annotationPropertyDomain rdf:datatype="&xsd;string">owl:Class</annotationPropertyDomain>
        <hasValidationMethod rdf:datatype="&xsd;string">sparql_verify_annotation_domain_and_range</hasValidationMethod>
    </owl:AnnotationProperty>
    <owl:AnnotationProperty rdf:about="&OBO_annotation_properties;sourceIndirection">
        <annotationType rdf:datatype="&xsd;string">http://www.w3.org/2004/02/skos/core#editorialNote</annotationType>
        <skos:definition xml:lang="en">An indication of an external source from which this class is a direct subclass.</skos:definition>
    </owl:AnnotationProperty>
    <owl:AnnotationProperty rdf:about="&OBO_annotation_properties;taxonomicCommonName">
        <annotationType rdf:datatype="&xsd;string">http://www.w3.org/2004/02/skos/core#altLabel</annotationType>
        <skos:definition xml:lang="en">The “common name” nametype is used for vernacular names associated with a particular taxon. These may be found at any level in the hierarchy; for example, “human”, “reptiles”, and “pale devil&#39;s-claw” are all used. Common names should be in lowercase letters, except where part of the name is derived from a proper noun, for example, “American butterfish” and “Robert&#39;s arbo- real rice rat”.
      The use of common names is inherently variable, regional, and often inconsistent. There is generally no authoritative reference that regulates the use of common names, and there is often not perfect correspondence between common names and formally described scientific taxa; therefore, there are some caveats to their use. For scientific discourse, there is no substitute for formal scientific names. Nevertheless, common names are invaluable for many indexing, retrieval, and display purposes. The combination “Oecomys roberti (Robert&#39;s arboreal rice rat)” conveys much more information than either name by itself. Issues raised by the variable, regional, and inexact use of common names are partly addressed by the “genbank common name” nametype (below) and the ability to customize names in the GenBank flatfile. (NCBI doc on NCBI Taxonomy, 2003).</skos:definition>
        <skos:definition xml:lang="en">This is the common name label frequently used to indicate a particular, species-level taxonomic group.</skos:definition>
    </owl:AnnotationProperty>
    <owl:AnnotationProperty rdf:about="&OBO_annotation_properties;termDerviedFrom">
        <annotationType rdf:datatype="&xsd;string">http://www.w3.org/2004/02/skos/core#historyNote</annotationType>
        <skos:definition xml:lang="en">Indicates a term derives from an external source but has been substantially altered from that source.  Is a type of skos_history_note.</skos:definition>
    </owl:AnnotationProperty>
    <owl:AnnotationProperty rdf:about="&OBO_annotation_properties;annotationPropertyRange"/>
    <owl:AnnotationProperty rdf:about="&OBO_annotation_properties;oboDefinition">
        <annotationType rdf:datatype="&xsd;string">http://www.w3.org/2004/02/skos/core#definition</annotationType>
        <skos:editorialNote xml:lang="en">It also will likely include the related Aristotelean genus-differentia approach to applying this manner of definition construction as used now (as of 2006) in The Gene Ontology.</skos:editorialNote>
        <skos:definition xml:lang="en">This is a class definition meeting the non-circular and Aristotelean requirements given by the OBO Foundry principles.</skos:definition>
    </owl:AnnotationProperty>
    <owl:AnnotationProperty rdf:about="&OBO_annotation_properties;definingCitationURI">
        <annotationType rdf:datatype="&xsd;string">http://purl.org/dc/elements/1.1/relation</annotationType>
        <skos:definition xml:lang="en">A publically accessible URI for a record in a citation database providing information fundamental to the definition of an ontology class.</skos:definition>
    </owl:AnnotationProperty>
    <owl:AnnotationProperty rdf:about="&OBO_annotation_properties;hasDefinitionSource">
        <annotationPropertyRange rdf:datatype="&xsd;string">http://ontology.neuinfo.org/NIF/Backend/OBO_annotation_properties.owl#EnumerationClass</annotationPropertyRange>
        <annotationPropertyDomain rdf:datatype="&xsd;string">owl:Class</annotationPropertyDomain>
        <hasValidationMethod rdf:datatype="&xsd;string">sparql_verify_annotation_domain_and_range</hasValidationMethod>
    </owl:AnnotationProperty>
    <owl:AnnotationProperty rdf:about="&OBO_annotation_properties;usageNote">
        <skos:definition xml:lang="en">A note providing guidance on the expected and appropriate usage of a given ontology class or relation.  Note that a core:scopeNote is a type of usageNote where the specific range of classes, instances, or relations to which a given class or relation applies is constrained or scoped.</skos:definition>
    </owl:AnnotationProperty>
    <owl:AnnotationProperty rdf:about="&OBO_annotation_properties;nifID">
        <annotationType rdf:datatype="&xsd;string">http://ontology.neuinfo.org/NIF/Backend/OBO_annotation_properties.owl#externalSourceId</annotationType>
        <skos:definition xml:lang="en">The ad-hoc ID created for entries in the Neuroscience Informatics Framework terminologies.</skos:definition>
    </owl:AnnotationProperty>
    <owl:AnnotationProperty rdf:about="&OBO_annotation_properties;pendingActionNote">
        <skos:altLabel rdf:datatype="&xsd;string">TODO</skos:altLabel>
        <annotationType rdf:datatype="&xsd;string">http://www.w3.org/2004/02/skos/core#editorialNote</annotationType>
        <skos:definition xml:lang="en">A note describing known tasks associate with a class that remain to be performed. This property should include a date in parenthesis to record when this pending action was first recognized as necessary.</skos:definition>
    </owl:AnnotationProperty>
    <owl:AnnotationProperty rdf:about="&OBO_annotation_properties;misnomer">
        <annotationType rdf:datatype="&xsd;string">http://www.w3.org/2004/02/skos/core#hiddenLabel</annotationType>
        <skos:definition xml:lang="en">incorrect term often found mistakenly used to refer to this class.</skos:definition>
    </owl:AnnotationProperty>
    <owl:AnnotationProperty rdf:about="&OBO_annotation_properties;antiquated">
        <annotationType rdf:datatype="&xsd;string">http://www.w3.org/2004/02/skos/core#altLabel</annotationType>
        <skos:definition xml:lang="en">A lexical variant carrying the same latent semantic value.</skos:definition>
        <skos:definition xml:lang="en">A synonym no longer in common use.</skos:definition>
    </owl:AnnotationProperty>
    <owl:AnnotationProperty rdf:about="&OBO_annotation_properties;misspelling">
        <annotationType rdf:datatype="&xsd;string">http://www.w3.org/2004/02/skos/core#hiddenLabel</annotationType>
        <skos:definition xml:lang="en">an incorrect spelling of either the preferred label or a synonym.</skos:definition>
    </owl:AnnotationProperty>
    <owl:AnnotationProperty rdf:about="&OBO_annotation_properties;createdDate">
        <annotationType rdf:datatype="&xsd;string">http://purl.org/dc/elements/1.1/date</annotationType>
        <skos:definition xml:lang="en">The date when a class was added to the file.</skos:definition>
    </owl:AnnotationProperty>
    <owl:AnnotationProperty rdf:about="&OBO_annotation_properties;curator">
        <annotationType rdf:datatype="&xsd;string">http://purl.org/dc/elements/1.1/contributor</annotationType>
        <skos:definition xml:lang="en">contributed to the properties, assertions, and other content associated with this class.</skos:definition>
    </owl:AnnotationProperty>
    <owl:AnnotationProperty rdf:about="&dc;date"/>
    <owl:AnnotationProperty rdf:about="&OBO_annotation_properties;definingCitationID">
        <annotationType rdf:datatype="&xsd;string">http://ontology.neuinfo.org/NIF/Backend/OBO_annotation_properties.owl#externalSourceId</annotationType>
        <skos:definition xml:lang="en">A namespace-specified ID for a record in a citation database providing information fundamental to the definition of an ontology class.</skos:definition>
    </owl:AnnotationProperty>
    <owl:AnnotationProperty rdf:about="&OBO_annotation_properties;annotationPropertyDomain"/>
    <owl:AnnotationProperty rdf:about="&OBO_annotation_properties;hasValidationMethod"/>
    <owl:AnnotationProperty rdf:about="&OBO_annotation_properties;modifiedDate">
        <annotationType rdf:datatype="&xsd;string">http://purl.org/dc/elements/1.1/date</annotationType>
        <skos:definition xml:lang="en">the date when a class was last altered.</skos:definition>
    </owl:AnnotationProperty>
    <owl:AnnotationProperty rdf:about="&OBO_annotation_properties;UmlsCui">
        <annotationType rdf:datatype="&xsd;string">http://ontology.neuinfo.org/NIF/Backend/OBO_annotation_properties.owl#externalSourceId</annotationType>
        <skos:editorialNote xml:lang="en">Is a type of obo_annot:obo_external_source_ID.</skos:editorialNote>
        <skos:definition xml:lang="en">This is the UMLS CUI ID for the concept associated with this class.</skos:definition>
    </owl:AnnotationProperty>
    <owl:AnnotationProperty rdf:about="&OBO_annotation_properties;synonym">
        <annotationType rdf:datatype="&xsd;string">http://www.w3.org/2004/02/skos/core#altLabel</annotationType>
        <skos:definition xml:lang="en">A lexical variant carrying the same latent semantic value.</skos:definition>
    </owl:AnnotationProperty>
    <owl:AnnotationProperty rdf:about="&OBO_annotation_properties;abbrev">
        <annotationType rdf:datatype="&xsd;string">http://www.w3.org/2004/02/skos/core#altLabel</annotationType>
        <skos:definition xml:lang="en">A lexical variant carrying the same latent semantic value.</skos:definition>
        <skos:definition xml:lang="en">A synonym that is a shortened version of either the preferred lexical label of one of its synonyms</skos:definition>
    </owl:AnnotationProperty>
    


    <!-- 
    ///////////////////////////////////////////////////////////////////////////////////////
    //
    // Datatypes
    //
    ///////////////////////////////////////////////////////////////////////////////////////
     -->

    


    <!-- 
    ///////////////////////////////////////////////////////////////////////////////////////
    //
    // Classes
    //
    ///////////////////////////////////////////////////////////////////////////////////////
     -->

    


    <!-- http://ontology.neuinfo.org/NIF/Backend/OBO_annotation_properties.owl#AbbrevSource -->

    <owl:Class rdf:about="&OBO_annotation_properties;AbbrevSource">
        <rdfs:subClassOf rdf:resource="&OBO_annotation_properties;EnumerationClass"/>
        <skos:definition xml:lang="en">The source authority for an externally derived class term abbreviation</skos:definition>
    </owl:Class>
    


    <!-- http://ontology.neuinfo.org/NIF/Backend/OBO_annotation_properties.owl#DefinitionSource -->

    <owl:Class rdf:about="&OBO_annotation_properties;DefinitionSource">
        <owl:equivalentClass>
            <owl:Class>
                <owl:oneOf rdf:parseType="Collection">
                    <rdf:Description rdf:about="&OBO_annotation_properties;Stanord_Encyclopedia_of_Philosophy_defSource"/>
                    <rdf:Description rdf:about="&OBO_annotation_properties;MeSH_defSource"/>
                    <rdf:Description rdf:about="&OBO_annotation_properties;OBI_defSource"/>
                    <rdf:Description rdf:about="&OBO_annotation_properties;Wikipedia_defSource"/>
                    <rdf:Description rdf:about="&OBO_annotation_properties;Meriam_Websters_Dictionary_online_ed_2006_defSource"/>
                    <rdf:Description rdf:about="&OBO_annotation_properties;FMA_defSource"/>
                    <rdf:Description rdf:about="&OBO_annotation_properties;American_Heritage_Dictionary_4th_ed_defSource"/>
                    <rdf:Description rdf:about="&OBO_annotation_properties;UMLS_defSource"/>
                    <rdf:Description rdf:about="&OBO_annotation_properties;GO_defSource"/>
                </owl:oneOf>
            </owl:Class>
        </owl:equivalentClass>
        <rdfs:subClassOf rdf:resource="&OBO_annotation_properties;EnumerationClass"/>
        <skos:definition xml:lang="en">The source authority for an externally derived definition</skos:definition>
    </owl:Class>
    


    <!-- http://ontology.neuinfo.org/NIF/Backend/OBO_annotation_properties.owl#EnumerationClass -->

    <owl:Class rdf:about="&OBO_annotation_properties;EnumerationClass">
        <dc:date rdf:datatype="&xsd;string">2007-05-04 (createdDate)</dc:date>
        <dc:date rdf:datatype="&xsd;string">2007-05-04 (modifedDate)</dc:date>
        <skos:scopeNote xml:lang="en">A parent class for all enumerations used for class annotation.</skos:scopeNote>
    </owl:Class>
    


    <!-- http://ontology.neuinfo.org/NIF/Backend/OBO_annotation_properties.owl#ExternalSource -->

    <owl:Class rdf:about="&OBO_annotation_properties;ExternalSource">
        <owl:equivalentClass>
            <owl:Class>
                <owl:oneOf rdf:parseType="Collection">
                    <rdf:Description rdf:about="&OBO_annotation_properties;SNOMED"/>
                    <rdf:Description rdf:about="&OBO_annotation_properties;Biodynamic_Ontology"/>
                    <rdf:Description rdf:about="&OBO_annotation_properties;MeSH"/>
                    <rdf:Description rdf:about="&OBO_annotation_properties;Simple_Bio_Upper_Ontology"/>
                    <rdf:Description rdf:about="&OBO_annotation_properties;NCBI_Taxonomy"/>
                    <rdf:Description rdf:about="&OBO_annotation_properties;MeSH-UMLS"/>
                    <rdf:Description rdf:about="&OBO_annotation_properties;OBR"/>
                    <rdf:Description rdf:about="&OBO_annotation_properties;UMLS"/>
                    <rdf:Description rdf:about="&OBO_annotation_properties;FMA"/>
                    <rdf:Description rdf:about="&OBO_annotation_properties;NLM"/>
                    <rdf:Description rdf:about="&OBO_annotation_properties;GBIF"/>
                </owl:oneOf>
            </owl:Class>
        </owl:equivalentClass>
        <rdfs:subClassOf rdf:resource="&OBO_annotation_properties;EnumerationClass"/>
        <skos:definition xml:lang="en">Class derived from an external knowledge source</skos:definition>
    </owl:Class>
    


    <!-- http://www.w3.org/1999/02/22-rdf-syntax-ns#List -->

    <owl:Class rdf:about="&rdf;List"/>
    


    <!-- 
    ///////////////////////////////////////////////////////////////////////////////////////
    //
    // Individuals
    //
    ///////////////////////////////////////////////////////////////////////////////////////
     -->

    


    <!-- http://ontology.neuinfo.org/NIF/Backend/OBO_annotation_properties.owl#American_Heritage_Dictionary_4th_ed_defSource -->

    <owl:NamedIndividual rdf:about="&OBO_annotation_properties;American_Heritage_Dictionary_4th_ed_defSource">
        <rdf:type rdf:resource="&OBO_annotation_properties;DefinitionSource"/>
    </owl:NamedIndividual>
    


    <!-- http://ontology.neuinfo.org/NIF/Backend/OBO_annotation_properties.owl#Biodynamic_Ontology -->

    <owl:NamedIndividual rdf:about="&OBO_annotation_properties;Biodynamic_Ontology">
        <rdf:type rdf:resource="&OBO_annotation_properties;ExternalSource"/>
    </owl:NamedIndividual>
    


    <!-- http://ontology.neuinfo.org/NIF/Backend/OBO_annotation_properties.owl#FMA -->

    <owl:NamedIndividual rdf:about="&OBO_annotation_properties;FMA">
        <rdf:type rdf:resource="&OBO_annotation_properties;ExternalSource"/>
    </owl:NamedIndividual>
    


    <!-- http://ontology.neuinfo.org/NIF/Backend/OBO_annotation_properties.owl#FMA_defSource -->

    <owl:NamedIndividual rdf:about="&OBO_annotation_properties;FMA_defSource">
        <rdf:type rdf:resource="&OBO_annotation_properties;DefinitionSource"/>
    </owl:NamedIndividual>
    


    <!-- http://ontology.neuinfo.org/NIF/Backend/OBO_annotation_properties.owl#GBIF -->

    <owl:NamedIndividual rdf:about="&OBO_annotation_properties;GBIF">
        <rdf:type rdf:resource="&OBO_annotation_properties;ExternalSource"/>
    </owl:NamedIndividual>
    


    <!-- http://ontology.neuinfo.org/NIF/Backend/OBO_annotation_properties.owl#GO_defSource -->

    <owl:NamedIndividual rdf:about="&OBO_annotation_properties;GO_defSource">
        <rdf:type rdf:resource="&OBO_annotation_properties;DefinitionSource"/>
    </owl:NamedIndividual>
    


    <!-- http://ontology.neuinfo.org/NIF/Backend/OBO_annotation_properties.owl#MeSH -->

    <owl:NamedIndividual rdf:about="&OBO_annotation_properties;MeSH">
        <rdf:type rdf:resource="&OBO_annotation_properties;ExternalSource"/>
    </owl:NamedIndividual>
    


    <!-- http://ontology.neuinfo.org/NIF/Backend/OBO_annotation_properties.owl#MeSH-UMLS -->

    <owl:NamedIndividual rdf:about="&OBO_annotation_properties;MeSH-UMLS">
        <rdf:type rdf:resource="&OBO_annotation_properties;ExternalSource"/>
    </owl:NamedIndividual>
    


    <!-- http://ontology.neuinfo.org/NIF/Backend/OBO_annotation_properties.owl#MeSH_defSource -->

    <owl:NamedIndividual rdf:about="&OBO_annotation_properties;MeSH_defSource">
        <rdf:type rdf:resource="&OBO_annotation_properties;DefinitionSource"/>
    </owl:NamedIndividual>
    


    <!-- http://ontology.neuinfo.org/NIF/Backend/OBO_annotation_properties.owl#Meriam_Websters_Dictionary_online_ed_2006_defSource -->

    <owl:NamedIndividual rdf:about="&OBO_annotation_properties;Meriam_Websters_Dictionary_online_ed_2006_defSource">
        <rdf:type rdf:resource="&OBO_annotation_properties;DefinitionSource"/>
    </owl:NamedIndividual>
    


    <!-- http://ontology.neuinfo.org/NIF/Backend/OBO_annotation_properties.owl#NCBI_Taxonomy -->

    <owl:NamedIndividual rdf:about="&OBO_annotation_properties;NCBI_Taxonomy">
        <rdf:type rdf:resource="&OBO_annotation_properties;ExternalSource"/>
    </owl:NamedIndividual>
    


    <!-- http://ontology.neuinfo.org/NIF/Backend/OBO_annotation_properties.owl#NLM -->

    <owl:NamedIndividual rdf:about="&OBO_annotation_properties;NLM">
        <rdf:type rdf:resource="&OBO_annotation_properties;ExternalSource"/>
    </owl:NamedIndividual>
    


    <!-- http://ontology.neuinfo.org/NIF/Backend/OBO_annotation_properties.owl#OBI_defSource -->

    <owl:NamedIndividual rdf:about="&OBO_annotation_properties;OBI_defSource">
        <rdf:type rdf:resource="&OBO_annotation_properties;DefinitionSource"/>
    </owl:NamedIndividual>
    


    <!-- http://ontology.neuinfo.org/NIF/Backend/OBO_annotation_properties.owl#OBR -->

    <owl:NamedIndividual rdf:about="&OBO_annotation_properties;OBR">
        <rdf:type rdf:resource="&OBO_annotation_properties;ExternalSource"/>
    </owl:NamedIndividual>
    


    <!-- http://ontology.neuinfo.org/NIF/Backend/OBO_annotation_properties.owl#SNOMED -->

    <owl:NamedIndividual rdf:about="&OBO_annotation_properties;SNOMED">
        <rdf:type rdf:resource="&OBO_annotation_properties;ExternalSource"/>
    </owl:NamedIndividual>
    


    <!-- http://ontology.neuinfo.org/NIF/Backend/OBO_annotation_properties.owl#Simple_Bio_Upper_Ontology -->

    <owl:NamedIndividual rdf:about="&OBO_annotation_properties;Simple_Bio_Upper_Ontology">
        <rdf:type rdf:resource="&OBO_annotation_properties;ExternalSource"/>
    </owl:NamedIndividual>
    


    <!-- http://ontology.neuinfo.org/NIF/Backend/OBO_annotation_properties.owl#Stanord_Encyclopedia_of_Philosophy_defSource -->

    <owl:NamedIndividual rdf:about="&OBO_annotation_properties;Stanord_Encyclopedia_of_Philosophy_defSource">
        <rdf:type rdf:resource="&OBO_annotation_properties;DefinitionSource"/>
    </owl:NamedIndividual>
    


    <!-- http://ontology.neuinfo.org/NIF/Backend/OBO_annotation_properties.owl#UMLS -->

    <owl:NamedIndividual rdf:about="&OBO_annotation_properties;UMLS">
        <rdf:type rdf:resource="&OBO_annotation_properties;ExternalSource"/>
    </owl:NamedIndividual>
    


    <!-- http://ontology.neuinfo.org/NIF/Backend/OBO_annotation_properties.owl#UMLS_defSource -->

    <owl:NamedIndividual rdf:about="&OBO_annotation_properties;UMLS_defSource">
        <rdf:type rdf:resource="&OBO_annotation_properties;DefinitionSource"/>
    </owl:NamedIndividual>
    


    <!-- http://ontology.neuinfo.org/NIF/Backend/OBO_annotation_properties.owl#Wikipedia_defSource -->

    <owl:NamedIndividual rdf:about="&OBO_annotation_properties;Wikipedia_defSource">
        <rdf:type rdf:resource="&OBO_annotation_properties;DefinitionSource"/>
    </owl:NamedIndividual>
    


    <!-- 
    ///////////////////////////////////////////////////////////////////////////////////////
    //
    // Annotations
    //
    ///////////////////////////////////////////////////////////////////////////////////////
     -->

    <rdf:Description rdf:about="&OBO_annotation_properties;pendingMereotopologicalRelationNote">
        <annotationType rdf:datatype="&xsd;string">http://ontology.neuinfo.org/NIF/Backend/OBO_annotation_properties.owl#pendingActionNote</annotationType>
        <skos:definition xml:lang="en">A note describing a known mereotopological spatial relation in which this class participates that is beyond pure subsumptive is_a relation.  Is a type of pending_object_relation_note.</skos:definition>
    </rdf:Description>
    <rdf:Description rdf:about="&OBO_annotation_properties;MeshUid">
        <annotationType rdf:datatype="&xsd;string">http://ontology.neuinfo.org/NIF/Backend/OBO_annotation_properties.owl#externalSourceId</annotationType>
        <skos:editorialNote xml:lang="en">Is a type of obo_annot:obo_external_source_ID.</skos:editorialNote>
        <skos:definition xml:lang="en">This is the Medical Subject Headings Unique ID for the concept associated with this class.</skos:definition>
    </rdf:Description>
    <rdf:Description rdf:about="&OBO_annotation_properties;altDefinition">
        <annotationType rdf:datatype="&xsd;string">http://www.w3.org/2004/02/skos/core#definition</annotationType>
        <skos:definition xml:lang="en">an additional, non-normative definition included while the curation status of a class is still pending.</skos:definition>
        <skos:editorialNote xml:lang="en">use of this property is discouraged.  A well defined ontology class cannot allow for alternative definitions.  This temporary_definition field should be used, when a definition is still pending full OBO definition status.</skos:editorialNote>
    </rdf:Description>
    


    <!-- 
    ///////////////////////////////////////////////////////////////////////////////////////
    //
    // General axioms
    //
    ///////////////////////////////////////////////////////////////////////////////////////
     -->

    <rdf:Description>
        <rdf:type rdf:resource="&owl;AllDifferent"/>
        <owl:distinctMembers rdf:parseType="Collection">
            <rdf:Description rdf:about="&OBO_annotation_properties;American_Heritage_Dictionary_4th_ed_defSource"/>
            <rdf:Description rdf:about="&OBO_annotation_properties;FMA_defSource"/>
            <rdf:Description rdf:about="&OBO_annotation_properties;GO_defSource"/>
            <rdf:Description rdf:about="&OBO_annotation_properties;MeSH_defSource"/>
            <rdf:Description rdf:about="&OBO_annotation_properties;Meriam_Websters_Dictionary_online_ed_2006_defSource"/>
            <rdf:Description rdf:about="&OBO_annotation_properties;OBI_defSource"/>
            <rdf:Description rdf:about="&OBO_annotation_properties;Stanord_Encyclopedia_of_Philosophy_defSource"/>
            <rdf:Description rdf:about="&OBO_annotation_properties;UMLS_defSource"/>
            <rdf:Description rdf:about="&OBO_annotation_properties;Wikipedia_defSource"/>
        </owl:distinctMembers>
    </rdf:Description>
    <rdf:Description>
        <rdf:type rdf:resource="&owl;AllDifferent"/>
        <owl:distinctMembers rdf:parseType="Collection">
            <rdf:Description rdf:about="&OBO_annotation_properties;Biodynamic_Ontology"/>
            <rdf:Description rdf:about="&OBO_annotation_properties;FMA"/>
            <rdf:Description rdf:about="&OBO_annotation_properties;GBIF"/>
            <rdf:Description rdf:about="&OBO_annotation_properties;MeSH"/>
            <rdf:Description rdf:about="&OBO_annotation_properties;MeSH-UMLS"/>
            <rdf:Description rdf:about="&OBO_annotation_properties;NCBI_Taxonomy"/>
            <rdf:Description rdf:about="&OBO_annotation_properties;NLM"/>
            <rdf:Description rdf:about="&OBO_annotation_properties;OBR"/>
            <rdf:Description rdf:about="&OBO_annotation_properties;SNOMED"/>
            <rdf:Description rdf:about="&OBO_annotation_properties;Simple_Bio_Upper_Ontology"/>
            <rdf:Description rdf:about="&OBO_annotation_properties;UMLS"/>
        </owl:distinctMembers>
    </rdf:Description>
</rdf:RDF>



<!-- Generated by the OWL API (version 3.2.3.22702) http://owlapi.sourceforge.net -->

