@prefix : <file:///ERROR/EMPTY/PREFIX/BANNED/> .
@prefix dc: <http://purl.org/dc/elements/1.1/> .
@prefix dcterms: <http://purl.org/dc/terms/> .
@prefix NIFRID: <http://uri.neuinfo.org/nif/nifstd/readable/> .
@prefix owl: <http://www.w3.org/2002/07/owl#> .
@prefix rdf: <http://www.w3.org/1999/02/22-rdf-syntax-ns#> .
@prefix rdfs: <http://www.w3.org/2000/01/rdf-schema#> .
@prefix skos: <http://www.w3.org/2004/02/skos/core#> .
@prefix xml: <http://www.w3.org/XML/1998/namespace> .
@prefix xsd: <http://www.w3.org/2001/XMLSchema#> .

<http://ontology.neuinfo.org/NIF/ttl/BIRNLex_annotation_properties.ttl> a owl:Ontology ;
    owl:imports <http://ontology.neuinfo.org/NIF/ttl/OBO_annotation_properties.ttl> ;
    dc:title "BIRNLex_annotation_properties"@en ;
    rdfs:comment "These are OWL Annotation Properties created by the BIRN OTF for the purposes of better managing the curation of the BIRNLex ontology."@en ;
    skos:changeNote " (2008-03-13) - finally added Template URLs for GO ID."@en,
        " (2008-03-21) - finally added ID property and Template URLs for ChEBI and PubChem CIDs."@en,
        " v1.2 (2007-03-20): Changed all Class identifiers to rdf:ID properties.  Some had previously been rdf:about properties.  Since Protege-OWL automatically sets new class identifiers to rdf:ID, I'm changing these across the files, to help make it more deterministic when parsing the RDF/XML."@en,
        "Have 'cleansed' the file to be OWL-DL (v1.2.2)."@en,
        "Now using a specific set of AnnotationProperties that link to specific Enumeration classes to specify annotations from a fixed list of values - e.g., ExternalSource, DefinitionSource.  This is the second iteration of this mechanism (first was put in v1.2.2).  This second version follows a patter recommended by Alan Ruttenberg which avoids using ObjectProperties as the Manchester design pattern for Value Partitions recommends, and instead sticks to AnnotationProperties only.  Note this version of OBO_annotation_properties uses the same EnumerationClasses from v1.2.2, and still includes the related ObjectProperties, so as to be able to support XSLT-based translation of the BIRNLex files that used the v1.2.2 pattern.  The next version of this file will eliminate the ObjectProperties and will rename the equivalent AnnotationProperties to remove the trailing '2' put in there to provide a unique name."@en,
        "Processed file with XSLT to remove the explicit DataTypeProperty declarations (v1.2.2)"@en,
        "v1.3.0 (2007-08-03) - Changed many things, but primarily: (1) removed rdf:datatype xsd:string specs for all AnnotationProperties, since they are now all untyped and should assume STRING as a the default; (2) added the typing of AnnotationProperties using annotationType which should aid in algorithmically processing; (3) added ReferenceURLTemplate to linked IDs to aid in algorithmically constructing URLs from IDs.  The reference URL template provides a URL template that includes a specification of how to combine it with the associated ID to build a putative URL for an external resource - putative in the sense that there is no guarantee the external curating authority will maintain this URL template; however, with these paired fields - ID and URL template template - it should be possible to update the template, when the authority changes their URL template - an updated that would then be algorithmicaly percollated to the use of that field across BIRNLex."@en,
        "v1.3.1 (2007-11-30) - Removed some UTF8 characters that dont translate well to other encodings (e.g., curly double quotes 0xE2809C)."@en ;
    owl:versionInfo "1.3.1"^^xsd:string ;
    NIFRID:createdDate "2006-09-26"^^xsd:string ;
    NIFRID:modifiedDate "2008-03-21"^^xsd:string ;
    dc:creator " xml:lang=\"en\"The BIRN Ontology Task Force"^^xsd:string .

### Annotation Properties

NIFRID:animalModel a owl:AnnotationProperty ;
    skos:definition "An organism providing a model system which mimics certain aspects of a particular human clinical syndrome or disease."@en .

NIFRID:atccID a owl:AnnotationProperty ;
    skos:definition "The unique ID for a biological material - typically a cell line - from the American Type Culture Collection database."@en ;
    rdfs:subPropertyOf NIFRID:externalSourceId ;
    NIFRID:annotationType NIFRID:externalSourceId .

NIFRID:bamsID a owl:AnnotationProperty ;
    skos:definition "The \"aidi\" ID from the Brain Architecture Management System (BAMS) corresponding to this class."@en ;
    rdfs:subPropertyOf NIFRID:externalSourceId ;
    NIFRID:annotationType NIFRID:externalSourceId .

NIFRID:birnlexComment a owl:AnnotationProperty ;
    rdfs:subPropertyOf skos:editorialNote ;
    skos:editorialNote "Is there a use for a BIRN-specific comment independent of rdfs:comment?"@en ;
    NIFRID:annotationType skos:editorialNote .

NIFRID:birnlexDefinition a owl:AnnotationProperty ;
    skos:definition "This is a type of OBO_definition that includes additional requirements specified by the BIRN OTF (additional requirements pending as of 2006-10-02)."@en ;
    rdfs:subPropertyOf NIFRID:oboDefinition ;
    NIFRID:annotationType NIFRID:oboDefinition .

NIFRID:birnlexPendingDifferentiaNote a owl:AnnotationProperty ;
    skos:definition "This is a note describing a pending class sub-genera."@en ;
    rdfs:subPropertyOf NIFRID:pendingActionNote,
        skos:scopeNote ;
    NIFRID:annotationType NIFRID:pendingActionNote,
        skos:scopeNote ;
    skos:example "\"Basal nucleus of Meynert\" is used for labeling the Basal nucleus in humans.  In a human specific neuroanatomical ontology layer, basal nucleus will receive the prefered lable \"Basal nucleus of Meynert\"."@en .

NIFRID:birnlexRetiredDefinition a owl:AnnotationProperty ;
    skos:definition "A former definition for a class.  It is kept for the purposes of interpreting annotations made when this definition was in effect and to monitor the evolution of class definitions.  Given this requirement, a \"retiredDate\" is added to the definition on the date of retirement."@en ;
    rdfs:subPropertyOf skos:definition ;
    NIFRID:annotationType skos:definition .

NIFRID:bonfireID a owl:AnnotationProperty ;
    skos:definition "This ID is derived from the BIRN BONFIRE vocubulary management system"@en ;
    rdfs:subPropertyOf NIFRID:externalSourceId ;
    NIFRID:annotationType NIFRID:externalSourceId .

NIFRID:cell_ontology_ID a owl:AnnotationProperty ;
    rdfs:subPropertyOf NIFRID:externalSourceId ;
    NIFRID:annotationType NIFRID:externalSourceId .

NIFRID:ChEBIid a owl:AnnotationProperty ;
    skos:definition "The ID from the Chemical Entities of Biological Interest (ChEBI) chemical taxonomy corresponding to this class."@en ;
    rdfs:subPropertyOf NIFRID:externalSourceId ;
    NIFRID:annotationType NIFRID:externalSourceId .

NIFRID:emapMouseStageDataID a owl:AnnotationProperty ;
    skos:definition "The unique ID for a Theiler mouse prenatal development stage as given by the EMAP Project."@en ;
    rdfs:subPropertyOf NIFRID:externalSourceId ;
    NIFRID:annotationType NIFRID:externalSourceId .

NIFRID:emapMouseStageDiagramID a owl:AnnotationProperty ;
    skos:definition "The unique ID type linked to a partiular URL Template.  An instance of this ID type can be combined algorithmically with a URL template ('$$ID$$') placeholder literal is replaced by an ID value to create a URL that links to the curated info associated with that ID."@en ;
    rdfs:subPropertyOf NIFRID:externalSourceId ;
    NIFRID:annotationType NIFRID:externalSourceId .

NIFRID:gbifID a owl:AnnotationProperty ;
    skos:definition "The unique ID for this taxonomic category in Global Biodiversity Information Facility taxonomic ,knowledgebase"@en ;
    rdfs:subPropertyOf NIFRID:externalSourceId ;
    NIFRID:annotationType NIFRID:externalSourceId .

NIFRID:gbifTaxonKeyID a owl:AnnotationProperty ;
    skos:definition "The unique ID for this taxonomy key in Global Biodiversity Information Facility taxonomic ,knowledgebase"@en ;
    rdfs:subPropertyOf NIFRID:externalSourceId ;
    NIFRID:annotationType NIFRID:externalSourceId .

NIFRID:gene_Ontology_ID a owl:AnnotationProperty ;
    rdfs:subPropertyOf NIFRID:externalSourceId ;
    NIFRID:annotationType NIFRID:externalSourceId .

NIFRID:hasBirnlexCurator a owl:AnnotationProperty ;
    NIFRID:annotationPropertyDomain owl:Class ;
    NIFRID:annotationPropertyRange NIFRID:BirnlexCurator ;
    NIFRID:hasValidationMethod "sparql_verify_annotation_domain_and_range"^^xsd:string .

NIFRID:hasCurationStatus a owl:AnnotationProperty ;
    rdfs:subPropertyOf skos:editorialNote ;
    NIFRID:annotationPropertyDomain owl:Class ;
    NIFRID:annotationPropertyRange NIFRID:CurationStatus ;
    NIFRID:annotationType skos:editorialNote ;
    NIFRID:hasValidationMethod "sparql_verify_annotation_domain_and_range"^^xsd:string .

NIFRID:hasFormerChildClass a owl:AnnotationProperty ;
    skos:definition "This annotation property is used to link back to an original child class for an obsoleted term.  The value of this property will simply be the ontology ID for the child class.  An obsoleted class can have greater than one former children.."@en ;
    NIFRID:annotationType dc:identifier,
        skos:historyNote .

NIFRID:hasFormerParentClass a owl:AnnotationProperty ;
    skos:definition "This annotation property is used to link back to the original parent class for an obsoleted term.  The value of this property will simply be the ontology ID for the parent class.  An obsoleted asserted class should have one and only one former parent class."@en ;
    NIFRID:annotationType dc:identifier,
        skos:historyNote .

NIFRID:hasKnownApplicationUses a owl:AnnotationProperty ;
    NIFRID:annotationPropertyDomain owl:Class ;
    NIFRID:annotationPropertyRange NIFRID:KnownApplicationUses ;
    NIFRID:hasValidationMethod "sparql_verify_annotation_domain_and_range"^^xsd:string .

NIFRID:hasReferenceURLTemplate a owl:AnnotationProperty ;
    NIFRID:annotationPropertyDomain owl:Class ;
    NIFRID:annotationPropertyRange "ReferenceURLTemplate"^^xsd:string ;
    NIFRID:annotationType dc:relation ;
    NIFRID:hasValidationMethod "sparql_verify_annotation_domain_and_range"^^xsd:string ;
    NIFRID:usageNote "A Class can be assigned more than one ReferenceURLTemplate assigned via distince hasReferenceURLTemplate properties"@en .

NIFRID:httpQueryUrlTemplate a owl:AnnotationProperty ;
    skos:definition "This is a template for constructing an HTTP-based dynamic query using an associated source ID."@en ;
    NIFRID:annotationType dc:relation ;
    NIFRID:usageNote "This URL will typically return a well-formed HTML page for viewing in a web browser, so long as the curating authority doesn't changed their HTTP Query template."@en .

NIFRID:imsrStandardStrainName a owl:AnnotationProperty ;
    skos:definition "This annotation property contains the approved strain name for an inbred mouse or rat as given by the International Mouse Strain Repository (IMSR)."@en ;
    NIFRID:annotationType dc:identifier,
        skos:altLabel .

NIFRID:isReplacedByClass a owl:AnnotationProperty ;
    skos:definition "This annotation property is used to link the new classes that now are used to represent the entities formerly represented by an obsoleted class.  The value of this property will simply be the ontology ID for the replacement class(es)."@en ;
    NIFRID:annotationType dc:identifier,
        skos:historyNote .

NIFRID:itisID a owl:AnnotationProperty ;
    skos:definition "The unique ID for this taxonomic category in the North American Integrated Taxonomic Information System (ITIS) taxonomic ,knowledgebase"@en ;
    rdfs:subPropertyOf NIFRID:externalSourceId ;
    NIFRID:annotationType NIFRID:externalSourceId .

NIFRID:jaxMiceID a owl:AnnotationProperty ;
    skos:definition "The unique ID for a mouse strain distributed by and tracked in the Jackson Laboratory Mouse database."@en ;
    rdfs:subPropertyOf NIFRID:externalSourceId ;
    NIFRID:annotationType NIFRID:externalSourceId .

NIFRID:ncbiIncludesName a owl:AnnotationProperty ;
    skos:definition "The \"includes\" nametype is the opposite of the in-part nametype and is included for retrieval terms that have a narrower scope of application than the taxon at which they appear. For example, we could list \"reptiles\" as an \"includes\" nametype for the Amniota (or at any higher node in the lineage) (NCBI doc on NCBI Taxonomy, 2003)."@en ;
    NIFRID:annotationType skos:scopeNote .

NIFRID:ncbiInPartName a owl:AnnotationProperty ;
    skos:definition """The "in-part" nametype is included for retrieval terms that have a broader range of application than the taxon or taxa at which they appear. For example, we list reptiles and Reptilia as in-part nametypes at our nodes Testudines (the turtles), Lepidosauria (the lizards and snakes), and Crocodylidae (the crocodilians).
         (NCBI doc on NCBI Taxonomy, 2003)."""@en ;
    NIFRID:annotationType skos:scopeNote .

NIFRID:ncbiTaxBlastName a owl:AnnotationProperty ;
    skos:definition """The "BLAST names" are a specially designated set of common names selected from the Taxonomy database. These were chosen to provide a pool of familiar names for large groups of organisms (such as "insects", "mammals", "fungi", and others) so that any particular species (which may not have an informative common name of its own) could inherit a meaningful collective common name from the Taxonomy database. This was originally developed for BLAST, because a list of BLAST results will typically include entries from many species identified by Latin binomials, which may not be familiar to all users. BLAST names may be nested; for example, "eukaryotes", "animals", "chordates", "mammals", and "primates" are all flagged as "blast names". 
         Blast names are now used in several other applications, for example the Tax BLAST displays, the Summary view in Entrez Taxonomy, and in the Summary display of the Common Tree
         format (NCBI doc on NCBI Taxonomy, 2003)."""@en ;
    NIFRID:annotationType skos:altLabel ;
    NIFRID:usageNote "The taxonomic name used in BLAST homology analysis given in NCBI Taxonomy"@en .

NIFRID:ncbiTaxGenbankCommonName a owl:AnnotationProperty ;
    skos:definition "The \"genbank common name\" was introduced to provide a mechanism by which, when there is more than one common name associated with a particular node in the taxonomy, one of them could be designated to be the common name that should be used by default in the GenBank flat- files and other applications that are trying to find a common name to use for display (or other) purposes. This is not intended to confer any special status or blessing on this particular common name over any of the other common names that might be associated with the same node, and we have developed mechanisms to override this choice for a common name on a case-by-case basis if another name is more appropriate or desirable for a particular sequence entry. Each node may have at most one \"genbank common name\" (NCBI doc on NCBI Taxonomy, 2003)."@en ;
    NIFRID:annotationType skos:altLabel ;
    NIFRID:usageNote "The common taxonomic name assigned by NCBI Taxonomy and applied to GENBANK sequence records."@en .

NIFRID:ncbiTaxID a owl:AnnotationProperty ;
    skos:definition "The unique ID for this taxonomic category in the NCBI Taxonomy database"@en ;
    rdfs:subPropertyOf NIFRID:externalSourceId ;
    NIFRID:annotationType NIFRID:externalSourceId .

NIFRID:ncbiTaxScientificName a owl:AnnotationProperty ;
    skos:definition "The preferred label for this taxonomic category in the NCBI Taxonomy database"@en ;
    NIFRID:annotationType NIFRID:synonym .

NIFRID:neuroNamesAncillaryTerm a owl:AnnotationProperty ;
    skos:definition " This class was derived from a NeuroNames ancillary term, indicated the NeuroNames developers were unable to fit it into the core NN hierarchy."@en,
        "\"(NeuroNames) defines the brain in terms of about 550 primary structures to which all other structures, names, and synonyms are related.  (It) provides standard English and Latin names for more than 850 unique structures including the primary structures, superstructures and related superficial features and shows hierarchical relations of each structure to its superstructures and substructures.  NeuroNames also defines more than 1500 other neuroanatomical entities in terms of structures in the Hierarchy. The structure you name may not be part of the Brain Hierarchy. For example, it may represent a different way of subdividing the brain or it may exist only at the embryonic stage of brain development. Such items are referred to as 'ancillary structures' (http://braininfo.rprc.washington.edu/indexabout.html)."@en .

NIFRID:neuronamesID a owl:AnnotationProperty ;
    skos:definition "The ID from the NeuroNames neuroanatomical thesaurus corresponding to this class."@en ;
    rdfs:subPropertyOf NIFRID:externalSourceId ;
    NIFRID:annotationType NIFRID:externalSourceId .

NIFRID:nitrc_ID a owl:AnnotationProperty ;
    rdfs:subPropertyOf NIFRID:externalSourceId ;
    NIFRID:annotationType NIFRID:externalSourceId .

NIFRID:PMID a owl:AnnotationProperty ;
    skos:definition "A PMID (PubMed Identifier or PubMed Unique Identifier) is a unique number assigned to each PubMed citation of life sciences and biomedical scientific journal articles."@en ;
    rdfs:subPropertyOf NIFRID:externalSourceId ;
    NIFRID:annotationType NIFRID:externalSourceId .

NIFRID:PubChemCID a owl:AnnotationProperty ;
    skos:definition "The ID from the NIH/NLM/NCBI PubChem chemical taxonomy corresponding to this class."@en ;
    rdfs:subPropertyOf NIFRID:externalSourceId ;
    NIFRID:annotationType NIFRID:externalSourceId .

NIFRID:PubMedID a owl:AnnotationProperty ;
    skos:definition "The ID from the NIH/NLM/NCBI PubMed literature related to this class."@en ;
    rdfs:subPropertyOf NIFRID:externalSourceId ;
    NIFRID:annotationType NIFRID:externalSourceId .

NIFRID:putativeClassExtension a owl:AnnotationProperty ;
    skos:definition "This is a note describing possible class sub-genera."@en ;
    NIFRID:annotationType NIFRID:pendingActionNote,
        skos:scopeNote .

NIFRID:sao_ID a owl:AnnotationProperty ;
    rdfs:subPropertyOf NIFRID:externalSourceId ;
    NIFRID:annotationType NIFRID:externalSourceId .

NIFRID:tacMiceID a owl:AnnotationProperty ;
    skos:definition "The unique ID for a mouse strain distributed by and tracked in the Taconic Farms Mouse database."@en ;
    rdfs:subPropertyOf NIFRID:externalSourceId ;
    NIFRID:annotationType NIFRID:externalSourceId .

NIFRID:umls_ID a owl:AnnotationProperty ;
    rdfs:subPropertyOf NIFRID:externalSourceId ;
    NIFRID:annotationType NIFRID:externalSourceId .

NIFRID:urlTemplateLinkedID a owl:AnnotationProperty ;
    skos:definition "This is a template for constructing an HTTP-based dynamic query using an associated source ID."@en ;
    rdfs:subPropertyOf NIFRID:externalSourceId ;
    NIFRID:annotationType NIFRID:externalSourceId ;
    NIFRID:usageNote "This URL constructed this way will typically return a well-formed HTML page for viewing in a web browser, so long as the curating authority doesn't changed their HTTP Query template."@en .

NIFRID:webServiceUrlTemplate a owl:AnnotationProperty ;
    skos:definition "This is the HTTP or WSDL URL with which a query can be constructed to return a data fragment describing the associated source ID."@en ;
    NIFRID:annotationType dc:relation ;
    NIFRID:usageNote "This is merely information and is designed to be associated with an ExternalSource, when a service is available to access related resource information using an External ID tracked in the ontology."@en .

### Classes

dcterms:DateScheme a owl:Class ;
    rdfs:subClassOf NIFRID:dctermsClass .

dcterms:DCMIType a owl:Class ;
    rdfs:subClassOf NIFRID:dctermsClass .

dcterms:FormatScheme a owl:Class ;
    rdfs:subClassOf NIFRID:dctermsClass .

dcterms:IdentifierScheme a owl:Class ;
    rdfs:subClassOf NIFRID:dctermsClass .

dcterms:LanguageScheme a owl:Class ;
    rdfs:subClassOf NIFRID:dctermsClass .

dcterms:RelationScheme a owl:Class ;
    rdfs:subClassOf NIFRID:dctermsClass .

dcterms:SourceScheme a owl:Class ;
    rdfs:subClassOf NIFRID:dctermsClass .

dcterms:SpatialScheme a owl:Class ;
    rdfs:subClassOf NIFRID:dctermsClass .

dcterms:SubjectScheme a owl:Class ;
    rdfs:subClassOf NIFRID:dctermsClass .

dcterms:TemporalScheme a owl:Class ;
    rdfs:subClassOf NIFRID:dctermsClass .

dcterms:TypeScheme a owl:Class ;
    rdfs:subClassOf NIFRID:dctermsClass .

NIFRID:BackendClass a owl:Class ;
    rdfs:label "_ Backend Class" ;
    rdfs:comment "Parent class of all the common 'backend' class entities for all the NIFSTD modules. These classes are imported from SKOS, Dublin Core Meta Data, Protege-DC, and 'extra' classes generated by OBO-to-OWL converted ontologies."@en ;
    NIFRID:createdDate "July 15, 2011"@en .

NIFRID:BirnlexAbbrevSource a owl:Class ;
    owl:equivalentClass [ a owl:Class ;
            owl:oneOf (
                    NIFRID:Hof-et-al-mouse-2000_abbrevSource
                    NIFRID:NeuroNames_abbrevSource
                    NIFRID:Paxinos-Franklin-mouse-2001_abbrevSource
                    NIFRID:Paxinos-Watson-rat-1998_abbrevSource
                    NIFRID:SumsDB_abbrevSource
                    NIFRID:Swanson-rat-1992_abbrevSource
                    NIFRID:Swanson-rat-1998_abbrevSource
                    NIFRID:Swanson-rat-2004_abbrevSource ) ] ;
    rdfs:subClassOf NIFRID:EnumerationClass .

NIFRID:BirnlexCurator a owl:Class ;
    owl:equivalentClass [ a owl:Class ;
            owl:oneOf (
                    NIFRID:Allan_MacKenzie-Graham
                    NIFRID:Amarnath_Gupta
                    NIFRID:Angie_Laird
                    NIFRID:Bill_Bug
                    NIFRID:BIRN_OTF
                    NIFRID:Brett_Peterson
                    NIFRID:Carol_Bean
                    NIFRID:Christine_Fennema-Notestine
                    NIFRID:David_Kennedy
                    NIFRID:Jeff_Grethe
                    NIFRID:Jessica_Turner
                    NIFRID:Jyl_Boline
                    NIFRID:Karen_Crawford
                    NIFRID:Karl_Helmer
                    NIFRID:Maryann_Martone
                    NIFRID:Michele_Diaz
                    NIFRID:Rob_Williams ) ] ;
    skos:definition "This property defines the BIRNLex ontology curators who've contributed to the definition of a class.  More than one instance of this property is valid.  In the case of multiple curators, the individual curator name may also be associated with the definition, if that person was primarily responsible for it."@en ;
    rdfs:subClassOf NIFRID:EnumerationClass .

NIFRID:BirnlexDefinitionSource a owl:Class ;
    owl:equivalentClass [ a owl:Class ;
            owl:oneOf (
                    NIFRID:ATCC_defSource
                    NIFRID:BAMS_defSource
                    NIFRID:BrainMap.org_defSource
                    NIFRID:ChEBI_defSource
                    NIFRID:IMSR_Glossary_defSource
                    NIFRID:MGI_defSource
                    NIFRID:NeuroNames_defSource
                    NIFRID:The_Sylvius_Project_defSource ) ] ;
    skos:definition "It indicates the external knowledge resource from which this class's definition derived."@en ;
    rdfs:subClassOf NIFRID:EnumerationClass .

NIFRID:BirnlexExternalSource a owl:Class ;
    owl:equivalentClass [ a owl:Class ;
            owl:oneOf (
                    NIFRID:ATCC
                    NIFRID:BAMS
                    NIFRID:BONFIRE
                    NIFRID:BrainMap.org
                    NIFRID:EMAP
                    NIFRID:Hof-et-al-mouse-2001
                    NIFRID:IMSR
                    NIFRID:JAX-mouse-stock
                    NIFRID:MGI
                    NIFRID:NeuroNames
                    NIFRID:Paxinos-Franklin-mouse-2001
                    NIFRID:PsychInfo_Thesaurus
                    NIFRID:SAO
                    NIFRID:SumsDB
                    NIFRID:TacFarms ) ] ;
    skos:definition "It indicates the external knowledge resource from which this class's definition derived."@en ;
    rdfs:subClassOf NIFRID:EnumerationClass .

NIFRID:birnlexLimboClass a owl:Class ;
    rdfs:label "_ Limbo Class"@en ;
    skos:prefLabel "_birnlex_limbo_class"^^xsd:string ;
    skos:definition "class in limbo since major refactoring of foundational community ontologies (e.g., BFO, OBI, SKOS). (BB:2007-03-05)."^^xsd:string ;
    rdfs:subClassOf owl:Thing ;
    NIFRID:createdDate "2007-03-05"^^xsd:string ;
    NIFRID:modifiedDate "2007-03-05"^^xsd:string ;
    NIFRID:hasBirnlexCurator NIFRID:Bill_Bug .

NIFRID:birnlexRetiredClass a owl:Class ;
    rdfs:label "_ Retired Class"@en ;
    skos:prefLabel "_birnlex_retired_class"^^xsd:string ;
    rdfs:subClassOf owl:Thing ;
    NIFRID:createdDate "2007-06-06"^^xsd:string ;
    NIFRID:modifiedDate "2007-06-06"^^xsd:string ;
    NIFRID:birnlexDefinition "These are classes for which the represented entities are now described using a different class.  A class is deprecated if it's semantic meaning required alteration or its entity is now represented directly in an imported foundational ontology.  Such obseleted classes are removed from the core subsumptive hierarchy and retired to this root branch of the tree for this ontology.  Deprecated classes maintain their original identifiers, so as to provide support for previous applications making use of the class prior to its being deprecated."^^xsd:string ;
    NIFRID:hasBirnlexCurator NIFRID:Bill_Bug .

NIFRID:CurationStatus a owl:Class ;
    owl:equivalentClass [ a owl:Class ;
            owl:oneOf (
                    NIFRID:curation_complete
                    NIFRID:definition_incomplete
                    NIFRID:graph_position_temporary
                    NIFRID:pending_final_vetting
                    NIFRID:raw_import
                    NIFRID:uncurated ) ] ;
    skos:definition "This provides specific info on the level of curation a given class has received and is specifically design to promote automated reporting on the status of classes in an ontology.  It is likely some classes will require more than one instance of this property to fully describe their status.   Is a type of skos_editorial_note."@en ;
    rdfs:subClassOf NIFRID:EnumerationClass ;
    skos:scopeNote "The current range of values for this property are: (1) raw_import :== a class derived directly via import of an entity form an existing knowledge resource.  Terms labeled as such has yet to receive any additional curation.  As they do, their status is likely to change, though the link back to the original entity in the external resource is maintained; (2) definition_incomplete :== the curators recognize the definition of the class remains incomplete in someway.  Many definitions are dervied from external sources (a fact tracked via an additional annotation property) and require considerable amending before they fully comply with the OBO Foundry Aristotelean genera/differentia & non-circular specification; (3) graph_position_temporary :== indicates the class may not be in its final preferred location within the ontology graph.  This label can be particularly useful during early ontology creation, as for certain entities, it may not be obvious where precisely a given class should reside until a sufficiently large portion of the graph has been settled; (4) uncurated :== indicates a class has been created by curators but has received minimal review; (5) pending_final_vetting :== indicates the term is likely ready for promotion to \"curation_complete\" status, and only requires a final review by the curators responsible.  A class may also be demoted to this status when a formerly \"complete\" class has been determined to require amendments.  In accordance with the emerging best practices, such a term will be moved to an obsolete branch of the ontology, when the new replacement class has been fully vetted and marked as such; (6) curation_complete :== indicates a class has been fully vetted by the curation authorities and to the best of their ability determined to be ready for use."@en .

NIFRID:dctermsClass a owl:Class ;
    rdfs:label "Dublin Core Terms Class"@en ;
    rdfs:subClassOf NIFRID:BackendClass ;
    rdfs:comment "Parent class of the class entities imported from DC terms."@en .

NIFRID:EnumerationClass a owl:Class ;
    rdfs:subClassOf NIFRID:BackendClass .

NIFRID:KnownApplicationUses a owl:Class ;
    owl:equivalentClass [ a owl:Class ;
            owl:oneOf (
                    NIFRID:ABA_app
                    NIFRID:BAMS_app
                    NIFRID:BrainInfo.org_app
                    NIFRID:BrainMap.org_app
                    NIFRID:BrainMaps.org_app
                    NIFRID:CoCoMac_app
                    NIFRID:Franklin-Paxinos-mouse-2001_app
                    NIFRID:FreeSurfer_app
                    NIFRID:GENSAT_app
                    NIFRID:IATR_app
                    NIFRID:MBAT_app
                    NIFRID:SenseLab_app ) ] ;
    skos:definition "A application where the class entity is known to currently be in use by annotators and users searching those annotations.  Multiple instances of this property can be used to identify more than one current application."@en ;
    rdfs:subClassOf NIFRID:EnumerationClass ;
    skos:scopeNote "This property is merely informative and not assumed to be an exhaustive list.  Rather, it is just an list of examples known to the BIRNLex curators at the time the term was last modified."@en .

NIFRID:ReferenceURLTemplate a owl:Class ;
    owl:equivalentClass [ a owl:Class ;
            owl:oneOf (
                    NIFRID:atccURLTemplate
                    NIFRID:bamsURLTemplate
                    NIFRID:chebiURLTemplate
                    NIFRID:emapMouseStageDataURLTemplate
                    NIFRID:emapMouseStageDiagramURLTemplate
                    NIFRID:gbifTaxonKeyURLTemplate
                    NIFRID:gbifURLTemplate
                    NIFRID:goURLTemplate
                    NIFRID:itisURLTemplate
                    NIFRID:jaxMiceURLTemplate
                    NIFRID:meshURLTemplate
                    NIFRID:ncbiTaxURLTemplate
                    NIFRID:neuronamesURLTemplate
                    NIFRID:pubchemCicURLTemplate
                    NIFRID:tacMiceURLTemplate ) ] ;
    rdfs:subClassOf NIFRID:EnumerationClass ;
    NIFRID:usageNote "Note that each instance of ReferenceURLTemplate will be named using the template name of the matching ID AnnotationProperty.  For example, the ReferenceURLTemplate ncbiTaxURLTemplate is linked to the ncbiTaxID AnnotationProperty, whose value can be combined algorithmically with this URL template to construct a working URL to the specific class reference.  This is a far from perfect solution to some of the limitations of imposed on the use of AnnotationProperties - in particular, the inability to explicitly link one annotation property to another (e.g., explicitly relating ncbiTaxID ncbiTaxURLTemplate as applied to a specific owl:Class).  However, this mechanism should suffice for now.  It will not only support more complete automatic processing of this critical information, but can also be algorithmically translated to whatever better mechanims may become available in future versions of OWL."@en,
        "The URL reference template is given exactly as posted in the form of a HTTP query, with the unique ID represented with the symbol '$$ID$$'"@en .

NIFRID:skosClass a owl:Class ;
    rdfs:label "SKOS Class"@en ;
    rdfs:subClassOf NIFRID:BackendClass ;
    rdfs:comment "Parent class of the class entities imported from SKOS."@en .

skos:Collection a owl:Class ;
    rdfs:subClassOf NIFRID:skosClass .

skos:ConceptScheme a owl:Class ;
    rdfs:subClassOf NIFRID:skosClass .

### Individuals

NIFRID:ABA_app a NIFRID:KnownApplicationUses,
        owl:NamedIndividual .

NIFRID:Allan_MacKenzie-Graham a NIFRID:BirnlexCurator,
        owl:NamedIndividual .

NIFRID:Amarnath_Gupta a NIFRID:BirnlexCurator,
        owl:NamedIndividual .

NIFRID:Angie_Laird a NIFRID:BirnlexCurator,
        owl:NamedIndividual .

NIFRID:ATCC a NIFRID:BirnlexExternalSource,
        owl:NamedIndividual .

NIFRID:ATCC_defSource a NIFRID:BirnlexDefinitionSource,
        owl:NamedIndividual .

NIFRID:atccURLTemplate a NIFRID:ReferenceURLTemplate,
        owl:NamedIndividual ;
    NIFRID:httpQueryUrlTemplate <http://www.atcc.org/common/catalog/numSearch/numResults.cfm?atccNum=$$ID$$> ;
    NIFRID:urlTemplateLinkedID NIFRID:atccID ;
    NIFRID:usageNote "The URL reference template for a resource page at the American Type Culture Collection catalog."@en .

NIFRID:BAMS a NIFRID:BirnlexExternalSource,
        owl:NamedIndividual ;
    dc:title "Brain Architecture Management System"^^xsd:string ;
    dc:publisher "Brain Architecture Center, University of Southern California, CA, USA"^^xsd:string ;
    dc:source <http://brancusi.usc.edu/bkms/> .

NIFRID:BAMS_app a NIFRID:KnownApplicationUses,
        owl:NamedIndividual .

NIFRID:BAMS_defSource a NIFRID:BirnlexDefinitionSource,
        owl:NamedIndividual .

NIFRID:bamsURLTemplate a NIFRID:ReferenceURLTemplate,
        owl:NamedIndividual ;
    NIFRID:httpQueryUrlTemplate <http://brancusi.usc.edu/bkms/brain/show-braing2.php?aidi=$$ID$$> ;
    NIFRID:urlTemplateLinkedID NIFRID:bamsID ;
    NIFRID:usageNote "The URL reference template for the main page in the Brain Architecture Management portal for a BAMS-defined neuroanatomical structure."@en .

NIFRID:Bill_Bug a NIFRID:BirnlexCurator,
        owl:NamedIndividual .

NIFRID:BIRN_OTF a NIFRID:BirnlexCurator,
        owl:NamedIndividual .

NIFRID:BONFIRE a NIFRID:BirnlexExternalSource,
        owl:NamedIndividual ;
    dc:title "The BIRN BONFIRE terminology server"^^xsd:string ;
    dc:publisher "The Biomedical Informatics Research Network (BIRN), NCRR, NIH"^^xsd:string .

NIFRID:BrainInfo.org_app a NIFRID:KnownApplicationUses,
        owl:NamedIndividual .

NIFRID:BrainMap.org a NIFRID:BirnlexExternalSource,
        owl:NamedIndividual ;
    dc:title "The BrainMap Project"^^xsd:string ;
    dc:publisher "Research Imaging Center, University of Texas Health Science Center, San Antonio, TX, USA"^^xsd:string ;
    dc:source <http://www.brainmap.org/> .

NIFRID:BrainMap.org_app a NIFRID:KnownApplicationUses,
        owl:NamedIndividual .

NIFRID:BrainMap.org_defSource a NIFRID:BirnlexDefinitionSource,
        owl:NamedIndividual .

NIFRID:BrainMaps.org_app a NIFRID:KnownApplicationUses,
        owl:NamedIndividual .

NIFRID:Brett_Peterson a NIFRID:BirnlexCurator,
        owl:NamedIndividual .

NIFRID:Carol_Bean a NIFRID:BirnlexCurator,
        owl:NamedIndividual .

NIFRID:ChEBI_defSource a NIFRID:BirnlexDefinitionSource,
        owl:NamedIndividual .

NIFRID:chebiURLTemplate a NIFRID:ReferenceURLTemplate,
        owl:NamedIndividual ;
    NIFRID:httpQueryUrlTemplate <http://www.ebi.ac.uk/ontology-lookup/?termId=CHEBI%3A$$ID$$> ;
    NIFRID:urlTemplateLinkedID NIFRID:ChEBIid ;
    NIFRID:usageNote "The URL reference template for an Ontology Lookup Service Browser page for a given ChEBI term."@en .

NIFRID:Christine_Fennema-Notestine a NIFRID:BirnlexCurator,
        owl:NamedIndividual .

NIFRID:CoCoMac_app a NIFRID:KnownApplicationUses,
        owl:NamedIndividual .

NIFRID:curation_complete a NIFRID:CurationStatus,
        owl:NamedIndividual ;
    skos:definition "indicates a class has been fully vetted by the curation authorities and to the best of their ability determined to be ready for use."@en .

NIFRID:David_Kennedy a NIFRID:BirnlexCurator,
        owl:NamedIndividual .

NIFRID:definition_incomplete a NIFRID:CurationStatus,
        owl:NamedIndividual ;
    skos:definition "the curators recognize the definition of the class remains incomplete in someway.  Many definitions are dervied from external sources (a fact tracked via an additional annotation property) and require considerable amending before they fully comply with the OBO Foundry Aristotelean genera/differentia & non-circular specification."@en .

NIFRID:EMAP a NIFRID:BirnlexExternalSource,
        owl:NamedIndividual ;
    dc:title "Edinburgh Mouse Atlas Project"^^xsd:string ;
    dc:publisher "MRC Human Genetics Unit, Western General Hospital, Edinburgh, UK"^^xsd:string ;
    dc:source <http://genex.hgu.mrc.ac.uk/> .

NIFRID:emapMouseStageDataURLTemplate a NIFRID:ReferenceURLTemplate,
        owl:NamedIndividual ;
    NIFRID:httpQueryUrlTemplate <http://genex.hgu.mrc.ac.uk/Databases/Anatomy/XML/$$ID$$.xml> ;
    NIFRID:urlTemplateLinkedID NIFRID:emapMouseStageDataID ;
    NIFRID:usageNote "The URL reference template for the data associated with a Theiler mouse prenatal development stage as given by the EMAP Project,"@en .

NIFRID:emapMouseStageDiagramURLTemplate a NIFRID:ReferenceURLTemplate,
        owl:NamedIndividual ;
    NIFRID:httpQueryUrlTemplate <http://genex.hgu.mrc.ac.uk/Databases/Anatomy/Diagrams/$$ID$$> ;
    NIFRID:urlTemplateLinkedID NIFRID:emapMouseStageDiagramID ;
    NIFRID:usageNote "The URL reference template for the diagram associated with a Theiler mouse prenatal development stage as given by the EMAP Project."@en .

NIFRID:Franklin-Paxinos-mouse-2001_app a NIFRID:KnownApplicationUses,
        owl:NamedIndividual .

NIFRID:FreeSurfer_app a NIFRID:KnownApplicationUses,
        owl:NamedIndividual .

NIFRID:gbifTaxonKeyURLTemplate a NIFRID:ReferenceURLTemplate,
        owl:NamedIndividual ;
    NIFRID:httpQueryUrlTemplate <http://www.europe.gbif.net/portal/ecat_browser.jsp?taxonKey=$$ID$$&countryKey=0&resourceKey=0> ;
    NIFRID:urlTemplateLinkedID NIFRID:gbifTaxonKeyID ;
    NIFRID:usageNote "The URL reference template for a taxonomy key in Global Biodiversity Information Facility taxonomic ,knowledgebase"@en .

NIFRID:gbifURLTemplate a NIFRID:ReferenceURLTemplate,
        owl:NamedIndividual ;
    NIFRID:httpQueryUrlTemplate <http://data.gbif.org/species/$$ID$$> ;
    NIFRID:urlTemplateLinkedID NIFRID:gbifID ;
    NIFRID:usageNote "The URL reference template for a taxonomic category in Global Biodiversity Information Facility taxonomic ,knowledgebase"@en .

NIFRID:GENSAT_app a NIFRID:KnownApplicationUses,
        owl:NamedIndividual .

NIFRID:goURLTemplate a NIFRID:ReferenceURLTemplate,
        owl:NamedIndividual ;
    NIFRID:httpQueryUrlTemplate <http://amigo.geneontology.org/cgi-bin/amigo/go.cgi?view=details&query=$$ID$$> ;
    NIFRID:urlTemplateLinkedID NIFRID:GOid ;
    NIFRID:usageNote "The URL reference template for an AmiGO Browser page for a given Gene Ontology term."@en ;
    NIFRID:webServiceUrlTemplate <http://amigo.geneontology.org/cgi-bin/amigo/go.cgi?format=xml&query=$$ID$$> .

NIFRID:graph_position_temporary a NIFRID:CurationStatus,
        owl:NamedIndividual ;
    skos:definition "indicates the class may not be in its final preferred location within the ontology graph.  This label can be particularly useful during early ontology creation, as for certain entities, it may not be obvious where precisely a given class should reside until a sufficiently large portion of the graph has been settled."@en .

NIFRID:Hof-et-al-mouse-2000_abbrevSource a NIFRID:BirnlexAbbrevSource,
        owl:NamedIndividual .

NIFRID:Hof-et-al-mouse-2001 a NIFRID:BirnlexExternalSource,
        owl:NamedIndividual .

NIFRID:IATR_app a NIFRID:KnownApplicationUses,
        owl:NamedIndividual .

NIFRID:IMSR a NIFRID:BirnlexExternalSource,
        owl:NamedIndividual .

NIFRID:IMSR_Glossary_defSource a NIFRID:BirnlexDefinitionSource,
        owl:NamedIndividual .

NIFRID:itisURLTemplate a NIFRID:ReferenceURLTemplate,
        owl:NamedIndividual ;
    NIFRID:httpQueryUrlTemplate <http://www.itis.gov/servlet/SingleRpt/SingleRpt?search_topic=TSN&search_value=$$ID$$> ;
    NIFRID:urlTemplateLinkedID NIFRID:itisID ;
    NIFRID:usageNote "The URL reference template for a taxonomic category in the North American Integrated Taxonomic Information System (ITIS) taxonomic ,knowledgebase"@en .

NIFRID:JAX-mouse-stock a NIFRID:BirnlexExternalSource,
        owl:NamedIndividual .

NIFRID:jaxMiceURLTemplate a NIFRID:ReferenceURLTemplate,
        owl:NamedIndividual ;
    NIFRID:httpQueryUrlTemplate <http://jaxmice.jax.org/strain/$$ID$$.html> ;
    NIFRID:urlTemplateLinkedID NIFRID:jaxMiceID ;
    NIFRID:usageNote "The URL reference template for a mouse strain tracked in the Jackson Laboratory Mouse database"@en .

NIFRID:Jeff_Grethe a NIFRID:BirnlexCurator,
        owl:NamedIndividual .

NIFRID:Jessica_Turner a NIFRID:BirnlexCurator,
        owl:NamedIndividual .

NIFRID:Jyl_Boline a NIFRID:BirnlexCurator,
        owl:NamedIndividual .

NIFRID:Karen_Crawford a NIFRID:BirnlexCurator,
        owl:NamedIndividual .

NIFRID:Karl_Helmer a NIFRID:BirnlexCurator,
        owl:NamedIndividual .

NIFRID:Maryann_Martone a NIFRID:BirnlexCurator,
        owl:NamedIndividual .

NIFRID:MBAT_app a NIFRID:KnownApplicationUses,
        owl:NamedIndividual .

NIFRID:meshURLTemplate a NIFRID:ReferenceURLTemplate,
        owl:NamedIndividual ;
    NIFRID:httpQueryUrlTemplate <http://www.nlm.nih.gov/cgi/mesh/2008/MB_cgi?field=uid&term=$$ID$$> ;
    NIFRID:urlTemplateLinkedID NIFRID:MeshUid ;
    NIFRID:usageNote "The URL reference template for an NLM MeSH Browser page for a given MeSH heading."@en ;
    NIFRID:webServiceUrlTemplate <http://eutils.ncbi.nlm.nih.gov/entrez/eutils/esummary.fcgi?db=mesh&id=$$ID$$> .

NIFRID:MGI a NIFRID:BirnlexExternalSource,
        owl:NamedIndividual .

NIFRID:MGI_defSource a NIFRID:BirnlexDefinitionSource,
        owl:NamedIndividual .

NIFRID:Michele_Diaz a NIFRID:BirnlexCurator,
        owl:NamedIndividual .

NIFRID:ncbiTaxURLTemplate a NIFRID:ReferenceURLTemplate,
        owl:NamedIndividual ;
    NIFRID:httpQueryUrlTemplate <http://www.ncbi.nlm.nih.gov/Taxonomy/Browser/wwwtax.cgi?mode=Info&id=$$ID$$> ;
    NIFRID:urlTemplateLinkedID NIFRID:ncbiTaxID ;
    NIFRID:usageNote "The URL reference template for a taxonomic category in NCBI Taxonomy"@en ;
    NIFRID:webServiceUrlTemplate <http://eutils.ncbi.nlm.nih.gov/entrez/eutils/esummary.fcgi?db=taxonomy&id=$$ID$$> .

NIFRID:NeuroNames a NIFRID:BirnlexExternalSource,
        owl:NamedIndividual ;
    dc:title "The NeuroNames Ontologies"^^xsd:string ;
    dc:publisher "The BrainInfo Project, Washington National Primate Research Center, University of Washington, Seattle, WA, USA"^^xsd:string ;
    dc:source <http://braininfo.rprc.washington.edu/nnont.html> .

NIFRID:NeuroNames_abbrevSource a NIFRID:BirnlexAbbrevSource,
        owl:NamedIndividual .

NIFRID:NeuroNames_defSource a NIFRID:BirnlexDefinitionSource,
        owl:NamedIndividual .

NIFRID:neuronamesURLTemplate a NIFRID:ReferenceURLTemplate,
        owl:NamedIndividual ;
    NIFRID:httpQueryUrlTemplate <http://braininfo.rprc.washington.edu/Scripts/hiercentraldirectory.aspx?ID=$$ID$$> ;
    NIFRID:urlTemplateLinkedID NIFRID:neuronamesID ;
    NIFRID:usageNote "The URL reference template for the main page in the BrainInfo.org portal for a NeuroNames neuroanatomical structure."@en .

NIFRID:nlx_000014 a NIFRID:BirnlexCurator,
        owl:NamedIndividual ;
    rdfs:label "Anita_Bandrowski"@en .

NIFRID:Paxinos-Franklin-mouse-2001 a NIFRID:BirnlexExternalSource,
        owl:NamedIndividual .

NIFRID:Paxinos-Franklin-mouse-2001_abbrevSource a NIFRID:BirnlexAbbrevSource,
        owl:NamedIndividual .

NIFRID:Paxinos-Watson-rat-1998_abbrevSource a NIFRID:BirnlexAbbrevSource,
        owl:NamedIndividual .

NIFRID:pending_final_vetting a NIFRID:CurationStatus,
        owl:NamedIndividual ;
    skos:definition "indicates the term is likely ready for promotion to \"curation_complete\" status, and only requires a final review by the curators responsible.  A class may also be demoted to this status when a formerly \"complete\" class has been determined to require amendments.  In accordance with the emerging best practices, such a term will be moved to an obsolete branch of the ontology, when the new replacement class has been fully vetted and marked as such."@en .

NIFRID:PsychInfo_Thesaurus a NIFRID:BirnlexExternalSource,
        owl:NamedIndividual .

NIFRID:pubchemCicURLTemplate a NIFRID:ReferenceURLTemplate,
        owl:NamedIndividual ;
    NIFRID:httpQueryUrlTemplate <http://pubchem.ncbi.nlm.nih.gov/summary/summary.cgi?cid=$$ID$$> ;
    NIFRID:urlTemplateLinkedID NIFRID:ChEBIid ;
    NIFRID:usageNote "The URL reference template for an PubChem Browser page for a given PubChem CID term."@en .

NIFRID:raw_import a NIFRID:CurationStatus,
        owl:NamedIndividual ;
    skos:definition "a class derived directly via import of an entity form an existing knowledge resource.  Terms labeled as such has yet to receive any additional curation.  As they do, their status is likely to change, though the link back to the original entity in the external resource is maintained."@en .

NIFRID:Rob_Williams a NIFRID:BirnlexCurator,
        owl:NamedIndividual .

NIFRID:SAO a NIFRID:BirnlexExternalSource,
        owl:NamedIndividual .

NIFRID:SenseLab_app a NIFRID:KnownApplicationUses,
        owl:NamedIndividual .

NIFRID:SumsDB a NIFRID:BirnlexExternalSource,
        owl:NamedIndividual .

NIFRID:SumsDB_abbrevSource a NIFRID:BirnlexAbbrevSource,
        owl:NamedIndividual .

NIFRID:Swanson-rat-1992_abbrevSource a NIFRID:BirnlexAbbrevSource,
        owl:NamedIndividual .

NIFRID:Swanson-rat-1998_abbrevSource a NIFRID:BirnlexAbbrevSource,
        owl:NamedIndividual .

NIFRID:Swanson-rat-2004_abbrevSource a NIFRID:BirnlexAbbrevSource,
        owl:NamedIndividual .

NIFRID:TacFarms a NIFRID:BirnlexExternalSource,
        owl:NamedIndividual .

NIFRID:tacMiceURLTemplate a NIFRID:ReferenceURLTemplate,
        owl:NamedIndividual ;
    NIFRID:httpQueryUrlTemplate <http://www.taconic.com/wmspage.cfm?parm1=$$ID$$> ;
    NIFRID:urlTemplateLinkedID NIFRID:tacMiceID ;
    NIFRID:usageNote "The URL reference template for a mouse strain tracked in the Taconic Farms Mouse database"@en .

NIFRID:The_Sylvius_Project_defSource a NIFRID:BirnlexDefinitionSource,
        owl:NamedIndividual .

NIFRID:uncurated a NIFRID:CurationStatus,
        owl:NamedIndividual ;
    skos:definition "indicates a class has been created by curators but has received minimal review."@en .

### Axioms

[ a owl:AllDifferent ;
    owl:distinctMembers (
            NIFRID:curation_complete
            NIFRID:definition_incomplete
            NIFRID:graph_position_temporary
            NIFRID:pending_final_vetting
            NIFRID:raw_import
            NIFRID:uncurated ) ] .

[ a owl:AllDifferent ;
    owl:distinctMembers (
            NIFRID:ATCC_defSource
            NIFRID:BAMS_defSource
            NIFRID:BrainMap.org_defSource
            NIFRID:ChEBI_defSource
            NIFRID:IMSR_Glossary_defSource
            NIFRID:MGI_defSource
            NIFRID:NeuroNames_defSource
            NIFRID:The_Sylvius_Project_defSource ) ] .

[ a owl:AllDifferent ;
    owl:distinctMembers (
            NIFRID:Hof-et-al-mouse-2000_abbrevSource
            NIFRID:NeuroNames_abbrevSource
            NIFRID:Paxinos-Franklin-mouse-2001_abbrevSource
            NIFRID:Paxinos-Watson-rat-1998_abbrevSource
            NIFRID:SumsDB_abbrevSource
            NIFRID:Swanson-rat-1992_abbrevSource
            NIFRID:Swanson-rat-1998_abbrevSource
            NIFRID:Swanson-rat-2004_abbrevSource ) ] .

[ a owl:AllDifferent ;
    owl:distinctMembers (
            NIFRID:ABA_app
            NIFRID:BAMS_app
            NIFRID:BrainInfo.org_app
            NIFRID:BrainMap.org_app
            NIFRID:BrainMaps.org_app
            NIFRID:CoCoMac_app
            NIFRID:Franklin-Paxinos-mouse-2001_app
            NIFRID:FreeSurfer_app
            NIFRID:GENSAT_app
            NIFRID:IATR_app
            NIFRID:MBAT_app
            NIFRID:SenseLab_app ) ] .

[ a owl:AllDifferent ;
    owl:distinctMembers (
            NIFRID:atccURLTemplate
            NIFRID:bamsURLTemplate
            NIFRID:chebiURLTemplate
            NIFRID:emapMouseStageDataURLTemplate
            NIFRID:emapMouseStageDiagramURLTemplate
            NIFRID:gbifTaxonKeyURLTemplate
            NIFRID:gbifURLTemplate
            NIFRID:goURLTemplate
            NIFRID:itisURLTemplate
            NIFRID:jaxMiceURLTemplate
            NIFRID:meshURLTemplate
            NIFRID:ncbiTaxURLTemplate
            NIFRID:neuronamesURLTemplate ) ] .

[ a owl:AllDifferent ;
    owl:distinctMembers (
            NIFRID:ATCC
            NIFRID:BAMS
            NIFRID:BONFIRE
            NIFRID:BrainMap.org
            NIFRID:EMAP
            NIFRID:Hof-et-al-mouse-2001
            NIFRID:IMSR
            NIFRID:JAX-mouse-stock
            NIFRID:MGI
            NIFRID:NeuroNames
            NIFRID:Paxinos-Franklin-mouse-2001
            NIFRID:PsychInfo_Thesaurus
            NIFRID:SAO
            NIFRID:SumsDB
            NIFRID:TacFarms ) ] .

[ a owl:AllDifferent ;
    owl:distinctMembers (
            NIFRID:Allan_MacKenzie-Graham
            NIFRID:Amarnath_Gupta
            NIFRID:Angie_Laird
            NIFRID:Bill_Bug
            NIFRID:BIRN_OTF
            NIFRID:Brett_Peterson
            NIFRID:Carol_Bean
            NIFRID:Christine_Fennema-Notestine
            NIFRID:David_Kennedy
            NIFRID:Jeff_Grethe
            NIFRID:Jessica_Turner
            NIFRID:Jyl_Boline
            NIFRID:Karen_Crawford
            NIFRID:Karl_Helmer
            NIFRID:Maryann_Martone
            NIFRID:Michele_Diaz
            NIFRID:Rob_Williams ) ] .

### Serialized using the nifstd custom serializer v1.0.7
