<?xml version="1.0"?>


<!DOCTYPE rdf:RDF [
    <!ENTITY dc "http://purl.org/dc/terms/" >
    <!ENTITY cito "http://purl.org/net/cito/" >
    <!ENTITY foaf "http://xmlns.com/foaf/0.1/" >
    <!ENTITY owl "http://www.w3.org/2002/07/owl#" >
    <!ENTITY obo "http://purl.obolibrary.org/obo/" >
    <!ENTITY OBO_REL "http://purl.org/obo/owl/OBO_REL#" >
    <!ENTITY xsd "http://www.w3.org/2001/XMLSchema#" >
    <!ENTITY snap "http://www.ifomis.org/bfo/1.1/snap#" >
    <!ENTITY span "http://www.ifomis.org/bfo/1.1/span#" >
    <!ENTITY ro "http://www.obofoundry.org/ro/ro.owl#" >
    <!ENTITY skos "http://www.w3.org/2004/02/skos/core#" >
    <!ENTITY rdfs "http://www.w3.org/2000/01/rdf-schema#" >
    <!ENTITY rdf "http://www.w3.org/1999/02/22-rdf-syntax-ns#" >
    <!ENTITY cogat "http://www.cognitiveatlas.org/ontology/cogat.owl#" >
]>


<rdf:RDF xmlns="http://www.cognitiveatlas.org/ontology/cogat.owl#"
     xml:base="http://www.cognitiveatlas.org/ontology/cogat.owl#"
     xmlns:obo="http://purl.obolibrary.org/obo/"
     xmlns:cogat="http://www.cognitiveatlas.org/ontology/cogat.owl#"
     xmlns:snap="http://www.ifomis.org/bfo/1.1/snap#"
     xmlns:ro="http://www.obofoundry.org/ro/ro.owl#"
     xmlns:xsd="http://www.w3.org/2001/XMLSchema#"
     xmlns:OBO_REL="http://purl.org/obo/owl/OBO_REL#"
     xmlns:cito="http://purl.org/net/cito/"
     xmlns:rdfs="http://www.w3.org/2000/01/rdf-schema#"
     xmlns:foaf="http://xmlns.com/foaf/0.1/"
     xmlns:owl="http://www.w3.org/2002/07/owl#"
     xmlns:skos="http://www.w3.org/2004/02/skos/core#"
     xmlns:dc="http://purl.org/dc/terms/"
     xmlns:span="http://www.ifomis.org/bfo/1.1/span#"
     xmlns:rdf="http://www.w3.org/1999/02/22-rdf-syntax-ns#">
    <owl:Ontology rdf:about="http://www.cognitiveatlas.org/ontology/cogat.owl#">
        <owl:versionInfo>0.3</owl:versionInfo>
    </owl:Ontology>
    


    <!-- 
    ///////////////////////////////////////////////////////////////////////////////////////
    //
    // Annotation properties
    //
    ///////////////////////////////////////////////////////////////////////////////////////
     -->

    <owl:AnnotationProperty rdf:about="&skos;hasTopConcept"/>
    <owl:AnnotationProperty rdf:about="&dc;Contributor"/>
    <owl:AnnotationProperty rdf:about="&skos;prefLabel"/>
    <owl:AnnotationProperty rdf:about="&dc;Title"/>
    <owl:AnnotationProperty rdf:about="&dc;Date"/>
    <owl:AnnotationProperty rdf:about="&dc;identifier"/>
    <owl:AnnotationProperty rdf:about="&cogat;measured_by">
        <rdfs:label>measured_by</rdfs:label>
        <obo:IAO_0000115>The relationship between a mental concept and a measurement that is thought to reflect the activity of that mental concept.</obo:IAO_0000115>
        <rdfs:domain rdf:resource="&cogat;MentalConcept"/>
    </owl:AnnotationProperty>
    <owl:AnnotationProperty rdf:about="&skos;definition"/>
    <owl:AnnotationProperty rdf:about="&obo;IAO_0000115"/>
    <owl:AnnotationProperty rdf:about="&skos;altLabel"/>
    


    <!-- 
    ///////////////////////////////////////////////////////////////////////////////////////
    //
    // Datatypes
    //
    ///////////////////////////////////////////////////////////////////////////////////////
     -->

    


    <!-- 
    ///////////////////////////////////////////////////////////////////////////////////////
    //
    // Object Properties
    //
    ///////////////////////////////////////////////////////////////////////////////////////
     -->

    


    <!-- http://www.cognitiveatlas.org/ontology/cogat.owl#descended_from -->

    <owl:ObjectProperty rdf:about="&cogat;descended_from">
        <rdfs:label>descended_from</rdfs:label>
        <obo:IAO_0000115>The relationship between a task and another task of which the former is an adaptation.</obo:IAO_0000115>
    </owl:ObjectProperty>
    


    <!-- http://www.cognitiveatlas.org/ontology/cogat.owl#measured_by -->

    <owl:ObjectProperty rdf:about="&cogat;measured_by">
        <rdfs:label>measured_by</rdfs:label>
        <obo:IAO_0000115>The relationship between a mental concept and a measurement that is thought to reflect the activity of that mental concept.</obo:IAO_0000115>
    </owl:ObjectProperty>
    


    <!-- http://www.obofoundry.org/ro/ro.owl#has_part -->

    <owl:ObjectProperty rdf:about="&ro;has_part"/>
    


    <!-- http://www.obofoundry.org/ro/ro.owl#part_of -->

    <owl:ObjectProperty rdf:about="&ro;part_of"/>
    


    <!-- 
    ///////////////////////////////////////////////////////////////////////////////////////
    //
    // Classes
    //
    ///////////////////////////////////////////////////////////////////////////////////////
     -->

    


    <!-- http://www.cognitiveatlas.org/ontology/cogat.owl#CAO_00001 -->

    <owl:Class rdf:about="&cogat;CAO_00001">
        <rdfs:subClassOf rdf:resource="&skos;Concept"/>
    </owl:Class>
    


    <!-- http://www.cognitiveatlas.org/ontology/cogat.owl#CAO_00101 -->

    <owl:Class rdf:about="&cogat;CAO_00101">
        <rdfs:label>Abductive reasoning</rdfs:label>
        <rdfs:subClassOf rdf:resource="&cogat;CAO_00480"/>
        <skos:definition>the process of adopting an explanatory hypothesis; inferring the cause A as a possible explanation for the consequence B </skos:definition>
        <dc:Title>Abductive reasoning</dc:Title>
        <dc:Contributor>Corey White</dc:Contributor>
        <dc:Date>2011-08-10 13:41:26</dc:Date>
        <skos:prefLabel>Abductive reasoning</skos:prefLabel>
        <skos:hasTopConcept>Reasoning and Decision Making</skos:hasTopConcept>
        <skos:altLabel></skos:altLabel>
        <dc:identifier>trm_4a3fd79d096be</dc:identifier>
    </owl:Class>
    


    <!-- http://www.cognitiveatlas.org/ontology/cogat.owl#CAO_00102 -->

    <owl:Class rdf:about="&cogat;CAO_00102">
        <rdfs:label>Abstract analogy</rdfs:label>
        <rdfs:subClassOf rdf:resource="&cogat;CAO_00126"/>
        <skos:altLabel></skos:altLabel>
        <dc:identifier>trm_4a3fd79d096e3</dc:identifier>
        <dc:Contributor>Russ Poldrack</dc:Contributor>
        <skos:hasTopConcept>Reasoning and Decision Making</skos:hasTopConcept>
        <skos:prefLabel>Abstract analogy</skos:prefLabel>
        <skos:definition>high-level analogy that retains general information relevant to many specific instances</skos:definition>
        <dc:Date>2012-03-28 08:36:11</dc:Date>
        <dc:Title>Abstract analogy</dc:Title>
    </owl:Class>
    


    <!-- http://www.cognitiveatlas.org/ontology/cogat.owl#CAO_00103 -->

    <owl:Class rdf:about="&cogat;CAO_00103">
        <rdfs:label>Abstract knowledge</rdfs:label>
        <rdfs:subClassOf rdf:resource="&cogat;CAO_00371"/>
        <skos:hasTopConcept>Reasoning and Decision Making</skos:hasTopConcept>
        <dc:identifier>trm_4a3fd79d096f0</dc:identifier>
        <skos:definition>Knowledge that is general and not tied to a specific instance.</skos:definition>
        <skos:altLabel></skos:altLabel>
        <dc:Date>2012-03-28 08:36:29</dc:Date>
        <dc:Contributor>Russ Poldrack</dc:Contributor>
        <dc:Title>Abstract knowledge</dc:Title>
        <skos:prefLabel>Abstract knowledge</skos:prefLabel>
    </owl:Class>
    


    <!-- http://www.cognitiveatlas.org/ontology/cogat.owl#CAO_00104 -->

    <owl:Class rdf:about="&cogat;CAO_00104">
        <rdfs:label>Acoustic coding</rdfs:label>
        <rdfs:subClassOf rdf:resource="&cogat;CAO_00001"/>
        <rdfs:subClassOf>
            <owl:Restriction>
                <owl:onProperty rdf:resource="&ro;part_of"/>
                <owl:someValuesFrom rdf:resource="&cogat;CAO_00164"/>
            </owl:Restriction>
        </rdfs:subClassOf>
        <skos:definition>a type of short term memory coding that represents the acoustic properties of the signal</skos:definition>
        <dc:Title>Acoustic coding</dc:Title>
        <skos:hasTopConcept>Perception</skos:hasTopConcept>
        <skos:prefLabel>Acoustic coding</skos:prefLabel>
        <dc:identifier>trm_4a3fd79d096fc</dc:identifier>
        <skos:altLabel></skos:altLabel>
        <dc:Date>2011-08-10 13:52:52</dc:Date>
        <dc:Contributor>Corey White</dc:Contributor>
    </owl:Class>
    


    <!-- http://www.cognitiveatlas.org/ontology/cogat.owl#CAO_00105 -->

    <owl:Class rdf:about="&cogat;CAO_00105">
        <rdfs:label>Acoustic encoding</rdfs:label>
        <rdfs:subClassOf rdf:resource="&cogat;CAO_00001"/>
        <rdfs:subClassOf>
            <owl:Restriction>
                <owl:onProperty rdf:resource="&ro;part_of"/>
                <owl:someValuesFrom rdf:resource="&cogat;CAO_00163"/>
            </owl:Restriction>
        </rdfs:subClassOf>
        <rdfs:subClassOf>
            <owl:Restriction>
                <owl:onProperty rdf:resource="&ro;part_of"/>
                <owl:someValuesFrom rdf:resource="&cogat;CAO_00154"/>
            </owl:Restriction>
        </rdfs:subClassOf>
        <rdfs:subClassOf>
            <owl:Restriction>
                <owl:onProperty rdf:resource="&ro;part_of"/>
                <owl:someValuesFrom rdf:resource="&cogat;CAO_00164"/>
            </owl:Restriction>
        </rdfs:subClassOf>
        <skos:hasTopConcept>Perception</skos:hasTopConcept>
        <skos:prefLabel>Acoustic encoding</skos:prefLabel>
        <skos:definition>the processing and encoding of auditory input for storage and later retrieval.</skos:definition>
        <dc:Contributor>Russ Poldrack</dc:Contributor>
        <skos:altLabel></skos:altLabel>
        <dc:identifier>trm_4a3fd79d09707</dc:identifier>
        <dc:Date>2012-03-28 08:36:53</dc:Date>
        <dc:Title>Acoustic encoding</dc:Title>
    </owl:Class>
    


    <!-- http://www.cognitiveatlas.org/ontology/cogat.owl#CAO_00106 -->

    <owl:Class rdf:about="&cogat;CAO_00106">
        <rdfs:label>Acoustic phonetic processing</rdfs:label>
        <rdfs:subClassOf rdf:resource="&cogat;CAO_00164"/>
        <rdfs:subClassOf>
            <owl:Restriction>
                <owl:onProperty rdf:resource="&ro;part_of"/>
                <owl:someValuesFrom rdf:resource="&cogat;CAO_00535"/>
            </owl:Restriction>
        </rdfs:subClassOf>
        <rdfs:subClassOf>
            <owl:Restriction>
                <owl:onProperty rdf:resource="&ro;part_of"/>
                <owl:someValuesFrom rdf:resource="&cogat;CAO_00164"/>
            </owl:Restriction>
        </rdfs:subClassOf>
        <dc:Title>Acoustic phonetic processing</dc:Title>
        <dc:Date>2012-03-28 08:37:10</dc:Date>
        <dc:identifier>trm_4a3fd79d09713</dc:identifier>
        <skos:prefLabel>Acoustic phonetic processing</skos:prefLabel>
        <skos:definition>the cognitive ability to discriminate items on the basis of contrasts in sonorance, manner, place, or voicing in auditory stimuli. </skos:definition>
        <skos:altLabel></skos:altLabel>
        <skos:hasTopConcept>Language</skos:hasTopConcept>
        <dc:Contributor>Russ Poldrack</dc:Contributor>
    </owl:Class>
    


    <!-- http://www.cognitiveatlas.org/ontology/cogat.owl#CAO_00107 -->

    <owl:Class rdf:about="&cogat;CAO_00107">
        <rdfs:label>Acoustic processing</rdfs:label>
        <rdfs:subClassOf rdf:resource="&cogat;CAO_00001"/>
        <skos:prefLabel>Acoustic processing</skos:prefLabel>
        <skos:definition>the extraction of information from signals propagated undersea, in the atmosphere, or in the solid earth in the presence of acoustic noise.</skos:definition>
        <dc:Contributor>Russ Poldrack</dc:Contributor>
        <dc:Date>2012-03-28 08:37:24</dc:Date>
        <dc:identifier>trm_4a3fd79d0971e</dc:identifier>
        <dc:Title>Acoustic processing</dc:Title>
        <skos:hasTopConcept>Perception</skos:hasTopConcept>
        <skos:altLabel></skos:altLabel>
    </owl:Class>
    


    <!-- http://www.cognitiveatlas.org/ontology/cogat.owl#CAO_00109 -->

    <owl:Class rdf:about="&cogat;CAO_00109">
        <rdfs:label>Action</rdfs:label>
        <rdfs:subClassOf rdf:resource="&cogat;CAO_00001"/>
        <skos:hasTopConcept>Action</skos:hasTopConcept>
        <dc:Contributor>Russ Poldrack</dc:Contributor>
        <skos:prefLabel>Action</skos:prefLabel>
        <dc:Date>2012-03-28 08:39:58</dc:Date>
        <skos:definition>the bringing about of an alteration by force or through a natural agency; expression by means of attitude, voice, and gesture; a function of the body or one of its parts; an act of will; a thing done; the accomplishment of a thing usually over a period of time, in stages, or with the possibility of repetition.</skos:definition>
        <dc:Title>Action</dc:Title>
        <dc:identifier>trm_4a3fd79d09735</dc:identifier>
        <skos:altLabel></skos:altLabel>
    </owl:Class>
    


    <!-- http://www.cognitiveatlas.org/ontology/cogat.owl#CAO_00110 -->

    <owl:Class rdf:about="&cogat;CAO_00110">
        <rdfs:label>Activation</rdfs:label>
        <rdfs:subClassOf rdf:resource="&cogat;CAO_00001"/>
        <dc:Contributor>Russ Poldrack</dc:Contributor>
        <skos:altLabel></skos:altLabel>
        <skos:hasTopConcept></skos:hasTopConcept>
        <dc:identifier>trm_4a3fd79d09741</dc:identifier>
        <dc:Title>Activation</dc:Title>
        <skos:prefLabel>Activation</skos:prefLabel>
        <skos:definition>the relative engagement of a particular mental representation compared to other representations</skos:definition>
        <dc:Date>2012-03-28 08:41:03</dc:Date>
    </owl:Class>
    


    <!-- http://www.cognitiveatlas.org/ontology/cogat.owl#CAO_00111 -->

    <owl:Class rdf:about="&cogat;CAO_00111">
        <rdfs:label>Activation level</rdfs:label>
        <rdfs:subClassOf rdf:resource="&cogat;CAO_00001"/>
        <skos:altLabel></skos:altLabel>
        <dc:Title>Activation level</dc:Title>
        <dc:identifier>trm_4a3fd79d0974d</dc:identifier>
        <dc:Date>2011-08-11 08:26:14</dc:Date>
        <skos:definition>quantity or amount of activation</skos:definition>
        <skos:hasTopConcept></skos:hasTopConcept>
        <dc:Contributor>Corey White</dc:Contributor>
        <skos:prefLabel>Activation level</skos:prefLabel>
    </owl:Class>
    


    <!-- http://www.cognitiveatlas.org/ontology/cogat.owl#CAO_00112 -->

    <owl:Class rdf:about="&cogat;CAO_00112">
        <rdfs:label>Adaptation</rdfs:label>
        <rdfs:subClassOf rdf:resource="&cogat;CAO_00001"/>
        <dc:Contributor>Russ Poldrack</dc:Contributor>
        <skos:altLabel></skos:altLabel>
        <dc:Title>Adaptation</dc:Title>
        <dc:Date>2012-03-28 08:43:33</dc:Date>
        <skos:definition>adjustment to environmental conditions; adjustment of a sense organ to the intensity or quality of stimulation; modification of an organism or its parts that makes it more fit for existence under the conditions of its environment. </skos:definition>
        <dc:identifier>trm_4a3fd79d09758</dc:identifier>
        <skos:prefLabel>Adaptation</skos:prefLabel>
        <skos:hasTopConcept>Learning and Memory</skos:hasTopConcept>
    </owl:Class>
    


    <!-- http://www.cognitiveatlas.org/ontology/cogat.owl#CAO_00113 -->

    <owl:Class rdf:about="&cogat;CAO_00113">
        <rdfs:label>Adaptive control</rdfs:label>
        <rdfs:subClassOf rdf:resource="&cogat;CAO_00001"/>
        <skos:prefLabel>Adaptive control</skos:prefLabel>
        <skos:altLabel></skos:altLabel>
        <skos:hasTopConcept>Action</skos:hasTopConcept>
        <dc:identifier>trm_4a3fd79d09764</dc:identifier>
        <dc:Title>Adaptive control</dc:Title>
        <dc:Contributor>Russ Poldrack</dc:Contributor>
        <dc:Date>2012-03-28 08:46:12</dc:Date>
        <skos:definition>modifying the control law used by a controller to cope with the fact that the parameters of the system being controlled are slowly time-varying or uncertain.</skos:definition>
    </owl:Class>
    


    <!-- http://www.cognitiveatlas.org/ontology/cogat.owl#CAO_00114 -->

    <owl:Class rdf:about="&cogat;CAO_00114">
        <rdfs:label>Affect perception</rdfs:label>
        <rdfs:subClassOf rdf:resource="&cogat;CAO_00001"/>
        <dc:Title>Affect perception</dc:Title>
        <skos:altLabel></skos:altLabel>
        <dc:Date>2011-04-18 13:12:11</dc:Date>
        <skos:prefLabel>Affect perception</skos:prefLabel>
        <dc:Contributor>Natalie Picchetti</dc:Contributor>
        <skos:definition>The ability to understand a facial, vocal, or gestural behavior that serves as an indicator of emotion.</skos:definition>
        <dc:identifier>trm_4a3fd79d09770</dc:identifier>
        <skos:hasTopConcept>Perception</skos:hasTopConcept>
    </owl:Class>
    


    <!-- http://www.cognitiveatlas.org/ontology/cogat.owl#CAO_00115 -->

    <owl:Class rdf:about="&cogat;CAO_00115">
        <rdfs:label>Affect recognition</rdfs:label>
        <rdfs:subClassOf rdf:resource="&cogat;CAO_00001"/>
        <skos:prefLabel>Affect recognition</skos:prefLabel>
        <skos:definition>The ability to understand a physical expression that serves as an indicator of emotion.</skos:definition>
        <dc:Title>Affect recognition</dc:Title>
        <skos:hasTopConcept>Emotion</skos:hasTopConcept>
        <dc:identifier>trm_4a3fd79d0977b</dc:identifier>
        <skos:altLabel></skos:altLabel>
        <dc:Contributor>Russ Poldrack</dc:Contributor>
        <dc:Date>2012-03-28 08:46:31</dc:Date>
    </owl:Class>
    


    <!-- http://www.cognitiveatlas.org/ontology/cogat.owl#CAO_00116 -->

    <owl:Class rdf:about="&cogat;CAO_00116">
        <rdfs:label>Altruism</rdfs:label>
        <rdfs:subClassOf rdf:resource="&cogat;CAO_00001"/>
        <skos:altLabel>selflessness, empathy</skos:altLabel>
        <dc:Date>2012-02-22 08:12:58</dc:Date>
        <skos:definition>the motivation to help others without reward.</skos:definition>
        <dc:Title>Altruism</dc:Title>
        <skos:prefLabel>Altruism</skos:prefLabel>
        <dc:Contributor>Michael Sharman</dc:Contributor>
        <skos:hasTopConcept>Motivation</skos:hasTopConcept>
        <dc:identifier>trm_4a3fd79d097b4</dc:identifier>
    </owl:Class>
    


    <!-- http://www.cognitiveatlas.org/ontology/cogat.owl#CAO_00117 -->

    <owl:Class rdf:about="&cogat;CAO_00117">
        <rdfs:label>Altruistic motivation</rdfs:label>
        <rdfs:subClassOf rdf:resource="&cogat;CAO_00001"/>
        <skos:prefLabel>Altruistic motivation</skos:prefLabel>
        <dc:Contributor>Russ Poldrack</dc:Contributor>
        <skos:altLabel></skos:altLabel>
        <dc:identifier>trm_4a3fd79d097bf</dc:identifier>
        <dc:Title>Altruistic motivation</dc:Title>
        <skos:hasTopConcept>Motivation</skos:hasTopConcept>
        <skos:definition>A desire or need to help others driven by selflessness.</skos:definition>
        <dc:Date>2012-03-28 08:46:51</dc:Date>
    </owl:Class>
    


    <!-- http://www.cognitiveatlas.org/ontology/cogat.owl#CAO_00118 -->

    <owl:Class rdf:about="&cogat;CAO_00118">
        <rdfs:label>Alveolar</rdfs:label>
        <rdfs:subClassOf rdf:resource="&cogat;CAO_00001"/>
        <skos:definition>speech sound articulated with the tip of the tongue touching or near the teethridge.</skos:definition>
        <dc:Contributor>Russ Poldrack</dc:Contributor>
        <dc:Title>Alveolar</dc:Title>
        <dc:identifier>trm_4a3fd79d097cb</dc:identifier>
        <dc:Date>2012-03-28 08:47:21</dc:Date>
        <skos:hasTopConcept>Language</skos:hasTopConcept>
        <skos:prefLabel>Alveolar</skos:prefLabel>
        <skos:altLabel></skos:altLabel>
    </owl:Class>
    


    <!-- http://www.cognitiveatlas.org/ontology/cogat.owl#CAO_00119 -->

    <owl:Class rdf:about="&cogat;CAO_00119">
        <rdfs:label>Amodal representation</rdfs:label>
        <rdfs:subClassOf rdf:resource="&cogat;CAO_00397"/>
        <dc:Title>Amodal representation</dc:Title>
        <skos:hasTopConcept></skos:hasTopConcept>
        <dc:Date>2011-08-11 12:18:12</dc:Date>
        <dc:identifier>trm_4a3fd79d097d6</dc:identifier>
        <skos:prefLabel>Amodal representation</skos:prefLabel>
        <dc:Contributor>Corey White</dc:Contributor>
        <skos:definition>The way the brain codes multiple inputs such as words and pictures to integrate and create a larger conceptual idea; independent of a particular modality</skos:definition>
        <skos:altLabel></skos:altLabel>
    </owl:Class>
    


    <!-- http://www.cognitiveatlas.org/ontology/cogat.owl#CAO_00120 -->

    <owl:Class rdf:about="&cogat;CAO_00120">
        <rdfs:label>Analog representation</rdfs:label>
        <rdfs:subClassOf rdf:resource="&cogat;CAO_00001"/>
        <dc:Contributor>Brenda Gregory</dc:Contributor>
        <skos:altLabel></skos:altLabel>
        <dc:Date>2011-05-12 15:34:10</dc:Date>
        <skos:definition>a value or variable in analog form.</skos:definition>
        <skos:hasTopConcept></skos:hasTopConcept>
        <dc:identifier>trm_4a3fd79d097e2</dc:identifier>
        <skos:prefLabel>Analog representation</skos:prefLabel>
        <dc:Title>Analog representation</dc:Title>
    </owl:Class>
    


    <!-- http://www.cognitiveatlas.org/ontology/cogat.owl#CAO_00121 -->

    <owl:Class rdf:about="&cogat;CAO_00121">
        <rdfs:label>Analogical encoding</rdfs:label>
        <rdfs:subClassOf rdf:resource="&cogat;CAO_00001"/>
        <dc:Title>Analogical encoding</dc:Title>
        <skos:definition>No definition submitted yet</skos:definition>
        <dc:Date>2009-07-10 14:06:30</dc:Date>
        <skos:hasTopConcept></skos:hasTopConcept>
        <dc:Contributor>System Administrator</dc:Contributor>
        <skos:altLabel></skos:altLabel>
        <skos:prefLabel>Analogical encoding</skos:prefLabel>
        <dc:identifier>trm_4a3fd79d097ed</dc:identifier>
    </owl:Class>
    


    <!-- http://www.cognitiveatlas.org/ontology/cogat.owl#CAO_00122 -->

    <owl:Class rdf:about="&cogat;CAO_00122">
        <rdfs:label>Analogical inference</rdfs:label>
        <rdfs:subClassOf rdf:resource="&cogat;CAO_00346"/>
        <skos:definition>is the ability to reason by permitting the extension of knowledge of a target domain by virtue of its similarity to a base domain. The general procedure for analogical inference involves copying structure from the base to the target in which missing information is generated, and substitutions are made for items for which analogical correspondences have already been found. </skos:definition>
        <dc:Title>Analogical inference</dc:Title>
        <skos:hasTopConcept></skos:hasTopConcept>
        <dc:identifier>trm_4a3fd79d097f9</dc:identifier>
        <dc:Date>2011-04-18 10:44:14</dc:Date>
        <skos:prefLabel>Analogical inference</skos:prefLabel>
        <dc:Contributor>Natalie Picchetti</dc:Contributor>
        <skos:altLabel></skos:altLabel>
    </owl:Class>
    


    <!-- http://www.cognitiveatlas.org/ontology/cogat.owl#CAO_00123 -->

    <owl:Class rdf:about="&cogat;CAO_00123">
        <rdfs:label>Analogical problem solving</rdfs:label>
        <rdfs:subClassOf rdf:resource="&cogat;CAO_00001"/>
        <skos:altLabel></skos:altLabel>
        <dc:Contributor>Russ Poldrack</dc:Contributor>
        <skos:hasTopConcept>Reasoning and Decision Making</skos:hasTopConcept>
        <dc:Date>2012-03-28 08:48:34</dc:Date>
        <dc:Title>Analogical problem solving</dc:Title>
        <skos:definition>using principles or concepts from a well-understood situation to solve problems in a new domain or area</skos:definition>
        <dc:identifier>trm_4a3fd79d09804</dc:identifier>
        <skos:prefLabel>Analogical problem solving</skos:prefLabel>
    </owl:Class>
    


    <!-- http://www.cognitiveatlas.org/ontology/cogat.owl#CAO_00124 -->

    <owl:Class rdf:about="&cogat;CAO_00124">
        <rdfs:label>Analogical reasoning</rdfs:label>
        <rdfs:subClassOf rdf:resource="&cogat;CAO_00480"/>
        <skos:prefLabel>Analogical reasoning</skos:prefLabel>
        <skos:hasTopConcept>Reasoning and Decision Making</skos:hasTopConcept>
        <dc:Title>Analogical reasoning</dc:Title>
        <skos:altLabel></skos:altLabel>
        <skos:definition>a method of processing information that compares the similarities between new and understood concepts, then uses those similarities to gain understanding of the new concept; a form of inductive reasoning.</skos:definition>
        <dc:Date>2012-03-28 08:32:06</dc:Date>
        <dc:identifier>trm_4a3fd79d09810</dc:identifier>
        <dc:Contributor>Russ Poldrack</dc:Contributor>
    </owl:Class>
    


    <!-- http://www.cognitiveatlas.org/ontology/cogat.owl#CAO_00125 -->

    <owl:Class rdf:about="&cogat;CAO_00125">
        <rdfs:label>Analogical transfer</rdfs:label>
        <rdfs:subClassOf rdf:resource="&cogat;CAO_00001"/>
        <dc:identifier>trm_4a3fd79d0981b</dc:identifier>
        <dc:Title>Analogical transfer</dc:Title>
        <skos:altLabel></skos:altLabel>
        <dc:Contributor>Russ Poldrack</dc:Contributor>
        <skos:hasTopConcept>Reasoning and Decision Making</skos:hasTopConcept>
        <skos:prefLabel>Analogical transfer</skos:prefLabel>
        <skos:definition>The transfer of knowledge from one situation to another by finding a set of one-to-one correspondences between aspects of one body of information and aspects of another.</skos:definition>
        <dc:Date>2012-03-28 08:48:50</dc:Date>
    </owl:Class>
    


    <!-- http://www.cognitiveatlas.org/ontology/cogat.owl#CAO_00126 -->

    <owl:Class rdf:about="&cogat;CAO_00126">
        <rdfs:label>Analogy</rdfs:label>
        <rdfs:subClassOf rdf:resource="&cogat;CAO_00346"/>
        <skos:altLabel></skos:altLabel>
        <dc:identifier>trm_4a3fd79d09827</dc:identifier>
        <dc:Contributor>Brenda Gregory</dc:Contributor>
        <skos:hasTopConcept></skos:hasTopConcept>
        <dc:Title>Analogy</dc:Title>
        <dc:Date>2011-05-10 15:01:10</dc:Date>
        <skos:prefLabel>Analogy</skos:prefLabel>
        <skos:definition>inference that if two or more things agree with one another in some respects they will probably agree in others; resemblance in some particulars between things otherwise unlike; correspondence between the members of pairs or sets of linguistic forms that serves as a basis for the creation of another form; correspondence in function between anatomical parts of different structure and origin.</skos:definition>
    </owl:Class>
    


    <!-- http://www.cognitiveatlas.org/ontology/cogat.owl#CAO_00127 -->

    <owl:Class rdf:about="&cogat;CAO_00127">
        <rdfs:label>Anchoring</rdfs:label>
        <rdfs:subClassOf rdf:resource="&cogat;CAO_00001"/>
        <dc:Title>Anchoring</dc:Title>
        <skos:prefLabel>Anchoring</skos:prefLabel>
        <skos:definition>a cognitive bias that describes the common human tendency to rely too heavily, or and#34;anchor,and#34; on one trait or piece of information when making decisions.</skos:definition>
        <skos:altLabel></skos:altLabel>
        <dc:identifier>trm_4a3fd79d09833</dc:identifier>
        <dc:Date>2011-04-09 08:03:06</dc:Date>
        <dc:Contributor>Russ Poldrack</dc:Contributor>
        <skos:hasTopConcept>Reasoning and Decision Making</skos:hasTopConcept>
    </owl:Class>
    


    <!-- http://www.cognitiveatlas.org/ontology/cogat.owl#CAO_00128 -->

    <owl:Class rdf:about="&cogat;CAO_00128">
        <rdfs:label>Anomaly detection</rdfs:label>
        <rdfs:subClassOf rdf:resource="&cogat;CAO_00001"/>
        <dc:Contributor>Brenda Gregory</dc:Contributor>
        <skos:altLabel></skos:altLabel>
        <dc:Date>2011-05-03 13:56:48</dc:Date>
        <skos:definition>detecting patterns in a given data set that do not conform to an established normal behavior. </skos:definition>
        <dc:Title>Anomaly detection</dc:Title>
        <skos:prefLabel>Anomaly detection</skos:prefLabel>
        <dc:identifier>trm_4a3fd79d0983e</dc:identifier>
        <skos:hasTopConcept></skos:hasTopConcept>
    </owl:Class>
    


    <!-- http://www.cognitiveatlas.org/ontology/cogat.owl#CAO_00129 -->

    <owl:Class rdf:about="&cogat;CAO_00129">
        <rdfs:label>Anticipation</rdfs:label>
        <rdfs:subClassOf rdf:resource="&cogat;CAO_00001"/>
        <skos:altLabel>intuition, foreknowledge, prescience, foresight, prediction, imaginative speculation</skos:altLabel>
        <dc:Title>Anticipation</dc:Title>
        <skos:definition>prior expectation of an event or occurrence, sometimes accompanied by an emotional reaction</skos:definition>
        <skos:hasTopConcept></skos:hasTopConcept>
        <dc:Contributor>Michael Sharman</dc:Contributor>
        <dc:identifier>trm_4a3fd79d09849</dc:identifier>
        <dc:Date>2012-02-22 08:10:30</dc:Date>
        <skos:prefLabel>Anticipation</skos:prefLabel>
    </owl:Class>
    


    <!-- http://www.cognitiveatlas.org/ontology/cogat.owl#CAO_00130 -->

    <owl:Class rdf:about="&cogat;CAO_00130">
        <rdfs:label>Apparent motion</rdfs:label>
        <rdfs:subClassOf rdf:resource="&cogat;CAO_00001"/>
        <skos:prefLabel>Apparent motion</skos:prefLabel>
        <dc:identifier>trm_4a3fd79d09855</dc:identifier>
        <dc:Contributor>Russ Poldrack</dc:Contributor>
        <skos:altLabel>apparent movement</skos:altLabel>
        <dc:Date>2012-03-28 08:53:06</dc:Date>
        <skos:hasTopConcept>Perception</skos:hasTopConcept>
        <dc:Title>Apparent motion</dc:Title>
        <skos:definition>The illusory perception that movement is occurring in one or more static images.</skos:definition>
    </owl:Class>
    


    <!-- http://www.cognitiveatlas.org/ontology/cogat.owl#CAO_00132 -->

    <owl:Class rdf:about="&cogat;CAO_00132">
        <rdfs:label>Apperception</rdfs:label>
        <rdfs:subClassOf rdf:resource="&cogat;CAO_00001"/>
        <skos:altLabel></skos:altLabel>
        <dc:Contributor>Brenda Gregory</dc:Contributor>
        <dc:Title>Apperception</dc:Title>
        <dc:Date>2011-05-18 09:47:09</dc:Date>
        <skos:definition>the process by which new experience is assimilated to and transformed by the residuum of past experience of an individual to form a new whole.</skos:definition>
        <skos:hasTopConcept></skos:hasTopConcept>
        <skos:prefLabel>Apperception</skos:prefLabel>
        <dc:identifier>trm_4a3fd79d0986c</dc:identifier>
    </owl:Class>
    


    <!-- http://www.cognitiveatlas.org/ontology/cogat.owl#CAO_00133 -->

    <owl:Class rdf:about="&cogat;CAO_00133">
        <rdfs:label>Appetitive motivation</rdfs:label>
        <rdfs:subClassOf rdf:resource="&cogat;CAO_00001"/>
        <dc:Title>Appetitive motivation</dc:Title>
        <skos:hasTopConcept>Motivation</skos:hasTopConcept>
        <skos:prefLabel>Appetitive motivation</skos:prefLabel>
        <dc:Date>2012-03-28 08:53:31</dc:Date>
        <skos:altLabel></skos:altLabel>
        <dc:identifier>trm_4a3fd79d09877</dc:identifier>
        <dc:Contributor>Russ Poldrack</dc:Contributor>
        <skos:definition>behavior directed toward goals that are usually associated with positive hedonic processes.  </skos:definition>
    </owl:Class>
    


    <!-- http://www.cognitiveatlas.org/ontology/cogat.owl#CAO_00134 -->

    <owl:Class rdf:about="&cogat;CAO_00134">
        <rdfs:label>Arousal</rdfs:label>
        <rdfs:subClassOf rdf:resource="&cogat;CAO_00001"/>
        <dc:Date>2012-03-28 08:54:29</dc:Date>
        <dc:Contributor>Russ Poldrack</dc:Contributor>
        <skos:prefLabel>Arousal</skos:prefLabel>
        <skos:hasTopConcept>Emotion</skos:hasTopConcept>
        <skos:altLabel></skos:altLabel>
        <dc:identifier>trm_4a3fd79d09883</dc:identifier>
        <dc:Title>Arousal</dc:Title>
        <skos:definition>physiological activation or readiness for activity</skos:definition>
    </owl:Class>
    


    <!-- http://www.cognitiveatlas.org/ontology/cogat.owl#CAO_00135 -->

    <owl:Class rdf:about="&cogat;CAO_00135">
        <rdfs:label>Articulation</rdfs:label>
        <rdfs:subClassOf rdf:resource="&cogat;CAO_00001"/>
        <skos:definition>the act of vocally producing an utterance or expression</skos:definition>
        <skos:altLabel></skos:altLabel>
        <dc:Title>Articulation</dc:Title>
        <skos:prefLabel>Articulation</skos:prefLabel>
        <skos:hasTopConcept>Language</skos:hasTopConcept>
        <dc:Date>2012-03-28 08:54:59</dc:Date>
        <dc:identifier>trm_4a3fd79d0988f</dc:identifier>
        <dc:Contributor>Russ Poldrack</dc:Contributor>
    </owl:Class>
    


    <!-- http://www.cognitiveatlas.org/ontology/cogat.owl#CAO_00136 -->

    <owl:Class rdf:about="&cogat;CAO_00136">
        <rdfs:label>Articulatory planning</rdfs:label>
        <rdfs:subClassOf rdf:resource="&cogat;CAO_00001"/>
        <rdfs:subClassOf>
            <owl:Restriction>
                <owl:onProperty rdf:resource="&ro;part_of"/>
                <owl:someValuesFrom rdf:resource="&cogat;CAO_00537"/>
            </owl:Restriction>
        </rdfs:subClassOf>
        <dc:Contributor>Natalie Picchetti</dc:Contributor>
        <skos:altLabel></skos:altLabel>
        <skos:definition>The action of coordinating complex tongue and mouth movements in order to produce sound. </skos:definition>
        <skos:prefLabel>Articulatory planning</skos:prefLabel>
        <dc:identifier>trm_4a3fd79d0989a</dc:identifier>
        <dc:Title>Articulatory planning</dc:Title>
        <skos:hasTopConcept>Language</skos:hasTopConcept>
        <dc:Date>2011-04-18 12:48:34</dc:Date>
    </owl:Class>
    


    <!-- http://www.cognitiveatlas.org/ontology/cogat.owl#CAO_00137 -->

    <owl:Class rdf:about="&cogat;CAO_00137">
        <rdfs:label>Articulatory rehearsal</rdfs:label>
        <rdfs:subClassOf rdf:resource="&cogat;CAO_00666"/>
        <rdfs:subClassOf>
            <owl:Restriction>
                <owl:onProperty rdf:resource="&ro;part_of"/>
                <owl:someValuesFrom rdf:resource="&cogat;CAO_00667"/>
            </owl:Restriction>
        </rdfs:subClassOf>
        <skos:definition>the process of subvocally repeating material that is to be stored in memory.  </skos:definition>
        <dc:identifier>trm_4a3fd79d098a6</dc:identifier>
        <skos:hasTopConcept>Learning and Memory</skos:hasTopConcept>
        <dc:Contributor>Natalie Picchetti</dc:Contributor>
        <dc:Title>Articulatory rehearsal</dc:Title>
        <dc:Date>2010-12-31 23:34:14</dc:Date>
        <skos:altLabel></skos:altLabel>
        <skos:prefLabel>Articulatory rehearsal</skos:prefLabel>
    </owl:Class>
    


    <!-- http://www.cognitiveatlas.org/ontology/cogat.owl#CAO_00138 -->

    <owl:Class rdf:about="&cogat;CAO_00138">
        <rdfs:label>Assimilation</rdfs:label>
        <rdfs:subClassOf rdf:resource="&cogat;CAO_00001"/>
        <rdfs:subClassOf>
            <owl:Restriction>
                <owl:onProperty rdf:resource="&ro;part_of"/>
                <owl:someValuesFrom rdf:resource="&cogat;CAO_00377"/>
            </owl:Restriction>
        </rdfs:subClassOf>
        <dc:Title>Assimilation</dc:Title>
        <dc:identifier>trm_4a3fd79d098b2</dc:identifier>
        <skos:hasTopConcept></skos:hasTopConcept>
        <skos:prefLabel>Assimilation</skos:prefLabel>
        <skos:altLabel></skos:altLabel>
        <skos:definition>the process of receiving new facts or of responding to new situations in conformity with what is already available to consciousness.</skos:definition>
        <dc:Contributor>Brenda Gregory</dc:Contributor>
        <dc:Date>2011-05-04 11:00:43</dc:Date>
    </owl:Class>
    


    <!-- http://www.cognitiveatlas.org/ontology/cogat.owl#CAO_00139 -->

    <owl:Class rdf:about="&cogat;CAO_00139">
        <rdfs:label>Association</rdfs:label>
        <rdfs:subClassOf rdf:resource="&cogat;CAO_00001"/>
        <rdfs:subClassOf>
            <owl:Restriction>
                <owl:onProperty rdf:resource="&ro;part_of"/>
                <owl:someValuesFrom rdf:resource="&cogat;CAO_00394"/>
            </owl:Restriction>
        </rdfs:subClassOf>
        <skos:altLabel></skos:altLabel>
        <dc:identifier>trm_4a3fd79d098bd</dc:identifier>
        <skos:prefLabel>Association</skos:prefLabel>
        <skos:definition>the process of forming mental connections or bonds between sensations, ideas, or memories.</skos:definition>
        <dc:Contributor>Russ Poldrack</dc:Contributor>
        <dc:Title>Association</dc:Title>
        <dc:Date>2012-03-28 08:55:56</dc:Date>
        <skos:hasTopConcept></skos:hasTopConcept>
    </owl:Class>
    


    <!-- http://www.cognitiveatlas.org/ontology/cogat.owl#CAO_00140 -->

    <owl:Class rdf:about="&cogat;CAO_00140">
        <rdfs:label>Association learning</rdfs:label>
        <rdfs:subClassOf rdf:resource="&cogat;CAO_00377"/>
        <rdfs:subClassOf>
            <owl:Restriction>
                <owl:onProperty rdf:resource="&ro;part_of"/>
                <owl:someValuesFrom rdf:resource="&cogat;CAO_00351"/>
            </owl:Restriction>
        </rdfs:subClassOf>
        <dc:identifier>trm_4a3fd79d098c9</dc:identifier>
        <dc:Contributor>Russ Poldrack</dc:Contributor>
        <skos:altLabel></skos:altLabel>
        <skos:definition>learning process in which two or more items or concepts become associated with each other; often used in relation to learned stimulus-response associations</skos:definition>
        <dc:Title>Association learning</dc:Title>
        <skos:hasTopConcept>Learning and Memory</skos:hasTopConcept>
        <dc:Date>2012-03-28 08:56:11</dc:Date>
        <skos:prefLabel>Association learning</skos:prefLabel>
    </owl:Class>
    


    <!-- http://www.cognitiveatlas.org/ontology/cogat.owl#CAO_00141 -->

    <owl:Class rdf:about="&cogat;CAO_00141">
        <rdfs:label>Attachment</rdfs:label>
        <rdfs:subClassOf rdf:resource="&cogat;CAO_00001"/>
        <dc:Date>2012-03-28 08:56:43</dc:Date>
        <skos:definition>a social connection between individuals</skos:definition>
        <dc:Contributor>Russ Poldrack</dc:Contributor>
        <skos:prefLabel>Attachment</skos:prefLabel>
        <dc:Title>Attachment</dc:Title>
        <dc:identifier>trm_4a3fd79d098e0</dc:identifier>
        <skos:hasTopConcept>Social Function</skos:hasTopConcept>
        <skos:altLabel></skos:altLabel>
    </owl:Class>
    


    <!-- http://www.cognitiveatlas.org/ontology/cogat.owl#CAO_00142 -->

    <owl:Class rdf:about="&cogat;CAO_00142">
        <rdfs:label>Attended channel</rdfs:label>
        <rdfs:subClassOf rdf:resource="&cogat;CAO_00001"/>
        <dc:identifier>trm_4a3fd79d098eb</dc:identifier>
        <skos:altLabel></skos:altLabel>
        <dc:Title>Attended channel</dc:Title>
        <skos:definition>the particular input, out of two or more, that is consciously perceived due to attention.  </skos:definition>
        <skos:hasTopConcept></skos:hasTopConcept>
        <dc:Contributor>Corey White</dc:Contributor>
        <skos:prefLabel>Attended channel</skos:prefLabel>
        <dc:Date>2011-08-15 07:58:43</dc:Date>
    </owl:Class>
    


    <!-- http://www.cognitiveatlas.org/ontology/cogat.owl#CAO_00143 -->

    <owl:Class rdf:about="&cogat;CAO_00143">
        <rdfs:label>Attended stimulus</rdfs:label>
        <rdfs:subClassOf rdf:resource="&cogat;CAO_00001"/>
        <dc:identifier>trm_4a3fd79d098f7</dc:identifier>
        <skos:definition>the specific object in the environment on which attention is focused.</skos:definition>
        <skos:hasTopConcept></skos:hasTopConcept>
        <skos:altLabel></skos:altLabel>
        <dc:Date>2011-08-15 08:04:46</dc:Date>
        <skos:prefLabel>Attended stimulus</skos:prefLabel>
        <dc:Title>Attended stimulus</dc:Title>
        <dc:Contributor>Corey White</dc:Contributor>
    </owl:Class>
    


    <!-- http://www.cognitiveatlas.org/ontology/cogat.owl#CAO_00144 -->

    <owl:Class rdf:about="&cogat;CAO_00144">
        <rdfs:label>Attention</rdfs:label>
        <rdfs:subClassOf rdf:resource="&cogat;CAO_00670"/>
        <skos:definition>the cognitive process of selectively concentrating on one aspect of the environment while ignoring other things.</skos:definition>
        <skos:hasTopConcept>Attention</skos:hasTopConcept>
        <dc:Title>Attention</dc:Title>
        <dc:Date>2011-04-28 16:11:01</dc:Date>
        <skos:altLabel></skos:altLabel>
        <skos:prefLabel>Attention</skos:prefLabel>
        <dc:identifier>trm_4a3fd79d09902</dc:identifier>
        <dc:Contributor>Brenda Gregory</dc:Contributor>
    </owl:Class>
    


    <!-- http://www.cognitiveatlas.org/ontology/cogat.owl#CAO_00145 -->

    <owl:Class rdf:about="&cogat;CAO_00145">
        <rdfs:label>Attention capacity</rdfs:label>
        <rdfs:subClassOf rdf:resource="&cogat;CAO_00001"/>
        <rdfs:subClassOf>
            <owl:Restriction>
                <owl:onProperty rdf:resource="&ro;part_of"/>
                <owl:someValuesFrom rdf:resource="&cogat;CAO_00144"/>
            </owl:Restriction>
        </rdfs:subClassOf>
        <dc:Date>2012-03-28 08:58:18</dc:Date>
        <dc:identifier>trm_4a3fd79d0990e</dc:identifier>
        <skos:prefLabel>Attention capacity</skos:prefLabel>
        <skos:altLabel></skos:altLabel>
        <dc:Contributor>Russ Poldrack</dc:Contributor>
        <skos:hasTopConcept>Attention</skos:hasTopConcept>
        <dc:Title>Attention capacity</dc:Title>
        <skos:definition>refers to the extent that one can allocate their processing resources.</skos:definition>
    </owl:Class>
    


    <!-- http://www.cognitiveatlas.org/ontology/cogat.owl#CAO_00146 -->

    <owl:Class rdf:about="&cogat;CAO_00146">
        <rdfs:label>Attentional effort</rdfs:label>
        <rdfs:subClassOf rdf:resource="&cogat;CAO_00001"/>
        <rdfs:subClassOf>
            <owl:Restriction>
                <owl:onProperty rdf:resource="&ro;part_of"/>
                <owl:someValuesFrom rdf:resource="&cogat;CAO_00205"/>
            </owl:Restriction>
        </rdfs:subClassOf>
        <skos:definition>a motivated activation of attention systems in order to stabilize or recover attentional performance in response to the detection of errors and reward loss or, more generally, deteriorating attentional performance; amount of attentional resources needed for a particular situation</skos:definition>
        <dc:Title>Attentional effort</dc:Title>
        <dc:Date>2012-03-28 08:58:32</dc:Date>
        <skos:altLabel></skos:altLabel>
        <skos:prefLabel>Attentional effort</skos:prefLabel>
        <skos:hasTopConcept>Attention</skos:hasTopConcept>
        <dc:Contributor>Russ Poldrack</dc:Contributor>
        <dc:identifier>trm_4a3fd79d09919</dc:identifier>
    </owl:Class>
    


    <!-- http://www.cognitiveatlas.org/ontology/cogat.owl#CAO_00148 -->

    <owl:Class rdf:about="&cogat;CAO_00148">
        <rdfs:label>Attentional state</rdfs:label>
        <rdfs:subClassOf rdf:resource="&cogat;CAO_00001"/>
        <dc:Title>Attentional state</dc:Title>
        <skos:definition>referring to amount of attentional resources being engaged;  a relaxed attentional state requires little attentional effort, whereas an alert, focused attentional state requires more</skos:definition>
        <dc:Date>2012-03-28 08:59:35</dc:Date>
        <skos:prefLabel>Attentional state</skos:prefLabel>
        <dc:Contributor>Russ Poldrack</dc:Contributor>
        <dc:identifier>trm_4a3fd79d09930</dc:identifier>
        <skos:altLabel></skos:altLabel>
        <skos:hasTopConcept>Attention</skos:hasTopConcept>
    </owl:Class>
    


    <!-- http://www.cognitiveatlas.org/ontology/cogat.owl#CAO_00149 -->

    <owl:Class rdf:about="&cogat;CAO_00149">
        <rdfs:label>Attitude</rdfs:label>
        <rdfs:subClassOf rdf:resource="&cogat;CAO_00001"/>
        <dc:Title>Attitude</dc:Title>
        <skos:hasTopConcept></skos:hasTopConcept>
        <dc:identifier>trm_4a3fd79d09947</dc:identifier>
        <skos:definition>a mental position with regard to a fact or state</skos:definition>
        <dc:Date>2012-03-28 09:00:01</dc:Date>
        <skos:prefLabel>Attitude</skos:prefLabel>
        <dc:Contributor>Russ Poldrack</dc:Contributor>
        <skos:altLabel></skos:altLabel>
    </owl:Class>
    


    <!-- http://www.cognitiveatlas.org/ontology/cogat.owl#CAO_00150 -->

    <owl:Class rdf:about="&cogat;CAO_00150">
        <rdfs:label>Audiovisual perception</rdfs:label>
        <rdfs:subClassOf rdf:resource="&cogat;CAO_00437"/>
        <dc:Date>2011-04-01 12:44:06</dc:Date>
        <dc:identifier>trm_4a3fd79d09953</dc:identifier>
        <dc:Title>Audiovisual perception</dc:Title>
        <skos:definition>a single unified awareness derived from the integration of auditory and visual sensory processes when a audiovisual stimulus is present.  </skos:definition>
        <dc:Contributor>Natalie Picchetti</dc:Contributor>
        <skos:prefLabel>Audiovisual perception</skos:prefLabel>
        <skos:altLabel></skos:altLabel>
        <skos:hasTopConcept>Perception</skos:hasTopConcept>
    </owl:Class>
    


    <!-- http://www.cognitiveatlas.org/ontology/cogat.owl#CAO_00151 -->

    <owl:Class rdf:about="&cogat;CAO_00151">
        <rdfs:label>Audition</rdfs:label>
        <rdfs:subClassOf rdf:resource="&cogat;CAO_00001"/>
        <rdfs:subClassOf>
            <owl:Restriction>
                <owl:onProperty rdf:resource="&ro;part_of"/>
                <owl:someValuesFrom rdf:resource="&cogat;CAO_00437"/>
            </owl:Restriction>
        </rdfs:subClassOf>
        <skos:prefLabel>Audition</skos:prefLabel>
        <skos:definition>the sense or act of hearing.</skos:definition>
        <skos:altLabel>auditory</skos:altLabel>
        <dc:Title>Audition</dc:Title>
        <dc:Date>2012-03-28 09:20:29</dc:Date>
        <dc:identifier>trm_4a3fd79d0995e</dc:identifier>
        <skos:hasTopConcept>Perception</skos:hasTopConcept>
        <dc:Contributor>Russ Poldrack</dc:Contributor>
    </owl:Class>
    


    <!-- http://www.cognitiveatlas.org/ontology/cogat.owl#CAO_00153 -->

    <owl:Class rdf:about="&cogat;CAO_00153">
        <rdfs:label>Auditory attention</rdfs:label>
        <rdfs:subClassOf rdf:resource="&cogat;CAO_00144"/>
        <dc:Title>Auditory attention</dc:Title>
        <skos:prefLabel>Auditory attention</skos:prefLabel>
        <dc:Date>2012-03-28 09:22:16</dc:Date>
        <dc:identifier>trm_4a3fd79d09a10</dc:identifier>
        <skos:altLabel></skos:altLabel>
        <skos:hasTopConcept>Attention</skos:hasTopConcept>
        <skos:definition>is the cognitive process of selectively concentrating on one auditory stream in the environment while ignoring others. </skos:definition>
        <dc:Contributor>Russ Poldrack</dc:Contributor>
    </owl:Class>
    


    <!-- http://www.cognitiveatlas.org/ontology/cogat.owl#CAO_00154 -->

    <owl:Class rdf:about="&cogat;CAO_00154">
        <rdfs:label>Auditory coding</rdfs:label>
        <rdfs:subClassOf rdf:resource="&cogat;CAO_00001"/>
        <rdfs:subClassOf>
            <owl:Restriction>
                <owl:onProperty rdf:resource="&ro;part_of"/>
                <owl:someValuesFrom rdf:resource="&cogat;CAO_00164"/>
            </owl:Restriction>
        </rdfs:subClassOf>
        <dc:Contributor>Brenda Gregory</dc:Contributor>
        <skos:prefLabel>Auditory coding</skos:prefLabel>
        <dc:Date>2011-04-19 12:16:40</dc:Date>
        <skos:hasTopConcept></skos:hasTopConcept>
        <dc:identifier>trm_4a3fd79d09a3d</dc:identifier>
        <dc:Title>Auditory coding</dc:Title>
        <skos:altLabel></skos:altLabel>
        <skos:definition>processing and encoding of sound, words, and all other auditory input for storage and later retrieval. According to Baddeley, processing of auditory information is aided by the concept of the phonological loop, which allows input within our echoic memory.</skos:definition>
    </owl:Class>
    


    <!-- http://www.cognitiveatlas.org/ontology/cogat.owl#CAO_00155 -->

    <owl:Class rdf:about="&cogat;CAO_00155">
        <rdfs:label>Auditory encoding</rdfs:label>
        <rdfs:subClassOf rdf:resource="&cogat;CAO_00001"/>
        <rdfs:subClassOf>
            <owl:Restriction>
                <owl:onProperty rdf:resource="&ro;part_of"/>
                <owl:someValuesFrom rdf:resource="&cogat;CAO_00642"/>
            </owl:Restriction>
        </rdfs:subClassOf>
        <dc:identifier>trm_4a3fd79d09a49</dc:identifier>
        <skos:hasTopConcept>Learning and Memory</skos:hasTopConcept>
        <skos:prefLabel>Auditory encoding</skos:prefLabel>
        <dc:Contributor>Natalie Picchetti</dc:Contributor>
        <skos:altLabel></skos:altLabel>
        <skos:definition>the process of storing auditory information in memory.  </skos:definition>
        <dc:Date>2010-12-31 23:48:05</dc:Date>
        <dc:Title>Auditory encoding</dc:Title>
    </owl:Class>
    


    <!-- http://www.cognitiveatlas.org/ontology/cogat.owl#CAO_00156 -->

    <owl:Class rdf:about="&cogat;CAO_00156">
        <rdfs:label>Auditory feedback</rdfs:label>
        <rdfs:subClassOf rdf:resource="&cogat;CAO_00303"/>
        <skos:definition>is provided by auditory stimulation in response to specific behavior. The feedback may be used to amend subsequent behavior, cognition, perception or performance. </skos:definition>
        <dc:identifier>trm_4a3fd79d09a55</dc:identifier>
        <dc:Title>Auditory feedback</dc:Title>
        <dc:Contributor>Natalie Picchetti</dc:Contributor>
        <dc:Date>2011-04-11 15:55:30</dc:Date>
        <skos:hasTopConcept></skos:hasTopConcept>
        <skos:altLabel></skos:altLabel>
        <skos:prefLabel>Auditory feedback</skos:prefLabel>
    </owl:Class>
    


    <!-- http://www.cognitiveatlas.org/ontology/cogat.owl#CAO_00157 -->

    <owl:Class rdf:about="&cogat;CAO_00157">
        <rdfs:label>Auditory grouping</rdfs:label>
        <rdfs:subClassOf rdf:resource="&cogat;CAO_00001"/>
        <rdfs:subClassOf>
            <owl:Restriction>
                <owl:onProperty rdf:resource="&ro;part_of"/>
                <owl:someValuesFrom rdf:resource="&cogat;CAO_00164"/>
            </owl:Restriction>
        </rdfs:subClassOf>
        <skos:altLabel></skos:altLabel>
        <dc:Contributor>Russ Poldrack</dc:Contributor>
        <dc:identifier>trm_4a3fd79d09a61</dc:identifier>
        <dc:Date>2012-03-28 09:23:16</dc:Date>
        <skos:prefLabel>Auditory grouping</skos:prefLabel>
        <skos:definition>joining disparate sounds together into one percept; assessing which acoustic streams belong together</skos:definition>
        <skos:hasTopConcept>Perception</skos:hasTopConcept>
        <dc:Title>Auditory grouping</dc:Title>
    </owl:Class>
    


    <!-- http://www.cognitiveatlas.org/ontology/cogat.owl#CAO_00158 -->

    <owl:Class rdf:about="&cogat;CAO_00158">
        <rdfs:label>Auditory imagery</rdfs:label>
        <rdfs:subClassOf rdf:resource="&cogat;CAO_00001"/>
        <dc:identifier>trm_4a3fd79d09a6c</dc:identifier>
        <dc:Date>2011-05-12 15:25:21</dc:Date>
        <skos:altLabel></skos:altLabel>
        <skos:prefLabel>Auditory imagery</skos:prefLabel>
        <dc:Title>Auditory imagery</dc:Title>
        <skos:hasTopConcept></skos:hasTopConcept>
        <skos:definition>the subjective experience of hearing in the absence of auditory stimulation.</skos:definition>
        <dc:Contributor>Brenda Gregory</dc:Contributor>
    </owl:Class>
    


    <!-- http://www.cognitiveatlas.org/ontology/cogat.owl#CAO_00159 -->

    <owl:Class rdf:about="&cogat;CAO_00159">
        <rdfs:label>Auditory learning</rdfs:label>
        <rdfs:subClassOf rdf:resource="&cogat;CAO_00001"/>
        <dc:Contributor>Russ Poldrack</dc:Contributor>
        <skos:altLabel></skos:altLabel>
        <skos:prefLabel>Auditory learning</skos:prefLabel>
        <dc:Date>2012-03-28 09:23:55</dc:Date>
        <dc:Title>Auditory learning</dc:Title>
        <skos:hasTopConcept>Learning and Memory</skos:hasTopConcept>
        <dc:identifier>trm_4a3fd79d09a78</dc:identifier>
        <skos:definition>learning of auditorily presented information</skos:definition>
    </owl:Class>
    


    <!-- http://www.cognitiveatlas.org/ontology/cogat.owl#CAO_00160 -->

    <owl:Class rdf:about="&cogat;CAO_00160">
        <rdfs:label>Auditory lexical access</rdfs:label>
        <rdfs:subClassOf rdf:resource="&cogat;CAO_00001"/>
        <rdfs:subClassOf>
            <owl:Restriction>
                <owl:onProperty rdf:resource="&ro;part_of"/>
                <owl:someValuesFrom rdf:resource="&cogat;CAO_00622"/>
            </owl:Restriction>
        </rdfs:subClassOf>
        <skos:hasTopConcept>Language</skos:hasTopConcept>
        <skos:prefLabel>Auditory lexical access</skos:prefLabel>
        <skos:definition>The process by which the basic sound-meaning connections of language, i.e., lexical entries, are activated. </skos:definition>
        <dc:Date>2011-04-19 12:17:49</dc:Date>
        <dc:Title>Auditory lexical access</dc:Title>
        <dc:identifier>trm_4a3fd79d09a84</dc:identifier>
        <dc:Contributor>Brenda Gregory</dc:Contributor>
        <skos:altLabel></skos:altLabel>
    </owl:Class>
    


    <!-- http://www.cognitiveatlas.org/ontology/cogat.owl#CAO_00161 -->

    <owl:Class rdf:about="&cogat;CAO_00161">
        <rdfs:label>Auditory localization</rdfs:label>
        <rdfs:subClassOf rdf:resource="&cogat;CAO_00001"/>
        <skos:definition>a listenerand#39;s ability to identify the location or origin of a detected sound.</skos:definition>
        <skos:hasTopConcept>Perception</skos:hasTopConcept>
        <dc:Title>Auditory localization</dc:Title>
        <skos:altLabel></skos:altLabel>
        <skos:prefLabel>Auditory localization</skos:prefLabel>
        <dc:Contributor>Russ Poldrack</dc:Contributor>
        <dc:Date>2012-03-28 09:24:09</dc:Date>
        <dc:identifier>trm_4a3fd79d09a8f</dc:identifier>
    </owl:Class>
    


    <!-- http://www.cognitiveatlas.org/ontology/cogat.owl#CAO_00162 -->

    <owl:Class rdf:about="&cogat;CAO_00162">
        <rdfs:label>Auditory masking</rdfs:label>
        <rdfs:subClassOf rdf:resource="&cogat;CAO_00001"/>
        <skos:definition>the perception of one sound is affected by the presence of another sound; presenting a sound to interfere with or terminate a target sound</skos:definition>
        <dc:Title>Auditory masking</dc:Title>
        <skos:altLabel></skos:altLabel>
        <dc:Contributor>Russ Poldrack</dc:Contributor>
        <dc:identifier>trm_4a3fd79d09a9b</dc:identifier>
        <dc:Date>2012-03-28 09:24:20</dc:Date>
        <skos:hasTopConcept>Perception</skos:hasTopConcept>
        <skos:prefLabel>Auditory masking</skos:prefLabel>
    </owl:Class>
    


    <!-- http://www.cognitiveatlas.org/ontology/cogat.owl#CAO_00163 -->

    <owl:Class rdf:about="&cogat;CAO_00163">
        <rdfs:label>Auditory memory</rdfs:label>
        <rdfs:subClassOf rdf:resource="&cogat;CAO_00394"/>
        <dc:Contributor>Natalie Picchetti</dc:Contributor>
        <dc:Title>Auditory memory</dc:Title>
        <skos:hasTopConcept>Learning and Memory</skos:hasTopConcept>
        <skos:definition>the cognitive capacity of storing and retrieving information related to sound.</skos:definition>
        <skos:altLabel></skos:altLabel>
        <dc:Date>2011-02-25 12:25:42</dc:Date>
        <skos:prefLabel>Auditory memory</skos:prefLabel>
        <dc:identifier>trm_4a3fd79d09aa7</dc:identifier>
    </owl:Class>
    


    <!-- http://www.cognitiveatlas.org/ontology/cogat.owl#CAO_00164 -->

    <owl:Class rdf:about="&cogat;CAO_00164">
        <rdfs:label>Auditory perception</rdfs:label>
        <rdfs:subClassOf rdf:resource="&cogat;CAO_00437"/>
        <rdfs:subClassOf>
            <owl:Restriction>
                <owl:onProperty rdf:resource="&ro;part_of"/>
                <owl:someValuesFrom rdf:resource="&cogat;CAO_00150"/>
            </owl:Restriction>
        </rdfs:subClassOf>
        <skos:altLabel></skos:altLabel>
        <dc:Contributor>Brenda Gregory</dc:Contributor>
        <dc:Date>2011-05-17 10:01:32</dc:Date>
        <skos:definition>The ability to identify, interpret, and attach meaning to sound.</skos:definition>
        <dc:Title>Auditory perception</dc:Title>
        <skos:prefLabel>Auditory perception</skos:prefLabel>
        <skos:hasTopConcept>Perception</skos:hasTopConcept>
        <dc:identifier>trm_4a3fd79d09ab2</dc:identifier>
    </owl:Class>
    


    <!-- http://www.cognitiveatlas.org/ontology/cogat.owl#CAO_00165 -->

    <owl:Class rdf:about="&cogat;CAO_00165">
        <rdfs:label>Auditory scene</rdfs:label>
        <rdfs:subClassOf rdf:resource="&cogat;CAO_00001"/>
        <skos:prefLabel>Auditory scene</skos:prefLabel>
        <skos:altLabel></skos:altLabel>
        <dc:identifier>trm_4a3fd79d09abe</dc:identifier>
        <dc:Contributor>Natalie Picchetti</dc:Contributor>
        <skos:definition>auditory scene analysis is the process by which the human auditory system organizes sound into perceptually meaningful elements.</skos:definition>
        <dc:Title>Auditory scene</dc:Title>
        <skos:hasTopConcept>Perception</skos:hasTopConcept>
        <dc:Date>2011-04-12 12:50:14</dc:Date>
    </owl:Class>
    


    <!-- http://www.cognitiveatlas.org/ontology/cogat.owl#CAO_00166 -->

    <owl:Class rdf:about="&cogat;CAO_00166">
        <rdfs:label>Auditory scene analysis</rdfs:label>
        <rdfs:subClassOf rdf:resource="&cogat;CAO_00001"/>
        <dc:Title>Auditory scene analysis</dc:Title>
        <dc:Contributor>Brenda Gregory</dc:Contributor>
        <dc:identifier>trm_4a3fd79d09aca</dc:identifier>
        <skos:hasTopConcept></skos:hasTopConcept>
        <dc:Date>2011-05-16 15:51:12</dc:Date>
        <skos:definition>the process by which the human auditory system organizes sound into perceptually meaningful elements.</skos:definition>
        <skos:prefLabel>Auditory scene analysis</skos:prefLabel>
        <skos:altLabel></skos:altLabel>
    </owl:Class>
    


    <!-- http://www.cognitiveatlas.org/ontology/cogat.owl#CAO_00167 -->

    <owl:Class rdf:about="&cogat;CAO_00167">
        <rdfs:label>Auditory sentence comprehension</rdfs:label>
        <rdfs:subClassOf rdf:resource="&cogat;CAO_00628"/>
        <dc:Title>Auditory sentence comprehension</dc:Title>
        <skos:hasTopConcept>Language</skos:hasTopConcept>
        <dc:Date>2012-03-28 08:30:43</dc:Date>
        <skos:prefLabel>Auditory sentence comprehension</skos:prefLabel>
        <skos:definition>ability to combine auditory words into a meaningful sentence unit. </skos:definition>
        <dc:Contributor>Russ Poldrack</dc:Contributor>
        <dc:identifier>trm_4a3fd79d09ad5</dc:identifier>
        <skos:altLabel></skos:altLabel>
    </owl:Class>
    


    <!-- http://www.cognitiveatlas.org/ontology/cogat.owl#CAO_00168 -->

    <owl:Class rdf:about="&cogat;CAO_00168">
        <rdfs:label>Auditory stream segregation</rdfs:label>
        <rdfs:subClassOf rdf:resource="&cogat;CAO_00001"/>
        <rdfs:subClassOf>
            <owl:Restriction>
                <owl:onProperty rdf:resource="&ro;part_of"/>
                <owl:someValuesFrom rdf:resource="&cogat;CAO_00164"/>
            </owl:Restriction>
        </rdfs:subClassOf>
        <rdfs:subClassOf>
            <owl:Restriction>
                <owl:onProperty rdf:resource="&ro;part_of"/>
                <owl:someValuesFrom rdf:resource="&cogat;CAO_00535"/>
            </owl:Restriction>
        </rdfs:subClassOf>
        <skos:prefLabel>Auditory stream segregation</skos:prefLabel>
        <dc:Date>2012-03-28 09:24:48</dc:Date>
        <skos:definition>the perceptual grouping of sounds to form coherent representations of objects in the acoustic scene; a fundamental aspect of hearing and speech perception.</skos:definition>
        <skos:altLabel></skos:altLabel>
        <skos:hasTopConcept>Perception</skos:hasTopConcept>
        <dc:Contributor>Russ Poldrack</dc:Contributor>
        <dc:Title>Auditory stream segregation</dc:Title>
        <dc:identifier>trm_4a3fd79d09ae1</dc:identifier>
    </owl:Class>
    


    <!-- http://www.cognitiveatlas.org/ontology/cogat.owl#CAO_00169 -->

    <owl:Class rdf:about="&cogat;CAO_00169">
        <rdfs:label>Auditory word comprehension</rdfs:label>
        <rdfs:subClassOf rdf:resource="&cogat;CAO_00579"/>
        <rdfs:subClassOf>
            <owl:Restriction>
                <owl:onProperty rdf:resource="&ro;part_of"/>
                <owl:someValuesFrom rdf:resource="&cogat;CAO_00535"/>
            </owl:Restriction>
        </rdfs:subClassOf>
        <dc:Title>Auditory word comprehension</dc:Title>
        <skos:definition>ability to parse acoustic signals into meaningful words</skos:definition>
        <dc:identifier>trm_4a3fd79d09aed</dc:identifier>
        <skos:altLabel></skos:altLabel>
        <skos:hasTopConcept>Language</skos:hasTopConcept>
        <dc:Date>2012-03-28 08:30:19</dc:Date>
        <dc:Contributor>Russ Poldrack</dc:Contributor>
        <skos:prefLabel>Auditory word comprehension</skos:prefLabel>
    </owl:Class>
    


    <!-- http://www.cognitiveatlas.org/ontology/cogat.owl#CAO_00170 -->

    <owl:Class rdf:about="&cogat;CAO_00170">
        <rdfs:label>Auditory word recognition</rdfs:label>
        <rdfs:subClassOf rdf:resource="&cogat;CAO_00001"/>
        <skos:prefLabel>Auditory word recognition</skos:prefLabel>
        <skos:hasTopConcept>Language</skos:hasTopConcept>
        <dc:Contributor>Russ Poldrack</dc:Contributor>
        <skos:altLabel></skos:altLabel>
        <skos:definition>ability to recognize acoustically presented words</skos:definition>
        <dc:Title>Auditory word recognition</dc:Title>
        <dc:Date>2012-03-28 08:30:32</dc:Date>
        <dc:identifier>trm_4a3fd79d09af8</dc:identifier>
    </owl:Class>
    


    <!-- http://www.cognitiveatlas.org/ontology/cogat.owl#CAO_00171 -->

    <owl:Class rdf:about="&cogat;CAO_00171">
        <rdfs:label>Auditory working memory</rdfs:label>
        <rdfs:subClassOf rdf:resource="&cogat;CAO_00587"/>
        <skos:definition>Working memory for auditory information</skos:definition>
        <dc:identifier>trm_4a3fd79d09b04</dc:identifier>
        <dc:Date>2009-07-10 14:06:31</dc:Date>
        <dc:Contributor>Russ Poldrack</dc:Contributor>
        <skos:hasTopConcept>Learning and Memory</skos:hasTopConcept>
        <skos:altLabel></skos:altLabel>
        <skos:prefLabel>Auditory working memory</skos:prefLabel>
        <dc:Title>Auditory working memory</dc:Title>
    </owl:Class>
    


    <!-- http://www.cognitiveatlas.org/ontology/cogat.owl#CAO_00172 -->

    <owl:Class rdf:about="&cogat;CAO_00172">
        <rdfs:label>Autobiographical memory</rdfs:label>
        <rdfs:subClassOf rdf:resource="&cogat;CAO_00285"/>
        <skos:prefLabel>Autobiographical memory</skos:prefLabel>
        <dc:Date>2011-05-04 10:59:03</dc:Date>
        <skos:hasTopConcept>Learning and Memory</skos:hasTopConcept>
        <skos:definition>a memory system consisting of episodes recollected from an individual’s life, based on a combination of episodic (personal experiences and specific objects, people and events experienced at particular time and place) and semantic (general knowledge and facts about the world) memory.</skos:definition>
        <dc:Title>Autobiographical memory</dc:Title>
        <skos:altLabel></skos:altLabel>
        <dc:identifier>trm_4a3fd79d09b10</dc:identifier>
        <dc:Contributor>Brenda Gregory</dc:Contributor>
    </owl:Class>
    


    <!-- http://www.cognitiveatlas.org/ontology/cogat.owl#CAO_00173 -->

    <owl:Class rdf:about="&cogat;CAO_00173">
        <rdfs:label>Autobiographical recall</rdfs:label>
        <rdfs:subClassOf rdf:resource="&cogat;CAO_00645"/>
        <rdfs:subClassOf>
            <owl:Restriction>
                <owl:onProperty rdf:resource="&ro;part_of"/>
                <owl:someValuesFrom rdf:resource="&cogat;CAO_00172"/>
            </owl:Restriction>
        </rdfs:subClassOf>
        <dc:identifier>trm_4a3fd79d09b1c</dc:identifier>
        <skos:prefLabel>Autobiographical recall</skos:prefLabel>
        <dc:Title>Autobiographical recall</dc:Title>
        <dc:Contributor>Brenda Gregory</dc:Contributor>
        <skos:hasTopConcept></skos:hasTopConcept>
        <dc:Date>2011-05-10 14:45:14</dc:Date>
        <skos:altLabel></skos:altLabel>
        <skos:definition>episodes recollected from an individual’s life, based on a combination of episodic (personal experiences and specific objects, people and events experienced at particular time and place) and semantic (general knowledge and facts about the world) memory. </skos:definition>
    </owl:Class>
    


    <!-- http://www.cognitiveatlas.org/ontology/cogat.owl#CAO_00174 -->

    <owl:Class rdf:about="&cogat;CAO_00174">
        <rdfs:label>Automaticity</rdfs:label>
        <rdfs:subClassOf rdf:resource="&cogat;CAO_00001"/>
        <skos:definition>behavior performed without intention</skos:definition>
        <dc:Date>2012-03-28 09:25:43</dc:Date>
        <skos:prefLabel>Automaticity</skos:prefLabel>
        <skos:hasTopConcept>Learning and Memory</skos:hasTopConcept>
        <dc:Contributor>Russ Poldrack</dc:Contributor>
        <dc:identifier>trm_4a3fd79d09b28</dc:identifier>
        <skos:altLabel></skos:altLabel>
        <dc:Title>Automaticity</dc:Title>
    </owl:Class>
    


    <!-- http://www.cognitiveatlas.org/ontology/cogat.owl#CAO_00175 -->

    <owl:Class rdf:about="&cogat;CAO_00175">
        <rdfs:label>Availability heuristic</rdfs:label>
        <rdfs:subClassOf rdf:resource="&cogat;CAO_00206"/>
        <skos:altLabel></skos:altLabel>
        <dc:Date>2009-07-10 14:06:31</dc:Date>
        <dc:Contributor>Emily Barkley-Levenson</dc:Contributor>
        <skos:hasTopConcept>Reasoning and Decision Making</skos:hasTopConcept>
        <skos:definition>A heuristic in which people predict the frequency of classes or the probability of events based on the ease with which relevant instances come to mind. </skos:definition>
        <dc:identifier>trm_4a3fd79d09b33</dc:identifier>
        <skos:prefLabel>Availability heuristic</skos:prefLabel>
        <dc:Title>Availability heuristic</dc:Title>
    </owl:Class>
    


    <!-- http://www.cognitiveatlas.org/ontology/cogat.owl#CAO_00176 -->

    <owl:Class rdf:about="&cogat;CAO_00176">
        <rdfs:label>Aversive learning</rdfs:label>
        <rdfs:subClassOf rdf:resource="&cogat;CAO_00001"/>
        <skos:definition>behavior modification using an adverse stimulus in response to the inappropriate or undesirable behavior.</skos:definition>
        <dc:Title>Aversive learning</dc:Title>
        <skos:hasTopConcept>Learning and Memory</skos:hasTopConcept>
        <skos:altLabel></skos:altLabel>
        <dc:Date>2011-05-16 15:54:48</dc:Date>
        <skos:prefLabel>Aversive learning</skos:prefLabel>
        <dc:Contributor>Brenda Gregory</dc:Contributor>
        <dc:identifier>trm_4a3fd79d09b3f</dc:identifier>
    </owl:Class>
    


    <!-- http://www.cognitiveatlas.org/ontology/cogat.owl#CAO_00177 -->

    <owl:Class rdf:about="&cogat;CAO_00177">
        <rdfs:label>Awareness</rdfs:label>
        <rdfs:subClassOf rdf:resource="&cogat;CAO_00001"/>
        <rdfs:subClassOf>
            <owl:Restriction>
                <owl:onProperty rdf:resource="&ro;part_of"/>
                <owl:someValuesFrom rdf:resource="&cogat;CAO_00223"/>
            </owl:Restriction>
        </rdfs:subClassOf>
        <skos:altLabel>consciousness</skos:altLabel>
        <skos:definition>having knowledge or cognizance. </skos:definition>
        <skos:hasTopConcept></skos:hasTopConcept>
        <dc:Title>Awareness</dc:Title>
        <dc:Contributor>Michael Sharman</dc:Contributor>
        <skos:prefLabel>Awareness</skos:prefLabel>
        <dc:Date>2012-02-22 03:02:05</dc:Date>
        <dc:identifier>trm_4a3fd79d09b4b</dc:identifier>
    </owl:Class>
    


    <!-- http://www.cognitiveatlas.org/ontology/cogat.owl#CAO_00178 -->

    <owl:Class rdf:about="&cogat;CAO_00178">
        <rdfs:label>Backward chaining</rdfs:label>
        <rdfs:subClassOf rdf:resource="&cogat;CAO_00001"/>
        <skos:hasTopConcept>Reasoning and Decision Making</skos:hasTopConcept>
        <dc:Contributor>Russ Poldrack</dc:Contributor>
        <dc:identifier>trm_4a3fd79d09b62</dc:identifier>
        <dc:Date>2012-03-28 09:26:22</dc:Date>
        <skos:altLabel></skos:altLabel>
        <skos:prefLabel>Backward chaining</skos:prefLabel>
        <skos:definition>an inference method used in automated theorem provers, proof assistants and other artificial intelligence applications.  Backward chaining starts with a list of goals (or a hypothesis) and works backwards from the consequent to the antecedent to see if there is data available that will support any of these consequents.</skos:definition>
        <dc:Title>Backward chaining</dc:Title>
    </owl:Class>
    


    <!-- http://www.cognitiveatlas.org/ontology/cogat.owl#CAO_00180 -->

    <owl:Class rdf:about="&cogat;CAO_00180">
        <rdfs:label>Belief</rdfs:label>
        <rdfs:subClassOf rdf:resource="&cogat;CAO_00001"/>
        <skos:prefLabel>Belief</skos:prefLabel>
        <dc:Contributor>Brenda Gregory</dc:Contributor>
        <skos:altLabel></skos:altLabel>
        <skos:hasTopConcept></skos:hasTopConcept>
        <skos:definition>a state or habit of mind in which trust or confidence is placed in some person or thing; conviction of the truth of some statement or the reality of some being or phenomenon especially when based on examination of evidence.</skos:definition>
        <dc:Title>Belief</dc:Title>
        <dc:identifier>trm_4a3fd79d09b85</dc:identifier>
        <dc:Date>2011-05-11 16:16:54</dc:Date>
    </owl:Class>
    


    <!-- http://www.cognitiveatlas.org/ontology/cogat.owl#CAO_00181 -->

    <owl:Class rdf:about="&cogat;CAO_00181">
        <rdfs:label>Binocular convergence</rdfs:label>
        <rdfs:subClassOf rdf:resource="&cogat;CAO_00001"/>
        <dc:Date>2011-04-19 12:11:26</dc:Date>
        <dc:Title>Binocular convergence</dc:Title>
        <skos:altLabel></skos:altLabel>
        <dc:Contributor>Brenda Gregory</dc:Contributor>
        <skos:hasTopConcept>Perception</skos:hasTopConcept>
        <skos:definition>when you look at an object that is closer than approximately 25 feet, your eyes must converge on the object to perceive it as a single object clearly in focus.and#34; </skos:definition>
        <skos:prefLabel>Binocular convergence</skos:prefLabel>
        <dc:identifier>trm_4a3fd79d09b9c</dc:identifier>
    </owl:Class>
    


    <!-- http://www.cognitiveatlas.org/ontology/cogat.owl#CAO_00182 -->

    <owl:Class rdf:about="&cogat;CAO_00182">
        <rdfs:label>Binocular disparity</rdfs:label>
        <rdfs:subClassOf rdf:resource="&cogat;CAO_00001"/>
        <skos:definition>the difference in image location of an object seen by the left and right eyes, resulting from the eyesand#39; horizontal separation. The brain uses binocular disparity to extract depth information from the two-dimensional retinal images  in stereopsis.</skos:definition>
        <dc:identifier>trm_4a3fd79d09bb3</dc:identifier>
        <dc:Contributor>Brenda Gregory</dc:Contributor>
        <dc:Date>2011-04-29 16:15:38</dc:Date>
        <skos:altLabel></skos:altLabel>
        <skos:hasTopConcept>Perception</skos:hasTopConcept>
        <skos:prefLabel>Binocular disparity</skos:prefLabel>
        <dc:Title>Binocular disparity</dc:Title>
    </owl:Class>
    


    <!-- http://www.cognitiveatlas.org/ontology/cogat.owl#CAO_00183 -->

    <owl:Class rdf:about="&cogat;CAO_00183">
        <rdfs:label>Binocular vision</rdfs:label>
        <rdfs:subClassOf rdf:resource="&cogat;CAO_00001"/>
        <skos:prefLabel>Binocular vision</skos:prefLabel>
        <dc:identifier>trm_4a3fd79d09bbf</dc:identifier>
        <skos:definition>is vision in which both eyes are used together.  Having two eyes confers at least four advantages over having one. First, it gives a creature a spare eye in case one is damaged. Second, it gives a wider field of view.  Third, it gives binocular summation in which the ability to detect faint objects is enhanced.  Fourth it can give stereopsis in which parallax provided by the two eyesand#39; different positions on the head give precise depth perception.  Such binocular vision is usually accompanied by singleness of vision or binocular fusion, in which a single image is seen despite each eyeand#39;s having its own image of any object.  Other phenomena of binocular vision include utrocular discrimination, eye dominance, allelotropia, and binocular rivalry.</skos:definition>
        <skos:hasTopConcept>Perception</skos:hasTopConcept>
        <dc:Contributor>Russ Poldrack</dc:Contributor>
        <dc:Date>2012-03-28 09:27:09</dc:Date>
        <skos:altLabel></skos:altLabel>
        <dc:Title>Binocular vision</dc:Title>
    </owl:Class>
    


    <!-- http://www.cognitiveatlas.org/ontology/cogat.owl#CAO_00184 -->

    <owl:Class rdf:about="&cogat;CAO_00184">
        <rdfs:label>Bitterness</rdfs:label>
        <rdfs:subClassOf rdf:resource="&cogat;CAO_00001"/>
        <skos:hasTopConcept>Perception</skos:hasTopConcept>
        <dc:Title>Bitterness</dc:Title>
        <dc:identifier>trm_4a3fd79d09bcb</dc:identifier>
        <dc:Contributor>Russ Poldrack</dc:Contributor>
        <skos:prefLabel>Bitterness</skos:prefLabel>
        <skos:definition>being or inducing the one of the four basic taste sensations that is peculiarly acrid, astringent, or disagreeable; marked by intensity or severity; marked by cynicism and rancor; intensely unpleasant especially in coldness or rawness; expressive of severe pain, grief, or regret.</skos:definition>
        <skos:altLabel></skos:altLabel>
        <dc:Date>2012-03-28 09:27:23</dc:Date>
    </owl:Class>
    


    <!-- http://www.cognitiveatlas.org/ontology/cogat.owl#CAO_00185 -->

    <owl:Class rdf:about="&cogat;CAO_00185">
        <rdfs:label>Body orientation</rdfs:label>
        <rdfs:subClassOf rdf:resource="&cogat;CAO_00001"/>
        <skos:hasTopConcept></skos:hasTopConcept>
        <skos:prefLabel>Body orientation</skos:prefLabel>
        <dc:Date>2009-07-10 14:06:31</dc:Date>
        <dc:identifier>trm_4a3fd79d09be2</dc:identifier>
        <skos:altLabel></skos:altLabel>
        <dc:Contributor>System Administrator</dc:Contributor>
        <skos:definition>No definition submitted yet</skos:definition>
        <dc:Title>Body orientation</dc:Title>
    </owl:Class>
    


    <!-- http://www.cognitiveatlas.org/ontology/cogat.owl#CAO_00186 -->

    <owl:Class rdf:about="&cogat;CAO_00186">
        <rdfs:label>Capacity limitation</rdfs:label>
        <rdfs:subClassOf rdf:resource="&cogat;CAO_00001"/>
        <rdfs:subClassOf>
            <owl:Restriction>
                <owl:onProperty rdf:resource="&ro;part_of"/>
                <owl:someValuesFrom rdf:resource="&cogat;CAO_00587"/>
            </owl:Restriction>
        </rdfs:subClassOf>
        <dc:identifier>trm_4a3fd79d09bee</dc:identifier>
        <skos:altLabel></skos:altLabel>
        <skos:hasTopConcept>Attention</skos:hasTopConcept>
        <skos:definition>a limitation on the capacity to process information</skos:definition>
        <dc:Contributor>Russ Poldrack</dc:Contributor>
        <dc:Title>Capacity limitation</dc:Title>
        <dc:Date>2012-03-28 09:30:42</dc:Date>
        <skos:prefLabel>Capacity limitation</skos:prefLabel>
    </owl:Class>
    


    <!-- http://www.cognitiveatlas.org/ontology/cogat.owl#CAO_00187 -->

    <owl:Class rdf:about="&cogat;CAO_00187">
        <rdfs:label>Case based reasoning</rdfs:label>
        <rdfs:subClassOf rdf:resource="&cogat;CAO_00001"/>
        <dc:identifier>trm_4a3fd79d09bf9</dc:identifier>
        <dc:Contributor>Brenda Gregory</dc:Contributor>
        <skos:prefLabel>Case based reasoning</skos:prefLabel>
        <skos:altLabel></skos:altLabel>
        <dc:Title>Case based reasoning</dc:Title>
        <skos:definition>the process of solving new problems based on the solutions of similar past problems.</skos:definition>
        <dc:Date>2011-05-16 11:07:36</dc:Date>
        <skos:hasTopConcept>Reasoning and Decision Making</skos:hasTopConcept>
    </owl:Class>
    


    <!-- http://www.cognitiveatlas.org/ontology/cogat.owl#CAO_00188 -->

    <owl:Class rdf:about="&cogat;CAO_00188">
        <rdfs:label>Categorical clustering</rdfs:label>
        <rdfs:subClassOf rdf:resource="&cogat;CAO_00001"/>
        <dc:Title>Categorical clustering</dc:Title>
        <dc:Contributor>Russ Poldrack</dc:Contributor>
        <skos:hasTopConcept>Learning and Memory</skos:hasTopConcept>
        <skos:altLabel></skos:altLabel>
        <skos:definition>the clustering of recalled items based on category membership</skos:definition>
        <dc:Date>2012-03-28 09:31:34</dc:Date>
        <skos:prefLabel>Categorical clustering</skos:prefLabel>
        <dc:identifier>trm_4a3fd79d09c05</dc:identifier>
    </owl:Class>
    


    <!-- http://www.cognitiveatlas.org/ontology/cogat.owl#CAO_00189 -->

    <owl:Class rdf:about="&cogat;CAO_00189">
        <rdfs:label>Categorical knowledge</rdfs:label>
        <rdfs:subClassOf rdf:resource="&cogat;CAO_00371"/>
        <skos:definition>knowledge about different attributes and uses of an object that allows it to be placed in a group of objects with similar attributes and uses. </skos:definition>
        <dc:Title>Categorical knowledge</dc:Title>
        <dc:identifier>trm_4a3fd79d09c11</dc:identifier>
        <skos:prefLabel>Categorical knowledge</skos:prefLabel>
        <dc:Contributor>Natalie Picchetti</dc:Contributor>
        <skos:altLabel></skos:altLabel>
        <dc:Date>2011-05-20 14:26:59</dc:Date>
        <skos:hasTopConcept></skos:hasTopConcept>
    </owl:Class>
    


    <!-- http://www.cognitiveatlas.org/ontology/cogat.owl#CAO_00190 -->

    <owl:Class rdf:about="&cogat;CAO_00190">
        <rdfs:label>Categorical perception</rdfs:label>
        <rdfs:subClassOf rdf:resource="&cogat;CAO_00001"/>
        <dc:Contributor>Russ Poldrack</dc:Contributor>
        <skos:altLabel></skos:altLabel>
        <dc:Date>2012-03-28 09:33:18</dc:Date>
        <skos:prefLabel>Categorical perception</skos:prefLabel>
        <dc:Title>Categorical perception</dc:Title>
        <skos:definition>A form of perception in which the individual perceives a categorical distinction rather than a continuous scale of a varying perceptual feature.  </skos:definition>
        <skos:hasTopConcept>Perception</skos:hasTopConcept>
        <dc:identifier>trm_4a3fd79d09c1c</dc:identifier>
    </owl:Class>
    


    <!-- http://www.cognitiveatlas.org/ontology/cogat.owl#CAO_00191 -->

    <owl:Class rdf:about="&cogat;CAO_00191">
        <rdfs:label>Categorization</rdfs:label>
        <rdfs:subClassOf rdf:resource="&cogat;CAO_00001"/>
        <dc:Title>Categorization</dc:Title>
        <skos:prefLabel>Categorization</skos:prefLabel>
        <skos:definition>the process in which ideas and objects are recognized, differentiated and understood.</skos:definition>
        <skos:altLabel></skos:altLabel>
        <dc:identifier>trm_4a3fd79d09c28</dc:identifier>
        <dc:Contributor>Russ Poldrack</dc:Contributor>
        <skos:hasTopConcept>Reasoning and Decision Making</skos:hasTopConcept>
        <dc:Date>2012-03-28 09:33:50</dc:Date>
    </owl:Class>
    


    <!-- http://www.cognitiveatlas.org/ontology/cogat.owl#CAO_00192 -->

    <owl:Class rdf:about="&cogat;CAO_00192">
        <rdfs:label>Category based induction</rdfs:label>
        <rdfs:subClassOf rdf:resource="&cogat;CAO_00001"/>
        <dc:Title>Category based induction</dc:Title>
        <skos:definition>requires that information about one set of categories is used to infer something about another category. A set of premises establishes that one or more categories possess a certain property.  The premises are followed by an assertion (the conclusion) that a target category also possesses that property. </skos:definition>
        <dc:Date>2012-03-28 09:34:02</dc:Date>
        <dc:identifier>trm_4a3fd79d09c34</dc:identifier>
        <skos:altLabel></skos:altLabel>
        <skos:prefLabel>Category based induction</skos:prefLabel>
        <skos:hasTopConcept>Reasoning and Decision Making</skos:hasTopConcept>
        <dc:Contributor>Russ Poldrack</dc:Contributor>
    </owl:Class>
    


    <!-- http://www.cognitiveatlas.org/ontology/cogat.owl#CAO_00193 -->

    <owl:Class rdf:about="&cogat;CAO_00193">
        <rdfs:label>Category learning</rdfs:label>
        <rdfs:subClassOf rdf:resource="&cogat;CAO_00001"/>
        <skos:definition>is a strategy which requires a learner to compare and contrast groups or categories that contain concept-relevant features with groups or categories that do not contain concept-relevant features. </skos:definition>
        <dc:Title>Category learning</dc:Title>
        <dc:identifier>trm_4a3fd79d09c3f</dc:identifier>
        <skos:hasTopConcept>Learning and Memory</skos:hasTopConcept>
        <dc:Date>2011-04-01 12:52:11</dc:Date>
        <dc:Contributor>Natalie Picchetti</dc:Contributor>
        <skos:prefLabel>Category learning</skos:prefLabel>
        <skos:altLabel></skos:altLabel>
    </owl:Class>
    


    <!-- http://www.cognitiveatlas.org/ontology/cogat.owl#CAO_00194 -->

    <owl:Class rdf:about="&cogat;CAO_00194">
        <rdfs:label>Causal inference</rdfs:label>
        <rdfs:subClassOf rdf:resource="&cogat;CAO_00001"/>
        <dc:Contributor>Russ Poldrack</dc:Contributor>
        <skos:hasTopConcept>Reasoning and Decision Making</skos:hasTopConcept>
        <dc:Title>Causal inference</dc:Title>
        <skos:definition>The process of inferring that one state-object-event causes the occurrence of another state-object-event.</skos:definition>
        <skos:prefLabel>Causal inference</skos:prefLabel>
        <skos:altLabel></skos:altLabel>
        <dc:Date>2012-03-28 09:34:36</dc:Date>
        <dc:identifier>trm_4a3fd79d09c5b</dc:identifier>
    </owl:Class>
    


    <!-- http://www.cognitiveatlas.org/ontology/cogat.owl#CAO_00195 -->

    <owl:Class rdf:about="&cogat;CAO_00195">
        <rdfs:label>Central attention</rdfs:label>
        <rdfs:subClassOf rdf:resource="&cogat;CAO_00001"/>
        <dc:Date>2011-04-18 12:33:38</dc:Date>
        <skos:definition>is the cognitive process that allows one to focus on the most important and relevant train of thought that needs to be attended to in a specific situation.</skos:definition>
        <skos:altLabel></skos:altLabel>
        <skos:prefLabel>Central attention</skos:prefLabel>
        <dc:Contributor>Natalie Picchetti</dc:Contributor>
        <dc:identifier>trm_4a3fd79d09c69</dc:identifier>
        <skos:hasTopConcept>Attention</skos:hasTopConcept>
        <dc:Title>Central attention</dc:Title>
    </owl:Class>
    


    <!-- http://www.cognitiveatlas.org/ontology/cogat.owl#CAO_00196 -->

    <owl:Class rdf:about="&cogat;CAO_00196">
        <rdfs:label>Centration</rdfs:label>
        <rdfs:subClassOf rdf:resource="&cogat;CAO_00001"/>
        <skos:hasTopConcept></skos:hasTopConcept>
        <dc:Date>2011-04-29 15:59:42</dc:Date>
        <skos:altLabel></skos:altLabel>
        <dc:Contributor>Brenda Gregory</dc:Contributor>
        <dc:Title>Centration</dc:Title>
        <skos:prefLabel>Centration</skos:prefLabel>
        <skos:definition>the tendency to focus on one aspect of a situation and neglect others.</skos:definition>
        <dc:identifier>trm_4a3fd79d09c74</dc:identifier>
    </owl:Class>
    


    <!-- http://www.cognitiveatlas.org/ontology/cogat.owl#CAO_00197 -->

    <owl:Class rdf:about="&cogat;CAO_00197">
        <rdfs:label>Chemonociception</rdfs:label>
        <rdfs:subClassOf rdf:resource="&cogat;CAO_00001"/>
        <skos:hasTopConcept>Perception</skos:hasTopConcept>
        <skos:definition>perception of stimulation by noxious chemical agents</skos:definition>
        <dc:Date>2012-03-28 09:36:36</dc:Date>
        <dc:Title>Chemonociception</dc:Title>
        <dc:Contributor>Russ Poldrack</dc:Contributor>
        <skos:altLabel></skos:altLabel>
        <skos:prefLabel>Chemonociception</skos:prefLabel>
        <dc:identifier>trm_4a3fd79d09c80</dc:identifier>
    </owl:Class>
    


    <!-- http://www.cognitiveatlas.org/ontology/cogat.owl#CAO_00198 -->

    <owl:Class rdf:about="&cogat;CAO_00198">
        <rdfs:label>Choice</rdfs:label>
        <rdfs:subClassOf rdf:resource="&cogat;CAO_00001"/>
        <skos:definition>the mental process of judging the merits of multiple options and selecting one of them.</skos:definition>
        <dc:identifier>trm_4a3fd79d09c8c</dc:identifier>
        <dc:Date>2012-03-28 09:36:50</dc:Date>
        <skos:prefLabel>Choice</skos:prefLabel>
        <skos:altLabel></skos:altLabel>
        <dc:Contributor>Russ Poldrack</dc:Contributor>
        <skos:hasTopConcept>Reasoning and Decision Making</skos:hasTopConcept>
        <dc:Title>Choice</dc:Title>
    </owl:Class>
    


    <!-- http://www.cognitiveatlas.org/ontology/cogat.owl#CAO_00199 -->

    <owl:Class rdf:about="&cogat;CAO_00199">
        <rdfs:label>Chromatic contrast</rdfs:label>
        <rdfs:subClassOf rdf:resource="&cogat;CAO_00001"/>
        <dc:Date>2011-04-19 12:19:59</dc:Date>
        <dc:Contributor>Brenda Gregory</dc:Contributor>
        <dc:Title>Chromatic contrast</dc:Title>
        <skos:hasTopConcept>Perception</skos:hasTopConcept>
        <dc:identifier>trm_4a3fd79d09c97</dc:identifier>
        <skos:prefLabel>Chromatic contrast</skos:prefLabel>
        <skos:definition>When a small patch is surrounded by a color field, the patch appears to be tinted in the opponent color of the surrounding field.</skos:definition>
        <skos:altLabel></skos:altLabel>
    </owl:Class>
    


    <!-- http://www.cognitiveatlas.org/ontology/cogat.owl#CAO_00200 -->

    <owl:Class rdf:about="&cogat;CAO_00200">
        <rdfs:label>Chunk</rdfs:label>
        <rdfs:subClassOf rdf:resource="&cogat;CAO_00001"/>
        <dc:Title>Chunk</dc:Title>
        <skos:hasTopConcept>Learning and Memory</skos:hasTopConcept>
        <skos:prefLabel>Chunk</skos:prefLabel>
        <skos:altLabel></skos:altLabel>
        <dc:identifier>trm_4a3fd79d09ca3</dc:identifier>
        <dc:Contributor>Agatha Lenartowicz</dc:Contributor>
        <dc:Date>2009-11-25 08:30:30</dc:Date>
        <skos:definition>Structure in memory that is used as a unit of knowledge representation. Also refers to the process of learning by which these units are acquired.</skos:definition>
    </owl:Class>
    


    <!-- http://www.cognitiveatlas.org/ontology/cogat.owl#CAO_00201 -->

    <owl:Class rdf:about="&cogat;CAO_00201">
        <rdfs:label>Chunking</rdfs:label>
        <rdfs:subClassOf rdf:resource="&cogat;CAO_00001"/>
        <dc:Contributor>Herbert Maier</dc:Contributor>
        <skos:definition>The process of recoding information by splitting or reorganizing it into smaller parts. Actually: combining several smaller items into a larger and#34;groupand#34; item, i.e.: 3 separate and#34;incoming aircraftand#34; considered as and#34;3 incoming aircraftand#34;. Significantly reduces the working memory space used. Likely concept model for computer programming data-forms that list pointers to numerous specific data. Larger classes of concepts include: Learning and Memory, Attention, Action (Planning), Executive Control.</skos:definition>
        <dc:Title>Chunking</dc:Title>
        <dc:identifier>trm_4a3fd79d09cae</dc:identifier>
        <skos:altLabel></skos:altLabel>
        <dc:Date>2011-11-16 09:13:26</dc:Date>
        <skos:hasTopConcept>Executive-Cognitive Control</skos:hasTopConcept>
        <skos:prefLabel>Chunking</skos:prefLabel>
    </owl:Class>
    


    <!-- http://www.cognitiveatlas.org/ontology/cogat.owl#CAO_00202 -->

    <owl:Class rdf:about="&cogat;CAO_00202">
        <rdfs:label>Cognition</rdfs:label>
        <rdfs:subClassOf rdf:resource="&cogat;CAO_00001"/>
        <skos:definition>The process of thought; includes all psychological-mental functions that allow for subsequent reflection given some information.</skos:definition>
        <dc:Title>Cognition</dc:Title>
        <skos:prefLabel>Cognition</skos:prefLabel>
        <skos:altLabel></skos:altLabel>
        <dc:identifier>trm_4a3fd79d09d29</dc:identifier>
        <dc:Date>2009-07-10 14:06:31</dc:Date>
        <skos:hasTopConcept></skos:hasTopConcept>
        <dc:Contributor>Agatha Lenartowicz</dc:Contributor>
    </owl:Class>
    


    <!-- http://www.cognitiveatlas.org/ontology/cogat.owl#CAO_00203 -->

    <owl:Class rdf:about="&cogat;CAO_00203">
        <rdfs:label>Cognitive development</rdfs:label>
        <rdfs:subClassOf rdf:resource="&cogat;CAO_00001"/>
        <skos:hasTopConcept></skos:hasTopConcept>
        <dc:Title>Cognitive development</dc:Title>
        <dc:Contributor>Brenda Gregory</dc:Contributor>
        <skos:altLabel></skos:altLabel>
        <skos:prefLabel>Cognitive development</skos:prefLabel>
        <dc:Date>2011-04-28 17:24:11</dc:Date>
        <dc:identifier>trm_4a3fd79d09d35</dc:identifier>
        <skos:definition>the construction of thought processes, including remembering, problem solving, and decision-making, from childhood through adolescence to adulthood.</skos:definition>
    </owl:Class>
    


    <!-- http://www.cognitiveatlas.org/ontology/cogat.owl#CAO_00204 -->

    <owl:Class rdf:about="&cogat;CAO_00204">
        <rdfs:label>Cognitive dissonance</rdfs:label>
        <rdfs:subClassOf rdf:resource="&cogat;CAO_00001"/>
        <skos:definition>The mental state in which a person holds multiple conflicting ideas simultaneously</skos:definition>
        <skos:hasTopConcept></skos:hasTopConcept>
        <dc:Date>2009-07-10 14:06:31</dc:Date>
        <skos:prefLabel>Cognitive dissonance</skos:prefLabel>
        <dc:Title>Cognitive dissonance</dc:Title>
        <dc:identifier>trm_4a3fd79d09d41</dc:identifier>
        <skos:altLabel></skos:altLabel>
        <dc:Contributor>Angela Rizk-Jackson</dc:Contributor>
    </owl:Class>
    


    <!-- http://www.cognitiveatlas.org/ontology/cogat.owl#CAO_00205 -->

    <owl:Class rdf:about="&cogat;CAO_00205">
        <rdfs:label>Cognitive effort</rdfs:label>
        <rdfs:subClassOf rdf:resource="&cogat;CAO_00001"/>
        <skos:hasTopConcept></skos:hasTopConcept>
        <skos:prefLabel>Cognitive effort</skos:prefLabel>
        <dc:Contributor>System Administrator</dc:Contributor>
        <skos:altLabel></skos:altLabel>
        <dc:identifier>trm_4a3fd79d09d4d</dc:identifier>
        <dc:Title>Cognitive effort</dc:Title>
        <skos:definition>No definition submitted yet</skos:definition>
        <dc:Date>2009-07-10 14:06:31</dc:Date>
    </owl:Class>
    


    <!-- http://www.cognitiveatlas.org/ontology/cogat.owl#CAO_00206 -->

    <owl:Class rdf:about="&cogat;CAO_00206">
        <rdfs:label>Cognitive heuristic</rdfs:label>
        <rdfs:subClassOf rdf:resource="&cogat;CAO_00001"/>
        <skos:altLabel></skos:altLabel>
        <skos:hasTopConcept>Reasoning and Decision Making</skos:hasTopConcept>
        <dc:Contributor>Russ Poldrack</dc:Contributor>
        <dc:Date>2012-03-28 09:38:39</dc:Date>
        <skos:definition>are simple, efficient rules, hard-coded by evolutionary processes or learned, which have been proposed to explain how people make decisions, come to judgments, and solve problems, typically when facing complex problems or incomplete information. These rules work well under most circumstances, but in certain cases lead to systematic errors or cognitive biases.</skos:definition>
        <dc:identifier>trm_4a3fd79d09d58</dc:identifier>
        <dc:Title>Cognitive heuristic</dc:Title>
        <skos:prefLabel>Cognitive heuristic</skos:prefLabel>
    </owl:Class>
    


    <!-- http://www.cognitiveatlas.org/ontology/cogat.owl#CAO_00207 -->

    <owl:Class rdf:about="&cogat;CAO_00207">
        <rdfs:label>Cognitive load</rdfs:label>
        <rdfs:subClassOf rdf:resource="&cogat;CAO_00001"/>
        <skos:prefLabel>Cognitive load</skos:prefLabel>
        <dc:Date>2009-07-10 14:06:31</dc:Date>
        <skos:hasTopConcept>Executive-Cognitive Control</skos:hasTopConcept>
        <dc:Title>Cognitive load</dc:Title>
        <dc:identifier>trm_4a3fd79d09d64</dc:identifier>
        <dc:Contributor>Agatha Lenartowicz</dc:Contributor>
        <skos:altLabel></skos:altLabel>
        <skos:definition>The amount of demand placed on working memory, typically expressed along some continuum and within a theoretical maximum.</skos:definition>
    </owl:Class>
    


    <!-- http://www.cognitiveatlas.org/ontology/cogat.owl#CAO_00208 -->

    <owl:Class rdf:about="&cogat;CAO_00208">
        <rdfs:label>Cognitive map</rdfs:label>
        <rdfs:subClassOf rdf:resource="&cogat;CAO_00001"/>
        <skos:hasTopConcept></skos:hasTopConcept>
        <skos:prefLabel>Cognitive map</skos:prefLabel>
        <skos:definition>a type of mental processing composed of a series of psychological transformations by which an individual can acquire, code, store, recall, and decode information about the relative locations and attributes of phenomena in their everyday or metaphorical spatial environment.</skos:definition>
        <skos:altLabel></skos:altLabel>
        <dc:Date>2011-05-16 13:24:24</dc:Date>
        <dc:Contributor>Brenda Gregory</dc:Contributor>
        <dc:Title>Cognitive map</dc:Title>
        <dc:identifier>trm_4a3fd79d09d70</dc:identifier>
    </owl:Class>
    


    <!-- http://www.cognitiveatlas.org/ontology/cogat.owl#CAO_00209 -->

    <owl:Class rdf:about="&cogat;CAO_00209">
        <rdfs:label>Color perception</rdfs:label>
        <rdfs:subClassOf rdf:resource="&cogat;CAO_00001"/>
        <skos:hasTopConcept>Perception</skos:hasTopConcept>
        <skos:altLabel></skos:altLabel>
        <dc:Title>Color perception</dc:Title>
        <dc:Date>2009-07-10 14:06:31</dc:Date>
        <dc:Contributor>Agatha Lenartowicz</dc:Contributor>
        <skos:definition>The process of distinguishing objects based on the wavelengths of the light they reflect or emit.</skos:definition>
        <skos:prefLabel>Color perception</skos:prefLabel>
        <dc:identifier>trm_4a3fd79d09d93</dc:identifier>
    </owl:Class>
    


    <!-- http://www.cognitiveatlas.org/ontology/cogat.owl#CAO_00210 -->

    <owl:Class rdf:about="&cogat;CAO_00210">
        <rdfs:label>Communication</rdfs:label>
        <rdfs:subClassOf rdf:resource="&cogat;CAO_00001"/>
        <skos:hasTopConcept>Social Function</skos:hasTopConcept>
        <skos:definition>a process by which information is exchanged between individuals through a common system of symbols, signs, or behavior.</skos:definition>
        <skos:prefLabel>Communication</skos:prefLabel>
        <dc:identifier>trm_4a3fd79d09d9e</dc:identifier>
        <skos:altLabel></skos:altLabel>
        <dc:Title>Communication</dc:Title>
        <dc:Date>2012-03-28 09:39:11</dc:Date>
        <dc:Contributor>Russ Poldrack</dc:Contributor>
    </owl:Class>
    


    <!-- http://www.cognitiveatlas.org/ontology/cogat.owl#CAO_00211 -->

    <owl:Class rdf:about="&cogat;CAO_00211">
        <rdfs:label>Competition</rdfs:label>
        <rdfs:subClassOf rdf:resource="&cogat;CAO_00001"/>
        <skos:hasTopConcept></skos:hasTopConcept>
        <skos:prefLabel>Competition</skos:prefLabel>
        <dc:identifier>trm_4a3fd79d09daa</dc:identifier>
        <dc:Title>Competition</dc:Title>
        <skos:altLabel></skos:altLabel>
        <dc:Contributor>Brenda Gregory</dc:Contributor>
        <dc:Date>2011-04-28 16:10:19</dc:Date>
        <skos:definition>the act or process of competing; active demand by two or more organisms or kinds of organisms for some environmental resource in short supply; a contest between rivals.</skos:definition>
    </owl:Class>
    


    <!-- http://www.cognitiveatlas.org/ontology/cogat.owl#CAO_00212 -->

    <owl:Class rdf:about="&cogat;CAO_00212">
        <rdfs:label>Concept</rdfs:label>
        <rdfs:subClassOf rdf:resource="&cogat;CAO_00001"/>
        <skos:altLabel></skos:altLabel>
        <dc:identifier>trm_4a3fd79d09db6</dc:identifier>
        <dc:Title>Concept</dc:Title>
        <skos:hasTopConcept></skos:hasTopConcept>
        <dc:Contributor>Brenda Gregory</dc:Contributor>
        <skos:definition>a cognitive unit of meaning—an abstract  idea or a mental symbol  sometimes defined as a and#34;unit of knowledge,and#34; built from other units which act as a conceptand#39;s characteristics.</skos:definition>
        <skos:prefLabel>Concept</skos:prefLabel>
        <dc:Date>2011-04-28 17:19:59</dc:Date>
    </owl:Class>
    


    <!-- http://www.cognitiveatlas.org/ontology/cogat.owl#CAO_00213 -->

    <owl:Class rdf:about="&cogat;CAO_00213">
        <rdfs:label>Concept learning</rdfs:label>
        <rdfs:subClassOf rdf:resource="&cogat;CAO_00001"/>
        <dc:identifier>trm_4a3fd79d09dc1</dc:identifier>
        <skos:hasTopConcept>Learning and Memory</skos:hasTopConcept>
        <dc:Title>Concept learning</dc:Title>
        <skos:definition>Concept learning, also known as category learning and concept attainment, is largely based on the works of the cognitive psychologist Jerome Bruner. Bruner, Goodnow, andamp; Austin (1967) defined concept attainment (or concept learning) as and#34;the search for and listing of attributes that can be used to distinguish exemplars from non exemplars of various categories.and#34; More simply put, concepts are the mental categories that help us classify objects, events, or ideas and each object, event, or idea has a set of common relevant features. Thus, concept learning is a strategy which requires a learner to compare and contrast groups or categories that contain concept-relevant features with groups or categories that do not contain concept-relevant features. </skos:definition>
        <skos:altLabel></skos:altLabel>
        <skos:prefLabel>Concept learning</skos:prefLabel>
        <dc:Contributor>Natalie Picchetti</dc:Contributor>
        <dc:Date>2011-04-18 10:51:41</dc:Date>
    </owl:Class>
    


    <!-- http://www.cognitiveatlas.org/ontology/cogat.owl#CAO_00214 -->

    <owl:Class rdf:about="&cogat;CAO_00214">
        <rdfs:label>Conceptual category</rdfs:label>
        <rdfs:subClassOf rdf:resource="&cogat;CAO_00001"/>
        <skos:hasTopConcept></skos:hasTopConcept>
        <skos:prefLabel>Conceptual category</skos:prefLabel>
        <dc:identifier>trm_4a3fd79d09dcd</dc:identifier>
        <skos:definition>No definition submitted yet</skos:definition>
        <dc:Date>2009-07-10 14:06:31</dc:Date>
        <dc:Title>Conceptual category</dc:Title>
        <skos:altLabel></skos:altLabel>
        <dc:Contributor>System Administrator</dc:Contributor>
    </owl:Class>
    


    <!-- http://www.cognitiveatlas.org/ontology/cogat.owl#CAO_00215 -->

    <owl:Class rdf:about="&cogat;CAO_00215">
        <rdfs:label>Conceptual coherence</rdfs:label>
        <rdfs:subClassOf rdf:resource="&cogat;CAO_00001"/>
        <skos:altLabel></skos:altLabel>
        <dc:Contributor>Brenda Gregory</dc:Contributor>
        <skos:definition>combining a set concepts to make sense of a situation or set of situations.</skos:definition>
        <dc:Title>Conceptual coherence</dc:Title>
        <dc:Date>2011-05-04 10:57:31</dc:Date>
        <skos:hasTopConcept></skos:hasTopConcept>
        <skos:prefLabel>Conceptual coherence</skos:prefLabel>
        <dc:identifier>trm_4a3fd79d09dd9</dc:identifier>
    </owl:Class>
    


    <!-- http://www.cognitiveatlas.org/ontology/cogat.owl#CAO_00216 -->

    <owl:Class rdf:about="&cogat;CAO_00216">
        <rdfs:label>Conceptual planning</rdfs:label>
        <rdfs:subClassOf rdf:resource="&cogat;CAO_00001"/>
        <skos:definition>No definition submitted yet</skos:definition>
        <dc:identifier>trm_4a3fd79d09de4</dc:identifier>
        <skos:altLabel></skos:altLabel>
        <dc:Title>Conceptual planning</dc:Title>
        <skos:prefLabel>Conceptual planning</skos:prefLabel>
        <skos:hasTopConcept></skos:hasTopConcept>
        <dc:Contributor>System Administrator</dc:Contributor>
        <dc:Date>2009-07-10 14:06:31</dc:Date>
    </owl:Class>
    


    <!-- http://www.cognitiveatlas.org/ontology/cogat.owl#CAO_00217 -->

    <owl:Class rdf:about="&cogat;CAO_00217">
        <rdfs:label>Conceptual skill</rdfs:label>
        <rdfs:subClassOf rdf:resource="&cogat;CAO_00001"/>
        <dc:Title>Conceptual skill</dc:Title>
        <skos:altLabel></skos:altLabel>
        <skos:hasTopConcept></skos:hasTopConcept>
        <dc:Date>2011-04-15 12:01:00</dc:Date>
        <skos:definition>is the ability to form concepts about abstract and complex ideas such as communication, language, time, and money, for example.</skos:definition>
        <dc:identifier>trm_4a3fd79d09df0</dc:identifier>
        <skos:prefLabel>Conceptual skill</skos:prefLabel>
        <dc:Contributor>Natalie Picchetti</dc:Contributor>
    </owl:Class>
    


    <!-- http://www.cognitiveatlas.org/ontology/cogat.owl#CAO_00218 -->

    <owl:Class rdf:about="&cogat;CAO_00218">
        <rdfs:label>Conceptualization</rdfs:label>
        <rdfs:subClassOf rdf:resource="&cogat;CAO_00001"/>
        <dc:Title>Conceptualization</dc:Title>
        <skos:definition>to form a concept of; to interpret.</skos:definition>
        <skos:prefLabel>Conceptualization</skos:prefLabel>
        <dc:Contributor>Brenda Gregory</dc:Contributor>
        <dc:Date>2011-05-10 14:46:23</dc:Date>
        <skos:altLabel></skos:altLabel>
        <skos:hasTopConcept></skos:hasTopConcept>
        <dc:identifier>trm_4a3fd79d09dfc</dc:identifier>
    </owl:Class>
    


    <!-- http://www.cognitiveatlas.org/ontology/cogat.owl#CAO_00219 -->

    <owl:Class rdf:about="&cogat;CAO_00219">
        <rdfs:label>Conditional reasoning</rdfs:label>
        <rdfs:subClassOf rdf:resource="&cogat;CAO_00480"/>
        <skos:altLabel></skos:altLabel>
        <dc:Title>Conditional reasoning</dc:Title>
        <skos:definition>the reasoner must draw a conclusion based on a conditional, or “if…then,” proposition.</skos:definition>
        <skos:hasTopConcept>Reasoning and Decision Making</skos:hasTopConcept>
        <skos:prefLabel>Conditional reasoning</skos:prefLabel>
        <dc:Date>2012-03-28 09:40:31</dc:Date>
        <dc:Contributor>Russ Poldrack</dc:Contributor>
        <dc:identifier>trm_4a3fd79d09e07</dc:identifier>
    </owl:Class>
    


    <!-- http://www.cognitiveatlas.org/ontology/cogat.owl#CAO_00220 -->

    <owl:Class rdf:about="&cogat;CAO_00220">
        <rdfs:label>Conflict detection</rdfs:label>
        <rdfs:subClassOf rdf:resource="&cogat;CAO_00001"/>
        <skos:prefLabel>Conflict detection</skos:prefLabel>
        <skos:definition>No definition submitted yet</skos:definition>
        <skos:hasTopConcept></skos:hasTopConcept>
        <dc:Contributor>System Administrator</dc:Contributor>
        <dc:identifier>trm_4a3fd79d09e13</dc:identifier>
        <dc:Date>2009-07-10 14:06:31</dc:Date>
        <dc:Title>Conflict detection</dc:Title>
        <skos:altLabel></skos:altLabel>
    </owl:Class>
    


    <!-- http://www.cognitiveatlas.org/ontology/cogat.owl#CAO_00221 -->

    <owl:Class rdf:about="&cogat;CAO_00221">
        <rdfs:label>Conjunction search</rdfs:label>
        <rdfs:subClassOf rdf:resource="&cogat;CAO_00001"/>
        <dc:Contributor>Russ Poldrack</dc:Contributor>
        <dc:Date>2012-03-28 09:41:04</dc:Date>
        <skos:prefLabel>Conjunction search</skos:prefLabel>
        <dc:Title>Conjunction search</dc:Title>
        <skos:definition>the process of searching for a target that is not defined by any single unique visual feature, but by a combination of two or more features.</skos:definition>
        <skos:altLabel></skos:altLabel>
        <dc:identifier>trm_4a3fd79d09e1e</dc:identifier>
        <skos:hasTopConcept>Attention</skos:hasTopConcept>
    </owl:Class>
    


    <!-- http://www.cognitiveatlas.org/ontology/cogat.owl#CAO_00222 -->

    <owl:Class rdf:about="&cogat;CAO_00222">
        <rdfs:label>Connotation</rdfs:label>
        <rdfs:subClassOf rdf:resource="&cogat;CAO_00001"/>
        <skos:definition>the suggesting of a meaning by a word apart from the thing it explicitly names or describes; something suggested by a word or thing; the signification of something; an essential property or group of properties of a thing named by a term in logic.</skos:definition>
        <dc:Title>Connotation</dc:Title>
        <skos:altLabel></skos:altLabel>
        <dc:Contributor>Russ Poldrack</dc:Contributor>
        <skos:hasTopConcept>Language</skos:hasTopConcept>
        <skos:prefLabel>Connotation</skos:prefLabel>
        <dc:Date>2012-03-28 09:41:22</dc:Date>
        <dc:identifier>trm_4a3fd79d09e2a</dc:identifier>
    </owl:Class>
    


    <!-- http://www.cognitiveatlas.org/ontology/cogat.owl#CAO_00223 -->

    <owl:Class rdf:about="&cogat;CAO_00223">
        <rdfs:label>Consciousness</rdfs:label>
        <rdfs:subClassOf rdf:resource="&cogat;CAO_00001"/>
        <dc:Contributor>Brenda Gregory</dc:Contributor>
        <skos:hasTopConcept></skos:hasTopConcept>
        <dc:Title>Consciousness</dc:Title>
        <dc:identifier>trm_4a3fd79d09e35</dc:identifier>
        <skos:prefLabel>Consciousness</skos:prefLabel>
        <dc:Date>2011-04-28 12:18:14</dc:Date>
        <skos:definition>the quality or state of being aware especially of something within oneself; the state or fact of being conscious of an external object, state, or fact; the state of being characterized by sensation, emotion, volition, and thought; the totality of conscious states of an individual; the normal state of conscious life,(regained consciousness); the upper level of mental life of which the person is aware as contrasted with unconscious processes. </skos:definition>
        <skos:altLabel></skos:altLabel>
    </owl:Class>
    


    <!-- http://www.cognitiveatlas.org/ontology/cogat.owl#CAO_00224 -->

    <owl:Class rdf:about="&cogat;CAO_00224">
        <rdfs:label>Constancy</rdfs:label>
        <rdfs:subClassOf rdf:resource="&cogat;CAO_00001"/>
        <dc:Title>Constancy</dc:Title>
        <dc:Contributor>Brenda Gregory</dc:Contributor>
        <dc:identifier>trm_4a3fd79d09e58</dc:identifier>
        <skos:altLabel></skos:altLabel>
        <skos:prefLabel>Constancy</skos:prefLabel>
        <dc:Date>2011-05-10 14:44:18</dc:Date>
        <skos:definition>steadfastness of mind under duress; a state of being constant or unchanging.</skos:definition>
        <skos:hasTopConcept></skos:hasTopConcept>
    </owl:Class>
    


    <!-- http://www.cognitiveatlas.org/ontology/cogat.owl#CAO_00225 -->

    <owl:Class rdf:about="&cogat;CAO_00225">
        <rdfs:label>Constituent structure</rdfs:label>
        <rdfs:subClassOf rdf:resource="&cogat;CAO_00001"/>
        <skos:altLabel></skos:altLabel>
        <dc:Date>2011-04-11 15:50:40</dc:Date>
        <dc:identifier>trm_4a3fd79d09e64</dc:identifier>
        <skos:definition>is an analysis, often in the form of a schematic representation, of the constituents of a construction, such as a sentence. </skos:definition>
        <skos:hasTopConcept></skos:hasTopConcept>
        <dc:Title>Constituent structure</dc:Title>
        <dc:Contributor>Natalie Picchetti</dc:Contributor>
        <skos:prefLabel>Constituent structure</skos:prefLabel>
    </owl:Class>
    


    <!-- http://www.cognitiveatlas.org/ontology/cogat.owl#CAO_00226 -->

    <owl:Class rdf:about="&cogat;CAO_00226">
        <rdfs:label>Context</rdfs:label>
        <rdfs:subClassOf rdf:resource="&cogat;CAO_00001"/>
        <dc:Contributor>Agatha Lenartowicz</dc:Contributor>
        <dc:identifier>trm_4a3fd79d09e6f</dc:identifier>
        <dc:Title>Context</dc:Title>
        <skos:altLabel></skos:altLabel>
        <skos:hasTopConcept></skos:hasTopConcept>
        <skos:definition>A set of interrelated conditions in which something exists or occurs (e.g., a style of language in a particular passage, activity of a given regions given sensory input).</skos:definition>
        <dc:Date>2009-07-10 14:06:31</dc:Date>
        <skos:prefLabel>Context</skos:prefLabel>
    </owl:Class>
    


    <!-- http://www.cognitiveatlas.org/ontology/cogat.owl#CAO_00227 -->

    <owl:Class rdf:about="&cogat;CAO_00227">
        <rdfs:label>Context dependent</rdfs:label>
        <rdfs:subClassOf rdf:resource="&cogat;CAO_00001"/>
        <skos:prefLabel>Context dependent</skos:prefLabel>
        <dc:Title>Context dependent</dc:Title>
        <dc:identifier>trm_4a3fd79d09e7b</dc:identifier>
        <dc:Date>2011-04-12 10:34:42</dc:Date>
        <dc:Contributor>Natalie Picchetti</dc:Contributor>
        <skos:altLabel></skos:altLabel>
        <skos:hasTopConcept>Learning and Memory</skos:hasTopConcept>
        <skos:definition>is a class of memory that refers to improved recall of specific episodes or information when the context present at encoding and retrieval are the same. </skos:definition>
    </owl:Class>
    


    <!-- http://www.cognitiveatlas.org/ontology/cogat.owl#CAO_00228 -->

    <owl:Class rdf:about="&cogat;CAO_00228">
        <rdfs:label>Context memory</rdfs:label>
        <rdfs:subClassOf rdf:resource="&cogat;CAO_00394"/>
        <skos:definition>refers to improved recall of specific episodes or information when the context present at encoding and retrieval are similar.</skos:definition>
        <skos:altLabel></skos:altLabel>
        <dc:identifier>trm_4a3fd79d09e87</dc:identifier>
        <dc:Title>Context memory</dc:Title>
        <skos:hasTopConcept>Learning and Memory</skos:hasTopConcept>
        <dc:Contributor>Natalie Picchetti</dc:Contributor>
        <skos:prefLabel>Context memory</skos:prefLabel>
        <dc:Date>2011-04-19 13:17:32</dc:Date>
    </owl:Class>
    


    <!-- http://www.cognitiveatlas.org/ontology/cogat.owl#CAO_00229 -->

    <owl:Class rdf:about="&cogat;CAO_00229">
        <rdfs:label>Contextual knowledge</rdfs:label>
        <rdfs:subClassOf rdf:resource="&cogat;CAO_00001"/>
        <skos:definition>information, and-or skills that have particular meaning because of the conditions that form part of their description. </skos:definition>
        <dc:Date>2011-04-28 17:25:15</dc:Date>
        <dc:Contributor>Brenda Gregory</dc:Contributor>
        <skos:prefLabel>Contextual knowledge</skos:prefLabel>
        <skos:altLabel></skos:altLabel>
        <dc:identifier>trm_4a3fd79d09e93</dc:identifier>
        <dc:Title>Contextual knowledge</dc:Title>
        <skos:hasTopConcept></skos:hasTopConcept>
    </owl:Class>
    


    <!-- http://www.cognitiveatlas.org/ontology/cogat.owl#CAO_00230 -->

    <owl:Class rdf:about="&cogat;CAO_00230">
        <rdfs:label>Contingency learning</rdfs:label>
        <rdfs:subClassOf rdf:resource="&cogat;CAO_00001"/>
        <dc:identifier>trm_4a3fd79d09e9e</dc:identifier>
        <dc:Date>2012-03-28 09:44:04</dc:Date>
        <dc:Title>Contingency learning</dc:Title>
        <skos:hasTopConcept>Learning and Memory</skos:hasTopConcept>
        <skos:prefLabel>Contingency learning</skos:prefLabel>
        <skos:altLabel></skos:altLabel>
        <skos:definition>Learning of the contingencies between different events</skos:definition>
        <dc:Contributor>Russ Poldrack</dc:Contributor>
    </owl:Class>
    


    <!-- http://www.cognitiveatlas.org/ontology/cogat.owl#CAO_00231 -->

    <owl:Class rdf:about="&cogat;CAO_00231">
        <rdfs:label>Contrastive stress</rdfs:label>
        <rdfs:subClassOf rdf:resource="&cogat;CAO_00001"/>
        <skos:altLabel></skos:altLabel>
        <skos:definition>No definition submitted yet</skos:definition>
        <skos:hasTopConcept></skos:hasTopConcept>
        <dc:Date>2009-07-10 14:06:31</dc:Date>
        <skos:prefLabel>Contrastive stress</skos:prefLabel>
        <dc:identifier>trm_4a3fd79d09eaa</dc:identifier>
        <dc:Title>Contrastive stress</dc:Title>
        <dc:Contributor>System Administrator</dc:Contributor>
    </owl:Class>
    


    <!-- http://www.cognitiveatlas.org/ontology/cogat.owl#CAO_00232 -->

    <owl:Class rdf:about="&cogat;CAO_00232">
        <rdfs:label>Conventionality</rdfs:label>
        <rdfs:subClassOf rdf:resource="&cogat;CAO_00001"/>
        <skos:altLabel></skos:altLabel>
        <dc:Contributor>Brenda Gregory</dc:Contributor>
        <skos:prefLabel>Conventionality</skos:prefLabel>
        <dc:Title>Conventionality</dc:Title>
        <dc:identifier>trm_4a3fd79d09eb6</dc:identifier>
        <skos:definition>the quality, fact, or condition of being conventional; conventional behavior or act; a conventional form, usage, or rule. </skos:definition>
        <skos:hasTopConcept></skos:hasTopConcept>
        <dc:Date>2011-05-12 15:34:31</dc:Date>
    </owl:Class>
    


    <!-- http://www.cognitiveatlas.org/ontology/cogat.owl#CAO_00233 -->

    <owl:Class rdf:about="&cogat;CAO_00233">
        <rdfs:label>Convergent thinking</rdfs:label>
        <rdfs:subClassOf rdf:resource="&cogat;CAO_00001"/>
        <dc:Title>Convergent thinking</dc:Title>
        <dc:Contributor>Brenda Gregory</dc:Contributor>
        <skos:definition>analytical, usually deductive, thinking in which ideas are examined for their logical validity or in which a set of rules is followed.</skos:definition>
        <dc:identifier>trm_4a3fd79d09ece</dc:identifier>
        <skos:prefLabel>Convergent thinking</skos:prefLabel>
        <dc:Date>2011-05-16 15:53:49</dc:Date>
        <skos:altLabel></skos:altLabel>
        <skos:hasTopConcept></skos:hasTopConcept>
    </owl:Class>
    


    <!-- http://www.cognitiveatlas.org/ontology/cogat.owl#CAO_00234 -->

    <owl:Class rdf:about="&cogat;CAO_00234">
        <rdfs:label>Conversation</rdfs:label>
        <rdfs:subClassOf rdf:resource="&cogat;CAO_00001"/>
        <skos:definition>An exchange of sentiments, observations, opinions, or ideas.</skos:definition>
        <dc:Title>Conversation</dc:Title>
        <dc:Contributor>Russ Poldrack</dc:Contributor>
        <skos:altLabel></skos:altLabel>
        <dc:Date>2012-03-28 09:44:32</dc:Date>
        <dc:identifier>trm_4a3fd79d09eda</dc:identifier>
        <skos:prefLabel>Conversation</skos:prefLabel>
        <skos:hasTopConcept>Language</skos:hasTopConcept>
    </owl:Class>
    


    <!-- http://www.cognitiveatlas.org/ontology/cogat.owl#CAO_00235 -->

    <owl:Class rdf:about="&cogat;CAO_00235">
        <rdfs:label>Conversational norm</rdfs:label>
        <rdfs:subClassOf rdf:resource="&cogat;CAO_00001"/>
        <skos:definition>No definition submitted yet</skos:definition>
        <skos:altLabel></skos:altLabel>
        <dc:Title>Conversational norm</dc:Title>
        <dc:Contributor>System Administrator</dc:Contributor>
        <skos:prefLabel>Conversational norm</skos:prefLabel>
        <dc:identifier>trm_4a3fd79d09ee6</dc:identifier>
        <dc:Date>2009-07-10 14:06:31</dc:Date>
        <skos:hasTopConcept></skos:hasTopConcept>
    </owl:Class>
    


    <!-- http://www.cognitiveatlas.org/ontology/cogat.owl#CAO_00236 -->

    <owl:Class rdf:about="&cogat;CAO_00236">
        <rdfs:label>Conversational speech</rdfs:label>
        <rdfs:subClassOf rdf:resource="&cogat;CAO_00001"/>
        <dc:identifier>trm_4a3fd79d09ef0</dc:identifier>
        <dc:Date>2012-03-28 09:44:44</dc:Date>
        <skos:altLabel></skos:altLabel>
        <dc:Contributor>Russ Poldrack</dc:Contributor>
        <skos:hasTopConcept>Language</skos:hasTopConcept>
        <skos:definition>is interactive, more-or-less spontaneous, communication between two or more conversants. Interactivity occurs because contributions to a conversation are response reactions to what has previously been said. Spontaneity occurs because a conversation must proceed, to some extent, and in some way, unpredictably.</skos:definition>
        <skos:prefLabel>Conversational speech</skos:prefLabel>
        <dc:Title>Conversational speech</dc:Title>
    </owl:Class>
    


    <!-- http://www.cognitiveatlas.org/ontology/cogat.owl#CAO_00237 -->

    <owl:Class rdf:about="&cogat;CAO_00237">
        <rdfs:label>Conversational structure</rdfs:label>
        <rdfs:subClassOf rdf:resource="&cogat;CAO_00001"/>
        <skos:altLabel></skos:altLabel>
        <dc:identifier>trm_4a3fd79d09efb</dc:identifier>
        <skos:hasTopConcept>Language</skos:hasTopConcept>
        <dc:Contributor>Natalie Picchetti</dc:Contributor>
        <dc:Date>2011-04-12 12:03:26</dc:Date>
        <skos:definition>is the organization of interactive, more-or-less spontaneous, communication between two or more conversants. </skos:definition>
        <skos:prefLabel>Conversational structure</skos:prefLabel>
        <dc:Title>Conversational structure</dc:Title>
    </owl:Class>
    


    <!-- http://www.cognitiveatlas.org/ontology/cogat.owl#CAO_00238 -->

    <owl:Class rdf:about="&cogat;CAO_00238">
        <rdfs:label>Coordination</rdfs:label>
        <rdfs:subClassOf rdf:resource="&cogat;CAO_00001"/>
        <skos:prefLabel>Coordination</skos:prefLabel>
        <dc:Date>2011-05-18 16:03:47</dc:Date>
        <skos:altLabel></skos:altLabel>
        <skos:hasTopConcept></skos:hasTopConcept>
        <dc:identifier>trm_4a3fd79d09f07</dc:identifier>
        <dc:Contributor>Natalie Picchetti</dc:Contributor>
        <skos:definition>is the act of coordinating, making different people or things work together for a goal or effect.  </skos:definition>
        <dc:Title>Coordination</dc:Title>
    </owl:Class>
    


    <!-- http://www.cognitiveatlas.org/ontology/cogat.owl#CAO_00239 -->

    <owl:Class rdf:about="&cogat;CAO_00239">
        <rdfs:label>Coproduction</rdfs:label>
        <rdfs:subClassOf rdf:resource="&cogat;CAO_00001"/>
        <skos:altLabel></skos:altLabel>
        <dc:identifier>trm_4a3fd79d09f12</dc:identifier>
        <dc:Contributor>System Administrator</dc:Contributor>
        <skos:prefLabel>Coproduction</skos:prefLabel>
        <skos:definition>No definition submitted yet</skos:definition>
        <dc:Date>2009-07-10 14:06:31</dc:Date>
        <dc:Title>Coproduction</dc:Title>
        <skos:hasTopConcept></skos:hasTopConcept>
    </owl:Class>
    


    <!-- http://www.cognitiveatlas.org/ontology/cogat.owl#CAO_00240 -->

    <owl:Class rdf:about="&cogat;CAO_00240">
        <rdfs:label>Coreference</rdfs:label>
        <rdfs:subClassOf rdf:resource="&cogat;CAO_00001"/>
        <skos:definition>a relationship between two words or phrases in which both refer to the same person or thing and one stands as a linguistic antecedent of the other.</skos:definition>
        <skos:altLabel></skos:altLabel>
        <dc:Title>Coreference</dc:Title>
        <skos:prefLabel>Coreference</skos:prefLabel>
        <dc:Date>2011-04-28 16:13:10</dc:Date>
        <skos:hasTopConcept>Language</skos:hasTopConcept>
        <dc:Contributor>Brenda Gregory</dc:Contributor>
        <dc:identifier>trm_4a3fd79d09f1e</dc:identifier>
    </owl:Class>
    


    <!-- http://www.cognitiveatlas.org/ontology/cogat.owl#CAO_00241 -->

    <owl:Class rdf:about="&cogat;CAO_00241">
        <rdfs:label>Creative cognition</rdfs:label>
        <rdfs:subClassOf rdf:resource="&cogat;CAO_00001"/>
        <dc:Title>Creative cognition</dc:Title>
        <skos:definition>involves two types of processes: generative processes and exploratory processes.  Generative processes are those that most of us think about when we think of creativity. They are the processes by which creative concepts are first born. These processes are highly visible in extreme acts of creativity, but they are also evident in ordinary, everyday cognition.  Examples (from Ward et al.(cited below)) include memory retrieval, association formation among information retrieved from memory, combinations of structures retrieved from memory, the synthesis of new structures, the transformation of retrieved structures into and#34;new forms,and#34; analogical transfer between domains, and and#34;categorical reduction,and#34; which involves reducing existing structures to and#34;more primitive constituentsand#34;.  Exploratory processes are the processes used to explore the structures produced by generative processes. Examples of exploratory processes (given by Ward, et al.) include searching retrieved structures for and#34;novel attributes,and#34; searching for and#34;metaphorical implications,and#34; searching for possible functions, and#34;the evaluation of structures from different perspectives or within different contexts,and#34; interpretation of structures from the perspective of the problem(s) to be solved, and and#34;the search for various practical or conceptual limitations that are suggested by the structures.and#34; </skos:definition>
        <skos:hasTopConcept></skos:hasTopConcept>
        <dc:Contributor>Natalie Picchetti</dc:Contributor>
        <skos:altLabel></skos:altLabel>
        <skos:prefLabel>Creative cognition</skos:prefLabel>
        <dc:Date>2011-04-11 15:16:37</dc:Date>
        <dc:identifier>trm_4a3fd79d09f2a</dc:identifier>
    </owl:Class>
    


    <!-- http://www.cognitiveatlas.org/ontology/cogat.owl#CAO_00242 -->

    <owl:Class rdf:about="&cogat;CAO_00242">
        <rdfs:label>Creative problem solving</rdfs:label>
        <rdfs:subClassOf rdf:resource="&cogat;CAO_00001"/>
        <dc:Title>Creative problem solving</dc:Title>
        <dc:Date>2012-03-28 09:45:09</dc:Date>
        <dc:Contributor>Russ Poldrack</dc:Contributor>
        <skos:prefLabel>Creative problem solving</skos:prefLabel>
        <skos:definition>the mental process of independently creating a solution to a problem without learned assistance.</skos:definition>
        <skos:hasTopConcept>Reasoning and Decision Making</skos:hasTopConcept>
        <skos:altLabel></skos:altLabel>
        <dc:identifier>trm_4a3fd79d09f36</dc:identifier>
    </owl:Class>
    


    <!-- http://www.cognitiveatlas.org/ontology/cogat.owl#CAO_00243 -->

    <owl:Class rdf:about="&cogat;CAO_00243">
        <rdfs:label>Creative thinking</rdfs:label>
        <rdfs:subClassOf rdf:resource="&cogat;CAO_00001"/>
        <skos:definition>the intellectually disciplined process of actively and skillfully conceptualizing, applying, analyzing, synthesizing, and-or evaluating information gathered from, or generated by, observation, experience, reflection, reasoning, or communication, as a guide to belief and action (Scriven andamp; Paul, 1992).</skos:definition>
        <skos:hasTopConcept></skos:hasTopConcept>
        <dc:Title>Creative thinking</dc:Title>
        <skos:altLabel></skos:altLabel>
        <dc:Contributor>Brenda Gregory</dc:Contributor>
        <dc:identifier>trm_4a3fd79d09f42</dc:identifier>
        <dc:Date>2011-04-19 12:17:09</dc:Date>
        <skos:prefLabel>Creative thinking</skos:prefLabel>
    </owl:Class>
    


    <!-- http://www.cognitiveatlas.org/ontology/cogat.owl#CAO_00244 -->

    <owl:Class rdf:about="&cogat;CAO_00244">
        <rdfs:label>Critical period</rdfs:label>
        <rdfs:subClassOf rdf:resource="&cogat;CAO_00001"/>
        <skos:definition>a limited time in which an event can occur, usually to result in some kind of transformation; in developmental psychology and developmental biology, it is a time in the early stages of an organismand#39;s life during which it displays a heightened sensitivity to certain environmental stimuli, and develops in particular ways due to experiences at this time.</skos:definition>
        <dc:Title>Critical period</dc:Title>
        <skos:altLabel></skos:altLabel>
        <skos:prefLabel>Critical period</skos:prefLabel>
        <dc:Contributor>Brenda Gregory</dc:Contributor>
        <dc:Date>2011-05-16 11:59:08</dc:Date>
        <dc:identifier>trm_4a3fd79d09f4d</dc:identifier>
        <skos:hasTopConcept></skos:hasTopConcept>
    </owl:Class>
    


    <!-- http://www.cognitiveatlas.org/ontology/cogat.owl#CAO_00245 -->

    <owl:Class rdf:about="&cogat;CAO_00245">
        <rdfs:label>Crosstalk</rdfs:label>
        <rdfs:subClassOf rdf:resource="&cogat;CAO_00001"/>
        <dc:identifier>trm_4a3fd79d09f59</dc:identifier>
        <skos:prefLabel>Crosstalk</skos:prefLabel>
        <dc:Date>2012-03-28 09:46:09</dc:Date>
        <skos:altLabel></skos:altLabel>
        <skos:hasTopConcept></skos:hasTopConcept>
        <dc:Title>Crosstalk</dc:Title>
        <dc:Contributor>Russ Poldrack</dc:Contributor>
        <skos:definition>interference by information presented via multiple channels</skos:definition>
    </owl:Class>
    


    <!-- http://www.cognitiveatlas.org/ontology/cogat.owl#CAO_00246 -->

    <owl:Class rdf:about="&cogat;CAO_00246">
        <rdfs:label>Crystallized intelligence</rdfs:label>
        <rdfs:subClassOf rdf:resource="&cogat;CAO_00001"/>
        <dc:Contributor>Russ Poldrack</dc:Contributor>
        <dc:Date>2012-03-28 09:46:29</dc:Date>
        <dc:identifier>trm_4a3fd79d09f64</dc:identifier>
        <skos:definition>the ability to utilize previously acquired knowledge and experience.</skos:definition>
        <skos:prefLabel>Crystallized intelligence</skos:prefLabel>
        <dc:Title>Crystallized intelligence</dc:Title>
        <skos:hasTopConcept>Reasoning and Decision Making</skos:hasTopConcept>
        <skos:altLabel></skos:altLabel>
    </owl:Class>
    


    <!-- http://www.cognitiveatlas.org/ontology/cogat.owl#CAO_00247 -->

    <owl:Class rdf:about="&cogat;CAO_00247">
        <rdfs:label>Cue dependent forgetting</rdfs:label>
        <rdfs:subClassOf rdf:resource="&cogat;CAO_00638"/>
        <dc:Title>Cue dependent forgetting</dc:Title>
        <skos:hasTopConcept>Learning and Memory</skos:hasTopConcept>
        <dc:Contributor>Natalie Picchetti</dc:Contributor>
        <dc:identifier>trm_4a3fd79d09f70</dc:identifier>
        <skos:definition>is the failure to recall a memory due to missing stimuli or cues that were present at the time the memory was encoded.</skos:definition>
        <skos:prefLabel>Cue dependent forgetting</skos:prefLabel>
        <dc:Date>2011-04-18 12:12:42</dc:Date>
        <skos:altLabel></skos:altLabel>
    </owl:Class>
    


    <!-- http://www.cognitiveatlas.org/ontology/cogat.owl#CAO_00248 -->

    <owl:Class rdf:about="&cogat;CAO_00248">
        <rdfs:label>Cue validity</rdfs:label>
        <rdfs:subClassOf rdf:resource="&cogat;CAO_00001"/>
        <dc:identifier>trm_4a3fd79d09f7c</dc:identifier>
        <dc:Contributor>Russ Poldrack</dc:Contributor>
        <skos:altLabel></skos:altLabel>
        <skos:prefLabel>Cue validity</skos:prefLabel>
        <skos:definition>the conditional probability that an object falls in a particular category given a particular feature or cue.</skos:definition>
        <skos:hasTopConcept>Attention</skos:hasTopConcept>
        <dc:Title>Cue validity</dc:Title>
        <dc:Date>2012-03-28 09:47:00</dc:Date>
    </owl:Class>
    


    <!-- http://www.cognitiveatlas.org/ontology/cogat.owl#CAO_00249 -->

    <owl:Class rdf:about="&cogat;CAO_00249">
        <rdfs:label>Cueing</rdfs:label>
        <rdfs:subClassOf rdf:resource="&cogat;CAO_00001"/>
        <dc:Contributor>Brenda Gregory</dc:Contributor>
        <skos:prefLabel>Cueing</skos:prefLabel>
        <skos:hasTopConcept></skos:hasTopConcept>
        <dc:Title>Cueing</dc:Title>
        <dc:Date>2010-04-29 13:10:21</dc:Date>
        <dc:identifier>trm_4a3fd79d09f87</dc:identifier>
        <skos:altLabel></skos:altLabel>
        <skos:definition>to give-present a stimulus that prompts a reaction.</skos:definition>
    </owl:Class>
    


    <!-- http://www.cognitiveatlas.org/ontology/cogat.owl#CAO_00250 -->

    <owl:Class rdf:about="&cogat;CAO_00250">
        <rdfs:label>Dative shift</rdfs:label>
        <rdfs:subClassOf rdf:resource="&cogat;CAO_00001"/>
        <dc:identifier>trm_4a3fd79d0a006</dc:identifier>
        <skos:prefLabel>Dative shift</skos:prefLabel>
        <dc:Contributor>Russ Poldrack</dc:Contributor>
        <dc:Date>2012-03-28 09:47:24</dc:Date>
        <skos:hasTopConcept>Language</skos:hasTopConcept>
        <skos:definition>a grammatical process by which an oblique  argument of a verb, usually one functioning as a recipient or a benefactive (roles often expressed by datives), is placed in the same grammatical role as a patient, increasing the valency of the verb and forming a clause with two objects.</skos:definition>
        <skos:altLabel></skos:altLabel>
        <dc:Title>Dative shift</dc:Title>
    </owl:Class>
    


    <!-- http://www.cognitiveatlas.org/ontology/cogat.owl#CAO_00251 -->

    <owl:Class rdf:about="&cogat;CAO_00251">
        <rdfs:label>Decay of activation</rdfs:label>
        <rdfs:subClassOf rdf:resource="&cogat;CAO_00001"/>
        <rdfs:subClassOf>
            <owl:Restriction>
                <owl:onProperty rdf:resource="&ro;part_of"/>
                <owl:someValuesFrom rdf:resource="&cogat;CAO_00538"/>
            </owl:Restriction>
        </rdfs:subClassOf>
        <dc:Date>2011-08-10 12:00:42</dc:Date>
        <dc:Contributor>Tyler Davis</dc:Contributor>
        <skos:prefLabel>Decay of activation</skos:prefLabel>
        <skos:hasTopConcept>Learning and Memory</skos:hasTopConcept>
        <skos:definition>An explanation for why spreading activation, in network-based models of knowledge representation, peters out as a function of the distance between nodes.</skos:definition>
        <dc:Title>Decay of activation</dc:Title>
        <dc:identifier>trm_4a3fd79d0a021</dc:identifier>
        <skos:altLabel></skos:altLabel>
    </owl:Class>
    


    <!-- http://www.cognitiveatlas.org/ontology/cogat.owl#CAO_00252 -->

    <owl:Class rdf:about="&cogat;CAO_00252">
        <rdfs:label>Deception</rdfs:label>
        <rdfs:subClassOf rdf:resource="&cogat;CAO_00001"/>
        <skos:definition>an act to propagate beliefs that are not true, or not the whole truth (as in half-truths or omission).</skos:definition>
        <dc:Contributor>Russ Poldrack</dc:Contributor>
        <dc:identifier>trm_4a3fd79d0a02c</dc:identifier>
        <skos:altLabel></skos:altLabel>
        <dc:Date>2012-03-28 09:47:39</dc:Date>
        <dc:Title>Deception</dc:Title>
        <skos:hasTopConcept>Social Function</skos:hasTopConcept>
        <skos:prefLabel>Deception</skos:prefLabel>
    </owl:Class>
    


    <!-- http://www.cognitiveatlas.org/ontology/cogat.owl#CAO_00253 -->

    <owl:Class rdf:about="&cogat;CAO_00253">
        <rdfs:label>Decision making</rdfs:label>
        <rdfs:subClassOf rdf:resource="&cogat;CAO_00001"/>
        <skos:hasTopConcept>Reasoning and Decision Making</skos:hasTopConcept>
        <dc:Date>2011-11-15 06:40:56</dc:Date>
        <dc:identifier>trm_4a3fd79d0a038</dc:identifier>
        <skos:definition>The selection of a course of action among several alternatives. </skos:definition>
        <skos:altLabel></skos:altLabel>
        <dc:Title>Decision making</dc:Title>
        <dc:Contributor>Michelle Johansen</dc:Contributor>
        <skos:prefLabel>Decision making</skos:prefLabel>
    </owl:Class>
    


    <!-- http://www.cognitiveatlas.org/ontology/cogat.owl#CAO_00254 -->

    <owl:Class rdf:about="&cogat;CAO_00254">
        <rdfs:label>Declarative knowledge</rdfs:label>
        <rdfs:subClassOf rdf:resource="&cogat;CAO_00371"/>
        <skos:prefLabel>Declarative knowledge</skos:prefLabel>
        <dc:Title>Declarative knowledge</dc:Title>
        <skos:definition>Knowledge that is descriptive and includes knowing and#34;thatand#34; rather than knowing and#34;howand#34; (can be expressed in declarative sentences).</skos:definition>
        <dc:Contributor>Agatha Lenartowicz</dc:Contributor>
        <skos:hasTopConcept>Learning and Memory</skos:hasTopConcept>
        <dc:identifier>trm_4a3fd79d0a044</dc:identifier>
        <skos:altLabel></skos:altLabel>
        <dc:Date>2009-07-10 14:06:31</dc:Date>
    </owl:Class>
    


    <!-- http://www.cognitiveatlas.org/ontology/cogat.owl#CAO_00255 -->

    <owl:Class rdf:about="&cogat;CAO_00255">
        <rdfs:label>Declarative memory</rdfs:label>
        <rdfs:subClassOf rdf:resource="&cogat;CAO_00397"/>
        <dc:identifier>trm_4a3fd79d0a04f</dc:identifier>
        <skos:altLabel></skos:altLabel>
        <dc:Date>2012-03-28 09:48:17</dc:Date>
        <skos:hasTopConcept>Learning and Memory</skos:hasTopConcept>
        <skos:definition>Memory for facts, and that can be intentionally articulated in some manner.</skos:definition>
        <skos:prefLabel>Declarative memory</skos:prefLabel>
        <dc:Title>Declarative memory</dc:Title>
        <dc:Contributor>Russ Poldrack</dc:Contributor>
    </owl:Class>
    


    <!-- http://www.cognitiveatlas.org/ontology/cogat.owl#CAO_00256 -->

    <owl:Class rdf:about="&cogat;CAO_00256">
        <rdfs:label>Declarative rule</rdfs:label>
        <rdfs:subClassOf rdf:resource="&cogat;CAO_00254"/>
        <rdfs:subClassOf>
            <owl:Restriction>
                <owl:onProperty rdf:resource="&ro;part_of"/>
                <owl:someValuesFrom rdf:resource="&cogat;CAO_00498"/>
            </owl:Restriction>
        </rdfs:subClassOf>
        <skos:definition>A criterion for which one possesses declarative knowledge. Contrasts with an implicit or non-declarative rule, which one might follow but not represent as a rule or even be aware that they are following.</skos:definition>
        <skos:prefLabel>Declarative rule</skos:prefLabel>
        <dc:Contributor>Tyler Davis</dc:Contributor>
        <dc:Title>Declarative rule</dc:Title>
        <dc:Date>2011-08-14 14:57:11</dc:Date>
        <skos:hasTopConcept>Learning and Memory</skos:hasTopConcept>
        <dc:identifier>trm_4a3fd79d0a05b</dc:identifier>
        <skos:altLabel></skos:altLabel>
    </owl:Class>
    


    <!-- http://www.cognitiveatlas.org/ontology/cogat.owl#CAO_00257 -->

    <owl:Class rdf:about="&cogat;CAO_00257">
        <rdfs:label>Deductive inference</rdfs:label>
        <rdfs:subClassOf rdf:resource="&cogat;CAO_00346"/>
        <skos:definition>A type of inference in which the conclusion always follows from the stated premises.If the premises are true, then the conclusion is valid.</skos:definition>
        <dc:Title>Deductive inference</dc:Title>
        <dc:identifier>trm_4a3fd79d0a066</dc:identifier>
        <dc:Date>2011-08-14 14:59:42</dc:Date>
        <skos:prefLabel>Deductive inference</skos:prefLabel>
        <skos:hasTopConcept>Reasoning and Decision Making</skos:hasTopConcept>
        <skos:altLabel></skos:altLabel>
        <dc:Contributor>Tyler Davis</dc:Contributor>
    </owl:Class>
    


    <!-- http://www.cognitiveatlas.org/ontology/cogat.owl#CAO_00258 -->

    <owl:Class rdf:about="&cogat;CAO_00258">
        <rdfs:label>Deductive reasoning</rdfs:label>
        <rdfs:subClassOf rdf:resource="&cogat;CAO_00480"/>
        <skos:prefLabel>Deductive reasoning</skos:prefLabel>
        <skos:definition>is reasoning which constructs or evaluates deductive arguments. Deductive arguments are attempts to show that a conclusion necessarily follows from a set of premises or hypotheses. </skos:definition>
        <dc:Title>Deductive reasoning</dc:Title>
        <skos:hasTopConcept>Reasoning and Decision Making</skos:hasTopConcept>
        <dc:Date>2011-04-11 15:54:01</dc:Date>
        <dc:Contributor>Natalie Picchetti</dc:Contributor>
        <dc:identifier>trm_4a3fd79d0a072</dc:identifier>
        <skos:altLabel></skos:altLabel>
    </owl:Class>
    


    <!-- http://www.cognitiveatlas.org/ontology/cogat.owl#CAO_00259 -->

    <owl:Class rdf:about="&cogat;CAO_00259">
        <rdfs:label>Deep processing</rdfs:label>
        <rdfs:subClassOf rdf:resource="&cogat;CAO_00001"/>
        <dc:identifier>trm_4a3fd79d0a07e</dc:identifier>
        <dc:Contributor>Tyler Davis</dc:Contributor>
        <dc:Date>2011-08-14 15:22:06</dc:Date>
        <skos:altLabel></skos:altLabel>
        <skos:prefLabel>Deep processing</skos:prefLabel>
        <skos:definition>Evaluating a piece of information in terms of meaning or associations to other concepts as opposed to surface or incidental characteristics.</skos:definition>
        <dc:Title>Deep processing</dc:Title>
        <skos:hasTopConcept>Learning and Memory</skos:hasTopConcept>
    </owl:Class>
    


    <!-- http://www.cognitiveatlas.org/ontology/cogat.owl#CAO_00260 -->

    <owl:Class rdf:about="&cogat;CAO_00260">
        <rdfs:label>Deep structure</rdfs:label>
        <rdfs:subClassOf rdf:resource="&cogat;CAO_00001"/>
        <dc:Contributor>Russ Poldrack</dc:Contributor>
        <skos:definition>The essential meaning of a sentence, without regard to the grammatical features (surface structure) of the sentence that are needed to express it in words.</skos:definition>
        <dc:Date>2012-03-28 09:48:58</dc:Date>
        <dc:Title>Deep structure</dc:Title>
        <skos:altLabel></skos:altLabel>
        <skos:hasTopConcept>Language</skos:hasTopConcept>
        <dc:identifier>trm_4a3fd79d0a08a</dc:identifier>
        <skos:prefLabel>Deep structure</skos:prefLabel>
    </owl:Class>
    


    <!-- http://www.cognitiveatlas.org/ontology/cogat.owl#CAO_00261 -->

    <owl:Class rdf:about="&cogat;CAO_00261">
        <rdfs:label>Depth cue</rdfs:label>
        <rdfs:subClassOf rdf:resource="&cogat;CAO_00001"/>
        <skos:altLabel></skos:altLabel>
        <dc:identifier>trm_4a3fd79d0a095</dc:identifier>
        <skos:definition>Depth perception arises from a variety of depth cues. These are typically classified into binocular cues that require input from both eyes and monocular cues that require the input from just one eye.  Binocular cues include stereopsis, yielding depth from binocular vision through exploitation of parallax. Monocular cues include size: distant objects subtend smaller visual angles than near objects.  A third class of cues requires synthetic integration of binocular and monocular cues.</skos:definition>
        <skos:prefLabel>Depth cue</skos:prefLabel>
        <dc:Contributor>Natalie Picchetti</dc:Contributor>
        <dc:Title>Depth cue</dc:Title>
        <skos:hasTopConcept>Perception</skos:hasTopConcept>
        <dc:Date>2011-04-12 11:15:44</dc:Date>
    </owl:Class>
    


    <!-- http://www.cognitiveatlas.org/ontology/cogat.owl#CAO_00262 -->

    <owl:Class rdf:about="&cogat;CAO_00262">
        <rdfs:label>Depth perception</rdfs:label>
        <rdfs:subClassOf rdf:resource="&cogat;CAO_00001"/>
        <dc:Title>Depth perception</dc:Title>
        <dc:identifier>trm_4a3fd79d0a0a1</dc:identifier>
        <skos:prefLabel>Depth perception</skos:prefLabel>
        <skos:hasTopConcept>Perception</skos:hasTopConcept>
        <dc:Contributor>Agatha Lenartowicz</dc:Contributor>
        <skos:altLabel></skos:altLabel>
        <dc:Date>2009-07-10 14:06:31</dc:Date>
        <skos:definition>Ability to perceive the visual world in three dimensions.</skos:definition>
    </owl:Class>
    


    <!-- http://www.cognitiveatlas.org/ontology/cogat.owl#CAO_00263 -->

    <owl:Class rdf:about="&cogat;CAO_00263">
        <rdfs:label>Desire</rdfs:label>
        <rdfs:subClassOf rdf:resource="&cogat;CAO_00001"/>
        <dc:Title>Desire</dc:Title>
        <dc:Date>2012-03-28 09:49:23</dc:Date>
        <skos:hasTopConcept>Motivation</skos:hasTopConcept>
        <skos:altLabel></skos:altLabel>
        <skos:prefLabel>Desire</skos:prefLabel>
        <dc:identifier>trm_4a3fd79d0a0ad</dc:identifier>
        <skos:definition>to long or hope for, exhibit or feel desire for; to express a wish for.</skos:definition>
        <dc:Contributor>Russ Poldrack</dc:Contributor>
    </owl:Class>
    


    <!-- http://www.cognitiveatlas.org/ontology/cogat.owl#CAO_00264 -->

    <owl:Class rdf:about="&cogat;CAO_00264">
        <rdfs:label>Diphthong</rdfs:label>
        <rdfs:subClassOf rdf:resource="&cogat;CAO_00001"/>
        <dc:Contributor>Brenda Gregory</dc:Contributor>
        <dc:identifier>trm_4a3fd79d0a0dc</dc:identifier>
        <skos:altLabel></skos:altLabel>
        <skos:hasTopConcept>Language</skos:hasTopConcept>
        <dc:Title>Diphthong</dc:Title>
        <dc:Date>2011-04-28 16:09:51</dc:Date>
        <skos:definition>a gliding monosyllabic speech sound (as the vowel combination at the end of toy) that starts at or near the articulatory position for one vowel and moves to or toward the position of another.</skos:definition>
        <skos:prefLabel>Diphthong</skos:prefLabel>
    </owl:Class>
    


    <!-- http://www.cognitiveatlas.org/ontology/cogat.owl#CAO_00265 -->

    <owl:Class rdf:about="&cogat;CAO_00265">
        <rdfs:label>Dispositions</rdfs:label>
        <rdfs:subClassOf rdf:resource="&cogat;CAO_00001"/>
        <dc:identifier>trm_4a3fd79d0a0e7</dc:identifier>
        <dc:Contributor>Tyler Davis</dc:Contributor>
        <skos:hasTopConcept></skos:hasTopConcept>
        <skos:definition>Tendency to act in a particular manner given a certain set of antecedents. </skos:definition>
        <dc:Date>2011-08-14 15:33:28</dc:Date>
        <skos:altLabel></skos:altLabel>
        <dc:Title>Dispositions</dc:Title>
        <skos:prefLabel>Dispositions</skos:prefLabel>
    </owl:Class>
    


    <!-- http://www.cognitiveatlas.org/ontology/cogat.owl#CAO_00266 -->

    <owl:Class rdf:about="&cogat;CAO_00266">
        <rdfs:label>Distraction</rdfs:label>
        <rdfs:subClassOf rdf:resource="&cogat;CAO_00001"/>
        <skos:altLabel></skos:altLabel>
        <dc:identifier>trm_4a3fd79d0a0f3</dc:identifier>
        <skos:definition>Any event that interrupts a mental process.</skos:definition>
        <skos:hasTopConcept>Attention</skos:hasTopConcept>
        <skos:prefLabel>Distraction</skos:prefLabel>
        <dc:Contributor>Russ Poldrack</dc:Contributor>
        <dc:Title>Distraction</dc:Title>
        <dc:Date>2012-03-28 09:51:06</dc:Date>
    </owl:Class>
    


    <!-- http://www.cognitiveatlas.org/ontology/cogat.owl#CAO_00267 -->

    <owl:Class rdf:about="&cogat;CAO_00267">
        <rdfs:label>Distributed coding</rdfs:label>
        <rdfs:subClassOf rdf:resource="&cogat;CAO_00001"/>
        <skos:definition>A type of coding in which the information that constitutes a concept (or mental representation) is spread amongst a number of constituent representations.</skos:definition>
        <skos:hasTopConcept>Learning and Memory</skos:hasTopConcept>
        <dc:Title>Distributed coding</dc:Title>
        <skos:altLabel></skos:altLabel>
        <dc:Date>2011-08-14 15:41:30</dc:Date>
        <dc:Contributor>Tyler Davis</dc:Contributor>
        <dc:identifier>trm_4a3fd79d0a0ff</dc:identifier>
        <skos:prefLabel>Distributed coding</skos:prefLabel>
    </owl:Class>
    


    <!-- http://www.cognitiveatlas.org/ontology/cogat.owl#CAO_00268 -->

    <owl:Class rdf:about="&cogat;CAO_00268">
        <rdfs:label>Divergent thinking</rdfs:label>
        <rdfs:subClassOf rdf:resource="&cogat;CAO_00001"/>
        <dc:identifier>trm_4a3fd79d0a10a</dc:identifier>
        <dc:Contributor>Russ Poldrack</dc:Contributor>
        <skos:prefLabel>Divergent thinking</skos:prefLabel>
        <skos:hasTopConcept>Reasoning and Decision Making</skos:hasTopConcept>
        <skos:definition>a thought process or method used to generate creative ideas by exploring many possible solutions.</skos:definition>
        <dc:Title>Divergent thinking</dc:Title>
        <dc:Date>2012-03-28 09:51:20</dc:Date>
        <skos:altLabel></skos:altLabel>
    </owl:Class>
    


    <!-- http://www.cognitiveatlas.org/ontology/cogat.owl#CAO_00269 -->

    <owl:Class rdf:about="&cogat;CAO_00269">
        <rdfs:label>Divided attention</rdfs:label>
        <rdfs:subClassOf rdf:resource="&cogat;CAO_00144"/>
        <dc:Contributor>Russ Poldrack</dc:Contributor>
        <dc:identifier>trm_4a3fd79d0a116</dc:identifier>
        <skos:definition>A state in which the focus of attention is spread across more than one object or event.</skos:definition>
        <skos:altLabel></skos:altLabel>
        <skos:hasTopConcept>Attention</skos:hasTopConcept>
        <skos:prefLabel>Divided attention</skos:prefLabel>
        <dc:Title>Divided attention</dc:Title>
        <dc:Date>2012-03-28 09:51:33</dc:Date>
    </owl:Class>
    


    <!-- http://www.cognitiveatlas.org/ontology/cogat.owl#CAO_00270 -->

    <owl:Class rdf:about="&cogat;CAO_00270">
        <rdfs:label>Dream</rdfs:label>
        <rdfs:subClassOf rdf:resource="&cogat;CAO_00001"/>
        <skos:hasTopConcept></skos:hasTopConcept>
        <skos:definition>a succession of thoughts, images, sounds or emotions which the mind experiences during sleep.</skos:definition>
        <dc:Date>2011-05-16 15:58:26</dc:Date>
        <dc:Contributor>Brenda Gregory</dc:Contributor>
        <skos:prefLabel>Dream</skos:prefLabel>
        <dc:Title>Dream</dc:Title>
        <dc:identifier>trm_4a3fd79d0a12d</dc:identifier>
        <skos:altLabel></skos:altLabel>
    </owl:Class>
    


    <!-- http://www.cognitiveatlas.org/ontology/cogat.owl#CAO_00271 -->

    <owl:Class rdf:about="&cogat;CAO_00271">
        <rdfs:label>Efficiency</rdfs:label>
        <rdfs:subClassOf rdf:resource="&cogat;CAO_00001"/>
        <dc:Date>2012-03-28 10:53:49</dc:Date>
        <skos:definition>effective operation as measured by a comparison of production with cost (as in energy, time, and money)</skos:definition>
        <dc:identifier>trm_4a3fd79d0a145</dc:identifier>
        <skos:altLabel></skos:altLabel>
        <dc:Title>Efficiency</dc:Title>
        <skos:hasTopConcept></skos:hasTopConcept>
        <skos:prefLabel>Efficiency</skos:prefLabel>
        <dc:Contributor>Russ Poldrack</dc:Contributor>
    </owl:Class>
    


    <!-- http://www.cognitiveatlas.org/ontology/cogat.owl#CAO_00272 -->

    <owl:Class rdf:about="&cogat;CAO_00272">
        <rdfs:label>Effort</rdfs:label>
        <rdfs:subClassOf rdf:resource="&cogat;CAO_00001"/>
        <skos:hasTopConcept></skos:hasTopConcept>
        <dc:Date>2011-08-14 15:51:16</dc:Date>
        <dc:Title>Effort</dc:Title>
        <dc:Contributor>Tyler Davis</dc:Contributor>
        <skos:altLabel></skos:altLabel>
        <dc:identifier>trm_4a3fd79d0a151</dc:identifier>
        <skos:prefLabel>Effort</skos:prefLabel>
        <skos:definition>Consciously or intentionally engaging cognitive resources in order to achieve a particular end.</skos:definition>
    </owl:Class>
    


    <!-- http://www.cognitiveatlas.org/ontology/cogat.owl#CAO_00273 -->

    <owl:Class rdf:about="&cogat;CAO_00273">
        <rdfs:label>Effortful processing</rdfs:label>
        <rdfs:subClassOf rdf:resource="&cogat;CAO_00001"/>
        <dc:Contributor>Brenda Gregory</dc:Contributor>
        <dc:Title>Effortful processing</dc:Title>
        <skos:prefLabel>Effortful processing</skos:prefLabel>
        <dc:Date>2011-04-29 11:03:59</dc:Date>
        <skos:altLabel></skos:altLabel>
        <dc:identifier>trm_4a3fd79d0a15c</dc:identifier>
        <skos:definition>learning or storing (encoding) that requires attention and effort.</skos:definition>
        <skos:hasTopConcept></skos:hasTopConcept>
    </owl:Class>
    


    <!-- http://www.cognitiveatlas.org/ontology/cogat.owl#CAO_00274 -->

    <owl:Class rdf:about="&cogat;CAO_00274">
        <rdfs:label>Egocentric</rdfs:label>
        <rdfs:subClassOf rdf:resource="&cogat;CAO_00001"/>
        <dc:identifier>trm_4a3fd79d0a168</dc:identifier>
        <dc:Contributor>Tyler Davis</dc:Contributor>
        <dc:Date>2011-08-14 15:52:33</dc:Date>
        <skos:hasTopConcept></skos:hasTopConcept>
        <skos:prefLabel>Egocentric</skos:prefLabel>
        <dc:Title>Egocentric</dc:Title>
        <skos:definition>A frame of reference centered around the self. In perception, a first-person frame of reference.</skos:definition>
        <skos:altLabel></skos:altLabel>
    </owl:Class>
    


    <!-- http://www.cognitiveatlas.org/ontology/cogat.owl#CAO_00275 -->

    <owl:Class rdf:about="&cogat;CAO_00275">
        <rdfs:label>Elaborative processing</rdfs:label>
        <rdfs:subClassOf rdf:resource="&cogat;CAO_00001"/>
        <skos:prefLabel>Elaborative processing</skos:prefLabel>
        <skos:hasTopConcept></skos:hasTopConcept>
        <dc:Title>Elaborative processing</dc:Title>
        <skos:definition>Processing in which semantic associations or relations between words-concepts are generated or elaborated on.</skos:definition>
        <dc:Date>2011-08-14 15:54:00</dc:Date>
        <skos:altLabel></skos:altLabel>
        <dc:identifier>trm_4a3fd79d0a173</dc:identifier>
        <dc:Contributor>Tyler Davis</dc:Contributor>
    </owl:Class>
    


    <!-- http://www.cognitiveatlas.org/ontology/cogat.owl#CAO_00276 -->

    <owl:Class rdf:about="&cogat;CAO_00276">
        <rdfs:label>Emotion</rdfs:label>
        <rdfs:subClassOf rdf:resource="&cogat;CAO_00001"/>
        <dc:Title>Emotion</dc:Title>
        <skos:hasTopConcept>Emotion</skos:hasTopConcept>
        <dc:Date>2012-03-28 10:54:40</dc:Date>
        <skos:altLabel></skos:altLabel>
        <dc:identifier>trm_4a3fd79d0a17f</dc:identifier>
        <skos:definition>a complex of psychological phenomena that involve some degree of arousal and valence (positive-negative)</skos:definition>
        <skos:prefLabel>Emotion</skos:prefLabel>
        <dc:Contributor>Russ Poldrack</dc:Contributor>
    </owl:Class>
    


    <!-- http://www.cognitiveatlas.org/ontology/cogat.owl#CAO_00277 -->

    <owl:Class rdf:about="&cogat;CAO_00277">
        <rdfs:label>Emotional decision making</rdfs:label>
        <rdfs:subClassOf rdf:resource="&cogat;CAO_00253"/>
        <skos:prefLabel>Emotional decision making</skos:prefLabel>
        <dc:Date>2011-08-14 16:04:41</dc:Date>
        <skos:definition>The use of affective information as information in a decision making process or as a basis for making a decision. Hot cognition.</skos:definition>
        <dc:identifier>trm_4a3fd79d0a18b</dc:identifier>
        <skos:altLabel></skos:altLabel>
        <skos:hasTopConcept>Emotion</skos:hasTopConcept>
        <dc:Title>Emotional decision making</dc:Title>
        <dc:Contributor>Tyler Davis</dc:Contributor>
    </owl:Class>
    


    <!-- http://www.cognitiveatlas.org/ontology/cogat.owl#CAO_00278 -->

    <owl:Class rdf:about="&cogat;CAO_00278">
        <rdfs:label>Emotional expression</rdfs:label>
        <rdfs:subClassOf rdf:resource="&cogat;CAO_00001"/>
        <skos:definition>observable verbal and nonverbal behavior that communicates emotion with or without self-awareness.</skos:definition>
        <skos:altLabel></skos:altLabel>
        <dc:Date>2012-03-28 10:55:25</dc:Date>
        <skos:hasTopConcept>Emotion</skos:hasTopConcept>
        <dc:Contributor>Russ Poldrack</dc:Contributor>
        <skos:prefLabel>Emotional expression</skos:prefLabel>
        <dc:Title>Emotional expression</dc:Title>
        <dc:identifier>trm_4a3fd79d0a196</dc:identifier>
    </owl:Class>
    


    <!-- http://www.cognitiveatlas.org/ontology/cogat.owl#CAO_00279 -->

    <owl:Class rdf:about="&cogat;CAO_00279">
        <rdfs:label>Emotional intelligence</rdfs:label>
        <rdfs:subClassOf rdf:resource="&cogat;CAO_00001"/>
        <dc:identifier>trm_4a3fd79d0a1a2</dc:identifier>
        <dc:Contributor>Russ Poldrack</dc:Contributor>
        <skos:altLabel></skos:altLabel>
        <skos:definition>the capacity, skill or ability to identify, assess, and manage the emotions of oneand#39;s self, of others, and of groups.</skos:definition>
        <skos:prefLabel>Emotional intelligence</skos:prefLabel>
        <dc:Date>2012-03-28 10:55:36</dc:Date>
        <dc:Title>Emotional intelligence</dc:Title>
        <skos:hasTopConcept>Emotion</skos:hasTopConcept>
    </owl:Class>
    


    <!-- http://www.cognitiveatlas.org/ontology/cogat.owl#CAO_00280 -->

    <owl:Class rdf:about="&cogat;CAO_00280">
        <rdfs:label>Emotional memory</rdfs:label>
        <rdfs:subClassOf rdf:resource="&cogat;CAO_00394"/>
        <dc:identifier>trm_4a3fd79d0a1ae</dc:identifier>
        <dc:Date>2011-04-18 10:48:40</dc:Date>
        <skos:prefLabel>Emotional memory</skos:prefLabel>
        <skos:altLabel></skos:altLabel>
        <skos:hasTopConcept>Learning and Memory</skos:hasTopConcept>
        <dc:Contributor>Natalie Picchetti</dc:Contributor>
        <dc:Title>Emotional memory</dc:Title>
        <skos:definition>Emotional memory is the storage and recall of events and details that are couple with the physiological response that was present when the event occurred.  </skos:definition>
    </owl:Class>
    


    <!-- http://www.cognitiveatlas.org/ontology/cogat.owl#CAO_00281 -->

    <owl:Class rdf:about="&cogat;CAO_00281">
        <rdfs:label>Emotional mimicry</rdfs:label>
        <rdfs:subClassOf rdf:resource="&cogat;CAO_00001"/>
        <dc:Contributor>Natalie Picchetti</dc:Contributor>
        <skos:prefLabel>Emotional mimicry</skos:prefLabel>
        <skos:altLabel></skos:altLabel>
        <dc:Title>Emotional mimicry</dc:Title>
        <dc:identifier>trm_4a3fd79d0a1b9</dc:identifier>
        <dc:Date>2011-03-31 13:36:52</dc:Date>
        <skos:hasTopConcept>Emotion</skos:hasTopConcept>
        <skos:definition>is the ability of a person to imitate, copy, and experience the physical and emotional characteristics of another persons emotion.  </skos:definition>
    </owl:Class>
    


    <!-- http://www.cognitiveatlas.org/ontology/cogat.owl#CAO_00284 -->

    <owl:Class rdf:about="&cogat;CAO_00284">
        <rdfs:label>Episodic learning</rdfs:label>
        <rdfs:subClassOf rdf:resource="&cogat;CAO_00001"/>
        <skos:altLabel></skos:altLabel>
        <dc:Date>2011-04-19 12:13:57</dc:Date>
        <dc:Contributor>Brenda Gregory</dc:Contributor>
        <dc:Title>Episodic learning</dc:Title>
        <dc:identifier>trm_4a3fd79d0a1e8</dc:identifier>
        <skos:hasTopConcept>Learning and Memory</skos:hasTopConcept>
        <skos:definition>a change in behavior that occurs as a result of an event; episodic learning is so named because events are recorded into episodic memory.</skos:definition>
        <skos:prefLabel>Episodic learning</skos:prefLabel>
    </owl:Class>
    


    <!-- http://www.cognitiveatlas.org/ontology/cogat.owl#CAO_00285 -->

    <owl:Class rdf:about="&cogat;CAO_00285">
        <rdfs:label>Episodic memory</rdfs:label>
        <rdfs:subClassOf rdf:resource="&cogat;CAO_00255"/>
        <dc:Date>2011-04-19 12:13:22</dc:Date>
        <dc:Title>Episodic memory</dc:Title>
        <skos:definition>memory of autobiographical events (times, places, associated emotions, and other contextual knowledge) that can be explicitly stated.</skos:definition>
        <dc:identifier>trm_4a3fd79d0a1f4</dc:identifier>
        <dc:Contributor>Brenda Gregory</dc:Contributor>
        <skos:altLabel></skos:altLabel>
        <skos:prefLabel>Episodic memory</skos:prefLabel>
        <skos:hasTopConcept>Learning and Memory</skos:hasTopConcept>
    </owl:Class>
    


    <!-- http://www.cognitiveatlas.org/ontology/cogat.owl#CAO_00286 -->

    <owl:Class rdf:about="&cogat;CAO_00286">
        <rdfs:label>Error detection</rdfs:label>
        <rdfs:subClassOf rdf:resource="&cogat;CAO_00001"/>
        <dc:Contributor>Tyler Davis</dc:Contributor>
        <skos:prefLabel>Error detection</skos:prefLabel>
        <skos:altLabel></skos:altLabel>
        <skos:definition>Processes that identify when mistakes have been made.</skos:definition>
        <dc:identifier>trm_4a3fd79d0a20c</dc:identifier>
        <dc:Date>2011-08-14 16:34:06</dc:Date>
        <skos:hasTopConcept></skos:hasTopConcept>
        <dc:Title>Error detection</dc:Title>
    </owl:Class>
    


    <!-- http://www.cognitiveatlas.org/ontology/cogat.owl#CAO_00287 -->

    <owl:Class rdf:about="&cogat;CAO_00287">
        <rdfs:label>Error signal</rdfs:label>
        <rdfs:subClassOf rdf:resource="&cogat;CAO_00001"/>
        <skos:altLabel></skos:altLabel>
        <dc:Title>Error signal</dc:Title>
        <skos:prefLabel>Error signal</skos:prefLabel>
        <dc:Date>2011-08-14 16:37:01</dc:Date>
        <skos:hasTopConcept></skos:hasTopConcept>
        <skos:definition>An event following error detection, in which a sign is relayed notifying the advent of an error.</skos:definition>
        <dc:Contributor>Tyler Davis</dc:Contributor>
        <dc:identifier>trm_4a3fd79d0a218</dc:identifier>
    </owl:Class>
    


    <!-- http://www.cognitiveatlas.org/ontology/cogat.owl#CAO_00288 -->

    <owl:Class rdf:about="&cogat;CAO_00288">
        <rdfs:label>Error trapping</rdfs:label>
        <rdfs:subClassOf rdf:resource="&cogat;CAO_00001"/>
        <skos:altLabel></skos:altLabel>
        <dc:Contributor>Brenda Gregory</dc:Contributor>
        <skos:definition>procedures that detect and correct errors before the errors cause further confusion.</skos:definition>
        <dc:Date>2011-04-19 13:53:02</dc:Date>
        <dc:identifier>trm_4a3fd79d0a223</dc:identifier>
        <skos:prefLabel>Error trapping</skos:prefLabel>
        <skos:hasTopConcept></skos:hasTopConcept>
        <dc:Title>Error trapping</dc:Title>
    </owl:Class>
    


    <!-- http://www.cognitiveatlas.org/ontology/cogat.owl#CAO_00289 -->

    <owl:Class rdf:about="&cogat;CAO_00289">
        <rdfs:label>Excitation</rdfs:label>
        <rdfs:subClassOf rdf:resource="&cogat;CAO_00001"/>
        <skos:hasTopConcept>Emotion</skos:hasTopConcept>
        <skos:altLabel></skos:altLabel>
        <dc:Date>2012-03-28 11:49:58</dc:Date>
        <dc:identifier>trm_4a3fd79d0a22f</dc:identifier>
        <dc:Title>Excitation</dc:Title>
        <dc:Contributor>Russ Poldrack</dc:Contributor>
        <skos:prefLabel>Excitation</skos:prefLabel>
        <skos:definition>a state of increased emotional arousal</skos:definition>
    </owl:Class>
    


    <!-- http://www.cognitiveatlas.org/ontology/cogat.owl#CAO_00291 -->

    <owl:Class rdf:about="&cogat;CAO_00291">
        <rdfs:label>Executive control</rdfs:label>
        <rdfs:subClassOf rdf:resource="&cogat;CAO_00001"/>
        <skos:prefLabel>Executive control</skos:prefLabel>
        <dc:Date>2010-01-10 14:48:58</dc:Date>
        <dc:Title>Executive control</dc:Title>
        <dc:identifier>trm_4a3fd79d0a246</dc:identifier>
        <skos:definition>A top-down system that manages and controls other cognitive processes, allowing goal-directed behavior.</skos:definition>
        <skos:hasTopConcept>Executive-Cognitive Control</skos:hasTopConcept>
        <skos:altLabel></skos:altLabel>
        <dc:Contributor>Russ Poldrack</dc:Contributor>
    </owl:Class>
    


    <!-- http://www.cognitiveatlas.org/ontology/cogat.owl#CAO_00292 -->

    <owl:Class rdf:about="&cogat;CAO_00292">
        <rdfs:label>Executive function</rdfs:label>
        <rdfs:subClassOf rdf:resource="&cogat;CAO_00001"/>
        <dc:Date>2010-01-10 14:56:27</dc:Date>
        <skos:definition>A top-down system that manages and controls other cognitive processes, allowing goal-directed behavior.</skos:definition>
        <skos:prefLabel>Executive function</skos:prefLabel>
        <dc:Contributor>Russ Poldrack</dc:Contributor>
        <skos:hasTopConcept>Executive-Cognitive Control</skos:hasTopConcept>
        <skos:altLabel></skos:altLabel>
        <dc:identifier>trm_4a3fd79d0a252</dc:identifier>
        <dc:Title>Executive function</dc:Title>
    </owl:Class>
    


    <!-- http://www.cognitiveatlas.org/ontology/cogat.owl#CAO_00293 -->

    <owl:Class rdf:about="&cogat;CAO_00293">
        <rdfs:label>Expertise</rdfs:label>
        <rdfs:subClassOf rdf:resource="&cogat;CAO_00001"/>
        <skos:definition>Having a highly cultivated level of skill in a particular domain. Occurs after prolonged experience in a domain.</skos:definition>
        <dc:Date>2012-03-28 11:51:15</dc:Date>
        <dc:Contributor>Russ Poldrack</dc:Contributor>
        <skos:hasTopConcept>Learning and Memory</skos:hasTopConcept>
        <dc:identifier>trm_4a3fd79d0a25e</dc:identifier>
        <skos:prefLabel>Expertise</skos:prefLabel>
        <skos:altLabel></skos:altLabel>
        <dc:Title>Expertise</dc:Title>
    </owl:Class>
    


    <!-- http://www.cognitiveatlas.org/ontology/cogat.owl#CAO_00294 -->

    <owl:Class rdf:about="&cogat;CAO_00294">
        <rdfs:label>Explicit knowledge</rdfs:label>
        <rdfs:subClassOf rdf:resource="&cogat;CAO_00371"/>
        <skos:altLabel></skos:altLabel>
        <dc:Contributor>Tyler Davis</dc:Contributor>
        <dc:Date>2011-08-14 16:42:15</dc:Date>
        <skos:prefLabel>Explicit knowledge</skos:prefLabel>
        <skos:definition>Knowledge that can be articulated or expressed intentionally.</skos:definition>
        <skos:hasTopConcept></skos:hasTopConcept>
        <dc:identifier>trm_4a3fd79d0a269</dc:identifier>
        <dc:Title>Explicit knowledge</dc:Title>
    </owl:Class>
    


    <!-- http://www.cognitiveatlas.org/ontology/cogat.owl#CAO_00295 -->

    <owl:Class rdf:about="&cogat;CAO_00295">
        <rdfs:label>Explicit learning</rdfs:label>
        <rdfs:subClassOf rdf:resource="&cogat;CAO_00377"/>
        <dc:Date>2009-07-10 14:06:31</dc:Date>
        <dc:identifier>trm_4a3fd79d0a275</dc:identifier>
        <skos:prefLabel>Explicit learning</skos:prefLabel>
        <dc:Title>Explicit learning</dc:Title>
        <skos:definition>Acquisition of skills and-or knowledge actively and with awareness. Typically such learning is accompanied by meta-awareness - individuals can explain how they acquired the skill-knowledge.</skos:definition>
        <skos:altLabel></skos:altLabel>
        <skos:hasTopConcept>Learning and Memory</skos:hasTopConcept>
        <dc:Contributor>Agatha Lenartowicz</dc:Contributor>
    </owl:Class>
    


    <!-- http://www.cognitiveatlas.org/ontology/cogat.owl#CAO_00296 -->

    <owl:Class rdf:about="&cogat;CAO_00296">
        <rdfs:label>Explicit memory</rdfs:label>
        <rdfs:subClassOf rdf:resource="&cogat;CAO_00255"/>
        <skos:altLabel></skos:altLabel>
        <skos:definition>the conscious, intentional recollection of previous experiences and information.</skos:definition>
        <dc:Contributor>Brenda Gregory</dc:Contributor>
        <skos:hasTopConcept>Learning and Memory</skos:hasTopConcept>
        <skos:prefLabel>Explicit memory</skos:prefLabel>
        <dc:Date>2011-05-12 15:18:53</dc:Date>
        <dc:Title>Explicit memory</dc:Title>
        <dc:identifier>trm_4a3fd79d0a281</dc:identifier>
    </owl:Class>
    


    <!-- http://www.cognitiveatlas.org/ontology/cogat.owl#CAO_00297 -->

    <owl:Class rdf:about="&cogat;CAO_00297">
        <rdfs:label>Extrinsic motivation</rdfs:label>
        <rdfs:subClassOf rdf:resource="&cogat;CAO_00001"/>
        <dc:Contributor>Brenda Gregory</dc:Contributor>
        <dc:Title>Extrinsic motivation</dc:Title>
        <skos:prefLabel>Extrinsic motivation</skos:prefLabel>
        <skos:altLabel></skos:altLabel>
        <skos:definition>motivated by external factors, as opposed to the internal drivers of intrinsic motivation. Extrinsic motivation drives one to do things for tangible rewards or pressures.</skos:definition>
        <skos:hasTopConcept>Motivation</skos:hasTopConcept>
        <dc:identifier>trm_4a3fd79d0a28c</dc:identifier>
        <dc:Date>2011-05-03 13:55:27</dc:Date>
    </owl:Class>
    


    <!-- http://www.cognitiveatlas.org/ontology/cogat.owl#CAO_00298 -->

    <owl:Class rdf:about="&cogat;CAO_00298">
        <rdfs:label>Face perception</rdfs:label>
        <rdfs:subClassOf rdf:resource="&cogat;CAO_00001"/>
        <skos:altLabel></skos:altLabel>
        <dc:Title>Face perception</dc:Title>
        <dc:identifier>trm_4a3fd79d0a300</dc:identifier>
        <dc:Date>2011-08-14 16:44:43</dc:Date>
        <dc:Contributor>Tyler Davis</dc:Contributor>
        <skos:definition>The processes by which faces are identified as such.</skos:definition>
        <skos:prefLabel>Face perception</skos:prefLabel>
        <skos:hasTopConcept>Perception</skos:hasTopConcept>
    </owl:Class>
    


    <!-- http://www.cognitiveatlas.org/ontology/cogat.owl#CAO_00299 -->

    <owl:Class rdf:about="&cogat;CAO_00299">
        <rdfs:label>Face recognition</rdfs:label>
        <rdfs:subClassOf rdf:resource="&cogat;CAO_00572"/>
        <dc:Date>2011-08-14 16:46:04</dc:Date>
        <skos:hasTopConcept>Learning and Memory</skos:hasTopConcept>
        <dc:Title>Face recognition</dc:Title>
        <skos:definition>The process of determining whether a face is the same as another face that has been previously encountered.</skos:definition>
        <dc:identifier>trm_4a3fd79d0a30c</dc:identifier>
        <skos:altLabel></skos:altLabel>
        <skos:prefLabel>Face recognition</skos:prefLabel>
        <dc:Contributor>Tyler Davis</dc:Contributor>
    </owl:Class>
    


    <!-- http://www.cognitiveatlas.org/ontology/cogat.owl#CAO_00300 -->

    <owl:Class rdf:about="&cogat;CAO_00300">
        <rdfs:label>Facial expression</rdfs:label>
        <rdfs:subClassOf rdf:resource="&cogat;CAO_00001"/>
        <dc:Date>2012-03-28 11:56:58</dc:Date>
        <skos:hasTopConcept>Emotion</skos:hasTopConcept>
        <dc:identifier>trm_4a3fd79d0a318</dc:identifier>
        <skos:prefLabel>Facial expression</skos:prefLabel>
        <skos:altLabel></skos:altLabel>
        <dc:Title>Facial expression</dc:Title>
        <skos:definition>Movements and positions of the facial muscles that can be used as a form of nonverbal communication, particularly in conveying emotional states.</skos:definition>
        <dc:Contributor>Russ Poldrack</dc:Contributor>
    </owl:Class>
    


    <!-- http://www.cognitiveatlas.org/ontology/cogat.owl#CAO_00301 -->

    <owl:Class rdf:about="&cogat;CAO_00301">
        <rdfs:label>False memory</rdfs:label>
        <rdfs:subClassOf rdf:resource="&cogat;CAO_00001"/>
        <skos:altLabel></skos:altLabel>
        <skos:definition>a memory that refers to an event that did not actually occur</skos:definition>
        <dc:Date>2011-04-09 08:15:38</dc:Date>
        <dc:Title>False memory</dc:Title>
        <skos:hasTopConcept>Learning and Memory</skos:hasTopConcept>
        <skos:prefLabel>False memory</skos:prefLabel>
        <dc:Contributor>Russ Poldrack</dc:Contributor>
        <dc:identifier>trm_4a3fd79d0a323</dc:identifier>
    </owl:Class>
    


    <!-- http://www.cognitiveatlas.org/ontology/cogat.owl#CAO_00302 -->

    <owl:Class rdf:about="&cogat;CAO_00302">
        <rdfs:label>Feature extraction</rdfs:label>
        <rdfs:subClassOf rdf:resource="&cogat;CAO_00001"/>
        <skos:hasTopConcept>Perception</skos:hasTopConcept>
        <dc:Date>2012-03-28 11:57:35</dc:Date>
        <dc:Title>Feature extraction</dc:Title>
        <skos:definition>Processes by which relevant aspects of a data stream are separated from irrelevant aspects.</skos:definition>
        <dc:Contributor>Russ Poldrack</dc:Contributor>
        <skos:altLabel></skos:altLabel>
        <dc:identifier>trm_4a3fd79d0a32f</dc:identifier>
        <skos:prefLabel>Feature extraction</skos:prefLabel>
    </owl:Class>
    


    <!-- http://www.cognitiveatlas.org/ontology/cogat.owl#CAO_00303 -->

    <owl:Class rdf:about="&cogat;CAO_00303">
        <rdfs:label>Feedback</rdfs:label>
        <rdfs:subClassOf rdf:resource="&cogat;CAO_00001"/>
        <skos:altLabel></skos:altLabel>
        <skos:prefLabel>Feedback</skos:prefLabel>
        <dc:Contributor>Tyler Davis</dc:Contributor>
        <dc:Title>Feedback</dc:Title>
        <skos:definition>Evaluative or corrective information about an action, event, or process delivered to the original or controlling source, often with the intent of modifying future actions.</skos:definition>
        <dc:identifier>trm_4a3fd79d0a33b</dc:identifier>
        <dc:Date>2011-08-14 17:02:21</dc:Date>
        <skos:hasTopConcept></skos:hasTopConcept>
    </owl:Class>
    


    <!-- http://www.cognitiveatlas.org/ontology/cogat.owl#CAO_00304 -->

    <owl:Class rdf:about="&cogat;CAO_00304">
        <rdfs:label>Filtering</rdfs:label>
        <rdfs:subClassOf rdf:resource="&cogat;CAO_00001"/>
        <skos:definition>a device or process that removes from a signal some unwanted component or feature.</skos:definition>
        <skos:altLabel></skos:altLabel>
        <dc:Date>2011-05-16 13:28:26</dc:Date>
        <dc:Title>Filtering</dc:Title>
        <skos:hasTopConcept></skos:hasTopConcept>
        <dc:Contributor>Brenda Gregory</dc:Contributor>
        <dc:identifier>trm_4a3fd79d0a352</dc:identifier>
        <skos:prefLabel>Filtering</skos:prefLabel>
    </owl:Class>
    


    <!-- http://www.cognitiveatlas.org/ontology/cogat.owl#CAO_00305 -->

    <owl:Class rdf:about="&cogat;CAO_00305">
        <rdfs:label>Fixation</rdfs:label>
        <rdfs:subClassOf rdf:resource="&cogat;CAO_00001"/>
        <skos:definition>Maintaining gaze or attention on some object or event. (Experimental design) A trial period in which a participant is instructed to direct attention toward a visual stimulus (often a cross).</skos:definition>
        <dc:Contributor>Tyler Davis</dc:Contributor>
        <skos:prefLabel>Fixation</skos:prefLabel>
        <dc:identifier>trm_4a3fd79d0a35e</dc:identifier>
        <skos:hasTopConcept>Attention</skos:hasTopConcept>
        <dc:Date>2011-08-14 17:14:56</dc:Date>
        <skos:altLabel></skos:altLabel>
        <dc:Title>Fixation</dc:Title>
    </owl:Class>
    


    <!-- http://www.cognitiveatlas.org/ontology/cogat.owl#CAO_00306 -->

    <owl:Class rdf:about="&cogat;CAO_00306">
        <rdfs:label>Fixed action patterns</rdfs:label>
        <rdfs:subClassOf rdf:resource="&cogat;CAO_00001"/>
        <skos:definition>an instinctive  behavioral  sequence that is indivisible and runs to completion.</skos:definition>
        <skos:altLabel></skos:altLabel>
        <dc:Contributor>Brenda Gregory</dc:Contributor>
        <dc:identifier>trm_4a3fd79d0a36a</dc:identifier>
        <dc:Date>2011-05-10 14:43:33</dc:Date>
        <skos:prefLabel>Fixed action patterns</skos:prefLabel>
        <dc:Title>Fixed action patterns</dc:Title>
        <skos:hasTopConcept></skos:hasTopConcept>
    </owl:Class>
    


    <!-- http://www.cognitiveatlas.org/ontology/cogat.owl#CAO_00307 -->

    <owl:Class rdf:about="&cogat;CAO_00307">
        <rdfs:label>Fluid intelligence</rdfs:label>
        <rdfs:subClassOf rdf:resource="&cogat;CAO_00001"/>
        <skos:hasTopConcept>Reasoning and Decision Making</skos:hasTopConcept>
        <dc:Contributor>Russ Poldrack</dc:Contributor>
        <skos:prefLabel>Fluid intelligence</skos:prefLabel>
        <skos:altLabel></skos:altLabel>
        <dc:Date>2012-03-28 11:59:36</dc:Date>
        <skos:definition>a factor of general intelligence originally identified by Raymond Cattell; Cattell defined fluid intelligence as and#34;…the ability to perceive relationships independent of previous specific practice or instruction concerning those relationships.and#34; Fluid intelligence is the ability to think and reason abstractly and solve problems. This ability is considered independent of learning, experience, and education.</skos:definition>
        <dc:identifier>trm_4a3fd79d0a375</dc:identifier>
        <dc:Title>Fluid intelligence</dc:Title>
    </owl:Class>
    


    <!-- http://www.cognitiveatlas.org/ontology/cogat.owl#CAO_00308 -->

    <owl:Class rdf:about="&cogat;CAO_00308">
        <rdfs:label>Focus</rdfs:label>
        <rdfs:subClassOf rdf:resource="&cogat;CAO_00001"/>
        <skos:definition>The center of attention or concentration. </skos:definition>
        <dc:Date>2011-08-14 17:16:17</dc:Date>
        <dc:Contributor>Tyler Davis</dc:Contributor>
        <skos:hasTopConcept>Attention</skos:hasTopConcept>
        <dc:Title>Focus</dc:Title>
        <skos:prefLabel>Focus</skos:prefLabel>
        <dc:identifier>trm_4a3fd79d0a381</dc:identifier>
        <skos:altLabel></skos:altLabel>
    </owl:Class>
    


    <!-- http://www.cognitiveatlas.org/ontology/cogat.owl#CAO_00309 -->

    <owl:Class rdf:about="&cogat;CAO_00309">
        <rdfs:label>Focused attention</rdfs:label>
        <rdfs:subClassOf rdf:resource="&cogat;CAO_00001"/>
        <skos:prefLabel>Focused attention</skos:prefLabel>
        <skos:hasTopConcept>Attention</skos:hasTopConcept>
        <dc:Title>Focused attention</dc:Title>
        <dc:Date>2011-04-29 11:01:09</dc:Date>
        <skos:altLabel></skos:altLabel>
        <dc:Contributor>Brenda Gregory</dc:Contributor>
        <skos:definition>the ability to respond discretely to specific visual, auditory or tactile stimuli.</skos:definition>
        <dc:identifier>trm_4a3fd79d0a38d</dc:identifier>
    </owl:Class>
    


    <!-- http://www.cognitiveatlas.org/ontology/cogat.owl#CAO_00310 -->

    <owl:Class rdf:about="&cogat;CAO_00310">
        <rdfs:label>Form perception</rdfs:label>
        <rdfs:subClassOf rdf:resource="&cogat;CAO_00001"/>
        <rdfs:subClassOf>
            <owl:Restriction>
                <owl:onProperty rdf:resource="&ro;part_of"/>
                <owl:someValuesFrom rdf:resource="&cogat;CAO_00427"/>
            </owl:Restriction>
        </rdfs:subClassOf>
        <skos:definition>the sensory discrimination of a pattern, shape or outline.</skos:definition>
        <skos:hasTopConcept>Perception</skos:hasTopConcept>
        <dc:Title>Form perception</dc:Title>
        <skos:prefLabel>Form perception</skos:prefLabel>
        <dc:Date>2011-04-28 16:16:53</dc:Date>
        <skos:altLabel></skos:altLabel>
        <dc:identifier>trm_4a3fd79d0a398</dc:identifier>
        <dc:Contributor>Brenda Gregory</dc:Contributor>
    </owl:Class>
    


    <!-- http://www.cognitiveatlas.org/ontology/cogat.owl#CAO_00311 -->

    <owl:Class rdf:about="&cogat;CAO_00311">
        <rdfs:label>Functional fixedness</rdfs:label>
        <rdfs:subClassOf rdf:resource="&cogat;CAO_00001"/>
        <dc:Contributor>Russ Poldrack</dc:Contributor>
        <skos:altLabel></skos:altLabel>
        <dc:identifier>trm_4a3fd79d0a3a4</dc:identifier>
        <skos:definition>a cognitive bias that limits a person to using an object only in the way it is traditionally used.</skos:definition>
        <dc:Date>2012-03-28 12:00:29</dc:Date>
        <dc:Title>Functional fixedness</dc:Title>
        <skos:prefLabel>Functional fixedness</skos:prefLabel>
        <skos:hasTopConcept>Reasoning and Decision Making</skos:hasTopConcept>
    </owl:Class>
    


    <!-- http://www.cognitiveatlas.org/ontology/cogat.owl#CAO_00312 -->

    <owl:Class rdf:about="&cogat;CAO_00312">
        <rdfs:label>Gaze</rdfs:label>
        <rdfs:subClassOf rdf:resource="&cogat;CAO_00305"/>
        <skos:definition>The act of fixating the eyes onto a location.  </skos:definition>
        <dc:Title>Gaze</dc:Title>
        <dc:Contributor>Tyler Davis</dc:Contributor>
        <skos:hasTopConcept></skos:hasTopConcept>
        <dc:identifier>trm_4a3fd79d0a3d2</dc:identifier>
        <skos:prefLabel>Gaze</skos:prefLabel>
        <dc:Date>2011-08-15 09:46:09</dc:Date>
        <skos:altLabel></skos:altLabel>
    </owl:Class>
    


    <!-- http://www.cognitiveatlas.org/ontology/cogat.owl#CAO_00313 -->

    <owl:Class rdf:about="&cogat;CAO_00313">
        <rdfs:label>Generalization</rdfs:label>
        <rdfs:subClassOf rdf:resource="&cogat;CAO_00346"/>
        <skos:altLabel></skos:altLabel>
        <skos:definition>The act of transferring knowledge learned from one event to a novel event that is similar in some respect.</skos:definition>
        <skos:prefLabel>Generalization</skos:prefLabel>
        <dc:Date>2011-08-15 09:52:59</dc:Date>
        <dc:Title>Generalization</dc:Title>
        <dc:identifier>trm_4a3fd79d0a3ea</dc:identifier>
        <dc:Contributor>Tyler Davis</dc:Contributor>
        <skos:hasTopConcept>Learning and Memory</skos:hasTopConcept>
    </owl:Class>
    


    <!-- http://www.cognitiveatlas.org/ontology/cogat.owl#CAO_00314 -->

    <owl:Class rdf:about="&cogat;CAO_00314">
        <rdfs:label>Generic knowledge</rdfs:label>
        <rdfs:subClassOf rdf:resource="&cogat;CAO_00001"/>
        <skos:hasTopConcept>Reasoning and Decision Making</skos:hasTopConcept>
        <skos:prefLabel>Generic knowledge</skos:prefLabel>
        <dc:Contributor>Ricardo Sanz</dc:Contributor>
        <dc:Title>Generic knowledge</dc:Title>
        <dc:Date>2011-03-15 14:04:58</dc:Date>
        <skos:altLabel></skos:altLabel>
        <skos:definition>Generic knowledge is knowledge that is applicable not just to a single entity but to a class of entities. </skos:definition>
        <dc:identifier>trm_4a3fd79d0a3f6</dc:identifier>
    </owl:Class>
    


    <!-- http://www.cognitiveatlas.org/ontology/cogat.owl#CAO_00315 -->

    <owl:Class rdf:about="&cogat;CAO_00315">
        <rdfs:label>Gestalt</rdfs:label>
        <rdfs:subClassOf rdf:resource="&cogat;CAO_00001"/>
        <skos:altLabel></skos:altLabel>
        <dc:Contributor>Russ Poldrack</dc:Contributor>
        <dc:Date>2012-03-28 12:00:57</dc:Date>
        <dc:Title>Gestalt</dc:Title>
        <skos:hasTopConcept>Perception</skos:hasTopConcept>
        <skos:definition>a collection of physical, biological, psychological or symbolic entities that creates a unified concept, configuration or pattern which is greater than the sum of its parts (of a character, personality, or being).</skos:definition>
        <dc:identifier>trm_4a3fd79d0a402</dc:identifier>
        <skos:prefLabel>Gestalt</skos:prefLabel>
    </owl:Class>
    


    <!-- http://www.cognitiveatlas.org/ontology/cogat.owl#CAO_00316 -->

    <owl:Class rdf:about="&cogat;CAO_00316">
        <rdfs:label>Goal</rdfs:label>
        <rdfs:subClassOf rdf:resource="&cogat;CAO_00001"/>
        <skos:hasTopConcept>Executive-Cognitive Control</skos:hasTopConcept>
        <skos:prefLabel>Goal</skos:prefLabel>
        <dc:Contributor>Russ Poldrack</dc:Contributor>
        <skos:altLabel></skos:altLabel>
        <dc:Date>2012-03-28 12:01:34</dc:Date>
        <skos:definition>The desired end-point of behavior(s).</skos:definition>
        <dc:identifier>trm_4a3fd79d0a419</dc:identifier>
        <dc:Title>Goal</dc:Title>
    </owl:Class>
    


    <!-- http://www.cognitiveatlas.org/ontology/cogat.owl#CAO_00317 -->

    <owl:Class rdf:about="&cogat;CAO_00317">
        <rdfs:label>Goal formation</rdfs:label>
        <rdfs:subClassOf rdf:resource="&cogat;CAO_00001"/>
        <skos:definition>The processes that create and maintain representations of goal states.</skos:definition>
        <dc:Title>Goal formation</dc:Title>
        <dc:Date>2012-03-28 12:01:09</dc:Date>
        <dc:identifier>trm_4a3fd79d0a425</dc:identifier>
        <dc:Contributor>Russ Poldrack</dc:Contributor>
        <skos:prefLabel>Goal formation</skos:prefLabel>
        <skos:hasTopConcept>Executive-Cognitive Control</skos:hasTopConcept>
        <skos:altLabel></skos:altLabel>
    </owl:Class>
    


    <!-- http://www.cognitiveatlas.org/ontology/cogat.owl#CAO_00318 -->

    <owl:Class rdf:about="&cogat;CAO_00318">
        <rdfs:label>Goal maintenance</rdfs:label>
        <rdfs:subClassOf rdf:resource="&cogat;CAO_00001"/>
        <dc:Date>2010-07-14 11:46:12</dc:Date>
        <dc:Contributor>Russ Poldrack</dc:Contributor>
        <skos:hasTopConcept>Executive-Cognitive Control</skos:hasTopConcept>
        <skos:prefLabel>Goal maintenance</skos:prefLabel>
        <skos:altLabel></skos:altLabel>
        <dc:Title>Goal maintenance</dc:Title>
        <dc:identifier>trm_4a3fd79d0a431</dc:identifier>
        <skos:definition>The maintenance of information regarding task goals in working memory.</skos:definition>
    </owl:Class>
    


    <!-- http://www.cognitiveatlas.org/ontology/cogat.owl#CAO_00319 -->

    <owl:Class rdf:about="&cogat;CAO_00319">
        <rdfs:label>Goal management</rdfs:label>
        <rdfs:subClassOf rdf:resource="&cogat;CAO_00001"/>
        <skos:altLabel></skos:altLabel>
        <skos:prefLabel>Goal management</skos:prefLabel>
        <skos:definition>consists of the process of recognizing or inferring goals, abandoning no longer relevant goals, identifying and resolving conflicts among goals, and prioritizing goals consistently for optimal success.</skos:definition>
        <dc:identifier>trm_4a3fd79d0a43c</dc:identifier>
        <dc:Title>Goal management</dc:Title>
        <skos:hasTopConcept>Executive-Cognitive Control</skos:hasTopConcept>
        <dc:Contributor>Russ Poldrack</dc:Contributor>
        <dc:Date>2012-03-28 12:01:22</dc:Date>
    </owl:Class>
    


    <!-- http://www.cognitiveatlas.org/ontology/cogat.owl#CAO_00320 -->

    <owl:Class rdf:about="&cogat;CAO_00320">
        <rdfs:label>Goal state</rdfs:label>
        <rdfs:subClassOf rdf:resource="&cogat;CAO_00001"/>
        <skos:definition>A point reached when goal directed behavior has successfully concluded. </skos:definition>
        <skos:hasTopConcept>Executive-Cognitive Control</skos:hasTopConcept>
        <dc:Date>2012-03-28 12:01:45</dc:Date>
        <dc:identifier>trm_4a3fd79d0a448</dc:identifier>
        <dc:Title>Goal state</dc:Title>
        <skos:altLabel></skos:altLabel>
        <skos:prefLabel>Goal state</skos:prefLabel>
        <dc:Contributor>Russ Poldrack</dc:Contributor>
    </owl:Class>
    


    <!-- http://www.cognitiveatlas.org/ontology/cogat.owl#CAO_00321 -->

    <owl:Class rdf:about="&cogat;CAO_00321">
        <rdfs:label>Gustatory learning</rdfs:label>
        <rdfs:subClassOf rdf:resource="&cogat;CAO_00377"/>
        <dc:identifier>trm_4a3fd79d0a460</dc:identifier>
        <skos:hasTopConcept>Learning and Memory</skos:hasTopConcept>
        <dc:Date>2011-08-15 10:06:15</dc:Date>
        <dc:Contributor>Tyler Davis</dc:Contributor>
        <skos:definition>The formation of a knowledge representation that contains information about gustatory percepts.</skos:definition>
        <skos:altLabel></skos:altLabel>
        <skos:prefLabel>Gustatory learning</skos:prefLabel>
        <dc:Title>Gustatory learning</dc:Title>
    </owl:Class>
    


    <!-- http://www.cognitiveatlas.org/ontology/cogat.owl#CAO_00322 -->

    <owl:Class rdf:about="&cogat;CAO_00322">
        <rdfs:label>Gustatory memory</rdfs:label>
        <rdfs:subClassOf rdf:resource="&cogat;CAO_00001"/>
        <skos:hasTopConcept>Learning and Memory</skos:hasTopConcept>
        <skos:prefLabel>Gustatory memory</skos:prefLabel>
        <dc:Date>2011-02-25 09:42:35</dc:Date>
        <skos:altLabel></skos:altLabel>
        <dc:Title>Gustatory memory</dc:Title>
        <skos:definition>the cognitive capacity of storing and retrieving information related to taste.  </skos:definition>
        <dc:Contributor>Natalie Picchetti</dc:Contributor>
        <dc:identifier>trm_4a3fd79d0a46b</dc:identifier>
    </owl:Class>
    


    <!-- http://www.cognitiveatlas.org/ontology/cogat.owl#CAO_00323 -->

    <owl:Class rdf:about="&cogat;CAO_00323">
        <rdfs:label>Gustatory perception</rdfs:label>
        <rdfs:subClassOf rdf:resource="&cogat;CAO_00001"/>
        <dc:Title>Gustatory perception</dc:Title>
        <skos:prefLabel>Gustatory perception</skos:prefLabel>
        <dc:identifier>trm_4a3fd79d0a477</dc:identifier>
        <dc:Date>2011-08-15 10:08:25</dc:Date>
        <skos:definition>The processes involved with representing gustatory sensations as such.</skos:definition>
        <skos:altLabel></skos:altLabel>
        <dc:Contributor>Tyler Davis</dc:Contributor>
        <skos:hasTopConcept>Perception</skos:hasTopConcept>
    </owl:Class>
    


    <!-- http://www.cognitiveatlas.org/ontology/cogat.owl#CAO_00324 -->

    <owl:Class rdf:about="&cogat;CAO_00324">
        <rdfs:label>Habit</rdfs:label>
        <rdfs:subClassOf rdf:resource="&cogat;CAO_00001"/>
        <skos:altLabel></skos:altLabel>
        <dc:Contributor>Agatha Lenartowicz</dc:Contributor>
        <dc:Title>Habit</dc:Title>
        <skos:hasTopConcept>Learning and Memory</skos:hasTopConcept>
        <dc:Date>2009-07-10 14:06:31</dc:Date>
        <skos:prefLabel>Habit</skos:prefLabel>
        <skos:definition>An acquired pattern of behavior that often occurs automatically and is reliably triggered by some event or stimulus.</skos:definition>
        <dc:identifier>trm_4a3fd79d0a483</dc:identifier>
    </owl:Class>
    


    <!-- http://www.cognitiveatlas.org/ontology/cogat.owl#CAO_00325 -->

    <owl:Class rdf:about="&cogat;CAO_00325">
        <rdfs:label>Habit learning</rdfs:label>
        <rdfs:subClassOf rdf:resource="&cogat;CAO_00001"/>
        <skos:altLabel></skos:altLabel>
        <dc:Contributor>Russ Poldrack</dc:Contributor>
        <dc:Title>Habit learning</dc:Title>
        <skos:hasTopConcept>Learning and Memory</skos:hasTopConcept>
        <skos:definition>The process of acquiring a habit</skos:definition>
        <dc:identifier>trm_4a3fd79d0a48e</dc:identifier>
        <skos:prefLabel>Habit learning</skos:prefLabel>
        <dc:Date>2012-03-28 12:50:34</dc:Date>
    </owl:Class>
    


    <!-- http://www.cognitiveatlas.org/ontology/cogat.owl#CAO_00326 -->

    <owl:Class rdf:about="&cogat;CAO_00326">
        <rdfs:label>Habit memory</rdfs:label>
        <rdfs:subClassOf rdf:resource="&cogat;CAO_00001"/>
        <dc:identifier>trm_4a3fd79d0a49a</dc:identifier>
        <skos:hasTopConcept>Learning and Memory</skos:hasTopConcept>
        <skos:altLabel></skos:altLabel>
        <dc:Date>2012-03-28 12:51:14</dc:Date>
        <skos:definition>the memory representation of a learned habit, generally thought to be represented as a stimulus-response association</skos:definition>
        <dc:Title>Habit memory</dc:Title>
        <skos:prefLabel>Habit memory</skos:prefLabel>
        <dc:Contributor>Russ Poldrack</dc:Contributor>
    </owl:Class>
    


    <!-- http://www.cognitiveatlas.org/ontology/cogat.owl#CAO_00327 -->

    <owl:Class rdf:about="&cogat;CAO_00327">
        <rdfs:label>Hallucination</rdfs:label>
        <rdfs:subClassOf rdf:resource="&cogat;CAO_00001"/>
        <skos:definition>in the broadest sense of the word, is a perception in the absence of a stimulus. In a stricter sense, hallucinations are defined as perceptions in a conscious and awake state in the absence of external stimuli which have qualities of real perception, in that they are vivid, substantial, and located in external objective space.  </skos:definition>
        <dc:Date>2011-04-12 09:33:17</dc:Date>
        <dc:Contributor>Natalie Picchetti</dc:Contributor>
        <dc:Title>Hallucination</dc:Title>
        <skos:hasTopConcept></skos:hasTopConcept>
        <dc:identifier>trm_4a3fd79d0a4a6</dc:identifier>
        <skos:prefLabel>Hallucination</skos:prefLabel>
        <skos:altLabel></skos:altLabel>
    </owl:Class>
    


    <!-- http://www.cognitiveatlas.org/ontology/cogat.owl#CAO_00328 -->

    <owl:Class rdf:about="&cogat;CAO_00328">
        <rdfs:label>Hedonism</rdfs:label>
        <rdfs:subClassOf rdf:resource="&cogat;CAO_00001"/>
        <skos:altLabel></skos:altLabel>
        <skos:prefLabel>Hedonism</skos:prefLabel>
        <dc:Contributor>Brenda Gregory</dc:Contributor>
        <dc:Date>2011-04-19 12:19:27</dc:Date>
        <dc:identifier>trm_4a3fd79d0a4b2</dc:identifier>
        <skos:definition>a school which argues that pleasure is the only intrinsic good, often used as a justification for evaluating actions in terms of how much pleasure and how little pain (i.e. suffering) they produce.</skos:definition>
        <dc:Title>Hedonism</dc:Title>
        <skos:hasTopConcept></skos:hasTopConcept>
    </owl:Class>
    


    <!-- http://www.cognitiveatlas.org/ontology/cogat.owl#CAO_00329 -->

    <owl:Class rdf:about="&cogat;CAO_00329">
        <rdfs:label>Heuristic search</rdfs:label>
        <rdfs:subClassOf rdf:resource="&cogat;CAO_00001"/>
        <skos:prefLabel>Heuristic search</skos:prefLabel>
        <dc:Contributor>Russ Poldrack</dc:Contributor>
        <skos:definition>refers to experience-based techniques for problem solving, learning, and discovery. Heuristic methods are used to speed up the process of finding a good enough solution, where an exhaustive search is impractical. Examples of this method include using a and#34;rule of thumband#34;, an educated guess, an intuitive judgment, or common sense.  In more precise terms, heuristics are strategies using readily accessible, though loosely applicable, information to control problem solving in human beings and machines</skos:definition>
        <dc:identifier>trm_4a3fd79d0a4be</dc:identifier>
        <skos:altLabel></skos:altLabel>
        <dc:Title>Heuristic search</dc:Title>
        <dc:Date>2012-03-28 12:52:13</dc:Date>
        <skos:hasTopConcept>Reasoning and Decision Making</skos:hasTopConcept>
    </owl:Class>
    


    <!-- http://www.cognitiveatlas.org/ontology/cogat.owl#CAO_00330 -->

    <owl:Class rdf:about="&cogat;CAO_00330">
        <rdfs:label>Hill climbing</rdfs:label>
        <rdfs:subClassOf rdf:resource="&cogat;CAO_00001"/>
        <skos:prefLabel>Hill climbing</skos:prefLabel>
        <skos:altLabel></skos:altLabel>
        <dc:Title>Hill climbing</dc:Title>
        <dc:Contributor>Russ Poldrack</dc:Contributor>
        <dc:identifier>trm_4a3fd79d0a4c9</dc:identifier>
        <skos:hasTopConcept>Reasoning and Decision Making</skos:hasTopConcept>
        <dc:Date>2012-03-28 12:52:23</dc:Date>
        <skos:definition>A fast but sometimes unreliable optimization method.  When searching for the minimum-maximum value of a function a random step is taken; if the value improves it replaces the current value, then another random step is taken.</skos:definition>
    </owl:Class>
    


    <!-- http://www.cognitiveatlas.org/ontology/cogat.owl#CAO_00331 -->

    <owl:Class rdf:about="&cogat;CAO_00331">
        <rdfs:label>Humiliation</rdfs:label>
        <rdfs:subClassOf rdf:resource="&cogat;CAO_00001"/>
        <dc:Contributor>Russ Poldrack</dc:Contributor>
        <dc:identifier>trm_4a3fd79d0a4e1</dc:identifier>
        <skos:altLabel></skos:altLabel>
        <dc:Date>2012-03-28 12:52:38</dc:Date>
        <skos:definition>to reduce to a lower position in oneand#39;s own eyes or othersand#39; eyes.</skos:definition>
        <skos:prefLabel>Humiliation</skos:prefLabel>
        <dc:Title>Humiliation</dc:Title>
        <skos:hasTopConcept>Emotion</skos:hasTopConcept>
    </owl:Class>
    


    <!-- http://www.cognitiveatlas.org/ontology/cogat.owl#CAO_00332 -->

    <owl:Class rdf:about="&cogat;CAO_00332">
        <rdfs:label>Humor</rdfs:label>
        <rdfs:subClassOf rdf:resource="&cogat;CAO_00001"/>
        <dc:Contributor>Russ Poldrack</dc:Contributor>
        <dc:Date>2012-03-28 12:52:47</dc:Date>
        <dc:Title>Humor</dc:Title>
        <skos:altLabel></skos:altLabel>
        <skos:hasTopConcept>Emotion</skos:hasTopConcept>
        <skos:definition>the tendency of particular cognitive experiences to provoke laughter  and provide amusement.</skos:definition>
        <skos:prefLabel>Humor</skos:prefLabel>
        <dc:identifier>trm_4a3fd79d0a4ed</dc:identifier>
    </owl:Class>
    


    <!-- http://www.cognitiveatlas.org/ontology/cogat.owl#CAO_00333 -->

    <owl:Class rdf:about="&cogat;CAO_00333">
        <rdfs:label>Iconic memory</rdfs:label>
        <rdfs:subClassOf rdf:resource="&cogat;CAO_00571"/>
        <skos:altLabel></skos:altLabel>
        <dc:Date>2011-05-04 11:01:59</dc:Date>
        <dc:Title>Iconic memory</dc:Title>
        <dc:Contributor>Brenda Gregory</dc:Contributor>
        <dc:identifier>trm_4a3fd79d0a4f9</dc:identifier>
        <skos:definition>very brief sensory memory of some visual stimuli, that occur in the form of mental pictures.</skos:definition>
        <skos:hasTopConcept>Learning and Memory</skos:hasTopConcept>
        <skos:prefLabel>Iconic memory</skos:prefLabel>
    </owl:Class>
    


    <!-- http://www.cognitiveatlas.org/ontology/cogat.owl#CAO_00334 -->

    <owl:Class rdf:about="&cogat;CAO_00334">
        <rdfs:label>Imageability</rdfs:label>
        <rdfs:subClassOf rdf:resource="&cogat;CAO_00001"/>
        <rdfs:subClassOf>
            <owl:Restriction>
                <owl:onProperty rdf:resource="&ro;part_of"/>
                <owl:someValuesFrom rdf:resource="&cogat;CAO_00372"/>
            </owl:Restriction>
        </rdfs:subClassOf>
        <dc:Date>2011-03-25 13:27:04</dc:Date>
        <skos:prefLabel>Imageability</skos:prefLabel>
        <skos:definition>is a property of a word or concept reflecting how easy or difficult it is to visually or acoustically imagine.  </skos:definition>
        <skos:hasTopConcept></skos:hasTopConcept>
        <dc:Contributor>Jianhui Wu</dc:Contributor>
        <dc:identifier>trm_4a3fd79d0a504</dc:identifier>
        <dc:Title>Imageability</dc:Title>
        <skos:altLabel></skos:altLabel>
    </owl:Class>
    


    <!-- http://www.cognitiveatlas.org/ontology/cogat.owl#CAO_00335 -->

    <owl:Class rdf:about="&cogat;CAO_00335">
        <rdfs:label>Imagery</rdfs:label>
        <rdfs:subClassOf rdf:resource="&cogat;CAO_00001"/>
        <dc:Title>Imagery</dc:Title>
        <skos:hasTopConcept></skos:hasTopConcept>
        <dc:Date>2011-04-29 16:17:03</dc:Date>
        <dc:Contributor>Brenda Gregory</dc:Contributor>
        <dc:identifier>trm_4a3fd79d0a510</dc:identifier>
        <skos:prefLabel>Imagery</skos:prefLabel>
        <skos:altLabel></skos:altLabel>
        <skos:definition>an experience that, on most occasions, significantly resembles the experience of perceiving some object, event, or scene, but occurs when the relevant object, event, or scene is not actually present to the senses.</skos:definition>
    </owl:Class>
    


    <!-- http://www.cognitiveatlas.org/ontology/cogat.owl#CAO_00336 -->

    <owl:Class rdf:about="&cogat;CAO_00336">
        <rdfs:label>Implicit knowledge</rdfs:label>
        <rdfs:subClassOf rdf:resource="&cogat;CAO_00371"/>
        <skos:definition>knowledge that is kept in a person’s mind without necessarily being expressed in words and is often acted on instinctively.</skos:definition>
        <dc:Title>Implicit knowledge</dc:Title>
        <dc:Contributor>Brenda Gregory</dc:Contributor>
        <skos:prefLabel>Implicit knowledge</skos:prefLabel>
        <skos:altLabel></skos:altLabel>
        <skos:hasTopConcept></skos:hasTopConcept>
        <dc:Date>2011-05-16 13:22:21</dc:Date>
        <dc:identifier>trm_4a3fd79d0a51c</dc:identifier>
    </owl:Class>
    


    <!-- http://www.cognitiveatlas.org/ontology/cogat.owl#CAO_00337 -->

    <owl:Class rdf:about="&cogat;CAO_00337">
        <rdfs:label>Implicit memory</rdfs:label>
        <rdfs:subClassOf rdf:resource="&cogat;CAO_00394"/>
        <skos:prefLabel>Implicit memory</skos:prefLabel>
        <skos:hasTopConcept>Learning and Memory</skos:hasTopConcept>
        <skos:altLabel></skos:altLabel>
        <dc:Date>2009-07-10 14:06:31</dc:Date>
        <dc:Title>Implicit memory</dc:Title>
        <skos:definition>Type of memory in which experiences increases performance of task without oneand#39;s conscious awareness of these previous experiences. This type of memory applies to habit learning, skills, conditioning.</skos:definition>
        <dc:identifier>trm_4a3fd79d0a533</dc:identifier>
        <dc:Contributor>Agatha Lenartowicz</dc:Contributor>
    </owl:Class>
    


    <!-- http://www.cognitiveatlas.org/ontology/cogat.owl#CAO_00338 -->

    <owl:Class rdf:about="&cogat;CAO_00338">
        <rdfs:label>Imprinting</rdfs:label>
        <rdfs:subClassOf rdf:resource="&cogat;CAO_00001"/>
        <skos:hasTopConcept></skos:hasTopConcept>
        <skos:definition>a rapid learning process that takes place early in the life of a social animal and establishes a behavior pattern (as recognition of and attraction to its own kind or a substitute).</skos:definition>
        <skos:altLabel></skos:altLabel>
        <dc:Date>2011-05-18 14:23:31</dc:Date>
        <skos:prefLabel>Imprinting</skos:prefLabel>
        <dc:Title>Imprinting</dc:Title>
        <dc:Contributor>Brenda Gregory</dc:Contributor>
        <dc:identifier>trm_4a3fd79d0a53f</dc:identifier>
    </owl:Class>
    


    <!-- http://www.cognitiveatlas.org/ontology/cogat.owl#CAO_00339 -->

    <owl:Class rdf:about="&cogat;CAO_00339">
        <rdfs:label>Inattention</rdfs:label>
        <rdfs:subClassOf rdf:resource="&cogat;CAO_00001"/>
        <dc:Title>Inattention</dc:Title>
        <skos:prefLabel>Inattention</skos:prefLabel>
        <dc:identifier>trm_4a3fd79d0a54b</dc:identifier>
        <skos:altLabel></skos:altLabel>
        <skos:hasTopConcept>Attention</skos:hasTopConcept>
        <dc:Contributor>Agatha Lenartowicz</dc:Contributor>
        <skos:definition>The failure to process an external stimulus (often refers to sensory stimuli).</skos:definition>
        <dc:Date>2009-07-10 14:06:31</dc:Date>
    </owl:Class>
    


    <!-- http://www.cognitiveatlas.org/ontology/cogat.owl#CAO_00340 -->

    <owl:Class rdf:about="&cogat;CAO_00340">
        <rdfs:label>Incidental learning</rdfs:label>
        <rdfs:subClassOf rdf:resource="&cogat;CAO_00377"/>
        <skos:definition>Learning without explicit knowledge of doing so, but occurring through interaction with the environment (e.g., by observation-copying of behavior or response to reinforcement).</skos:definition>
        <skos:hasTopConcept>Learning and Memory</skos:hasTopConcept>
        <skos:altLabel></skos:altLabel>
        <skos:prefLabel>Incidental learning</skos:prefLabel>
        <dc:Contributor>Agatha Lenartowicz</dc:Contributor>
        <dc:identifier>trm_4a3fd79d0a556</dc:identifier>
        <dc:Date>2009-12-21 14:32:56</dc:Date>
        <dc:Title>Incidental learning</dc:Title>
    </owl:Class>
    


    <!-- http://www.cognitiveatlas.org/ontology/cogat.owl#CAO_00341 -->

    <owl:Class rdf:about="&cogat;CAO_00341">
        <rdfs:label>Incubation</rdfs:label>
        <rdfs:subClassOf rdf:resource="&cogat;CAO_00001"/>
        <dc:Contributor>Russ Poldrack</dc:Contributor>
        <skos:prefLabel>Incubation</skos:prefLabel>
        <dc:Title>Incubation</dc:Title>
        <dc:Date>2012-03-28 17:02:50</dc:Date>
        <dc:identifier>trm_4a3fd79d0a562</dc:identifier>
        <skos:hasTopConcept>Reasoning and Decision Making</skos:hasTopConcept>
        <skos:altLabel></skos:altLabel>
        <skos:definition>the process of thinking about a problem subconsciously while being involved in other activities</skos:definition>
    </owl:Class>
    


    <!-- http://www.cognitiveatlas.org/ontology/cogat.owl#CAO_00342 -->

    <owl:Class rdf:about="&cogat;CAO_00342">
        <rdfs:label>Indignation</rdfs:label>
        <rdfs:subClassOf rdf:resource="&cogat;CAO_00001"/>
        <dc:Contributor>Russ Poldrack</dc:Contributor>
        <skos:definition>anger aroused by something unjust, unworthy, or mean.</skos:definition>
        <skos:altLabel></skos:altLabel>
        <skos:hasTopConcept>Emotion</skos:hasTopConcept>
        <skos:prefLabel>Indignation</skos:prefLabel>
        <dc:Title>Indignation</dc:Title>
        <dc:Date>2012-03-28 17:03:07</dc:Date>
        <dc:identifier>trm_4a3fd79d0a56e</dc:identifier>
    </owl:Class>
    


    <!-- http://www.cognitiveatlas.org/ontology/cogat.owl#CAO_00343 -->

    <owl:Class rdf:about="&cogat;CAO_00343">
        <rdfs:label>Induction</rdfs:label>
        <rdfs:subClassOf rdf:resource="&cogat;CAO_00001"/>
        <skos:prefLabel>Induction</skos:prefLabel>
        <skos:hasTopConcept></skos:hasTopConcept>
        <dc:Title>Induction</dc:Title>
        <skos:altLabel></skos:altLabel>
        <skos:definition>No definition submitted yet</skos:definition>
        <dc:Contributor>System Administrator</dc:Contributor>
        <dc:identifier>trm_4a3fd79d0a579</dc:identifier>
        <dc:Date>2009-07-10 14:06:31</dc:Date>
    </owl:Class>
    


    <!-- http://www.cognitiveatlas.org/ontology/cogat.owl#CAO_00345 -->

    <owl:Class rdf:about="&cogat;CAO_00345">
        <rdfs:label>Inductive reasoning</rdfs:label>
        <rdfs:subClassOf rdf:resource="&cogat;CAO_00346"/>
        <skos:hasTopConcept>Reasoning and Decision Making</skos:hasTopConcept>
        <dc:Title>Inductive reasoning</dc:Title>
        <skos:altLabel>inductive inference</skos:altLabel>
        <skos:definition>reasoning from a specific case or cases and deriving a general rule, drawing inferences from observations in order to make generalizations. </skos:definition>
        <skos:prefLabel>Inductive reasoning</skos:prefLabel>
        <dc:identifier>trm_4a3fd79d0a590</dc:identifier>
        <dc:Date>2012-03-28 17:04:17</dc:Date>
        <dc:Contributor>Russ Poldrack</dc:Contributor>
    </owl:Class>
    


    <!-- http://www.cognitiveatlas.org/ontology/cogat.owl#CAO_00346 -->

    <owl:Class rdf:about="&cogat;CAO_00346">
        <rdfs:label>Inference</rdfs:label>
        <rdfs:subClassOf rdf:resource="&cogat;CAO_00001"/>
        <skos:prefLabel>Inference</skos:prefLabel>
        <dc:identifier>trm_4a3fd79d0a5ed</dc:identifier>
        <skos:altLabel></skos:altLabel>
        <skos:definition>the act of passing from one proposition, statement, or judgment considered as true to another whose truth is believed to follow from that of the former; the act of passing from statistical sample data to generalizations (as of the value of population parameters) usually with calculated degrees of certainty.</skos:definition>
        <dc:Date>2012-03-28 17:04:58</dc:Date>
        <dc:Contributor>Russ Poldrack</dc:Contributor>
        <dc:Title>Inference</dc:Title>
        <skos:hasTopConcept>Reasoning and Decision Making</skos:hasTopConcept>
    </owl:Class>
    


    <!-- http://www.cognitiveatlas.org/ontology/cogat.owl#CAO_00347 -->

    <owl:Class rdf:about="&cogat;CAO_00347">
        <rdfs:label>Inhibition</rdfs:label>
        <rdfs:subClassOf rdf:resource="&cogat;CAO_00001"/>
        <dc:Title>Inhibition</dc:Title>
        <dc:Date>2012-03-28 17:05:31</dc:Date>
        <skos:hasTopConcept>Executive-Cognitive Control</skos:hasTopConcept>
        <skos:definition>The process by which a response or thought is suppressed.</skos:definition>
        <skos:altLabel></skos:altLabel>
        <skos:prefLabel>Inhibition</skos:prefLabel>
        <dc:Contributor>Russ Poldrack</dc:Contributor>
        <dc:identifier>trm_4a3fd79d0a613</dc:identifier>
    </owl:Class>
    


    <!-- http://www.cognitiveatlas.org/ontology/cogat.owl#CAO_00348 -->

    <owl:Class rdf:about="&cogat;CAO_00348">
        <rdfs:label>Inhibition of return</rdfs:label>
        <rdfs:subClassOf rdf:resource="&cogat;CAO_00001"/>
        <skos:hasTopConcept>Executive-Cognitive Control</skos:hasTopConcept>
        <dc:Title>Inhibition of return</dc:Title>
        <skos:definition>the phenomenon in which the speed and accuracy with which an object is detected are first briefly enhanced (for perhaps 100-300 milliseconds) after the object is attended, and then detection speed and accuracy are impaired (for perhaps 500-3000 milliseconds).</skos:definition>
        <dc:Contributor>Russ Poldrack</dc:Contributor>
        <dc:identifier>trm_4a3fd79d0a61f</dc:identifier>
        <dc:Date>2012-03-28 17:06:11</dc:Date>
        <skos:altLabel></skos:altLabel>
        <skos:prefLabel>Inhibition of return</skos:prefLabel>
    </owl:Class>
    


    <!-- http://www.cognitiveatlas.org/ontology/cogat.owl#CAO_00349 -->

    <owl:Class rdf:about="&cogat;CAO_00349">
        <rdfs:label>Insight</rdfs:label>
        <rdfs:subClassOf rdf:resource="&cogat;CAO_00001"/>
        <skos:definition>In problem solving, the moment at which an underlying relation between cause and effect is discovered-identified.</skos:definition>
        <skos:hasTopConcept>Reasoning and Decision Making</skos:hasTopConcept>
        <dc:Title>Insight</dc:Title>
        <skos:altLabel></skos:altLabel>
        <dc:identifier>trm_4a3fd79d0a62b</dc:identifier>
        <dc:Date>2009-07-10 14:06:31</dc:Date>
        <dc:Contributor>Agatha Lenartowicz</dc:Contributor>
        <skos:prefLabel>Insight</skos:prefLabel>
    </owl:Class>
    


    <!-- http://www.cognitiveatlas.org/ontology/cogat.owl#CAO_00350 -->

    <owl:Class rdf:about="&cogat;CAO_00350">
        <rdfs:label>Instinct</rdfs:label>
        <rdfs:subClassOf rdf:resource="&cogat;CAO_00001"/>
        <dc:Date>2011-04-28 12:21:03</dc:Date>
        <dc:Title>Instinct</dc:Title>
        <skos:altLabel></skos:altLabel>
        <dc:identifier>trm_4a3fd79d0a637</dc:identifier>
        <skos:hasTopConcept></skos:hasTopConcept>
        <dc:Contributor>Brenda Gregory</dc:Contributor>
        <skos:definition>a natural or inherent aptitude, impulse, or capacity; a largely inheritable and unalterable tendency of an organism to make a complex and specific response to environmental stimuli without involving reason, behavior that is mediated by reactions below the conscious level.</skos:definition>
        <skos:prefLabel>Instinct</skos:prefLabel>
    </owl:Class>
    


    <!-- http://www.cognitiveatlas.org/ontology/cogat.owl#CAO_00351 -->

    <owl:Class rdf:about="&cogat;CAO_00351">
        <rdfs:label>Instrumental conditioning</rdfs:label>
        <rdfs:subClassOf rdf:resource="&cogat;CAO_00001"/>
        <skos:hasTopConcept>Learning and Memory</skos:hasTopConcept>
        <dc:Contributor>Agatha Lenartowicz</dc:Contributor>
        <skos:definition>A learning process in which the consequences of an action are used to modify the likelihood that that action will reoccur.</skos:definition>
        <dc:Title>Instrumental conditioning</dc:Title>
        <dc:identifier>trm_4a3fd79d0a642</dc:identifier>
        <skos:prefLabel>Instrumental conditioning</skos:prefLabel>
        <dc:Date>2009-07-10 14:06:31</dc:Date>
        <skos:altLabel></skos:altLabel>
    </owl:Class>
    


    <!-- http://www.cognitiveatlas.org/ontology/cogat.owl#CAO_00352 -->

    <owl:Class rdf:about="&cogat;CAO_00352">
        <rdfs:label>Instrumental learning</rdfs:label>
        <rdfs:subClassOf rdf:resource="&cogat;CAO_00001"/>
        <skos:hasTopConcept>Learning and Memory</skos:hasTopConcept>
        <skos:altLabel></skos:altLabel>
        <skos:definition>learning based on reward; a form of learning that takes place as a direct consequence of a reward or pleasant outcome for the learner.</skos:definition>
        <skos:prefLabel>Instrumental learning</skos:prefLabel>
        <dc:Title>Instrumental learning</dc:Title>
        <dc:Contributor>Brenda Gregory</dc:Contributor>
        <dc:Date>2011-05-03 13:50:59</dc:Date>
        <dc:identifier>trm_4a3fd79d0a64e</dc:identifier>
    </owl:Class>
    


    <!-- http://www.cognitiveatlas.org/ontology/cogat.owl#CAO_00353 -->

    <owl:Class rdf:about="&cogat;CAO_00353">
        <rdfs:label>Integration</rdfs:label>
        <rdfs:subClassOf rdf:resource="&cogat;CAO_00001"/>
        <skos:hasTopConcept></skos:hasTopConcept>
        <dc:identifier>trm_4a3fd79d0a65a</dc:identifier>
        <skos:definition>coordination of mental processes into a normal effective personality or with the individualand#39;s environment</skos:definition>
        <dc:Date>2012-03-28 17:06:53</dc:Date>
        <dc:Title>Integration</dc:Title>
        <dc:Contributor>Russ Poldrack</dc:Contributor>
        <skos:prefLabel>Integration</skos:prefLabel>
        <skos:altLabel></skos:altLabel>
    </owl:Class>
    


    <!-- http://www.cognitiveatlas.org/ontology/cogat.owl#CAO_00354 -->

    <owl:Class rdf:about="&cogat;CAO_00354">
        <rdfs:label>Intelligence</rdfs:label>
        <rdfs:subClassOf rdf:resource="&cogat;CAO_00001"/>
        <dc:Date>2012-03-28 17:07:15</dc:Date>
        <dc:identifier>trm_4a3fd79d0a666</dc:identifier>
        <dc:Title>Intelligence</dc:Title>
        <skos:altLabel></skos:altLabel>
        <skos:prefLabel>Intelligence</skos:prefLabel>
        <skos:hasTopConcept>Reasoning and Decision Making</skos:hasTopConcept>
        <skos:definition>the ability to learn or understand or to deal with new or trying situations; the skilled use of reason; the ability to apply knowledge to manipulate oneand#39;s environment or to think abstractly as measured by objective criteria</skos:definition>
        <dc:Contributor>Russ Poldrack</dc:Contributor>
    </owl:Class>
    


    <!-- http://www.cognitiveatlas.org/ontology/cogat.owl#CAO_00355 -->

    <owl:Class rdf:about="&cogat;CAO_00355">
        <rdfs:label>Intention</rdfs:label>
        <rdfs:subClassOf rdf:resource="&cogat;CAO_00001"/>
        <skos:hasTopConcept></skos:hasTopConcept>
        <dc:Contributor>Brenda Gregory</dc:Contributor>
        <skos:definition>an act or instance of determining mentally upon some action or result; meaning or significance.</skos:definition>
        <skos:altLabel></skos:altLabel>
        <dc:Title>Intention</dc:Title>
        <dc:Date>2011-05-18 12:19:55</dc:Date>
        <skos:prefLabel>Intention</skos:prefLabel>
        <dc:identifier>trm_4a3fd79d0a67d</dc:identifier>
    </owl:Class>
    


    <!-- http://www.cognitiveatlas.org/ontology/cogat.owl#CAO_00356 -->

    <owl:Class rdf:about="&cogat;CAO_00356">
        <rdfs:label>Intentional forgetting</rdfs:label>
        <rdfs:subClassOf rdf:resource="&cogat;CAO_00638"/>
        <dc:Title>Intentional forgetting</dc:Title>
        <dc:Contributor>Russ Poldrack</dc:Contributor>
        <skos:hasTopConcept>Learning and Memory</skos:hasTopConcept>
        <dc:identifier>trm_4a3fd79d0a689</dc:identifier>
        <dc:Date>2012-03-28 17:07:32</dc:Date>
        <skos:definition>the purposeful forgetting of information that is no longer needed.</skos:definition>
        <skos:altLabel></skos:altLabel>
        <skos:prefLabel>Intentional forgetting</skos:prefLabel>
    </owl:Class>
    


    <!-- http://www.cognitiveatlas.org/ontology/cogat.owl#CAO_00357 -->

    <owl:Class rdf:about="&cogat;CAO_00357">
        <rdfs:label>Intentional learning</rdfs:label>
        <rdfs:subClassOf rdf:resource="&cogat;CAO_00377"/>
        <skos:prefLabel>Intentional learning</skos:prefLabel>
        <skos:definition>learning that is motivated  with intention and is usually goal directed.</skos:definition>
        <dc:Contributor>Russ Poldrack</dc:Contributor>
        <skos:altLabel></skos:altLabel>
        <dc:Title>Intentional learning</dc:Title>
        <skos:hasTopConcept>Learning and Memory</skos:hasTopConcept>
        <dc:Date>2012-03-28 17:07:59</dc:Date>
        <dc:identifier>trm_4a3fd79d0a695</dc:identifier>
    </owl:Class>
    


    <!-- http://www.cognitiveatlas.org/ontology/cogat.owl#CAO_00358 -->

    <owl:Class rdf:about="&cogat;CAO_00358">
        <rdfs:label>Intentionality</rdfs:label>
        <rdfs:subClassOf rdf:resource="&cogat;CAO_00001"/>
        <skos:prefLabel>Intentionality</skos:prefLabel>
        <dc:identifier>trm_4a3fd79d0a6a1</dc:identifier>
        <skos:definition>the state of having or being formed by an intention; (philosophy) the property of being about or directed toward a subject, as inherent in conscious states, beliefs, or creations of the mind, such as sentences or books. </skos:definition>
        <dc:Date>2011-05-10 14:47:29</dc:Date>
        <skos:altLabel></skos:altLabel>
        <dc:Contributor>Brenda Gregory</dc:Contributor>
        <skos:hasTopConcept></skos:hasTopConcept>
        <dc:Title>Intentionality</dc:Title>
    </owl:Class>
    


    <!-- http://www.cognitiveatlas.org/ontology/cogat.owl#CAO_00359 -->

    <owl:Class rdf:about="&cogat;CAO_00359">
        <rdfs:label>Interference</rdfs:label>
        <rdfs:subClassOf rdf:resource="&cogat;CAO_00001"/>
        <dc:Title>Interference</dc:Title>
        <dc:Date>2012-03-28 17:09:25</dc:Date>
        <skos:prefLabel>Interference</skos:prefLabel>
        <dc:Contributor>Russ Poldrack</dc:Contributor>
        <dc:identifier>trm_4a3fd79d0a6ad</dc:identifier>
        <skos:definition>the disturbing effect of new information on the other information with which it is inconsistent</skos:definition>
        <skos:altLabel></skos:altLabel>
        <skos:hasTopConcept></skos:hasTopConcept>
    </owl:Class>
    


    <!-- http://www.cognitiveatlas.org/ontology/cogat.owl#CAO_00360 -->

    <owl:Class rdf:about="&cogat;CAO_00360">
        <rdfs:label>Intermediate term memory</rdfs:label>
        <rdfs:subClassOf rdf:resource="&cogat;CAO_00394"/>
        <skos:prefLabel>Intermediate term memory</skos:prefLabel>
        <dc:Title>Intermediate term memory</dc:Title>
        <skos:hasTopConcept>Learning and Memory</skos:hasTopConcept>
        <skos:definition>a specialized term referring for information about a current task.</skos:definition>
        <dc:identifier>trm_4a3fd79d0a6b9</dc:identifier>
        <dc:Date>2011-04-29 11:01:54</dc:Date>
        <skos:altLabel></skos:altLabel>
        <dc:Contributor>Brenda Gregory</dc:Contributor>
    </owl:Class>
    


    <!-- http://www.cognitiveatlas.org/ontology/cogat.owl#CAO_00361 -->

    <owl:Class rdf:about="&cogat;CAO_00361">
        <rdfs:label>Internal speech</rdfs:label>
        <rdfs:subClassOf rdf:resource="&cogat;CAO_00001"/>
        <skos:definition>also known as inner voice, internal speech, or verbal stream of consciousness is thinking in words. It also refers to the semi-constant internal monologue one has with oneself at a conscious or semi-conscious level.  </skos:definition>
        <skos:prefLabel>Internal speech</skos:prefLabel>
        <dc:Date>2011-04-11 15:18:46</dc:Date>
        <dc:Title>Internal speech</dc:Title>
        <dc:Contributor>Natalie Picchetti</dc:Contributor>
        <skos:hasTopConcept>Language</skos:hasTopConcept>
        <skos:altLabel></skos:altLabel>
        <dc:identifier>trm_4a3fd79d0a6c5</dc:identifier>
    </owl:Class>
    


    <!-- http://www.cognitiveatlas.org/ontology/cogat.owl#CAO_00362 -->

    <owl:Class rdf:about="&cogat;CAO_00362">
        <rdfs:label>Interrogative</rdfs:label>
        <rdfs:subClassOf rdf:resource="&cogat;CAO_00001"/>
        <dc:Date>2012-03-28 17:11:00</dc:Date>
        <dc:Title>Interrogative</dc:Title>
        <skos:altLabel></skos:altLabel>
        <skos:hasTopConcept>Language</skos:hasTopConcept>
        <dc:Contributor>Russ Poldrack</dc:Contributor>
        <skos:definition>of, pertaining to, or conveying a question.</skos:definition>
        <skos:prefLabel>Interrogative</skos:prefLabel>
        <dc:identifier>trm_4a3fd79d0a6d0</dc:identifier>
    </owl:Class>
    


    <!-- http://www.cognitiveatlas.org/ontology/cogat.owl#CAO_00363 -->

    <owl:Class rdf:about="&cogat;CAO_00363">
        <rdfs:label>Intonation</rdfs:label>
        <rdfs:subClassOf rdf:resource="&cogat;CAO_00001"/>
        <skos:hasTopConcept>Language</skos:hasTopConcept>
        <dc:Date>2011-05-11 16:14:48</dc:Date>
        <skos:definition>the ability to play or sing notes in tune; manner of utterance, specifically the rise and fall in pitch of the voice in speech.</skos:definition>
        <dc:identifier>trm_4a3fd79d0a6dc</dc:identifier>
        <dc:Contributor>Brenda Gregory</dc:Contributor>
        <skos:prefLabel>Intonation</skos:prefLabel>
        <dc:Title>Intonation</dc:Title>
        <skos:altLabel></skos:altLabel>
    </owl:Class>
    


    <!-- http://www.cognitiveatlas.org/ontology/cogat.owl#CAO_00364 -->

    <owl:Class rdf:about="&cogat;CAO_00364">
        <rdfs:label>Intrinsic motivation</rdfs:label>
        <rdfs:subClassOf rdf:resource="&cogat;CAO_00001"/>
        <skos:definition>a highly desired form of incentive that stems from a personand#39;s internal desire for self-satisfaction or pleasure in performing the task itself.</skos:definition>
        <dc:Contributor>Russ Poldrack</dc:Contributor>
        <skos:altLabel></skos:altLabel>
        <dc:Title>Intrinsic motivation</dc:Title>
        <dc:Date>2012-03-28 17:11:16</dc:Date>
        <dc:identifier>trm_4a3fd79d0a6e8</dc:identifier>
        <skos:prefLabel>Intrinsic motivation</skos:prefLabel>
        <skos:hasTopConcept>Motivation</skos:hasTopConcept>
    </owl:Class>
    


    <!-- http://www.cognitiveatlas.org/ontology/cogat.owl#CAO_00365 -->

    <owl:Class rdf:about="&cogat;CAO_00365">
        <rdfs:label>Introspection</rdfs:label>
        <rdfs:subClassOf rdf:resource="&cogat;CAO_00001"/>
        <skos:hasTopConcept></skos:hasTopConcept>
        <skos:prefLabel>Introspection</skos:prefLabel>
        <dc:Date>2011-04-29 15:55:50</dc:Date>
        <dc:identifier>trm_4a3fd79d0a6f4</dc:identifier>
        <dc:Contributor>Brenda Gregory</dc:Contributor>
        <dc:Title>Introspection</dc:Title>
        <skos:definition>the self-observation and reporting of conscious inner thoughts, desires  and sensations. It is a conscious mental and usually purposive process relying on thinking, reasoning, and examining oneand#39;s own thoughts, feelings.</skos:definition>
        <skos:altLabel></skos:altLabel>
    </owl:Class>
    


    <!-- http://www.cognitiveatlas.org/ontology/cogat.owl#CAO_00366 -->

    <owl:Class rdf:about="&cogat;CAO_00366">
        <rdfs:label>Involuntary attention</rdfs:label>
        <rdfs:subClassOf rdf:resource="&cogat;CAO_00001"/>
        <dc:Contributor>Natalie Picchetti</dc:Contributor>
        <skos:altLabel></skos:altLabel>
        <dc:identifier>trm_4a3fd79d0a700</dc:identifier>
        <skos:definition>results when the conscious mind changes focus to sudden changes in the environment (big sound, intensity of light, unique situation etc.).  The person is not prepared for the attention and the attention is not under control of the individual.  The persons attention is less concerned with motives, interests, and needs and the stimulus is usually more important than any functional factors.</skos:definition>
        <skos:prefLabel>Involuntary attention</skos:prefLabel>
        <skos:hasTopConcept>Attention</skos:hasTopConcept>
        <dc:Title>Involuntary attention</dc:Title>
        <dc:Date>2011-04-12 09:55:50</dc:Date>
    </owl:Class>
    


    <!-- http://www.cognitiveatlas.org/ontology/cogat.owl#CAO_00367 -->

    <owl:Class rdf:about="&cogat;CAO_00367">
        <rdfs:label>Irony</rdfs:label>
        <rdfs:subClassOf rdf:resource="&cogat;CAO_00001"/>
        <dc:Contributor>Brenda Gregory</dc:Contributor>
        <skos:hasTopConcept></skos:hasTopConcept>
        <dc:Title>Irony</dc:Title>
        <dc:Date>2011-05-16 11:33:38</dc:Date>
        <skos:definition>a situation, literary technique, or rhetorical device, in which there is an incongruity or discordance that goes strikingly beyond the most simple and evident meaning of words or actions.</skos:definition>
        <dc:identifier>trm_4a3fd79d0a70b</dc:identifier>
        <skos:prefLabel>Irony</skos:prefLabel>
        <skos:altLabel></skos:altLabel>
    </owl:Class>
    


    <!-- http://www.cognitiveatlas.org/ontology/cogat.owl#CAO_00368 -->

    <owl:Class rdf:about="&cogat;CAO_00368">
        <rdfs:label>Judgment</rdfs:label>
        <rdfs:subClassOf rdf:resource="&cogat;CAO_00001"/>
        <dc:Contributor>Russ Poldrack</dc:Contributor>
        <skos:prefLabel>Judgment</skos:prefLabel>
        <dc:Title>Judgment</dc:Title>
        <dc:identifier>trm_4a3fd79d0a723</dc:identifier>
        <dc:Date>2012-03-28 17:12:13</dc:Date>
        <skos:definition>the process of forming an opinion or evaluation by discerning and comparing, or an opinion or estimate so formed</skos:definition>
        <skos:altLabel></skos:altLabel>
        <skos:hasTopConcept>Reasoning and Decision Making</skos:hasTopConcept>
    </owl:Class>
    


    <!-- http://www.cognitiveatlas.org/ontology/cogat.owl#CAO_00369 -->

    <owl:Class rdf:about="&cogat;CAO_00369">
        <rdfs:label>Kinaesthetic representation</rdfs:label>
        <rdfs:subClassOf rdf:resource="&cogat;CAO_00691"/>
        <rdfs:subClassOf>
            <owl:Restriction>
                <owl:onProperty rdf:resource="&ro;part_of"/>
                <owl:someValuesFrom rdf:resource="&cogat;CAO_00370"/>
            </owl:Restriction>
        </rdfs:subClassOf>
        <skos:prefLabel>Kinaesthetic representation</skos:prefLabel>
        <dc:identifier>trm_4a3fd79d0a72e</dc:identifier>
        <skos:altLabel>kinesthetic representation</skos:altLabel>
        <dc:Contributor>Russ Poldrack</dc:Contributor>
        <skos:hasTopConcept></skos:hasTopConcept>
        <dc:Title>Kinaesthetic representation</dc:Title>
        <skos:definition>is a representation of sensory inputs from muscles, tendons, and joints (e.g.,the joint angles used to reach a point in space).  </skos:definition>
        <dc:Date>2011-08-24 07:12:35</dc:Date>
    </owl:Class>
    


    <!-- http://www.cognitiveatlas.org/ontology/cogat.owl#CAO_00370 -->

    <owl:Class rdf:about="&cogat;CAO_00370">
        <rdfs:label>Kinesthesia</rdfs:label>
        <rdfs:subClassOf rdf:resource="&cogat;CAO_00525"/>
        <dc:Contributor>Russ Poldrack</dc:Contributor>
        <dc:Title>Kinesthesia</dc:Title>
        <skos:definition>a sense mediated by receptors located in muscles, tendons, and joints and stimulated by bodily movements and tensions. </skos:definition>
        <dc:identifier>trm_4a3fd79d0a73a</dc:identifier>
        <skos:hasTopConcept>Perception</skos:hasTopConcept>
        <skos:prefLabel>Kinesthesia</skos:prefLabel>
        <skos:altLabel>kinaesthesia</skos:altLabel>
        <dc:Date>2012-03-28 17:12:39</dc:Date>
    </owl:Class>
    


    <!-- http://www.cognitiveatlas.org/ontology/cogat.owl#CAO_00371 -->

    <owl:Class rdf:about="&cogat;CAO_00371">
        <rdfs:label>Knowledge</rdfs:label>
        <rdfs:subClassOf rdf:resource="&cogat;CAO_00001"/>
        <dc:identifier>trm_4a3fd79d0a746</dc:identifier>
        <skos:altLabel></skos:altLabel>
        <skos:prefLabel>Knowledge</skos:prefLabel>
        <dc:Date>2012-03-28 17:13:17</dc:Date>
        <skos:definition>information acquired and represented by a person through experience or education</skos:definition>
        <dc:Title>Knowledge</dc:Title>
        <skos:hasTopConcept></skos:hasTopConcept>
        <dc:Contributor>Russ Poldrack</dc:Contributor>
    </owl:Class>
    


    <!-- http://www.cognitiveatlas.org/ontology/cogat.owl#CAO_00372 -->

    <owl:Class rdf:about="&cogat;CAO_00372">
        <rdfs:label>Language</rdfs:label>
        <rdfs:subClassOf rdf:resource="&cogat;CAO_00001"/>
        <skos:altLabel></skos:altLabel>
        <skos:hasTopConcept>Language</skos:hasTopConcept>
        <dc:Contributor>Agatha Lenartowicz</dc:Contributor>
        <dc:Date>2009-07-10 14:06:32</dc:Date>
        <skos:prefLabel>Language</skos:prefLabel>
        <skos:definition>The mental ability to encode and decode information, and translate this information into verbal, acoustic and visual representations, according to a set of rules that are common across a population.</skos:definition>
        <dc:Title>Language</dc:Title>
        <dc:identifier>trm_4a3fd79d0a769</dc:identifier>
    </owl:Class>
    


    <!-- http://www.cognitiveatlas.org/ontology/cogat.owl#CAO_00373 -->

    <owl:Class rdf:about="&cogat;CAO_00373">
        <rdfs:label>Language comprehension</rdfs:label>
        <rdfs:subClassOf rdf:resource="&cogat;CAO_00001"/>
        <dc:identifier>trm_4a3fd79d0a775</dc:identifier>
        <skos:altLabel></skos:altLabel>
        <dc:Date>2011-05-11 16:22:12</dc:Date>
        <dc:Contributor>Brenda Gregory</dc:Contributor>
        <skos:hasTopConcept>Language</skos:hasTopConcept>
        <dc:Title>Language comprehension</dc:Title>
        <skos:prefLabel>Language comprehension</skos:prefLabel>
        <skos:definition>The ability to understand communication from others, such as speech, written text, gestures, or sign language.</skos:definition>
    </owl:Class>
    


    <!-- http://www.cognitiveatlas.org/ontology/cogat.owl#CAO_00374 -->

    <owl:Class rdf:about="&cogat;CAO_00374">
        <rdfs:label>Language learning</rdfs:label>
        <rdfs:subClassOf rdf:resource="&cogat;CAO_00377"/>
        <skos:hasTopConcept>Language</skos:hasTopConcept>
        <dc:Date>2011-04-19 13:50:16</dc:Date>
        <dc:Contributor>Brenda Gregory</dc:Contributor>
        <skos:definition>the process by which humans acquire the capacity to perceive, produce and use words to understand and communicate, this capacity involves the picking up of diverse capacities including syntax, phonetics, and an extensive vocabulary, the language might be vocal as with speech or manual as in sign.</skos:definition>
        <skos:prefLabel>Language learning</skos:prefLabel>
        <dc:Title>Language learning</dc:Title>
        <skos:altLabel></skos:altLabel>
        <dc:identifier>trm_4a3fd79d0a781</dc:identifier>
    </owl:Class>
    


    <!-- http://www.cognitiveatlas.org/ontology/cogat.owl#CAO_00375 -->

    <owl:Class rdf:about="&cogat;CAO_00375">
        <rdfs:label>Language production</rdfs:label>
        <rdfs:subClassOf rdf:resource="&cogat;CAO_00001"/>
        <rdfs:subClassOf>
            <owl:Restriction>
                <owl:onProperty rdf:resource="&ro;part_of"/>
                <owl:someValuesFrom rdf:resource="&cogat;CAO_00372"/>
            </owl:Restriction>
        </rdfs:subClassOf>
        <dc:Date>2010-01-31 02:15:29</dc:Date>
        <dc:identifier>trm_4a3fd79d0a78d</dc:identifier>
        <dc:Title>Language production</dc:Title>
        <dc:Contributor>Joseph Devlin</dc:Contributor>
        <skos:prefLabel>Language production</skos:prefLabel>
        <skos:hasTopConcept>Language</skos:hasTopConcept>
        <skos:definition>is translating a concept or set of ideas into spoken, signed or written form</skos:definition>
        <skos:altLabel></skos:altLabel>
    </owl:Class>
    


    <!-- http://www.cognitiveatlas.org/ontology/cogat.owl#CAO_00377 -->

    <owl:Class rdf:about="&cogat;CAO_00377">
        <rdfs:label>Learning</rdfs:label>
        <rdfs:subClassOf rdf:resource="&cogat;CAO_00001"/>
        <dc:Date>2009-07-10 14:06:32</dc:Date>
        <skos:definition>The process of acquiring new skills-knowledge-information </skos:definition>
        <dc:identifier>trm_4a3fd79d0a7bb</dc:identifier>
        <dc:Title>Learning</dc:Title>
        <skos:altLabel></skos:altLabel>
        <dc:Contributor>Tom Schonberg</dc:Contributor>
        <skos:prefLabel>Learning</skos:prefLabel>
        <skos:hasTopConcept>Learning and Memory</skos:hasTopConcept>
    </owl:Class>
    


    <!-- http://www.cognitiveatlas.org/ontology/cogat.owl#CAO_00378 -->

    <owl:Class rdf:about="&cogat;CAO_00378">
        <rdfs:label>Lemma</rdfs:label>
        <rdfs:subClassOf rdf:resource="&cogat;CAO_00001"/>
        <skos:definition>an intermediate form a word about to be uttered takes during speech production</skos:definition>
        <skos:prefLabel>Lemma</skos:prefLabel>
        <dc:Title>Lemma</dc:Title>
        <dc:identifier>trm_4a3fd79d0a7c7</dc:identifier>
        <skos:altLabel></skos:altLabel>
        <skos:hasTopConcept>Language</skos:hasTopConcept>
        <dc:Date>2012-03-28 17:15:10</dc:Date>
        <dc:Contributor>Russ Poldrack</dc:Contributor>
    </owl:Class>
    


    <!-- http://www.cognitiveatlas.org/ontology/cogat.owl#CAO_00379 -->

    <owl:Class rdf:about="&cogat;CAO_00379">
        <rdfs:label>Lexical encoding</rdfs:label>
        <rdfs:subClassOf rdf:resource="&cogat;CAO_00001"/>
        <skos:altLabel></skos:altLabel>
        <dc:Contributor>Russ Poldrack</dc:Contributor>
        <skos:definition>converting vocabulary, words, or morphemes of a language into a code. </skos:definition>
        <dc:identifier>trm_4a3fd79d0a7d4</dc:identifier>
        <dc:Title>Lexical encoding</dc:Title>
        <skos:prefLabel>Lexical encoding</skos:prefLabel>
        <dc:Date>2012-03-28 17:15:32</dc:Date>
        <skos:hasTopConcept>Language</skos:hasTopConcept>
    </owl:Class>
    


    <!-- http://www.cognitiveatlas.org/ontology/cogat.owl#CAO_00380 -->

    <owl:Class rdf:about="&cogat;CAO_00380">
        <rdfs:label>Lexical retrieval</rdfs:label>
        <rdfs:subClassOf rdf:resource="&cogat;CAO_00490"/>
        <dc:Contributor>Russ Poldrack</dc:Contributor>
        <dc:Title>Lexical retrieval</dc:Title>
        <skos:definition>retrieval of a lexical entry</skos:definition>
        <skos:hasTopConcept>Language</skos:hasTopConcept>
        <dc:Date>2012-03-28 17:27:58</dc:Date>
        <dc:identifier>trm_4a3fd79d0a7e0</dc:identifier>
        <skos:prefLabel>Lexical retrieval</skos:prefLabel>
        <skos:altLabel></skos:altLabel>
    </owl:Class>
    


    <!-- http://www.cognitiveatlas.org/ontology/cogat.owl#CAO_00381 -->

    <owl:Class rdf:about="&cogat;CAO_00381">
        <rdfs:label>Lexicon</rdfs:label>
        <rdfs:subClassOf rdf:resource="&cogat;CAO_00001"/>
        <skos:hasTopConcept>Language</skos:hasTopConcept>
        <skos:prefLabel>Lexicon</skos:prefLabel>
        <dc:Date>2010-06-05 13:03:20</dc:Date>
        <skos:definition>The vocabulary of a language, including its words and expressions.</skos:definition>
        <skos:altLabel></skos:altLabel>
        <dc:identifier>trm_4a3fd79d0a7ec</dc:identifier>
        <dc:Contributor>Tal Yarkoni</dc:Contributor>
        <dc:Title>Lexicon</dc:Title>
    </owl:Class>
    


    <!-- http://www.cognitiveatlas.org/ontology/cogat.owl#CAO_00382 -->

    <owl:Class rdf:about="&cogat;CAO_00382">
        <rdfs:label>Linguistic competence</rdfs:label>
        <rdfs:subClassOf rdf:resource="&cogat;CAO_00001"/>
        <dc:Title>Linguistic competence</dc:Title>
        <dc:Contributor>Brenda Gregory</dc:Contributor>
        <skos:prefLabel>Linguistic competence</skos:prefLabel>
        <skos:hasTopConcept>Language</skos:hasTopConcept>
        <dc:identifier>trm_4a3fd79d0a7f8</dc:identifier>
        <skos:definition>a speakerand#39;s implicit, internalized knowledge of the rules of their language.</skos:definition>
        <dc:Date>2011-04-19 13:54:10</dc:Date>
        <skos:altLabel></skos:altLabel>
    </owl:Class>
    


    <!-- http://www.cognitiveatlas.org/ontology/cogat.owl#CAO_00383 -->

    <owl:Class rdf:about="&cogat;CAO_00383">
        <rdfs:label>Listening</rdfs:label>
        <rdfs:subClassOf rdf:resource="&cogat;CAO_00153"/>
        <skos:altLabel></skos:altLabel>
        <skos:hasTopConcept></skos:hasTopConcept>
        <skos:prefLabel>Listening</skos:prefLabel>
        <dc:Title>Listening</dc:Title>
        <skos:definition>to pay attention to sound; to hear something with thoughtful attention, give consideration; to be alert to catch an expected sound.</skos:definition>
        <dc:identifier>trm_4a3fd79d0a803</dc:identifier>
        <dc:Date>2011-04-28 17:25:32</dc:Date>
        <dc:Contributor>Brenda Gregory</dc:Contributor>
    </owl:Class>
    


    <!-- http://www.cognitiveatlas.org/ontology/cogat.owl#CAO_00384 -->

    <owl:Class rdf:about="&cogat;CAO_00384">
        <rdfs:label>Logic</rdfs:label>
        <rdfs:subClassOf rdf:resource="&cogat;CAO_00001"/>
        <skos:definition>a science that deals with the principles and criteria of validity of inference and demonstration; the science of the formal principles of reasoning.</skos:definition>
        <skos:prefLabel>Logic</skos:prefLabel>
        <dc:Title>Logic</dc:Title>
        <dc:Contributor>Brenda Gregory</dc:Contributor>
        <skos:altLabel></skos:altLabel>
        <skos:hasTopConcept>Reasoning and Decision Making</skos:hasTopConcept>
        <dc:Date>2011-05-16 15:44:00</dc:Date>
        <dc:identifier>trm_4a3fd79d0a80f</dc:identifier>
    </owl:Class>
    


    <!-- http://www.cognitiveatlas.org/ontology/cogat.owl#CAO_00385 -->

    <owl:Class rdf:about="&cogat;CAO_00385">
        <rdfs:label>Logical reasoning</rdfs:label>
        <rdfs:subClassOf rdf:resource="&cogat;CAO_00480"/>
        <dc:Date>2011-04-18 11:38:13</dc:Date>
        <skos:hasTopConcept>Reasoning and Decision Making</skos:hasTopConcept>
        <dc:Title>Logical reasoning</dc:Title>
        <skos:prefLabel>Logical reasoning</skos:prefLabel>
        <dc:identifier>trm_4a3fd79d0a81b</dc:identifier>
        <skos:altLabel></skos:altLabel>
        <dc:Contributor>Natalie Picchetti</dc:Contributor>
        <skos:definition>The strategy when  one uses deduction, induction, or abduction to evaluate preconditions and rules to determnie a conclusion.  </skos:definition>
    </owl:Class>
    


    <!-- http://www.cognitiveatlas.org/ontology/cogat.owl#CAO_00387 -->

    <owl:Class rdf:about="&cogat;CAO_00387">
        <rdfs:label>Long term memory</rdfs:label>
        <rdfs:subClassOf rdf:resource="&cogat;CAO_00394"/>
        <dc:Contributor>Brenda Gregory</dc:Contributor>
        <skos:hasTopConcept>Learning and Memory</skos:hasTopConcept>
        <skos:prefLabel>Long term memory</skos:prefLabel>
        <dc:identifier>trm_4a3fd79d0a833</dc:identifier>
        <dc:Title>Long term memory</dc:Title>
        <skos:altLabel></skos:altLabel>
        <dc:Date>2011-04-28 12:20:19</dc:Date>
        <skos:definition>a system for permanently storing, managing, and retrieving information for later use, items of information stored as long-term memory may be available for a lifetime.</skos:definition>
    </owl:Class>
    


    <!-- http://www.cognitiveatlas.org/ontology/cogat.owl#CAO_00388 -->

    <owl:Class rdf:about="&cogat;CAO_00388">
        <rdfs:label>Loss aversion</rdfs:label>
        <rdfs:subClassOf rdf:resource="&cogat;CAO_00001"/>
        <skos:definition>The tendency of individuals to be more sensitive to the possibility of losing objects or money than they are to the possibility of gaining the same objects or amounts of money.</skos:definition>
        <dc:Date>2009-07-10 14:06:32</dc:Date>
        <skos:hasTopConcept>Reasoning and Decision Making</skos:hasTopConcept>
        <dc:identifier>trm_4a3fd79d0a83f</dc:identifier>
        <dc:Contributor>Emily Barkley-Levenson</dc:Contributor>
        <dc:Title>Loss aversion</dc:Title>
        <skos:altLabel></skos:altLabel>
        <skos:prefLabel>Loss aversion</skos:prefLabel>
    </owl:Class>
    


    <!-- http://www.cognitiveatlas.org/ontology/cogat.owl#CAO_00389 -->

    <owl:Class rdf:about="&cogat;CAO_00389">
        <rdfs:label>Lying</rdfs:label>
        <rdfs:subClassOf rdf:resource="&cogat;CAO_00001"/>
        <dc:Title>Lying</dc:Title>
        <skos:prefLabel>Lying</skos:prefLabel>
        <dc:identifier>trm_4a3fd79d0a84a</dc:identifier>
        <dc:Contributor>Russ Poldrack</dc:Contributor>
        <dc:Date>2012-03-28 17:29:43</dc:Date>
        <skos:hasTopConcept>Social Function</skos:hasTopConcept>
        <skos:altLabel></skos:altLabel>
        <skos:definition>the expression of a falsehood</skos:definition>
    </owl:Class>
    


    <!-- http://www.cognitiveatlas.org/ontology/cogat.owl#CAO_00390 -->

    <owl:Class rdf:about="&cogat;CAO_00390">
        <rdfs:label>Mathematical reasoning</rdfs:label>
        <rdfs:subClassOf rdf:resource="&cogat;CAO_00480"/>
        <skos:hasTopConcept>Reasoning and Decision Making</skos:hasTopConcept>
        <dc:Title>Mathematical reasoning</dc:Title>
        <dc:Date>2012-03-28 17:30:58</dc:Date>
        <skos:prefLabel>Mathematical reasoning</skos:prefLabel>
        <skos:definition>Reasoning about mathematical objects</skos:definition>
        <dc:identifier>trm_4a3fd79d0a862</dc:identifier>
        <skos:altLabel></skos:altLabel>
        <dc:Contributor>Russ Poldrack</dc:Contributor>
    </owl:Class>
    


    <!-- http://www.cognitiveatlas.org/ontology/cogat.owl#CAO_00391 -->

    <owl:Class rdf:about="&cogat;CAO_00391">
        <rdfs:label>Meaning</rdfs:label>
        <rdfs:subClassOf rdf:resource="&cogat;CAO_00001"/>
        <dc:identifier>trm_4a3fd79d0a86e</dc:identifier>
        <dc:Date>2012-03-28 17:31:39</dc:Date>
        <skos:definition>the connotation of a word or phrase</skos:definition>
        <skos:altLabel></skos:altLabel>
        <skos:hasTopConcept>Language</skos:hasTopConcept>
        <skos:prefLabel>Meaning</skos:prefLabel>
        <dc:Contributor>Russ Poldrack</dc:Contributor>
        <dc:Title>Meaning</dc:Title>
    </owl:Class>
    


    <!-- http://www.cognitiveatlas.org/ontology/cogat.owl#CAO_00392 -->

    <owl:Class rdf:about="&cogat;CAO_00392">
        <rdfs:label>Mechanical reasoning</rdfs:label>
        <rdfs:subClassOf rdf:resource="&cogat;CAO_00480"/>
        <dc:Contributor>Russ Poldrack</dc:Contributor>
        <dc:Title>Mechanical reasoning</dc:Title>
        <dc:Date>2012-03-28 17:32:07</dc:Date>
        <skos:prefLabel>Mechanical reasoning</skos:prefLabel>
        <skos:altLabel></skos:altLabel>
        <dc:identifier>trm_4a3fd79d0a87a</dc:identifier>
        <skos:definition>Reasoning about mechanical objects or functions</skos:definition>
        <skos:hasTopConcept>Reasoning and Decision Making</skos:hasTopConcept>
    </owl:Class>
    


    <!-- http://www.cognitiveatlas.org/ontology/cogat.owl#CAO_00393 -->

    <owl:Class rdf:about="&cogat;CAO_00393">
        <rdfs:label>Melody</rdfs:label>
        <rdfs:subClassOf rdf:resource="&cogat;CAO_00001"/>
        <skos:definition>a linear succession of musical tones which is perceived as a single entity.</skos:definition>
        <dc:identifier>trm_4a3fd79d0a886</dc:identifier>
        <skos:prefLabel>Melody</skos:prefLabel>
        <dc:Title>Melody</dc:Title>
        <skos:hasTopConcept>Perception</skos:hasTopConcept>
        <dc:Date>2012-03-28 17:32:29</dc:Date>
        <dc:Contributor>Russ Poldrack</dc:Contributor>
        <skos:altLabel>tune</skos:altLabel>
    </owl:Class>
    


    <!-- http://www.cognitiveatlas.org/ontology/cogat.owl#CAO_00394 -->

    <owl:Class rdf:about="&cogat;CAO_00394">
        <rdfs:label>Memory</rdfs:label>
        <rdfs:subClassOf rdf:resource="&cogat;CAO_00001"/>
        <skos:prefLabel>Memory</skos:prefLabel>
        <skos:altLabel></skos:altLabel>
        <dc:Contributor>Russ Poldrack</dc:Contributor>
        <skos:hasTopConcept>Learning and Memory</skos:hasTopConcept>
        <dc:Date>2012-03-28 17:32:42</dc:Date>
        <dc:Title>Memory</dc:Title>
        <dc:identifier>trm_4a3fd79d0a891</dc:identifier>
        <skos:definition>The ability of an organism to use past events to inform-influence current actions </skos:definition>
    </owl:Class>
    


    <!-- http://www.cognitiveatlas.org/ontology/cogat.owl#CAO_00395 -->

    <owl:Class rdf:about="&cogat;CAO_00395">
        <rdfs:label>Mental arithmetic</rdfs:label>
        <rdfs:subClassOf rdf:resource="&cogat;CAO_00001"/>
        <dc:Contributor>Russ Poldrack</dc:Contributor>
        <dc:Title>Mental arithmetic</dc:Title>
        <skos:definition>mathematical calculations done mentally, without writing them down.</skos:definition>
        <skos:hasTopConcept>Reasoning and Decision Making</skos:hasTopConcept>
        <dc:Date>2012-03-28 17:35:19</dc:Date>
        <skos:altLabel></skos:altLabel>
        <skos:prefLabel>Mental arithmetic</skos:prefLabel>
        <dc:identifier>trm_4a3fd79d0a8ed</dc:identifier>
    </owl:Class>
    


    <!-- http://www.cognitiveatlas.org/ontology/cogat.owl#CAO_00396 -->

    <owl:Class rdf:about="&cogat;CAO_00396">
        <rdfs:label>Mental imagery</rdfs:label>
        <rdfs:subClassOf rdf:resource="&cogat;CAO_00001"/>
        <skos:hasTopConcept>Perception</skos:hasTopConcept>
        <skos:altLabel></skos:altLabel>
        <dc:Title>Mental imagery</dc:Title>
        <dc:Contributor>Natalie Picchetti</dc:Contributor>
        <dc:Date>2011-04-18 12:23:36</dc:Date>
        <dc:identifier>trm_4a3fd79d0a8fc</dc:identifier>
        <skos:definition>is an experience that, on most occasions, significantly resembles the experience of perceiving (through any of the senses) of some object, event, or scene, but occurs when the relevant object, event, or scene is not actually present to the senses.</skos:definition>
        <skos:prefLabel>Mental imagery</skos:prefLabel>
    </owl:Class>
    


    <!-- http://www.cognitiveatlas.org/ontology/cogat.owl#CAO_00397 -->

    <owl:Class rdf:about="&cogat;CAO_00397">
        <rdfs:label>Mental representation</rdfs:label>
        <rdfs:subClassOf rdf:resource="&cogat;CAO_00001"/>
        <skos:definition>a presentation to the mind in the form of an idea or image.</skos:definition>
        <skos:prefLabel>Mental representation</skos:prefLabel>
        <skos:hasTopConcept></skos:hasTopConcept>
        <dc:Title>Mental representation</dc:Title>
        <dc:identifier>trm_4a3fd79d0a908</dc:identifier>
        <dc:Contributor>Brenda Gregory</dc:Contributor>
        <dc:Date>2011-04-29 16:00:20</dc:Date>
        <skos:altLabel></skos:altLabel>
    </owl:Class>
    


    <!-- http://www.cognitiveatlas.org/ontology/cogat.owl#CAO_00398 -->

    <owl:Class rdf:about="&cogat;CAO_00398">
        <rdfs:label>Mental rotation</rdfs:label>
        <rdfs:subClassOf rdf:resource="&cogat;CAO_00001"/>
        <skos:altLabel></skos:altLabel>
        <skos:definition>Ability to rotate an object in oneand#39;s mind; ability to make perceptual judgments on a new spatial configuration of an object.</skos:definition>
        <skos:prefLabel>Mental rotation</skos:prefLabel>
        <skos:hasTopConcept>Perception</skos:hasTopConcept>
        <dc:Title>Mental rotation</dc:Title>
        <dc:Date>2009-07-10 14:06:32</dc:Date>
        <dc:Contributor>Agatha Lenartowicz</dc:Contributor>
        <dc:identifier>trm_4a3fd79d0a914</dc:identifier>
    </owl:Class>
    


    <!-- http://www.cognitiveatlas.org/ontology/cogat.owl#CAO_00399 -->

    <owl:Class rdf:about="&cogat;CAO_00399">
        <rdfs:label>Metacognition</rdfs:label>
        <rdfs:subClassOf rdf:resource="&cogat;CAO_00001"/>
        <dc:identifier>trm_4a3fd79d0a920</dc:identifier>
        <dc:Contributor>Brenda Gregory</dc:Contributor>
        <dc:Date>2011-05-16 15:50:20</dc:Date>
        <skos:hasTopConcept></skos:hasTopConcept>
        <skos:prefLabel>Metacognition</skos:prefLabel>
        <skos:definition>awareness or analysis of oneand#39;s own learning or thinking processes.</skos:definition>
        <skos:altLabel></skos:altLabel>
        <dc:Title>Metacognition</dc:Title>
    </owl:Class>
    


    <!-- http://www.cognitiveatlas.org/ontology/cogat.owl#CAO_00400 -->

    <owl:Class rdf:about="&cogat;CAO_00400">
        <rdfs:label>Metacognitive skill</rdfs:label>
        <rdfs:subClassOf rdf:resource="&cogat;CAO_00001"/>
        <dc:Date>2011-04-07 11:09:01</dc:Date>
        <dc:identifier>trm_4a3fd79d0a92b</dc:identifier>
        <skos:definition>a learnersand#39; automatic awareness of their own knowledge and their ability to understand, control, and manipulate their own cognitive processes. </skos:definition>
        <skos:altLabel></skos:altLabel>
        <dc:Title>Metacognitive skill</dc:Title>
        <skos:prefLabel>Metacognitive skill</skos:prefLabel>
        <skos:hasTopConcept>Learning and Memory</skos:hasTopConcept>
        <dc:Contributor>Natalie Picchetti</dc:Contributor>
    </owl:Class>
    


    <!-- http://www.cognitiveatlas.org/ontology/cogat.owl#CAO_00401 -->

    <owl:Class rdf:about="&cogat;CAO_00401">
        <rdfs:label>Metaphor</rdfs:label>
        <rdfs:subClassOf rdf:resource="&cogat;CAO_00001"/>
        <dc:Contributor>Brenda Gregory</dc:Contributor>
        <skos:prefLabel>Metaphor</skos:prefLabel>
        <dc:Date>2011-04-29 10:58:00</dc:Date>
        <dc:Title>Metaphor</dc:Title>
        <skos:hasTopConcept>Language</skos:hasTopConcept>
        <skos:altLabel></skos:altLabel>
        <skos:definition>a figure of speech in which a word or phrase literally denoting one kind of object or idea is used in place of another to suggest a likeness or analogy between them.</skos:definition>
        <dc:identifier>trm_4a3fd79d0a937</dc:identifier>
    </owl:Class>
    


    <!-- http://www.cognitiveatlas.org/ontology/cogat.owl#CAO_00402 -->

    <owl:Class rdf:about="&cogat;CAO_00402">
        <rdfs:label>Misattribution</rdfs:label>
        <rdfs:subClassOf rdf:resource="&cogat;CAO_00001"/>
        <skos:definition>attributing an event to something with which it has no connection or association.</skos:definition>
        <dc:Date>2011-04-19 13:56:00</dc:Date>
        <skos:prefLabel>Misattribution</skos:prefLabel>
        <skos:altLabel></skos:altLabel>
        <dc:Contributor>Brenda Gregory</dc:Contributor>
        <dc:identifier>trm_4a3fd79d0a943</dc:identifier>
        <skos:hasTopConcept></skos:hasTopConcept>
        <dc:Title>Misattribution</dc:Title>
    </owl:Class>
    


    <!-- http://www.cognitiveatlas.org/ontology/cogat.owl#CAO_00403 -->

    <owl:Class rdf:about="&cogat;CAO_00403">
        <rdfs:label>Monitoring</rdfs:label>
        <rdfs:subClassOf rdf:resource="&cogat;CAO_00001"/>
        <skos:hasTopConcept>Executive-Cognitive Control</skos:hasTopConcept>
        <dc:Date>2012-03-28 17:36:34</dc:Date>
        <dc:Contributor>Russ Poldrack</dc:Contributor>
        <dc:identifier>trm_4a3fd79d0a94f</dc:identifier>
        <skos:prefLabel>Monitoring</skos:prefLabel>
        <skos:definition>the act of checking for particular kinds of information</skos:definition>
        <dc:Title>Monitoring</dc:Title>
        <skos:altLabel></skos:altLabel>
    </owl:Class>
    


    <!-- http://www.cognitiveatlas.org/ontology/cogat.owl#CAO_00404 -->

    <owl:Class rdf:about="&cogat;CAO_00404">
        <rdfs:label>Mood</rdfs:label>
        <rdfs:subClassOf rdf:resource="&cogat;CAO_00001"/>
        <dc:identifier>trm_4a3fd79d0a95a</dc:identifier>
        <skos:definition>a conscious state of mind or predominant emotion.</skos:definition>
        <skos:prefLabel>Mood</skos:prefLabel>
        <skos:hasTopConcept>Emotion</skos:hasTopConcept>
        <dc:Contributor>Brenda Gregory</dc:Contributor>
        <dc:Title>Mood</dc:Title>
        <skos:altLabel></skos:altLabel>
        <dc:Date>2011-05-16 13:23:45</dc:Date>
    </owl:Class>
    


    <!-- http://www.cognitiveatlas.org/ontology/cogat.owl#CAO_00405 -->

    <owl:Class rdf:about="&cogat;CAO_00405">
        <rdfs:label>Motor control</rdfs:label>
        <rdfs:subClassOf rdf:resource="&cogat;CAO_00001"/>
        <skos:definition>The function of supervising motor activities</skos:definition>
        <skos:prefLabel>Motor control</skos:prefLabel>
        <dc:Contributor>Russ Poldrack</dc:Contributor>
        <dc:Date>2012-03-28 17:37:24</dc:Date>
        <dc:Title>Motor control</dc:Title>
        <skos:altLabel></skos:altLabel>
        <dc:identifier>trm_4a3fd79d0a972</dc:identifier>
        <skos:hasTopConcept>Action</skos:hasTopConcept>
    </owl:Class>
    


    <!-- http://www.cognitiveatlas.org/ontology/cogat.owl#CAO_00406 -->

    <owl:Class rdf:about="&cogat;CAO_00406">
        <rdfs:label>Motor execution</rdfs:label>
        <rdfs:subClassOf rdf:resource="&cogat;CAO_00001"/>
        <dc:identifier>trm_4a3fd79d0a97e</dc:identifier>
        <dc:Contributor>Russ Poldrack</dc:Contributor>
        <skos:prefLabel>Motor execution</skos:prefLabel>
        <dc:Date>2012-03-28 17:37:50</dc:Date>
        <skos:hasTopConcept>Action</skos:hasTopConcept>
        <skos:definition>The implementation of a motor movement</skos:definition>
        <skos:altLabel></skos:altLabel>
        <dc:Title>Motor execution</dc:Title>
    </owl:Class>
    


    <!-- http://www.cognitiveatlas.org/ontology/cogat.owl#CAO_00408 -->

    <owl:Class rdf:about="&cogat;CAO_00408">
        <rdfs:label>Motor learning</rdfs:label>
        <rdfs:subClassOf rdf:resource="&cogat;CAO_00001"/>
        <dc:Contributor>Russ Poldrack</dc:Contributor>
        <skos:hasTopConcept>Learning and Memory</skos:hasTopConcept>
        <dc:Date>2012-03-28 17:38:24</dc:Date>
        <skos:definition>the process of improving motor skills, the smoothness and accuracy of movements.</skos:definition>
        <dc:identifier>trm_4a3fd79d0a995</dc:identifier>
        <skos:prefLabel>Motor learning</skos:prefLabel>
        <skos:altLabel></skos:altLabel>
        <dc:Title>Motor learning</dc:Title>
    </owl:Class>
    


    <!-- http://www.cognitiveatlas.org/ontology/cogat.owl#CAO_00409 -->

    <owl:Class rdf:about="&cogat;CAO_00409">
        <rdfs:label>Motor planning</rdfs:label>
        <rdfs:subClassOf rdf:resource="&cogat;CAO_00001"/>
        <skos:definition>the conception of a future motoric action </skos:definition>
        <dc:Date>2012-03-28 17:42:32</dc:Date>
        <dc:Contributor>Russ Poldrack</dc:Contributor>
        <skos:altLabel>movement planning</skos:altLabel>
        <skos:prefLabel>Motor planning</skos:prefLabel>
        <dc:Title>Motor planning</dc:Title>
        <dc:identifier>trm_4a3fd79d0a9a1</dc:identifier>
        <skos:hasTopConcept>Action</skos:hasTopConcept>
    </owl:Class>
    


    <!-- http://www.cognitiveatlas.org/ontology/cogat.owl#CAO_00410 -->

    <owl:Class rdf:about="&cogat;CAO_00410">
        <rdfs:label>Motor program</rdfs:label>
        <rdfs:subClassOf rdf:resource="&cogat;CAO_00001"/>
        <skos:definition>abstract representation of a movement</skos:definition>
        <skos:prefLabel>Motor program</skos:prefLabel>
        <dc:identifier>trm_4a3fd79d0a9ad</dc:identifier>
        <skos:hasTopConcept>Action</skos:hasTopConcept>
        <dc:Contributor>Russ Poldrack</dc:Contributor>
        <skos:altLabel></skos:altLabel>
        <dc:Date>2012-03-28 17:40:05</dc:Date>
        <dc:Title>Motor program</dc:Title>
    </owl:Class>
    


    <!-- http://www.cognitiveatlas.org/ontology/cogat.owl#CAO_00411 -->

    <owl:Class rdf:about="&cogat;CAO_00411">
        <rdfs:label>Motor sequence learning</rdfs:label>
        <rdfs:subClassOf rdf:resource="&cogat;CAO_00510"/>
        <skos:hasTopConcept>Learning and Memory</skos:hasTopConcept>
        <skos:definition>The acquisition of knowledge regarding sequences of motor action</skos:definition>
        <skos:altLabel></skos:altLabel>
        <skos:prefLabel>Motor sequence learning</skos:prefLabel>
        <dc:Date>2012-03-28 17:41:31</dc:Date>
        <dc:identifier>trm_4a3fd79d0a9b9</dc:identifier>
        <dc:Title>Motor sequence learning</dc:Title>
        <dc:Contributor>Russ Poldrack</dc:Contributor>
    </owl:Class>
    


    <!-- http://www.cognitiveatlas.org/ontology/cogat.owl#CAO_00412 -->

    <owl:Class rdf:about="&cogat;CAO_00412">
        <rdfs:label>Movement</rdfs:label>
        <rdfs:subClassOf rdf:resource="&cogat;CAO_00001"/>
        <skos:altLabel></skos:altLabel>
        <dc:Title>Movement</dc:Title>
        <dc:Date>2012-03-28 17:41:51</dc:Date>
        <dc:identifier>trm_4a3fd79d0a9c4</dc:identifier>
        <skos:definition>change of place or position or posture</skos:definition>
        <dc:Contributor>Russ Poldrack</dc:Contributor>
        <skos:prefLabel>Movement</skos:prefLabel>
        <skos:hasTopConcept>Action</skos:hasTopConcept>
    </owl:Class>
    


    <!-- http://www.cognitiveatlas.org/ontology/cogat.owl#CAO_00414 -->

    <owl:Class rdf:about="&cogat;CAO_00414">
        <rdfs:label>Naming</rdfs:label>
        <rdfs:subClassOf rdf:resource="&cogat;CAO_00001"/>
        <skos:prefLabel>Naming</skos:prefLabel>
        <skos:altLabel></skos:altLabel>
        <skos:definition>the expression of the name of an object</skos:definition>
        <dc:Title>Naming</dc:Title>
        <dc:Contributor>Russ Poldrack</dc:Contributor>
        <skos:hasTopConcept>Language</skos:hasTopConcept>
        <dc:Date>2012-03-28 17:47:23</dc:Date>
        <dc:identifier>trm_4a3fd79d0a9dc</dc:identifier>
    </owl:Class>
    


    <!-- http://www.cognitiveatlas.org/ontology/cogat.owl#CAO_00415 -->

    <owl:Class rdf:about="&cogat;CAO_00415">
        <rdfs:label>Narrative</rdfs:label>
        <rdfs:subClassOf rdf:resource="&cogat;CAO_00001"/>
        <dc:Date>2012-03-28 17:47:36</dc:Date>
        <skos:prefLabel>Narrative</skos:prefLabel>
        <skos:definition>a story that is created in a constructive format (as a work of writing, speech, poetry, prose, pictures, song, motion pictures, video games, theater or dance) that describes a sequence of fictional or non-fictional events.</skos:definition>
        <dc:identifier>trm_4a3fd79d0a9e8</dc:identifier>
        <dc:Title>Narrative</dc:Title>
        <dc:Contributor>Russ Poldrack</dc:Contributor>
        <skos:hasTopConcept>Language</skos:hasTopConcept>
        <skos:altLabel></skos:altLabel>
    </owl:Class>
    


    <!-- http://www.cognitiveatlas.org/ontology/cogat.owl#CAO_00416 -->

    <owl:Class rdf:about="&cogat;CAO_00416">
        <rdfs:label>Navigation</rdfs:label>
        <rdfs:subClassOf rdf:resource="&cogat;CAO_00001"/>
        <skos:prefLabel>Navigation</skos:prefLabel>
        <skos:altLabel></skos:altLabel>
        <skos:definition>The process of controlling the movement of a body-entity-vehicle through space from one point to another.</skos:definition>
        <dc:identifier>trm_4a3fd79d0aa00</dc:identifier>
        <skos:hasTopConcept>Perception</skos:hasTopConcept>
        <dc:Date>2009-07-10 14:06:32</dc:Date>
        <dc:Contributor>Agatha Lenartowicz</dc:Contributor>
        <dc:Title>Navigation</dc:Title>
    </owl:Class>
    


    <!-- http://www.cognitiveatlas.org/ontology/cogat.owl#CAO_00417 -->

    <owl:Class rdf:about="&cogat;CAO_00417">
        <rdfs:label>Nociception</rdfs:label>
        <rdfs:subClassOf rdf:resource="&cogat;CAO_00001"/>
        <skos:definition>the processes of encoding and processing noxious stimuli.</skos:definition>
        <dc:Title>Nociception</dc:Title>
        <skos:prefLabel>Nociception</skos:prefLabel>
        <dc:Contributor>Russ Poldrack</dc:Contributor>
        <dc:identifier>trm_4a3fd79d0aa0c</dc:identifier>
        <skos:hasTopConcept>Perception</skos:hasTopConcept>
        <dc:Date>2012-03-28 17:48:12</dc:Date>
        <skos:altLabel></skos:altLabel>
    </owl:Class>
    


    <!-- http://www.cognitiveatlas.org/ontology/cogat.owl#CAO_00418 -->

    <owl:Class rdf:about="&cogat;CAO_00418">
        <rdfs:label>Nondeclarative knowledge</rdfs:label>
        <rdfs:subClassOf rdf:resource="&cogat;CAO_00001"/>
        <skos:altLabel></skos:altLabel>
        <skos:definition>The nonconscious or implicit ability to express and practice learned information.</skos:definition>
        <skos:prefLabel>Nondeclarative knowledge</skos:prefLabel>
        <dc:Contributor>Brenda Gregory</dc:Contributor>
        <dc:identifier>trm_4a3fd79d0aa23</dc:identifier>
        <dc:Date>2011-04-29 16:02:35</dc:Date>
        <dc:Title>Nondeclarative knowledge</dc:Title>
        <skos:hasTopConcept></skos:hasTopConcept>
    </owl:Class>
    


    <!-- http://www.cognitiveatlas.org/ontology/cogat.owl#CAO_00419 -->

    <owl:Class rdf:about="&cogat;CAO_00419">
        <rdfs:label>Nondeclarative memory</rdfs:label>
        <rdfs:subClassOf rdf:resource="&cogat;CAO_00394"/>
        <skos:hasTopConcept>Learning and Memory</skos:hasTopConcept>
        <dc:Date>2009-07-10 14:06:32</dc:Date>
        <skos:altLabel></skos:altLabel>
        <dc:Contributor>Agatha Lenartowicz</dc:Contributor>
        <dc:identifier>trm_4a3fd79d0aa2f</dc:identifier>
        <skos:prefLabel>Nondeclarative memory</skos:prefLabel>
        <dc:Title>Nondeclarative memory</dc:Title>
        <skos:definition>Memory acquired through experience and which can not be consciously articulated (such as by recall or recognition). This type of memory includes priming, conditioning, skill-acquisition, and habits.</skos:definition>
    </owl:Class>
    


    <!-- http://www.cognitiveatlas.org/ontology/cogat.owl#CAO_00420 -->

    <owl:Class rdf:about="&cogat;CAO_00420">
        <rdfs:label>Novelty detection</rdfs:label>
        <rdfs:subClassOf rdf:resource="&cogat;CAO_00001"/>
        <skos:prefLabel>Novelty detection</skos:prefLabel>
        <skos:altLabel></skos:altLabel>
        <skos:definition>the identification of new or unknown information</skos:definition>
        <dc:Date>2012-03-28 17:48:55</dc:Date>
        <dc:Contributor>Russ Poldrack</dc:Contributor>
        <dc:identifier>trm_4a3fd79d0aa47</dc:identifier>
        <dc:Title>Novelty detection</dc:Title>
        <skos:hasTopConcept></skos:hasTopConcept>
    </owl:Class>
    


    <!-- http://www.cognitiveatlas.org/ontology/cogat.owl#CAO_00421 -->

    <owl:Class rdf:about="&cogat;CAO_00421">
        <rdfs:label>Object categorization</rdfs:label>
        <rdfs:subClassOf rdf:resource="&cogat;CAO_00001"/>
        <dc:Title>Object categorization</dc:Title>
        <skos:prefLabel>Object categorization</skos:prefLabel>
        <skos:definition>the assignment of an object to a particular category</skos:definition>
        <dc:Date>2012-03-28 17:49:25</dc:Date>
        <dc:identifier>trm_4a3fd79d0aa5e</dc:identifier>
        <dc:Contributor>Russ Poldrack</dc:Contributor>
        <skos:altLabel></skos:altLabel>
        <skos:hasTopConcept></skos:hasTopConcept>
    </owl:Class>
    


    <!-- http://www.cognitiveatlas.org/ontology/cogat.owl#CAO_00422 -->

    <owl:Class rdf:about="&cogat;CAO_00422">
        <rdfs:label>Object centered representation</rdfs:label>
        <rdfs:subClassOf rdf:resource="&cogat;CAO_00397"/>
        <rdfs:subClassOf>
            <owl:Restriction>
                <owl:onProperty rdf:resource="&ro;part_of"/>
                <owl:someValuesFrom rdf:resource="&cogat;CAO_00428"/>
            </owl:Restriction>
        </rdfs:subClassOf>
        <dc:Date>2011-04-11 15:32:18</dc:Date>
        <dc:Title>Object centered representation</dc:Title>
        <dc:identifier>trm_4a3fd79d0aa6a</dc:identifier>
        <skos:hasTopConcept></skos:hasTopConcept>
        <skos:prefLabel>Object centered representation</skos:prefLabel>
        <dc:Contributor>Natalie Picchetti</dc:Contributor>
        <skos:definition>In an object-centered representation, the position of the subparts of an object are encoded with respect to a set of axes and an origin centered on the object. Several physiological and neuropsychological results support the existence of such representations in humans and monkeys. An explicit representation would involve neurons with invariant response properties in object-centered coordinates. </skos:definition>
        <skos:altLabel></skos:altLabel>
    </owl:Class>
    


    <!-- http://www.cognitiveatlas.org/ontology/cogat.owl#CAO_00423 -->

    <owl:Class rdf:about="&cogat;CAO_00423">
        <rdfs:label>Object detection</rdfs:label>
        <rdfs:subClassOf rdf:resource="&cogat;CAO_00001"/>
        <dc:Date>2012-03-28 17:49:53</dc:Date>
        <skos:altLabel></skos:altLabel>
        <skos:hasTopConcept>Perception</skos:hasTopConcept>
        <dc:identifier>trm_4a3fd79d0aa76</dc:identifier>
        <dc:Title>Object detection</dc:Title>
        <dc:Contributor>Russ Poldrack</dc:Contributor>
        <skos:prefLabel>Object detection</skos:prefLabel>
        <skos:definition>deals with detecting instances of semantic objects of a certain class (such as humans, buildings, cars, etc.).</skos:definition>
    </owl:Class>
    


    <!-- http://www.cognitiveatlas.org/ontology/cogat.owl#CAO_00425 -->

    <owl:Class rdf:about="&cogat;CAO_00425">
        <rdfs:label>Object manipulation</rdfs:label>
        <rdfs:subClassOf rdf:resource="&cogat;CAO_00001"/>
        <skos:prefLabel>Object manipulation</skos:prefLabel>
        <skos:hasTopConcept>Action</skos:hasTopConcept>
        <skos:definition>is a form of dexterity play or performance in which one or more artists physically interact with props such as balls, hoops, rings, poi, staff, devil sticks, or clubs. Object manipulation can be considered an advanced combinatorial form of sports, dance, and games.</skos:definition>
        <dc:Date>2012-03-28 17:50:34</dc:Date>
        <skos:altLabel></skos:altLabel>
        <dc:Title>Object manipulation</dc:Title>
        <dc:Contributor>Russ Poldrack</dc:Contributor>
        <dc:identifier>trm_4a3fd79d0aa8d</dc:identifier>
    </owl:Class>
    


    <!-- http://www.cognitiveatlas.org/ontology/cogat.owl#CAO_00426 -->

    <owl:Class rdf:about="&cogat;CAO_00426">
        <rdfs:label>Object orientation</rdfs:label>
        <rdfs:subClassOf rdf:resource="&cogat;CAO_00001"/>
        <dc:Title>Object orientation</dc:Title>
        <dc:Contributor>System Administrator</dc:Contributor>
        <skos:altLabel></skos:altLabel>
        <dc:Date>2009-07-10 14:06:32</dc:Date>
        <skos:definition>No definition submitted yet</skos:definition>
        <dc:identifier>trm_4a3fd79d0aa99</dc:identifier>
        <skos:prefLabel>Object orientation</skos:prefLabel>
        <skos:hasTopConcept></skos:hasTopConcept>
    </owl:Class>
    


    <!-- http://www.cognitiveatlas.org/ontology/cogat.owl#CAO_00427 -->

    <owl:Class rdf:about="&cogat;CAO_00427">
        <rdfs:label>Object perception</rdfs:label>
        <rdfs:subClassOf rdf:resource="&cogat;CAO_00001"/>
        <dc:identifier>trm_4a3fd79d0aaa4</dc:identifier>
        <skos:definition>The process of transforming basic visual sensory input (such as contrast, edge, motion, color etc) into a more abstract and semantically identifiable whole.</skos:definition>
        <dc:Contributor>Agatha Lenartowicz</dc:Contributor>
        <skos:altLabel></skos:altLabel>
        <dc:Date>2009-07-10 14:06:32</dc:Date>
        <skos:hasTopConcept>Perception</skos:hasTopConcept>
        <dc:Title>Object perception</dc:Title>
        <skos:prefLabel>Object perception</skos:prefLabel>
    </owl:Class>
    


    <!-- http://www.cognitiveatlas.org/ontology/cogat.owl#CAO_00428 -->

    <owl:Class rdf:about="&cogat;CAO_00428">
        <rdfs:label>Object recognition</rdfs:label>
        <rdfs:subClassOf rdf:resource="&cogat;CAO_00646"/>
        <skos:definition>is the ability to perceive an object’s physical properties (such as shape, colour and texture) and apply semantic attributes to the object, which includes the understanding of its use, previous experience with the object and how it relates to others. </skos:definition>
        <dc:Contributor>Russ Poldrack</dc:Contributor>
        <dc:identifier>trm_4a3fd79d0aab0</dc:identifier>
        <skos:altLabel>object identification</skos:altLabel>
        <skos:prefLabel>Object recognition</skos:prefLabel>
        <dc:Date>2012-03-28 17:51:30</dc:Date>
        <skos:hasTopConcept>Perception</skos:hasTopConcept>
        <dc:Title>Object recognition</dc:Title>
    </owl:Class>
    


    <!-- http://www.cognitiveatlas.org/ontology/cogat.owl#CAO_00429 -->

    <owl:Class rdf:about="&cogat;CAO_00429">
        <rdfs:label>Olfaction</rdfs:label>
        <rdfs:subClassOf rdf:resource="&cogat;CAO_00001"/>
        <rdfs:subClassOf>
            <owl:Restriction>
                <owl:onProperty rdf:resource="&ro;part_of"/>
                <owl:someValuesFrom rdf:resource="&cogat;CAO_00437"/>
            </owl:Restriction>
        </rdfs:subClassOf>
        <skos:hasTopConcept>Perception</skos:hasTopConcept>
        <dc:Contributor>Russ Poldrack</dc:Contributor>
        <skos:prefLabel>Olfaction</skos:prefLabel>
        <dc:Date>2012-03-28 17:51:44</dc:Date>
        <skos:altLabel></skos:altLabel>
        <dc:identifier>trm_4a3fd79d0aabc</dc:identifier>
        <dc:Title>Olfaction</dc:Title>
        <skos:definition>the sense of smell; the act or process of smelling.</skos:definition>
    </owl:Class>
    


    <!-- http://www.cognitiveatlas.org/ontology/cogat.owl#CAO_00430 -->

    <owl:Class rdf:about="&cogat;CAO_00430">
        <rdfs:label>Olfactory perception</rdfs:label>
        <rdfs:subClassOf rdf:resource="&cogat;CAO_00437"/>
        <dc:Contributor>Brenda Gregory</dc:Contributor>
        <skos:altLabel></skos:altLabel>
        <skos:prefLabel>Olfactory perception</skos:prefLabel>
        <skos:hasTopConcept>Perception</skos:hasTopConcept>
        <skos:definition>the sensation that results when olfactory receptors in the nose are stimulated by particular chemicals in gaseous form. </skos:definition>
        <dc:Date>2011-04-29 16:19:58</dc:Date>
        <dc:Title>Olfactory perception</dc:Title>
        <dc:identifier>trm_4a3fd79d0aac8</dc:identifier>
    </owl:Class>
    


    <!-- http://www.cognitiveatlas.org/ontology/cogat.owl#CAO_00431 -->

    <owl:Class rdf:about="&cogat;CAO_00431">
        <rdfs:label>Orthographic lexicon</rdfs:label>
        <rdfs:subClassOf rdf:resource="&cogat;CAO_00381"/>
        <skos:definition>A set of representations of orthographic information</skos:definition>
        <dc:identifier>trm_4a3fd79d0aad4</dc:identifier>
        <dc:Date>2012-03-28 17:53:02</dc:Date>
        <skos:altLabel></skos:altLabel>
        <skos:hasTopConcept>Language</skos:hasTopConcept>
        <dc:Title>Orthographic lexicon</dc:Title>
        <dc:Contributor>Russ Poldrack</dc:Contributor>
        <skos:prefLabel>Orthographic lexicon</skos:prefLabel>
    </owl:Class>
    


    <!-- http://www.cognitiveatlas.org/ontology/cogat.owl#CAO_00432 -->

    <owl:Class rdf:about="&cogat;CAO_00432">
        <rdfs:label>Parsing</rdfs:label>
        <rdfs:subClassOf rdf:resource="&cogat;CAO_00001"/>
        <dc:identifier>trm_4a3fd79d0ab42</dc:identifier>
        <skos:definition>to resolve (as a sentence) into component parts of speech and describe them grammatically</skos:definition>
        <dc:Title>Parsing</dc:Title>
        <skos:hasTopConcept>Language</skos:hasTopConcept>
        <skos:altLabel></skos:altLabel>
        <dc:Date>2012-03-28 17:54:29</dc:Date>
        <dc:Contributor>Russ Poldrack</dc:Contributor>
        <skos:prefLabel>Parsing</skos:prefLabel>
    </owl:Class>
    


    <!-- http://www.cognitiveatlas.org/ontology/cogat.owl#CAO_00433 -->

    <owl:Class rdf:about="&cogat;CAO_00433">
        <rdfs:label>Passive attention</rdfs:label>
        <rdfs:subClassOf rdf:resource="&cogat;CAO_00144"/>
        <dc:Contributor>Natalie Picchetti</dc:Contributor>
        <dc:Date>2011-04-12 09:38:58</dc:Date>
        <skos:prefLabel>Passive attention</skos:prefLabel>
        <dc:Title>Passive attention</dc:Title>
        <skos:hasTopConcept>Attention</skos:hasTopConcept>
        <dc:identifier>trm_4a3fd79d0ab4d</dc:identifier>
        <skos:altLabel></skos:altLabel>
        <skos:definition>refers to the involuntary process directed by external events that stand out from their environment, such as a bright flash, a strong odor, or a sudden loud noise. </skos:definition>
    </owl:Class>
    


    <!-- http://www.cognitiveatlas.org/ontology/cogat.owl#CAO_00434 -->

    <owl:Class rdf:about="&cogat;CAO_00434">
        <rdfs:label>Past tense</rdfs:label>
        <rdfs:subClassOf rdf:resource="&cogat;CAO_00001"/>
        <rdfs:subClassOf>
            <owl:Restriction>
                <owl:onProperty rdf:resource="&ro;part_of"/>
                <owl:someValuesFrom rdf:resource="&cogat;CAO_00372"/>
            </owl:Restriction>
        </rdfs:subClassOf>
        <skos:altLabel></skos:altLabel>
        <dc:Title>Past tense</dc:Title>
        <dc:Contributor>Joseph Devlin</dc:Contributor>
        <skos:prefLabel>Past tense</skos:prefLabel>
        <skos:hasTopConcept>Language</skos:hasTopConcept>
        <skos:definition>refers to a form of a verb that indicates that the action already has occurred </skos:definition>
        <dc:Date>2010-01-30 14:22:27</dc:Date>
        <dc:identifier>trm_4a3fd79d0ab59</dc:identifier>
    </owl:Class>
    


    <!-- http://www.cognitiveatlas.org/ontology/cogat.owl#CAO_00435 -->

    <owl:Class rdf:about="&cogat;CAO_00435">
        <rdfs:label>Pattern recognition</rdfs:label>
        <rdfs:subClassOf rdf:resource="&cogat;CAO_00001"/>
        <dc:identifier>trm_4a3fd79d0ab65</dc:identifier>
        <dc:Contributor>Tal Yarkoni</dc:Contributor>
        <dc:Date>2010-04-27 07:35:02</dc:Date>
        <skos:hasTopConcept>Perception</skos:hasTopConcept>
        <skos:altLabel></skos:altLabel>
        <skos:definition>The process of identifying a meaningful pattern in raw data.</skos:definition>
        <dc:Title>Pattern recognition</dc:Title>
        <skos:prefLabel>Pattern recognition</skos:prefLabel>
    </owl:Class>
    


    <!-- http://www.cognitiveatlas.org/ontology/cogat.owl#CAO_00436 -->

    <owl:Class rdf:about="&cogat;CAO_00436">
        <rdfs:label>Pavlovian conditioning</rdfs:label>
        <rdfs:subClassOf rdf:resource="&cogat;CAO_00001"/>
        <skos:prefLabel>Pavlovian conditioning</skos:prefLabel>
        <dc:Contributor>Brenda Gregory</dc:Contributor>
        <skos:hasTopConcept></skos:hasTopConcept>
        <dc:Date>2011-05-18 12:23:11</dc:Date>
        <skos:definition>a form of learning in which either (1) a given stimulus (or signal) becomes increasingly effective in evoking a response or (2) a response occurs with increasing regularity in a well-specified and stable environment. The type of reinforcement used will determine the outcome. When two stimuli are presented in an appropriate time and intensity relationship, one of them will eventually induce a response resembling that of the other. The process can be described as one of stimulus substitution. This procedure is called classical (or respondent) conditioning; based on the work of the Russian physiologist Ivan P. Pavlov.</skos:definition>
        <dc:Title>Pavlovian conditioning</dc:Title>
        <dc:identifier>trm_4a3fd79d0ab70</dc:identifier>
        <skos:altLabel></skos:altLabel>
    </owl:Class>
    


    <!-- http://www.cognitiveatlas.org/ontology/cogat.owl#CAO_00437 -->

    <owl:Class rdf:about="&cogat;CAO_00437">
        <rdfs:label>Perception</rdfs:label>
        <rdfs:subClassOf rdf:resource="&cogat;CAO_00001"/>
        <skos:altLabel></skos:altLabel>
        <dc:Contributor>Naomi Kenner</dc:Contributor>
        <skos:prefLabel>Perception</skos:prefLabel>
        <skos:definition>the conscious experience or mental registration of a sensory stimulus</skos:definition>
        <dc:identifier>trm_4a3fd79d0ab7c</dc:identifier>
        <skos:hasTopConcept>Perception</skos:hasTopConcept>
        <dc:Date>2009-07-10 14:06:32</dc:Date>
        <dc:Title>Perception</dc:Title>
    </owl:Class>
    


    <!-- http://www.cognitiveatlas.org/ontology/cogat.owl#CAO_00438 -->

    <owl:Class rdf:about="&cogat;CAO_00438">
        <rdfs:label>Perceptual binding</rdfs:label>
        <rdfs:subClassOf rdf:resource="&cogat;CAO_00001"/>
        <dc:identifier>trm_4a3fd79d0ab88</dc:identifier>
        <dc:Title>Perceptual binding</dc:Title>
        <dc:Date>2011-04-07 11:39:48</dc:Date>
        <skos:prefLabel>Perceptual binding</skos:prefLabel>
        <skos:definition>is the cognitive ability to couple characteristics between items that one is perceiving.  This can be illustrated by the one observing a blue square and a yellow circle.  Through the neural mechanisms of perceptual binding, one can ensure that the sensing of blue is coupled to that of a square shape and that of yellow is coupled to that of a circle. </skos:definition>
        <dc:Contributor>Natalie Picchetti</dc:Contributor>
        <skos:altLabel></skos:altLabel>
        <skos:hasTopConcept>Perception</skos:hasTopConcept>
    </owl:Class>
    


    <!-- http://www.cognitiveatlas.org/ontology/cogat.owl#CAO_00439 -->

    <owl:Class rdf:about="&cogat;CAO_00439">
        <rdfs:label>Perceptual categorization</rdfs:label>
        <rdfs:subClassOf rdf:resource="&cogat;CAO_00001"/>
        <dc:Date>2011-04-07 11:21:36</dc:Date>
        <dc:identifier>trm_4a3fd79d0ab93</dc:identifier>
        <dc:Title>Perceptual categorization</dc:Title>
        <skos:definition>A selective system that can have no a priori information about the particular stimuli that might be encountered in its environment, other than boundary conditions implicit in the construction of its recognizing elements. Perceptual categorization, according to this view, does not involve the and#34;reading inand#34; of readily available information about the stimulus category; rather, it involves the utilization of multiple cues in degenerate, overlapping sets and under the influence of context. </skos:definition>
        <skos:prefLabel>Perceptual categorization</skos:prefLabel>
        <dc:Contributor>Natalie Picchetti</dc:Contributor>
        <skos:hasTopConcept>Perception</skos:hasTopConcept>
        <skos:altLabel></skos:altLabel>
    </owl:Class>
    


    <!-- http://www.cognitiveatlas.org/ontology/cogat.owl#CAO_00440 -->

    <owl:Class rdf:about="&cogat;CAO_00440">
        <rdfs:label>Perceptual fluency</rdfs:label>
        <rdfs:subClassOf rdf:resource="&cogat;CAO_00001"/>
        <skos:hasTopConcept>Perception</skos:hasTopConcept>
        <skos:altLabel></skos:altLabel>
        <dc:Title>Perceptual fluency</dc:Title>
        <skos:prefLabel>Perceptual fluency</skos:prefLabel>
        <skos:definition>is the ease at which the brain can process information. </skos:definition>
        <dc:Date>2011-04-12 09:30:51</dc:Date>
        <dc:Contributor>Natalie Picchetti</dc:Contributor>
        <dc:identifier>trm_4a3fd79d0ab9f</dc:identifier>
    </owl:Class>
    


    <!-- http://www.cognitiveatlas.org/ontology/cogat.owl#CAO_00441 -->

    <owl:Class rdf:about="&cogat;CAO_00441">
        <rdfs:label>Perceptual identification</rdfs:label>
        <rdfs:subClassOf rdf:resource="&cogat;CAO_00001"/>
        <dc:Date>2011-04-11 15:45:46</dc:Date>
        <skos:definition>has two different processing stages.  The first stage yields a state of of perceptual information about the stimulus presented.  The second stage is the processing of attained perceptual information in a response. </skos:definition>
        <skos:hasTopConcept>Perception</skos:hasTopConcept>
        <skos:prefLabel>Perceptual identification</skos:prefLabel>
        <dc:identifier>trm_4a3fd79d0abaa</dc:identifier>
        <dc:Title>Perceptual identification</dc:Title>
        <dc:Contributor>Natalie Picchetti</dc:Contributor>
        <skos:altLabel></skos:altLabel>
    </owl:Class>
    


    <!-- http://www.cognitiveatlas.org/ontology/cogat.owl#CAO_00442 -->

    <owl:Class rdf:about="&cogat;CAO_00442">
        <rdfs:label>Perceptual learning</rdfs:label>
        <rdfs:subClassOf rdf:resource="&cogat;CAO_00377"/>
        <dc:Title>Perceptual learning</dc:Title>
        <skos:hasTopConcept>Learning and Memory</skos:hasTopConcept>
        <skos:prefLabel>Perceptual learning</skos:prefLabel>
        <dc:Contributor>Brenda Gregory</dc:Contributor>
        <skos:definition>long lasting improvement in performing perceptual  (visual, auditory, tactile, olfactory or taste) tasks as a function of experience.</skos:definition>
        <dc:Date>2011-05-04 11:06:32</dc:Date>
        <skos:altLabel></skos:altLabel>
        <dc:identifier>trm_4a3fd79d0abb6</dc:identifier>
    </owl:Class>
    


    <!-- http://www.cognitiveatlas.org/ontology/cogat.owl#CAO_00443 -->

    <owl:Class rdf:about="&cogat;CAO_00443">
        <rdfs:label>Perceptual similarity</rdfs:label>
        <rdfs:subClassOf rdf:resource="&cogat;CAO_00001"/>
        <dc:Contributor>Matt Craddock</dc:Contributor>
        <skos:definition>Perceptual similarity is the subjective similarity between two stimuli as perceived by the observer. Thus, object A may be rated as more similar to object B than to object C despite a greater difference in some physical metric (such as height or width) between objects A and C than between objects A and B. This may differ across modalities: for example, two objects may be rated as more similar when seen than when touched. However, the physical, objective similarity between the two objects remains the same regardless of which modality is used to explore them.</skos:definition>
        <skos:prefLabel>Perceptual similarity</skos:prefLabel>
        <dc:Title>Perceptual similarity</dc:Title>
        <skos:altLabel></skos:altLabel>
        <dc:Date>2011-10-03 05:34:23</dc:Date>
        <skos:hasTopConcept>Perception</skos:hasTopConcept>
        <dc:identifier>trm_4a3fd79d0abc1</dc:identifier>
    </owl:Class>
    


    <!-- http://www.cognitiveatlas.org/ontology/cogat.owl#CAO_00444 -->

    <owl:Class rdf:about="&cogat;CAO_00444">
        <rdfs:label>Perceptual skill</rdfs:label>
        <rdfs:subClassOf rdf:resource="&cogat;CAO_00001"/>
        <skos:prefLabel>Perceptual skill</skos:prefLabel>
        <dc:Contributor>Brenda Gregory</dc:Contributor>
        <dc:identifier>trm_4a3fd79d0abcd</dc:identifier>
        <dc:Date>2010-03-11 15:54:28</dc:Date>
        <dc:Title>Perceptual skill</dc:Title>
        <skos:definition>The ability to observe and understand the events surrounding an individual.</skos:definition>
        <skos:altLabel></skos:altLabel>
        <skos:hasTopConcept>Perception</skos:hasTopConcept>
    </owl:Class>
    


    <!-- http://www.cognitiveatlas.org/ontology/cogat.owl#CAO_00445 -->

    <owl:Class rdf:about="&cogat;CAO_00445">
        <rdfs:label>Performance monitoring</rdfs:label>
        <rdfs:subClassOf rdf:resource="&cogat;CAO_00001"/>
        <skos:hasTopConcept>Executive-Cognitive Control</skos:hasTopConcept>
        <skos:prefLabel>Performance monitoring</skos:prefLabel>
        <dc:identifier>trm_4a3fd79d0ac30</dc:identifier>
        <dc:Title>Performance monitoring</dc:Title>
        <dc:Contributor>Russ Poldrack</dc:Contributor>
        <skos:altLabel></skos:altLabel>
        <dc:Date>2012-03-28 17:56:20</dc:Date>
        <skos:definition>the online evaluation of oneand#39;s performance on a task</skos:definition>
    </owl:Class>
    


    <!-- http://www.cognitiveatlas.org/ontology/cogat.owl#CAO_00446 -->

    <owl:Class rdf:about="&cogat;CAO_00446">
        <rdfs:label>Phonation</rdfs:label>
        <rdfs:subClassOf rdf:resource="&cogat;CAO_00001"/>
        <skos:definition>process by which the vocal folds produce certain sounds through quasi-periodic vibration; any oscillatory state of any part of the larynx that modifies the airstream.</skos:definition>
        <dc:identifier>trm_4a3fd79d0ac4a</dc:identifier>
        <skos:prefLabel>Phonation</skos:prefLabel>
        <dc:Date>2011-04-19 13:55:33</dc:Date>
        <dc:Title>Phonation</dc:Title>
        <skos:altLabel></skos:altLabel>
        <skos:hasTopConcept>Language</skos:hasTopConcept>
        <dc:Contributor>Brenda Gregory</dc:Contributor>
    </owl:Class>
    


    <!-- http://www.cognitiveatlas.org/ontology/cogat.owl#CAO_00447 -->

    <owl:Class rdf:about="&cogat;CAO_00447">
        <rdfs:label>Phonological buffer</rdfs:label>
        <rdfs:subClassOf rdf:resource="&cogat;CAO_00001"/>
        <rdfs:subClassOf>
            <owl:Restriction>
                <owl:onProperty rdf:resource="&ro;part_of"/>
                <owl:someValuesFrom rdf:resource="&cogat;CAO_00171"/>
            </owl:Restriction>
        </rdfs:subClassOf>
        <dc:Title>Phonological buffer</dc:Title>
        <skos:prefLabel>Phonological buffer</skos:prefLabel>
        <dc:identifier>trm_4a3fd79d0ac61</dc:identifier>
        <dc:Contributor>Russ Poldrack</dc:Contributor>
        <skos:hasTopConcept>Language</skos:hasTopConcept>
        <dc:Date>2012-03-28 17:57:17</dc:Date>
        <skos:altLabel></skos:altLabel>
        <skos:definition>a passive storage device that is part of the articulatory rehearsal loop; serves as a part of the mechanisms ordinarily needed for hearing.  In rehearsal, the buffer is loaded by means of subvocalization.</skos:definition>
    </owl:Class>
    


    <!-- http://www.cognitiveatlas.org/ontology/cogat.owl#CAO_00448 -->

    <owl:Class rdf:about="&cogat;CAO_00448">
        <rdfs:label>Phonological code</rdfs:label>
        <rdfs:subClassOf rdf:resource="&cogat;CAO_00001"/>
        <dc:Date>2012-03-28 17:57:45</dc:Date>
        <skos:altLabel></skos:altLabel>
        <dc:Contributor>Russ Poldrack</dc:Contributor>
        <dc:identifier>trm_4a3fd79d0ac7a</dc:identifier>
        <dc:Title>Phonological code</dc:Title>
        <skos:definition>A representation of information using phonological features</skos:definition>
        <skos:hasTopConcept></skos:hasTopConcept>
        <skos:prefLabel>Phonological code</skos:prefLabel>
    </owl:Class>
    


    <!-- http://www.cognitiveatlas.org/ontology/cogat.owl#CAO_00449 -->

    <owl:Class rdf:about="&cogat;CAO_00449">
        <rdfs:label>Phonological encoding</rdfs:label>
        <rdfs:subClassOf rdf:resource="&cogat;CAO_00001"/>
        <rdfs:subClassOf>
            <owl:Restriction>
                <owl:onProperty rdf:resource="&ro;part_of"/>
                <owl:someValuesFrom rdf:resource="&cogat;CAO_00154"/>
            </owl:Restriction>
        </rdfs:subClassOf>
        <dc:Contributor>Natalie Picchetti</dc:Contributor>
        <dc:Title>Phonological encoding</dc:Title>
        <dc:identifier>trm_4a3fd79d0ac87</dc:identifier>
        <skos:prefLabel>Phonological encoding</skos:prefLabel>
        <skos:altLabel></skos:altLabel>
        <skos:hasTopConcept>Language</skos:hasTopConcept>
        <skos:definition>involves retrieval of segmental and supra-segmental information and the generation of a syllabified phonological word, and the computation of the phonetic form of the intended utterance, referred to as phonetic encoding.  </skos:definition>
        <dc:Date>2011-04-11 13:26:04</dc:Date>
    </owl:Class>
    


    <!-- http://www.cognitiveatlas.org/ontology/cogat.owl#CAO_00450 -->

    <owl:Class rdf:about="&cogat;CAO_00450">
        <rdfs:label>Phonological retrieval</rdfs:label>
        <rdfs:subClassOf rdf:resource="&cogat;CAO_00490"/>
        <skos:hasTopConcept>Language</skos:hasTopConcept>
        <dc:Date>2012-03-28 17:59:31</dc:Date>
        <skos:definition>The retrieval of phonological representations based on other cues</skos:definition>
        <dc:Title>Phonological retrieval</dc:Title>
        <skos:altLabel></skos:altLabel>
        <dc:Contributor>Russ Poldrack</dc:Contributor>
        <skos:prefLabel>Phonological retrieval</skos:prefLabel>
        <dc:identifier>trm_4a3fd79d0ac93</dc:identifier>
    </owl:Class>
    


    <!-- http://www.cognitiveatlas.org/ontology/cogat.owl#CAO_00451 -->

    <owl:Class rdf:about="&cogat;CAO_00451">
        <rdfs:label>Phonological working memory</rdfs:label>
        <rdfs:subClassOf rdf:resource="&cogat;CAO_00587"/>
        <skos:definition>The process of maintaining sound information online for a limited amount of time.</skos:definition>
        <skos:altLabel></skos:altLabel>
        <skos:hasTopConcept>Executive-Cognitive Control</skos:hasTopConcept>
        <skos:prefLabel>Phonological working memory</skos:prefLabel>
        <dc:identifier>trm_4a3fd79d0ac9e</dc:identifier>
        <dc:Contributor>Agatha Lenartowicz</dc:Contributor>
        <dc:Title>Phonological working memory</dc:Title>
        <dc:Date>2009-07-10 14:06:32</dc:Date>
    </owl:Class>
    


    <!-- http://www.cognitiveatlas.org/ontology/cogat.owl#CAO_00452 -->

    <owl:Class rdf:about="&cogat;CAO_00452">
        <rdfs:label>Planning</rdfs:label>
        <rdfs:subClassOf rdf:resource="&cogat;CAO_00001"/>
        <dc:Date>2012-02-23 08:46:45</dc:Date>
        <dc:Contributor>Michael Sharman</dc:Contributor>
        <dc:identifier>trm_4a3fd79d0acc1</dc:identifier>
        <dc:Title>Planning</dc:Title>
        <skos:definition>formulation, evaluation and selection of a sequence of actions to achieve a desired goal.</skos:definition>
        <skos:hasTopConcept>Executive-Cognitive Control</skos:hasTopConcept>
        <skos:altLabel></skos:altLabel>
        <skos:prefLabel>Planning</skos:prefLabel>
    </owl:Class>
    


    <!-- http://www.cognitiveatlas.org/ontology/cogat.owl#CAO_00453 -->

    <owl:Class rdf:about="&cogat;CAO_00453">
        <rdfs:label>Pragmatic inference</rdfs:label>
        <rdfs:subClassOf rdf:resource="&cogat;CAO_00346"/>
        <skos:definition>Inferences are made when a person (or machine) goes beyond available evidence to form a conclusion. A pragmatic inference (also known as an inductive inference) is one which is likely to be true because of the state of the world. Unlike deductive inferences, pragmatic (inductive) inferences do yield conclusions that increase the semantic information over and above that found in the initial premises. </skos:definition>
        <skos:altLabel></skos:altLabel>
        <skos:hasTopConcept>Reasoning and Decision Making</skos:hasTopConcept>
        <skos:prefLabel>Pragmatic inference</skos:prefLabel>
        <dc:Title>Pragmatic inference</dc:Title>
        <dc:identifier>trm_4a3fd79d0ad12</dc:identifier>
        <dc:Contributor>Natalie Picchetti</dc:Contributor>
        <dc:Date>2011-04-18 11:12:02</dc:Date>
    </owl:Class>
    


    <!-- http://www.cognitiveatlas.org/ontology/cogat.owl#CAO_00454 -->

    <owl:Class rdf:about="&cogat;CAO_00454">
        <rdfs:label>Pragmatic knowledge</rdfs:label>
        <rdfs:subClassOf rdf:resource="&cogat;CAO_00371"/>
        <skos:altLabel></skos:altLabel>
        <dc:identifier>trm_4a3fd79d0ad1d</dc:identifier>
        <skos:prefLabel>Pragmatic knowledge</skos:prefLabel>
        <dc:Contributor>Natalie Picchetti</dc:Contributor>
        <dc:Date>2011-04-12 11:51:53</dc:Date>
        <skos:definition>is how individuals communicate meaning and how they produce contextually appropriate utterances, sentences, or texts.  Pragmatic knowledge includes sociolinguistic and functional knowledge.  </skos:definition>
        <skos:hasTopConcept></skos:hasTopConcept>
        <dc:Title>Pragmatic knowledge</dc:Title>
    </owl:Class>
    


    <!-- http://www.cognitiveatlas.org/ontology/cogat.owl#CAO_00455 -->

    <owl:Class rdf:about="&cogat;CAO_00455">
        <rdfs:label>Pragmatic reasoning</rdfs:label>
        <rdfs:subClassOf rdf:resource="&cogat;CAO_00480"/>
        <skos:altLabel></skos:altLabel>
        <dc:Date>2012-03-28 18:02:00</dc:Date>
        <skos:prefLabel>Pragmatic reasoning</skos:prefLabel>
        <dc:Contributor>Russ Poldrack</dc:Contributor>
        <skos:hasTopConcept>Reasoning and Decision Making</skos:hasTopConcept>
        <dc:Title>Pragmatic reasoning</dc:Title>
        <skos:definition>Pragmatic reasoning is defined as the process of finding the intended meaning(s) of the given, and it is suggested that this amounts to the process of inferring the appropriate context(s) in which to interpret the given.</skos:definition>
        <dc:identifier>trm_4a3fd79d0ad29</dc:identifier>
    </owl:Class>
    


    <!-- http://www.cognitiveatlas.org/ontology/cogat.owl#CAO_00456 -->

    <owl:Class rdf:about="&cogat;CAO_00456">
        <rdfs:label>Preattentive processing</rdfs:label>
        <rdfs:subClassOf rdf:resource="&cogat;CAO_00001"/>
        <dc:Title>Preattentive processing</dc:Title>
        <skos:prefLabel>Preattentive processing</skos:prefLabel>
        <dc:identifier>trm_4a3fd79d0ad41</dc:identifier>
        <skos:definition>background activity that necessarily precedes conscious mental activity; major purpose is the preparation of sensory input for use in focal-attentive processes including encoding of the basic properties of sensory input.</skos:definition>
        <skos:hasTopConcept>Attention</skos:hasTopConcept>
        <dc:Date>2012-03-28 18:02:16</dc:Date>
        <dc:Contributor>Russ Poldrack</dc:Contributor>
        <skos:altLabel></skos:altLabel>
    </owl:Class>
    


    <!-- http://www.cognitiveatlas.org/ontology/cogat.owl#CAO_00457 -->

    <owl:Class rdf:about="&cogat;CAO_00457">
        <rdfs:label>Preconscious perception</rdfs:label>
        <rdfs:subClassOf rdf:resource="&cogat;CAO_00001"/>
        <rdfs:subClassOf>
            <owl:Restriction>
                <owl:onProperty rdf:resource="&ro;part_of"/>
                <owl:someValuesFrom rdf:resource="&cogat;CAO_00683"/>
            </owl:Restriction>
        </rdfs:subClassOf>
        <dc:Date>2011-04-12 09:24:58</dc:Date>
        <skos:prefLabel>Preconscious perception</skos:prefLabel>
        <dc:identifier>trm_4a3fd79d0ad4c</dc:identifier>
        <skos:altLabel></skos:altLabel>
        <skos:hasTopConcept>Perception</skos:hasTopConcept>
        <dc:Title>Preconscious perception</dc:Title>
        <skos:definition>is the subthreshold process of visual perception.  </skos:definition>
        <dc:Contributor>Natalie Picchetti</dc:Contributor>
    </owl:Class>
    


    <!-- http://www.cognitiveatlas.org/ontology/cogat.owl#CAO_00459 -->

    <owl:Class rdf:about="&cogat;CAO_00459">
        <rdfs:label>Prejudice</rdfs:label>
        <rdfs:subClassOf rdf:resource="&cogat;CAO_00001"/>
        <dc:Title>Prejudice</dc:Title>
        <skos:prefLabel>Prejudice</skos:prefLabel>
        <skos:definition>preconceived judgment or opinion; an adverse opinion or leaning formed without just grounds or before sufficient knowledge; an irrational attitude of hostility directed against an individual, a group, a race, or their supposed characteristics.</skos:definition>
        <dc:identifier>trm_4a3fd79d0ad64</dc:identifier>
        <dc:Contributor>Brenda Gregory</dc:Contributor>
        <skos:hasTopConcept></skos:hasTopConcept>
        <dc:Date>2011-05-17 10:07:32</dc:Date>
        <skos:altLabel></skos:altLabel>
    </owl:Class>
    


    <!-- http://www.cognitiveatlas.org/ontology/cogat.owl#CAO_00460 -->

    <owl:Class rdf:about="&cogat;CAO_00460">
        <rdfs:label>Primary memory</rdfs:label>
        <rdfs:subClassOf rdf:resource="&cogat;CAO_00394"/>
        <skos:altLabel></skos:altLabel>
        <skos:prefLabel>Primary memory</skos:prefLabel>
        <skos:hasTopConcept>Learning and Memory</skos:hasTopConcept>
        <dc:Contributor>Brenda Gregory</dc:Contributor>
        <skos:definition>the temporary maintenance system for conscious processing of information.</skos:definition>
        <dc:Title>Primary memory</dc:Title>
        <dc:identifier>trm_4a3fd79d0ad94</dc:identifier>
        <dc:Date>2011-04-28 16:07:46</dc:Date>
    </owl:Class>
    


    <!-- http://www.cognitiveatlas.org/ontology/cogat.owl#CAO_00462 -->

    <owl:Class rdf:about="&cogat;CAO_00462">
        <rdfs:label>Proactive interference</rdfs:label>
        <rdfs:subClassOf rdf:resource="&cogat;CAO_00001"/>
        <skos:prefLabel>Proactive interference</skos:prefLabel>
        <dc:Date>2012-03-28 18:09:21</dc:Date>
        <skos:hasTopConcept>Learning and Memory</skos:hasTopConcept>
        <dc:Contributor>Russ Poldrack</dc:Contributor>
        <dc:identifier>trm_4a3fd79d0adab</dc:identifier>
        <skos:altLabel></skos:altLabel>
        <dc:Title>Proactive interference</dc:Title>
        <skos:definition>the forgetting of information due to interference from the traces of events or learning that occurred prior to the materials to be remembered; occurs when in any given context, past memories inhibit an individual’s full potential to retain new memories.</skos:definition>
    </owl:Class>
    


    <!-- http://www.cognitiveatlas.org/ontology/cogat.owl#CAO_00463 -->

    <owl:Class rdf:about="&cogat;CAO_00463">
        <rdfs:label>Problem solving</rdfs:label>
        <rdfs:subClassOf rdf:resource="&cogat;CAO_00480"/>
        <dc:Contributor>Naomi Kenner</dc:Contributor>
        <dc:Title>Problem solving</dc:Title>
        <dc:identifier>trm_4a3fd79d0adb7</dc:identifier>
        <skos:prefLabel>Problem solving</skos:prefLabel>
        <skos:altLabel></skos:altLabel>
        <skos:definition>Broadly, the mental processes involved in finding a solution to a problem.</skos:definition>
        <skos:hasTopConcept>Reasoning and Decision Making</skos:hasTopConcept>
        <dc:Date>2009-07-10 14:06:32</dc:Date>
    </owl:Class>
    


    <!-- http://www.cognitiveatlas.org/ontology/cogat.owl#CAO_00464 -->

    <owl:Class rdf:about="&cogat;CAO_00464">
        <rdfs:label>Procedural knowledge</rdfs:label>
        <rdfs:subClassOf rdf:resource="&cogat;CAO_00371"/>
        <dc:Date>2012-03-28 18:10:20</dc:Date>
        <skos:altLabel></skos:altLabel>
        <dc:Contributor>Russ Poldrack</dc:Contributor>
        <skos:definition>Knowledge exercised in the performance of a task-activity. Its acquisition or structure is often unavailable to the actor.</skos:definition>
        <dc:identifier>trm_4a3fd79d0adc3</dc:identifier>
        <skos:prefLabel>Procedural knowledge</skos:prefLabel>
        <skos:hasTopConcept>Learning and Memory</skos:hasTopConcept>
        <dc:Title>Procedural knowledge</dc:Title>
    </owl:Class>
    


    <!-- http://www.cognitiveatlas.org/ontology/cogat.owl#CAO_00465 -->

    <owl:Class rdf:about="&cogat;CAO_00465">
        <rdfs:label>Procedural learning</rdfs:label>
        <rdfs:subClassOf rdf:resource="&cogat;CAO_00377"/>
        <dc:Title>Procedural learning</dc:Title>
        <dc:Date>2012-03-28 18:11:17</dc:Date>
        <skos:hasTopConcept>Learning and Memory</skos:hasTopConcept>
        <skos:definition>The acquisition of a skill or ability through practice which is not accessible to verbalization or conscious awareness.</skos:definition>
        <skos:altLabel></skos:altLabel>
        <dc:identifier>trm_4a3fd79d0adcf</dc:identifier>
        <dc:Contributor>Russ Poldrack</dc:Contributor>
        <skos:prefLabel>Procedural learning</skos:prefLabel>
    </owl:Class>
    


    <!-- http://www.cognitiveatlas.org/ontology/cogat.owl#CAO_00466 -->

    <owl:Class rdf:about="&cogat;CAO_00466">
        <rdfs:label>Procedural memory</rdfs:label>
        <rdfs:subClassOf rdf:resource="&cogat;CAO_00419"/>
        <dc:Contributor>Brenda Gregory</dc:Contributor>
        <skos:prefLabel>Procedural memory</skos:prefLabel>
        <skos:altLabel></skos:altLabel>
        <skos:hasTopConcept></skos:hasTopConcept>
        <skos:definition>memory for how to do things; procedural memories are automatically retrieved and utilized for the execution of the step-by-step procedures involved in both cognitive and motor skills.</skos:definition>
        <dc:Title>Procedural memory</dc:Title>
        <dc:Date>2011-05-10 14:43:54</dc:Date>
        <dc:identifier>trm_4a3fd79d0addc</dc:identifier>
    </owl:Class>
    


    <!-- http://www.cognitiveatlas.org/ontology/cogat.owl#CAO_00467 -->

    <owl:Class rdf:about="&cogat;CAO_00467">
        <rdfs:label>Procedural rule</rdfs:label>
        <rdfs:subClassOf rdf:resource="&cogat;CAO_00001"/>
        <dc:Date>2009-07-10 14:06:32</dc:Date>
        <skos:prefLabel>Procedural rule</skos:prefLabel>
        <dc:Title>Procedural rule</dc:Title>
        <skos:definition>No definition submitted yet</skos:definition>
        <dc:Contributor>System Administrator</dc:Contributor>
        <dc:identifier>trm_4a3fd79d0ade8</dc:identifier>
        <skos:hasTopConcept></skos:hasTopConcept>
        <skos:altLabel></skos:altLabel>
    </owl:Class>
    


    <!-- http://www.cognitiveatlas.org/ontology/cogat.owl#CAO_00468 -->

    <owl:Class rdf:about="&cogat;CAO_00468">
        <rdfs:label>Processing capacity</rdfs:label>
        <rdfs:subClassOf rdf:resource="&cogat;CAO_00001"/>
        <skos:hasTopConcept></skos:hasTopConcept>
        <skos:altLabel></skos:altLabel>
        <skos:definition>No definition submitted yet</skos:definition>
        <dc:Date>2009-07-10 14:06:32</dc:Date>
        <dc:Contributor>System Administrator</dc:Contributor>
        <dc:Title>Processing capacity</dc:Title>
        <skos:prefLabel>Processing capacity</skos:prefLabel>
        <dc:identifier>trm_4a3fd79d0adf4</dc:identifier>
    </owl:Class>
    


    <!-- http://www.cognitiveatlas.org/ontology/cogat.owl#CAO_00469 -->

    <owl:Class rdf:about="&cogat;CAO_00469">
        <rdfs:label>Processing stage</rdfs:label>
        <rdfs:subClassOf rdf:resource="&cogat;CAO_00001"/>
        <skos:definition>A subset of mental operations that are confined some feature space of information within a stream and-or hierarchy of mental operations.</skos:definition>
        <skos:hasTopConcept></skos:hasTopConcept>
        <dc:Contributor>Russ Poldrack</dc:Contributor>
        <skos:prefLabel>Processing stage</skos:prefLabel>
        <skos:altLabel></skos:altLabel>
        <dc:Date>2012-03-28 18:12:25</dc:Date>
        <dc:Title>Processing stage</dc:Title>
        <dc:identifier>trm_4a3fd79d0ae00</dc:identifier>
    </owl:Class>
    


    <!-- http://www.cognitiveatlas.org/ontology/cogat.owl#CAO_00470 -->

    <owl:Class rdf:about="&cogat;CAO_00470">
        <rdfs:label>Pronunciation</rdfs:label>
        <rdfs:subClassOf rdf:resource="&cogat;CAO_00001"/>
        <dc:Title>Pronunciation</dc:Title>
        <dc:identifier>trm_4a3fd79d0ae17</dc:identifier>
        <skos:altLabel></skos:altLabel>
        <skos:prefLabel>Pronunciation</skos:prefLabel>
        <dc:Contributor>Brenda Gregory</dc:Contributor>
        <skos:definition>the way a word or a language is spoken, or the manner in which someone utters a word.</skos:definition>
        <dc:Date>2011-05-04 11:00:18</dc:Date>
        <skos:hasTopConcept>Language</skos:hasTopConcept>
    </owl:Class>
    


    <!-- http://www.cognitiveatlas.org/ontology/cogat.owl#CAO_00471 -->

    <owl:Class rdf:about="&cogat;CAO_00471">
        <rdfs:label>Proper noun</rdfs:label>
        <rdfs:subClassOf rdf:resource="&cogat;CAO_00001"/>
        <skos:definition>A subject that usually indicates a particular person, place, or object.</skos:definition>
        <dc:Title>Proper noun</dc:Title>
        <dc:Date>2012-03-28 18:12:43</dc:Date>
        <skos:altLabel></skos:altLabel>
        <skos:prefLabel>Proper noun</skos:prefLabel>
        <skos:hasTopConcept>Language</skos:hasTopConcept>
        <dc:identifier>trm_4a3fd79d0ae2b</dc:identifier>
        <dc:Contributor>Russ Poldrack</dc:Contributor>
    </owl:Class>
    


    <!-- http://www.cognitiveatlas.org/ontology/cogat.owl#CAO_00472 -->

    <owl:Class rdf:about="&cogat;CAO_00472">
        <rdfs:label>Proprioception</rdfs:label>
        <rdfs:subClassOf rdf:resource="&cogat;CAO_00001"/>
        <skos:hasTopConcept>Perception</skos:hasTopConcept>
        <skos:definition>the sense of the relative position of neighboring parts of the body.</skos:definition>
        <dc:identifier>trm_4a3fd79d0ae3d</dc:identifier>
        <dc:Contributor>Brenda Gregory</dc:Contributor>
        <dc:Date>2011-05-17 10:02:47</dc:Date>
        <skos:prefLabel>Proprioception</skos:prefLabel>
        <dc:Title>Proprioception</dc:Title>
        <skos:altLabel></skos:altLabel>
    </owl:Class>
    


    <!-- http://www.cognitiveatlas.org/ontology/cogat.owl#CAO_00473 -->

    <owl:Class rdf:about="&cogat;CAO_00473">
        <rdfs:label>Prosodic stress</rdfs:label>
        <rdfs:subClassOf rdf:resource="&cogat;CAO_00001"/>
        <skos:prefLabel>Prosodic stress</skos:prefLabel>
        <dc:Date>2011-05-19 15:09:30</dc:Date>
        <skos:altLabel></skos:altLabel>
        <dc:identifier>trm_4a3fd79d0ae58</dc:identifier>
        <skos:hasTopConcept>Language</skos:hasTopConcept>
        <dc:Title>Prosodic stress</dc:Title>
        <dc:Contributor>Natalie Picchetti</dc:Contributor>
        <skos:definition>the stress and intonation patterns of an utterance. </skos:definition>
    </owl:Class>
    


    <!-- http://www.cognitiveatlas.org/ontology/cogat.owl#CAO_00474 -->

    <owl:Class rdf:about="&cogat;CAO_00474">
        <rdfs:label>Prosody</rdfs:label>
        <rdfs:subClassOf rdf:resource="&cogat;CAO_00001"/>
        <skos:altLabel></skos:altLabel>
        <skos:hasTopConcept>Language</skos:hasTopConcept>
        <dc:identifier>trm_4a3fd79d0ae64</dc:identifier>
        <skos:prefLabel>Prosody</skos:prefLabel>
        <dc:Date>2012-03-28 18:13:04</dc:Date>
        <dc:Contributor>Russ Poldrack</dc:Contributor>
        <skos:definition>the rhythm, stress, and intonation of speech.</skos:definition>
        <dc:Title>Prosody</dc:Title>
    </owl:Class>
    


    <!-- http://www.cognitiveatlas.org/ontology/cogat.owl#CAO_00475 -->

    <owl:Class rdf:about="&cogat;CAO_00475">
        <rdfs:label>Prospective memory</rdfs:label>
        <rdfs:subClassOf rdf:resource="&cogat;CAO_00394"/>
        <dc:Contributor>Brenda Gregory</dc:Contributor>
        <skos:altLabel></skos:altLabel>
        <dc:identifier>trm_4a3fd79d0ae70</dc:identifier>
        <skos:definition>remembering to perform an intended action...prospective memory is self-initiated and does not operate directly on external stimuli.</skos:definition>
        <dc:Date>2011-05-17 10:05:01</dc:Date>
        <skos:hasTopConcept>Learning and Memory</skos:hasTopConcept>
        <skos:prefLabel>Prospective memory</skos:prefLabel>
        <dc:Title>Prospective memory</dc:Title>
    </owl:Class>
    


    <!-- http://www.cognitiveatlas.org/ontology/cogat.owl#CAO_00476 -->

    <owl:Class rdf:about="&cogat;CAO_00476">
        <rdfs:label>Prospective planning</rdfs:label>
        <rdfs:subClassOf rdf:resource="&cogat;CAO_00452"/>
        <skos:prefLabel>Prospective planning</skos:prefLabel>
        <skos:hasTopConcept></skos:hasTopConcept>
        <dc:Title>Prospective planning</dc:Title>
        <dc:Date>2009-07-10 14:06:32</dc:Date>
        <skos:definition>No definition submitted yet</skos:definition>
        <dc:identifier>trm_4a3fd79d0ae7b</dc:identifier>
        <dc:Contributor>System Administrator</dc:Contributor>
        <skos:altLabel></skos:altLabel>
    </owl:Class>
    


    <!-- http://www.cognitiveatlas.org/ontology/cogat.owl#CAO_00477 -->

    <owl:Class rdf:about="&cogat;CAO_00477">
        <rdfs:label>Prototype</rdfs:label>
        <rdfs:subClassOf rdf:resource="&cogat;CAO_00397"/>
        <skos:definition>A most common, standard or basic mental representation of some category.</skos:definition>
        <dc:Date>2009-07-10 14:06:32</dc:Date>
        <skos:prefLabel>Prototype</skos:prefLabel>
        <skos:altLabel></skos:altLabel>
        <dc:identifier>trm_4a3fd79d0ae87</dc:identifier>
        <skos:hasTopConcept>Learning and Memory</skos:hasTopConcept>
        <dc:Contributor>Agatha Lenartowicz</dc:Contributor>
        <dc:Title>Prototype</dc:Title>
    </owl:Class>
    


    <!-- http://www.cognitiveatlas.org/ontology/cogat.owl#CAO_00478 -->

    <owl:Class rdf:about="&cogat;CAO_00478">
        <rdfs:label>Quantitative skill</rdfs:label>
        <rdfs:subClassOf rdf:resource="&cogat;CAO_00519"/>
        <dc:Date>2012-02-23 13:30:09</dc:Date>
        <skos:definition>the ability to to use mathematical concepts to solve problems. </skos:definition>
        <dc:Title>Quantitative skill</dc:Title>
        <skos:prefLabel>Quantitative skill</skos:prefLabel>
        <skos:hasTopConcept></skos:hasTopConcept>
        <dc:identifier>trm_4a3fd79d0aeaa</dc:identifier>
        <skos:altLabel></skos:altLabel>
        <dc:Contributor>Michael Sharman</dc:Contributor>
    </owl:Class>
    


    <!-- http://www.cognitiveatlas.org/ontology/cogat.owl#CAO_00479 -->

    <owl:Class rdf:about="&cogat;CAO_00479">
        <rdfs:label>Reading</rdfs:label>
        <rdfs:subClassOf rdf:resource="&cogat;CAO_00572"/>
        <rdfs:subClassOf>
            <owl:Restriction>
                <owl:onProperty rdf:resource="&ro;part_of"/>
                <owl:someValuesFrom rdf:resource="&cogat;CAO_00619"/>
            </owl:Restriction>
        </rdfs:subClassOf>
        <skos:prefLabel>Reading</skos:prefLabel>
        <skos:definition>Decoding symbols to derive their meaning.</skos:definition>
        <skos:altLabel></skos:altLabel>
        <dc:Title>Reading</dc:Title>
        <dc:Date>2012-03-28 18:15:04</dc:Date>
        <dc:identifier>trm_4a3fd79d0aeb6</dc:identifier>
        <skos:hasTopConcept>Language</skos:hasTopConcept>
        <dc:Contributor>Russ Poldrack</dc:Contributor>
    </owl:Class>
    


    <!-- http://www.cognitiveatlas.org/ontology/cogat.owl#CAO_00480 -->

    <owl:Class rdf:about="&cogat;CAO_00480">
        <rdfs:label>Reasoning</rdfs:label>
        <rdfs:subClassOf rdf:resource="&cogat;CAO_00001"/>
        <dc:Date>2011-05-16 10:57:30</dc:Date>
        <skos:definition>drawing of inferences or conclusions through the use of reason.</skos:definition>
        <skos:altLabel></skos:altLabel>
        <skos:prefLabel>Reasoning</skos:prefLabel>
        <dc:Title>Reasoning</dc:Title>
        <dc:Contributor>Brenda Gregory</dc:Contributor>
        <dc:identifier>trm_4a3fd79d0aec1</dc:identifier>
        <skos:hasTopConcept>Reasoning and Decision Making</skos:hasTopConcept>
    </owl:Class>
    


    <!-- http://www.cognitiveatlas.org/ontology/cogat.owl#CAO_00481 -->

    <owl:Class rdf:about="&cogat;CAO_00481">
        <rdfs:label>Regret</rdfs:label>
        <rdfs:subClassOf rdf:resource="&cogat;CAO_00001"/>
        <skos:hasTopConcept>Emotion</skos:hasTopConcept>
        <skos:definition>an emotional response to remembrance of a past state, condition, or experience that one wishes had been different</skos:definition>
        <dc:Contributor>Akram Bakkour</dc:Contributor>
        <skos:altLabel></skos:altLabel>
        <dc:Title>Regret</dc:Title>
        <dc:Date>2011-08-12 08:24:49</dc:Date>
        <skos:prefLabel>Regret</skos:prefLabel>
        <dc:identifier>trm_4a3fd79d0aecd</dc:identifier>
    </owl:Class>
    


    <!-- http://www.cognitiveatlas.org/ontology/cogat.owl#CAO_00482 -->

    <owl:Class rdf:about="&cogat;CAO_00482">
        <rdfs:label>Relational learning</rdfs:label>
        <rdfs:subClassOf rdf:resource="&cogat;CAO_00377"/>
        <skos:definition>learning to differentiate among stimuli on the basis of relational properties (e.g., the larger of two stimuli) rather than absolute properties (e.g., the stimulus that has a given size).</skos:definition>
        <dc:Date>2011-08-12 09:11:12</dc:Date>
        <skos:prefLabel>Relational learning</skos:prefLabel>
        <dc:Contributor>Akram Bakkour</dc:Contributor>
        <dc:Title>Relational learning</dc:Title>
        <skos:altLabel></skos:altLabel>
        <dc:identifier>trm_4a3fd79d0aed8</dc:identifier>
        <skos:hasTopConcept>Learning and Memory</skos:hasTopConcept>
    </owl:Class>
    


    <!-- http://www.cognitiveatlas.org/ontology/cogat.owl#CAO_00483 -->

    <owl:Class rdf:about="&cogat;CAO_00483">
        <rdfs:label>Remote memory</rdfs:label>
        <rdfs:subClassOf rdf:resource="&cogat;CAO_00394"/>
        <rdfs:subClassOf>
            <owl:Restriction>
                <owl:onProperty rdf:resource="&ro;part_of"/>
                <owl:someValuesFrom rdf:resource="&cogat;CAO_00387"/>
            </owl:Restriction>
        </rdfs:subClassOf>
        <dc:Contributor>Brenda Gregory</dc:Contributor>
        <dc:identifier>trm_4a3fd79d0aee4</dc:identifier>
        <skos:altLabel></skos:altLabel>
        <skos:definition>memory for events of long ago as opposed to recent events.</skos:definition>
        <skos:hasTopConcept>Learning and Memory</skos:hasTopConcept>
        <dc:Title>Remote memory</dc:Title>
        <skos:prefLabel>Remote memory</skos:prefLabel>
        <dc:Date>2011-05-16 15:48:23</dc:Date>
    </owl:Class>
    


    <!-- http://www.cognitiveatlas.org/ontology/cogat.owl#CAO_00484 -->

    <owl:Class rdf:about="&cogat;CAO_00484">
        <rdfs:label>Repressed memory</rdfs:label>
        <rdfs:subClassOf rdf:resource="&cogat;CAO_00394"/>
        <skos:hasTopConcept>Learning and Memory</skos:hasTopConcept>
        <skos:altLabel></skos:altLabel>
        <dc:identifier>trm_4a3fd79d0aeef</dc:identifier>
        <skos:prefLabel>Repressed memory</skos:prefLabel>
        <dc:Contributor>Agatha Lenartowicz</dc:Contributor>
        <dc:Date>2009-12-21 14:42:08</dc:Date>
        <dc:Title>Repressed memory</dc:Title>
        <skos:definition>A memory (often traumatic) that is unavailable for recall.</skos:definition>
    </owl:Class>
    


    <!-- http://www.cognitiveatlas.org/ontology/cogat.owl#CAO_00485 -->

    <owl:Class rdf:about="&cogat;CAO_00485">
        <rdfs:label>Resource limit</rdfs:label>
        <rdfs:subClassOf rdf:resource="&cogat;CAO_00001"/>
        <dc:Contributor>Michael Sharman</dc:Contributor>
        <skos:altLabel></skos:altLabel>
        <skos:prefLabel>Resource limit</skos:prefLabel>
        <dc:Title>Resource limit</dc:Title>
        <skos:hasTopConcept>Executive-Cognitive Control</skos:hasTopConcept>
        <dc:Date>2012-02-23 08:07:25</dc:Date>
        <dc:identifier>trm_4a3fd79d0af4c</dc:identifier>
        <skos:definition>the maximum amount of cognitive resources that can be allocated to various, often competing tasks</skos:definition>
    </owl:Class>
    


    <!-- http://www.cognitiveatlas.org/ontology/cogat.owl#CAO_00486 -->

    <owl:Class rdf:about="&cogat;CAO_00486">
        <rdfs:label>Resource sharing</rdfs:label>
        <rdfs:subClassOf rdf:resource="&cogat;CAO_00001"/>
        <skos:definition>is a unique characteristic of humans and several primates that involve sharing resources such as food, shelter, etc., as a collective risk-reduction against variability in resource supply. </skos:definition>
        <skos:altLabel></skos:altLabel>
        <skos:hasTopConcept>Social Function</skos:hasTopConcept>
        <dc:identifier>trm_4a3fd79d0af5a</dc:identifier>
        <dc:Date>2012-03-28 18:19:07</dc:Date>
        <skos:prefLabel>Resource sharing</skos:prefLabel>
        <dc:Title>Resource sharing</dc:Title>
        <dc:Contributor>Russ Poldrack</dc:Contributor>
    </owl:Class>
    


    <!-- http://www.cognitiveatlas.org/ontology/cogat.owl#CAO_00488 -->

    <owl:Class rdf:about="&cogat;CAO_00488">
        <rdfs:label>Response selection</rdfs:label>
        <rdfs:subClassOf rdf:resource="&cogat;CAO_00001"/>
        <skos:definition>The selection of one action from a set of possible actions.</skos:definition>
        <dc:Contributor>Russ Poldrack</dc:Contributor>
        <skos:altLabel></skos:altLabel>
        <dc:Date>2012-03-28 18:20:12</dc:Date>
        <dc:identifier>trm_4a3fd79d0af71</dc:identifier>
        <skos:prefLabel>Response selection</skos:prefLabel>
        <skos:hasTopConcept>Action</skos:hasTopConcept>
        <dc:Title>Response selection</dc:Title>
    </owl:Class>
    


    <!-- http://www.cognitiveatlas.org/ontology/cogat.owl#CAO_00489 -->

    <owl:Class rdf:about="&cogat;CAO_00489">
        <rdfs:label>Retention</rdfs:label>
        <rdfs:subClassOf rdf:resource="&cogat;CAO_00001"/>
        <rdfs:subClassOf>
            <owl:Restriction>
                <owl:onProperty rdf:resource="&ro;part_of"/>
                <owl:someValuesFrom rdf:resource="&cogat;CAO_00394"/>
            </owl:Restriction>
        </rdfs:subClassOf>
        <dc:Title>Retention</dc:Title>
        <skos:altLabel></skos:altLabel>
        <skos:prefLabel>Retention</skos:prefLabel>
        <dc:Date>2011-08-12 10:08:31</dc:Date>
        <dc:Contributor>Akram Bakkour</dc:Contributor>
        <skos:definition>a preservation of the aftereffects of experience and learning that makes recall or recognition possible. Persistence of learned behavior or experience during a period when it is not being performed o r practiced. Retention is the second stage of memory after encoding and before retrival</skos:definition>
        <skos:hasTopConcept>Learning and Memory</skos:hasTopConcept>
        <dc:identifier>trm_4a3fd79d0af7d</dc:identifier>
    </owl:Class>
    


    <!-- http://www.cognitiveatlas.org/ontology/cogat.owl#CAO_00490 -->

    <owl:Class rdf:about="&cogat;CAO_00490">
        <rdfs:label>Retrieval</rdfs:label>
        <rdfs:subClassOf rdf:resource="&cogat;CAO_00001"/>
        <rdfs:subClassOf>
            <owl:Restriction>
                <owl:onProperty rdf:resource="&ro;part_of"/>
                <owl:someValuesFrom rdf:resource="&cogat;CAO_00394"/>
            </owl:Restriction>
        </rdfs:subClassOf>
        <skos:definition>The process of accessing information from memory or other storage devices; the possibility of recovery, restoration, or rectification. Retrieval is the third stage of memory after encoding and retention.</skos:definition>
        <dc:Title>Retrieval</dc:Title>
        <dc:Contributor>Akram Bakkour</dc:Contributor>
        <skos:prefLabel>Retrieval</skos:prefLabel>
        <skos:hasTopConcept>Learning and Memory</skos:hasTopConcept>
        <dc:Date>2011-08-12 10:12:09</dc:Date>
        <dc:identifier>trm_4a3fd79d0af94</dc:identifier>
        <skos:altLabel></skos:altLabel>
    </owl:Class>
    


    <!-- http://www.cognitiveatlas.org/ontology/cogat.owl#CAO_00491 -->

    <owl:Class rdf:about="&cogat;CAO_00491">
        <rdfs:label>Retrieval cue</rdfs:label>
        <rdfs:subClassOf rdf:resource="&cogat;CAO_00001"/>
        <skos:definition>An event or experience that facilitates retrieval of information from long-term memory because of its association to that information.</skos:definition>
        <dc:identifier>trm_4a3fd79d0afa0</dc:identifier>
        <skos:altLabel></skos:altLabel>
        <skos:hasTopConcept>Learning and Memory</skos:hasTopConcept>
        <dc:Title>Retrieval cue</dc:Title>
        <skos:prefLabel>Retrieval cue</skos:prefLabel>
        <dc:Contributor>Agatha Lenartowicz</dc:Contributor>
        <dc:Date>2009-07-10 14:06:32</dc:Date>
    </owl:Class>
    


    <!-- http://www.cognitiveatlas.org/ontology/cogat.owl#CAO_00492 -->

    <owl:Class rdf:about="&cogat;CAO_00492">
        <rdfs:label>Retroactive interference</rdfs:label>
        <rdfs:subClassOf rdf:resource="&cogat;CAO_00359"/>
        <dc:Contributor>Akram Bakkour</dc:Contributor>
        <skos:prefLabel>Retroactive interference</skos:prefLabel>
        <dc:identifier>trm_4a3fd79d0afab</dc:identifier>
        <dc:Title>Retroactive interference</dc:Title>
        <skos:altLabel>retroactive inhibition</skos:altLabel>
        <skos:hasTopConcept>Learning and Memory</skos:hasTopConcept>
        <skos:definition>impeded retrieval and performance of previously learnt information due to newly acquired and practiced information.</skos:definition>
        <dc:Date>2011-08-12 11:56:47</dc:Date>
    </owl:Class>
    


    <!-- http://www.cognitiveatlas.org/ontology/cogat.owl#CAO_00493 -->

    <owl:Class rdf:about="&cogat;CAO_00493">
        <rdfs:label>Rhythm</rdfs:label>
        <rdfs:subClassOf rdf:resource="&cogat;CAO_00001"/>
        <dc:Contributor>Russ Poldrack</dc:Contributor>
        <dc:identifier>trm_4a3fd79d0afc3</dc:identifier>
        <skos:definition>Movement marked by the regulated succession of strong and weak elements, or of opposite or different conditions.  While rhythm most commonly applies to sound, such as music and spoken language, it may also refer to visual presentation, as timed movement through space.</skos:definition>
        <dc:Title>Rhythm</dc:Title>
        <dc:Date>2012-03-28 18:27:15</dc:Date>
        <skos:prefLabel>Rhythm</skos:prefLabel>
        <skos:hasTopConcept>Perception</skos:hasTopConcept>
        <skos:altLabel></skos:altLabel>
    </owl:Class>
    


    <!-- http://www.cognitiveatlas.org/ontology/cogat.owl#CAO_00494 -->

    <owl:Class rdf:about="&cogat;CAO_00494">
        <rdfs:label>Risk</rdfs:label>
        <rdfs:subClassOf rdf:resource="&cogat;CAO_00001"/>
        <skos:prefLabel>Risk</skos:prefLabel>
        <skos:hasTopConcept>Reasoning and Decision Making</skos:hasTopConcept>
        <skos:altLabel></skos:altLabel>
        <dc:Date>2012-03-28 18:27:26</dc:Date>
        <skos:definition>the probability or likelihood that an event will occur; possibility of loss or injury; someone or something that creates or suggests a hazard; the chance that an investment will lose value.</skos:definition>
        <dc:Title>Risk</dc:Title>
        <dc:Contributor>Russ Poldrack</dc:Contributor>
        <dc:identifier>trm_4a3fd79d0afcf</dc:identifier>
    </owl:Class>
    


    <!-- http://www.cognitiveatlas.org/ontology/cogat.owl#CAO_00495 -->

    <owl:Class rdf:about="&cogat;CAO_00495">
        <rdfs:label>Route knowledge</rdfs:label>
        <rdfs:subClassOf rdf:resource="&cogat;CAO_00371"/>
        <skos:prefLabel>Route knowledge</skos:prefLabel>
        <dc:Contributor>Akram Bakkour</dc:Contributor>
        <dc:Title>Route knowledge</dc:Title>
        <dc:Date>2011-08-12 12:17:07</dc:Date>
        <skos:hasTopConcept></skos:hasTopConcept>
        <dc:identifier>trm_4a3fd79d0afda</dc:identifier>
        <skos:altLabel></skos:altLabel>
        <skos:definition>is represented as a series of directions to follow to get from one place to another.</skos:definition>
    </owl:Class>
    


    <!-- http://www.cognitiveatlas.org/ontology/cogat.owl#CAO_00496 -->

    <owl:Class rdf:about="&cogat;CAO_00496">
        <rdfs:label>Routine</rdfs:label>
        <rdfs:subClassOf rdf:resource="&cogat;CAO_00001"/>
        <skos:altLabel></skos:altLabel>
        <dc:Date>2011-05-10 14:42:43</dc:Date>
        <skos:prefLabel>Routine</skos:prefLabel>
        <skos:definition>a regular course of procedure; habitual or mechanical performance of an established procedure; a reiterated speech or formula; a sequence of computer instructions for performing a particular task.</skos:definition>
        <skos:hasTopConcept></skos:hasTopConcept>
        <dc:Title>Routine</dc:Title>
        <dc:Contributor>Brenda Gregory</dc:Contributor>
        <dc:identifier>trm_4a3fd79d0afe6</dc:identifier>
    </owl:Class>
    


    <!-- http://www.cognitiveatlas.org/ontology/cogat.owl#CAO_00497 -->

    <owl:Class rdf:about="&cogat;CAO_00497">
        <rdfs:label>Rule</rdfs:label>
        <rdfs:subClassOf rdf:resource="&cogat;CAO_00001"/>
        <dc:Title>Rule</dc:Title>
        <dc:Date>2012-03-28 18:28:27</dc:Date>
        <dc:identifier>trm_4a3fd79d0aff2</dc:identifier>
        <skos:altLabel></skos:altLabel>
        <skos:definition>a method for performing a psychological operation</skos:definition>
        <skos:hasTopConcept></skos:hasTopConcept>
        <dc:Contributor>Russ Poldrack</dc:Contributor>
        <skos:prefLabel>Rule</skos:prefLabel>
    </owl:Class>
    


    <!-- http://www.cognitiveatlas.org/ontology/cogat.owl#CAO_00498 -->

    <owl:Class rdf:about="&cogat;CAO_00498">
        <rdfs:label>Rule learning</rdfs:label>
        <rdfs:subClassOf rdf:resource="&cogat;CAO_00377"/>
        <rdfs:subClassOf>
            <owl:Restriction>
                <owl:onProperty rdf:resource="&ro;part_of"/>
                <owl:someValuesFrom rdf:resource="&cogat;CAO_00191"/>
            </owl:Restriction>
        </rdfs:subClassOf>
        <dc:Contributor>Akram Bakkour</dc:Contributor>
        <dc:Title>Rule learning</dc:Title>
        <dc:identifier>trm_4a3fd79d0affd</dc:identifier>
        <dc:Date>2011-08-12 12:35:05</dc:Date>
        <skos:definition>process in which a participant gradually acquires knowledge about a fixed but unstated standard that defines, for example, the acceptability of a response or membership of category</skos:definition>
        <skos:altLabel></skos:altLabel>
        <skos:hasTopConcept>Learning and Memory</skos:hasTopConcept>
        <skos:prefLabel>Rule learning</skos:prefLabel>
    </owl:Class>
    


    <!-- http://www.cognitiveatlas.org/ontology/cogat.owl#CAO_00499 -->

    <owl:Class rdf:about="&cogat;CAO_00499">
        <rdfs:label>Sadness</rdfs:label>
        <rdfs:subClassOf rdf:resource="&cogat;CAO_00276"/>
        <skos:altLabel></skos:altLabel>
        <dc:Date>2011-08-12 12:59:49</dc:Date>
        <skos:definition>an emotion  characterized by feelings of unhappiness, disadvantage, loss, and helplessness.</skos:definition>
        <skos:hasTopConcept>Emotion</skos:hasTopConcept>
        <skos:prefLabel>Sadness</skos:prefLabel>
        <dc:Title>Sadness</dc:Title>
        <dc:identifier>trm_4a3fd79d0b014</dc:identifier>
        <dc:Contributor>Akram Bakkour</dc:Contributor>
    </owl:Class>
    


    <!-- http://www.cognitiveatlas.org/ontology/cogat.owl#CAO_00500 -->

    <owl:Class rdf:about="&cogat;CAO_00500">
        <rdfs:label>Salience</rdfs:label>
        <rdfs:subClassOf rdf:resource="&cogat;CAO_00001"/>
        <dc:Date>2011-08-12 13:06:31</dc:Date>
        <dc:Contributor>Akram Bakkour</dc:Contributor>
        <skos:altLabel></skos:altLabel>
        <dc:Title>Salience</dc:Title>
        <skos:prefLabel>Salience</skos:prefLabel>
        <skos:hasTopConcept></skos:hasTopConcept>
        <skos:definition>a parameter of a stimulus that indexes its effectiveness.</skos:definition>
        <dc:identifier>trm_4a3fd79d0b020</dc:identifier>
    </owl:Class>
    


    <!-- http://www.cognitiveatlas.org/ontology/cogat.owl#CAO_00501 -->

    <owl:Class rdf:about="&cogat;CAO_00501">
        <rdfs:label>Schema</rdfs:label>
        <rdfs:subClassOf rdf:resource="&cogat;CAO_00001"/>
        <rdfs:subClassOf>
            <owl:Restriction>
                <owl:onProperty rdf:resource="&ro;part_of"/>
                <owl:someValuesFrom rdf:resource="&cogat;CAO_00463"/>
            </owl:Restriction>
        </rdfs:subClassOf>
        <rdfs:subClassOf>
            <owl:Restriction>
                <owl:onProperty rdf:resource="&ro;part_of"/>
                <owl:someValuesFrom rdf:resource="&cogat;CAO_00437"/>
            </owl:Restriction>
        </rdfs:subClassOf>
        <dc:Contributor>Russ Poldrack</dc:Contributor>
        <skos:definition>a structured representation that includes a particular organized way of perceiving and responding to a complex situation or set of stimuli.</skos:definition>
        <skos:altLabel></skos:altLabel>
        <skos:hasTopConcept>Reasoning and Decision Making</skos:hasTopConcept>
        <dc:Title>Schema</dc:Title>
        <dc:Date>2012-03-28 18:29:43</dc:Date>
        <skos:prefLabel>Schema</skos:prefLabel>
        <dc:identifier>trm_4a3fd79d0b02c</dc:identifier>
    </owl:Class>
    


    <!-- http://www.cognitiveatlas.org/ontology/cogat.owl#CAO_00502 -->

    <owl:Class rdf:about="&cogat;CAO_00502">
        <rdfs:label>Search</rdfs:label>
        <rdfs:subClassOf rdf:resource="&cogat;CAO_00001"/>
        <dc:identifier>trm_4a3fd79d0b037</dc:identifier>
        <dc:Date>2011-05-04 10:55:36</dc:Date>
        <dc:Title>Search</dc:Title>
        <dc:Contributor>Brenda Gregory</dc:Contributor>
        <skos:hasTopConcept></skos:hasTopConcept>
        <skos:prefLabel>Search</skos:prefLabel>
        <skos:definition>to look into or over carefully or thoroughly in an effort to find or discover something; to look through or explore by inspecting possible places of concealment or investigating suspicious circumstances; to look at as if to discover or penetrate intention or nature; to uncover, find, or come to know by inquiry or scrutiny.</skos:definition>
        <skos:altLabel></skos:altLabel>
    </owl:Class>
    


    <!-- http://www.cognitiveatlas.org/ontology/cogat.owl#CAO_00503 -->

    <owl:Class rdf:about="&cogat;CAO_00503">
        <rdfs:label>Selective attention</rdfs:label>
        <rdfs:subClassOf rdf:resource="&cogat;CAO_00001"/>
        <skos:definition>When multiple external sensory inputs are present, the process of dedicating cognitive and perceptual resources to one type-set of input and attenuating receptiveness to other inputs.</skos:definition>
        <skos:prefLabel>Selective attention</skos:prefLabel>
        <dc:identifier>trm_4a3fd79d0b043</dc:identifier>
        <dc:Title>Selective attention</dc:Title>
        <dc:Date>2011-08-17 09:56:16</dc:Date>
        <skos:altLabel>controlled attention, directed attention</skos:altLabel>
        <skos:hasTopConcept>Attention</skos:hasTopConcept>
        <dc:Contributor>Akram Bakkour</dc:Contributor>
    </owl:Class>
    


    <!-- http://www.cognitiveatlas.org/ontology/cogat.owl#CAO_00504 -->

    <owl:Class rdf:about="&cogat;CAO_00504">
        <rdfs:label>Self monitoring</rdfs:label>
        <rdfs:subClassOf rdf:resource="&cogat;CAO_00001"/>
        <skos:hasTopConcept>Executive-Cognitive Control</skos:hasTopConcept>
        <dc:Contributor>Russ Poldrack</dc:Contributor>
        <dc:Date>2012-03-28 18:30:15</dc:Date>
        <skos:definition>monitoring of oneand#39;s own behavior.</skos:definition>
        <dc:identifier>trm_4a3fd79d0b05e</dc:identifier>
        <dc:Title>Self monitoring</dc:Title>
        <skos:altLabel></skos:altLabel>
        <skos:prefLabel>Self monitoring</skos:prefLabel>
    </owl:Class>
    


    <!-- http://www.cognitiveatlas.org/ontology/cogat.owl#CAO_00505 -->

    <owl:Class rdf:about="&cogat;CAO_00505">
        <rdfs:label>Semantic category</rdfs:label>
        <rdfs:subClassOf rdf:resource="&cogat;CAO_00001"/>
        <dc:identifier>trm_4a3fd79d0b06b</dc:identifier>
        <skos:hasTopConcept>Language</skos:hasTopConcept>
        <skos:altLabel></skos:altLabel>
        <skos:prefLabel>Semantic category</skos:prefLabel>
        <dc:Title>Semantic category</dc:Title>
        <dc:Contributor>Natalie Picchetti</dc:Contributor>
        <skos:definition>is a grouping of vocabulary within a language, organizing words which are interrelated and define each other in various ways. Also referred to as a semantic field.  </skos:definition>
        <dc:Date>2011-04-01 12:50:06</dc:Date>
    </owl:Class>
    


    <!-- http://www.cognitiveatlas.org/ontology/cogat.owl#CAO_00506 -->

    <owl:Class rdf:about="&cogat;CAO_00506">
        <rdfs:label>Semantic knowledge</rdfs:label>
        <rdfs:subClassOf rdf:resource="&cogat;CAO_00387"/>
        <rdfs:subClassOf>
            <owl:Restriction>
                <owl:onProperty rdf:resource="&ro;part_of"/>
                <owl:someValuesFrom rdf:resource="&cogat;CAO_00372"/>
            </owl:Restriction>
        </rdfs:subClassOf>
        <skos:definition>long-established knowledge about objects, facts, and word meanings.</skos:definition>
        <dc:Contributor>Russ Poldrack</dc:Contributor>
        <dc:identifier>trm_4a3fd79d0b077</dc:identifier>
        <skos:prefLabel>Semantic knowledge</skos:prefLabel>
        <skos:hasTopConcept>Language</skos:hasTopConcept>
        <dc:Title>Semantic knowledge</dc:Title>
        <skos:altLabel></skos:altLabel>
        <dc:Date>2012-03-28 18:31:37</dc:Date>
    </owl:Class>
    


    <!-- http://www.cognitiveatlas.org/ontology/cogat.owl#CAO_00507 -->

    <owl:Class rdf:about="&cogat;CAO_00507">
        <rdfs:label>Semantic memory</rdfs:label>
        <rdfs:subClassOf rdf:resource="&cogat;CAO_00255"/>
        <rdfs:subClassOf>
            <owl:Restriction>
                <owl:onProperty rdf:resource="&ro;part_of"/>
                <owl:someValuesFrom rdf:resource="&cogat;CAO_00372"/>
            </owl:Restriction>
        </rdfs:subClassOf>
        <skos:definition>refers to oneand#39;s conceptual knowledge and includes the meanings of words, factual information about the world, and other information not related to specific events or episodes</skos:definition>
        <skos:hasTopConcept>Language</skos:hasTopConcept>
        <skos:prefLabel>Semantic memory</skos:prefLabel>
        <dc:Title>Semantic memory</dc:Title>
        <dc:Contributor>Joseph Devlin</dc:Contributor>
        <dc:Date>2010-05-09 00:46:27</dc:Date>
        <skos:altLabel></skos:altLabel>
        <dc:identifier>trm_4a3fd79d0b083</dc:identifier>
    </owl:Class>
    


    <!-- http://www.cognitiveatlas.org/ontology/cogat.owl#CAO_00508 -->

    <owl:Class rdf:about="&cogat;CAO_00508">
        <rdfs:label>Semantic working memory</rdfs:label>
        <rdfs:subClassOf rdf:resource="&cogat;CAO_00587"/>
        <skos:definition>Working memory for meaning</skos:definition>
        <dc:Contributor>Russ Poldrack</dc:Contributor>
        <dc:identifier>trm_4a3fd79d0b08f</dc:identifier>
        <skos:hasTopConcept>Executive-Cognitive Control</skos:hasTopConcept>
        <skos:altLabel></skos:altLabel>
        <dc:Date>2010-01-10 15:04:12</dc:Date>
        <skos:prefLabel>Semantic working memory</skos:prefLabel>
        <dc:Title>Semantic working memory</dc:Title>
    </owl:Class>
    


    <!-- http://www.cognitiveatlas.org/ontology/cogat.owl#CAO_00509 -->

    <owl:Class rdf:about="&cogat;CAO_00509">
        <rdfs:label>Sensory memory</rdfs:label>
        <rdfs:subClassOf rdf:resource="&cogat;CAO_00394"/>
        <dc:Date>2011-08-12 14:35:38</dc:Date>
        <skos:hasTopConcept>Learning and Memory</skos:hasTopConcept>
        <skos:prefLabel>Sensory memory</skos:prefLabel>
        <skos:altLabel>sensory-information store; sensory register</skos:altLabel>
        <dc:Title>Sensory memory</dc:Title>
        <dc:identifier>trm_4a3fd79d0b09a</dc:identifier>
        <dc:Contributor>Akram Bakkour</dc:Contributor>
        <skos:definition>brief storage of sensory information in each of the senses, which temporarily holds material (e.g., a perceptual experience) for recoding into another memory (such as short-term memory) or for comprehension.</skos:definition>
    </owl:Class>
    


    <!-- http://www.cognitiveatlas.org/ontology/cogat.owl#CAO_00510 -->

    <owl:Class rdf:about="&cogat;CAO_00510">
        <rdfs:label>Sequence learning</rdfs:label>
        <rdfs:subClassOf rdf:resource="&cogat;CAO_00377"/>
        <skos:prefLabel>Sequence learning</skos:prefLabel>
        <dc:Contributor>Akram Bakkour</dc:Contributor>
        <dc:identifier>trm_4a3fd79d0b0a6</dc:identifier>
        <skos:altLabel></skos:altLabel>
        <dc:Date>2011-08-17 10:06:58</dc:Date>
        <dc:Title>Sequence learning</dc:Title>
        <skos:hasTopConcept>Learning and Memory</skos:hasTopConcept>
        <skos:definition>learning of a sequence of items or responses in the precise order of their presentation.</skos:definition>
    </owl:Class>
    


    <!-- http://www.cognitiveatlas.org/ontology/cogat.owl#CAO_00511 -->

    <owl:Class rdf:about="&cogat;CAO_00511">
        <rdfs:label>Serial learning</rdfs:label>
        <rdfs:subClassOf rdf:resource="&cogat;CAO_00377"/>
        <skos:definition>The process of acquiring information in sequence and following an order that must be preserved at recall.</skos:definition>
        <dc:Contributor>Agatha Lenartowicz</dc:Contributor>
        <dc:Title>Serial learning</dc:Title>
        <skos:hasTopConcept>Learning and Memory</skos:hasTopConcept>
        <dc:identifier>trm_4a3fd79d0b0b1</dc:identifier>
        <skos:prefLabel>Serial learning</skos:prefLabel>
        <skos:altLabel></skos:altLabel>
        <dc:Date>2009-11-25 08:36:00</dc:Date>
    </owl:Class>
    


    <!-- http://www.cognitiveatlas.org/ontology/cogat.owl#CAO_00512 -->

    <owl:Class rdf:about="&cogat;CAO_00512">
        <rdfs:label>Serial processing</rdfs:label>
        <rdfs:subClassOf rdf:resource="&cogat;CAO_00001"/>
        <skos:definition>information processing in which only one sequence of processing operations is carried on at a time.</skos:definition>
        <dc:Title>Serial processing</dc:Title>
        <dc:Contributor>Akram Bakkour</dc:Contributor>
        <skos:prefLabel>Serial processing</skos:prefLabel>
        <skos:hasTopConcept></skos:hasTopConcept>
        <dc:identifier>trm_4a3fd79d0b0bd</dc:identifier>
        <skos:altLabel>intermittent processing, sequential processing</skos:altLabel>
        <dc:Date>2011-08-19 09:32:01</dc:Date>
    </owl:Class>
    


    <!-- http://www.cognitiveatlas.org/ontology/cogat.owl#CAO_00513 -->

    <owl:Class rdf:about="&cogat;CAO_00513">
        <rdfs:label>Serial search</rdfs:label>
        <rdfs:subClassOf rdf:resource="&cogat;CAO_00502"/>
        <dc:identifier>trm_4a3fd79d0b0c8</dc:identifier>
        <skos:altLabel></skos:altLabel>
        <dc:Title>Serial search</dc:Title>
        <dc:Date>2009-07-10 14:06:32</dc:Date>
        <skos:definition>The process of identifying a target within a set of candidate elements by testing the identity of each element against the identity of the sought after target one at a time.</skos:definition>
        <skos:prefLabel>Serial search</skos:prefLabel>
        <dc:Contributor>Agatha Lenartowicz</dc:Contributor>
        <skos:hasTopConcept>Attention</skos:hasTopConcept>
    </owl:Class>
    


    <!-- http://www.cognitiveatlas.org/ontology/cogat.owl#CAO_00515 -->

    <owl:Class rdf:about="&cogat;CAO_00515">
        <rdfs:label>Shallow processing</rdfs:label>
        <rdfs:subClassOf rdf:resource="&cogat;CAO_00001"/>
        <skos:hasTopConcept></skos:hasTopConcept>
        <dc:Title>Shallow processing</dc:Title>
        <skos:prefLabel>Shallow processing</skos:prefLabel>
        <skos:definition>a mode of thinking in which one pays attention only to appearances and other superficial aspects of the material, typically leading to poor memory retention.</skos:definition>
        <dc:identifier>trm_4a3fd79d0b0df</dc:identifier>
        <dc:Contributor>Brenda Gregory</dc:Contributor>
        <skos:altLabel></skos:altLabel>
        <dc:Date>2011-05-11 16:15:06</dc:Date>
    </owl:Class>
    


    <!-- http://www.cognitiveatlas.org/ontology/cogat.owl#CAO_00516 -->

    <owl:Class rdf:about="&cogat;CAO_00516">
        <rdfs:label>Shame</rdfs:label>
        <rdfs:subClassOf rdf:resource="&cogat;CAO_00276"/>
        <skos:prefLabel>Shame</skos:prefLabel>
        <dc:Contributor>Brenda Gregory</dc:Contributor>
        <skos:definition>a painful emotion caused by consciousness of guilt, shortcoming, or impropriety; a condition of humiliating disgrace or disrepute; something that brings censure or reproach.</skos:definition>
        <dc:identifier>trm_4a3fd79d0b0eb</dc:identifier>
        <dc:Date>2011-05-12 15:24:59</dc:Date>
        <skos:altLabel></skos:altLabel>
        <skos:hasTopConcept>Emotion</skos:hasTopConcept>
        <dc:Title>Shame</dc:Title>
    </owl:Class>
    


    <!-- http://www.cognitiveatlas.org/ontology/cogat.owl#CAO_00517 -->

    <owl:Class rdf:about="&cogat;CAO_00517">
        <rdfs:label>Short term memory</rdfs:label>
        <rdfs:subClassOf rdf:resource="&cogat;CAO_00394"/>
        <dc:Title>Short term memory</dc:Title>
        <skos:prefLabel>Short term memory</skos:prefLabel>
        <dc:Date>2011-08-19 09:46:00</dc:Date>
        <dc:Contributor>Akram Bakkour</dc:Contributor>
        <skos:definition>A limited-capacity and short-lasting representation of information in the mind. The duration of short-term memory is on the order of seconds, while its capacity is on the order of 4 to 9 independent items.</skos:definition>
        <dc:identifier>trm_4a3fd79d0b0f7</dc:identifier>
        <skos:altLabel></skos:altLabel>
        <skos:hasTopConcept>Learning and Memory</skos:hasTopConcept>
    </owl:Class>
    


    <!-- http://www.cognitiveatlas.org/ontology/cogat.owl#CAO_00518 -->

    <owl:Class rdf:about="&cogat;CAO_00518">
        <rdfs:label>Skepticism</rdfs:label>
        <rdfs:subClassOf rdf:resource="&cogat;CAO_00001"/>
        <dc:identifier>trm_4a3fd79d0b10e</dc:identifier>
        <skos:hasTopConcept></skos:hasTopConcept>
        <dc:Contributor>Brenda Gregory</dc:Contributor>
        <dc:Title>Skepticism</dc:Title>
        <dc:Date>2011-04-28 12:20:42</dc:Date>
        <skos:prefLabel>Skepticism</skos:prefLabel>
        <skos:altLabel></skos:altLabel>
        <skos:definition>an attitude of doubt or a disposition to incredulity either in general or toward a particular object.</skos:definition>
    </owl:Class>
    


    <!-- http://www.cognitiveatlas.org/ontology/cogat.owl#CAO_00519 -->

    <owl:Class rdf:about="&cogat;CAO_00519">
        <rdfs:label>Skill</rdfs:label>
        <rdfs:subClassOf rdf:resource="&cogat;CAO_00001"/>
        <dc:Date>2011-05-17 09:58:34</dc:Date>
        <dc:Title>Skill</dc:Title>
        <skos:definition> Proficiency, facility, or dexterity that is acquired or developed through training or experience.</skos:definition>
        <skos:altLabel></skos:altLabel>
        <skos:prefLabel>Skill</skos:prefLabel>
        <skos:hasTopConcept></skos:hasTopConcept>
        <dc:identifier>trm_4a3fd79d0b11a</dc:identifier>
        <dc:Contributor>Brenda Gregory</dc:Contributor>
    </owl:Class>
    


    <!-- http://www.cognitiveatlas.org/ontology/cogat.owl#CAO_00520 -->

    <owl:Class rdf:about="&cogat;CAO_00520">
        <rdfs:label>Skill acquisition</rdfs:label>
        <rdfs:subClassOf rdf:resource="&cogat;CAO_00377"/>
        <dc:identifier>trm_4a3fd79d0b125</dc:identifier>
        <dc:Title>Skill acquisition</dc:Title>
        <dc:Date>2012-03-28 18:38:04</dc:Date>
        <skos:definition>The process of learning to perform a task or set of tasks with increasing facility. Typically implies the formation of procedural (as distinct from semantic or episodic) memories.</skos:definition>
        <skos:hasTopConcept>Learning and Memory</skos:hasTopConcept>
        <skos:altLabel>skill learning</skos:altLabel>
        <skos:prefLabel>Skill acquisition</skos:prefLabel>
        <dc:Contributor>Russ Poldrack</dc:Contributor>
    </owl:Class>
    


    <!-- http://www.cognitiveatlas.org/ontology/cogat.owl#CAO_00522 -->

    <owl:Class rdf:about="&cogat;CAO_00522">
        <rdfs:label>Social cognition</rdfs:label>
        <rdfs:subClassOf rdf:resource="&cogat;CAO_00001"/>
        <dc:identifier>trm_4a3fd79d0b13d</dc:identifier>
        <dc:Date>2012-03-28 18:38:21</dc:Date>
        <dc:Contributor>Russ Poldrack</dc:Contributor>
        <skos:prefLabel>Social cognition</skos:prefLabel>
        <dc:Title>Social cognition</dc:Title>
        <skos:definition>the encoding, storage, retrieval, and processing, in the brain, of information relating to conspecifics, or members of the same species.</skos:definition>
        <skos:hasTopConcept>Social Function</skos:hasTopConcept>
        <skos:altLabel></skos:altLabel>
    </owl:Class>
    


    <!-- http://www.cognitiveatlas.org/ontology/cogat.owl#CAO_00523 -->

    <owl:Class rdf:about="&cogat;CAO_00523">
        <rdfs:label>Social context</rdfs:label>
        <rdfs:subClassOf rdf:resource="&cogat;CAO_00001"/>
        <skos:prefLabel>Social context</skos:prefLabel>
        <skos:definition>the identical or similar social positions and social roles as a whole that influence the individuals of a group.</skos:definition>
        <dc:Title>Social context</dc:Title>
        <dc:identifier>trm_4a3fd79d0b148</dc:identifier>
        <dc:Date>2012-03-28 18:38:34</dc:Date>
        <dc:Contributor>Russ Poldrack</dc:Contributor>
        <skos:hasTopConcept>Social Function</skos:hasTopConcept>
        <skos:altLabel></skos:altLabel>
    </owl:Class>
    


    <!-- http://www.cognitiveatlas.org/ontology/cogat.owl#CAO_00524 -->

    <owl:Class rdf:about="&cogat;CAO_00524">
        <rdfs:label>Social intelligence</rdfs:label>
        <rdfs:subClassOf rdf:resource="&cogat;CAO_00001"/>
        <dc:identifier>trm_4a3fd79d0b154</dc:identifier>
        <dc:Date>2012-03-28 18:38:50</dc:Date>
        <dc:Contributor>Russ Poldrack</dc:Contributor>
        <skos:hasTopConcept>Social Function</skos:hasTopConcept>
        <skos:prefLabel>Social intelligence</skos:prefLabel>
        <skos:altLabel></skos:altLabel>
        <dc:Title>Social intelligence</dc:Title>
        <skos:definition>the ability to function successfully in interpersonal situations.</skos:definition>
    </owl:Class>
    


    <!-- http://www.cognitiveatlas.org/ontology/cogat.owl#CAO_00525 -->

    <owl:Class rdf:about="&cogat;CAO_00525">
        <rdfs:label>Somatosensation</rdfs:label>
        <rdfs:subClassOf rdf:resource="&cogat;CAO_00001"/>
        <dc:Title>Somatosensation</dc:Title>
        <dc:Contributor>Russ Poldrack</dc:Contributor>
        <skos:prefLabel>Somatosensation</skos:prefLabel>
        <skos:altLabel>somatosensory perception</skos:altLabel>
        <skos:definition>the components of the central and peripheral nervous systems that receive and interpret sensory information from organs in the joints, ligaments, muscles, and skin. This system processes information about the length, degree of stretch, tension, and contraction of muscles; pain; temperature; pressure; and joint position.</skos:definition>
        <dc:Date>2012-03-28 18:40:09</dc:Date>
        <dc:identifier>trm_4a3fd79d0b160</dc:identifier>
        <skos:hasTopConcept>Perception</skos:hasTopConcept>
    </owl:Class>
    


    <!-- http://www.cognitiveatlas.org/ontology/cogat.owl#CAO_00527 -->

    <owl:Class rdf:about="&cogat;CAO_00527">
        <rdfs:label>Source memory</rdfs:label>
        <rdfs:subClassOf rdf:resource="&cogat;CAO_00285"/>
        <dc:Date>2011-04-19 12:12:49</dc:Date>
        <skos:hasTopConcept>Learning and Memory</skos:hasTopConcept>
        <dc:Title>Source memory</dc:Title>
        <dc:Contributor>Brenda Gregory</dc:Contributor>
        <dc:identifier>trm_4a3fd79d0b18f</dc:identifier>
        <skos:definition>the episodic source from which a specific item was acquired (e.g., from a person, a book, or television (Schacter, Kaszniak, Kihlstrom, andamp; Valdiserri, 1991, p. 559).</skos:definition>
        <skos:altLabel></skos:altLabel>
        <skos:prefLabel>Source memory</skos:prefLabel>
    </owl:Class>
    


    <!-- http://www.cognitiveatlas.org/ontology/cogat.owl#CAO_00528 -->

    <owl:Class rdf:about="&cogat;CAO_00528">
        <rdfs:label>Source monitoring</rdfs:label>
        <rdfs:subClassOf rdf:resource="&cogat;CAO_00001"/>
        <skos:altLabel></skos:altLabel>
        <skos:hasTopConcept>Learning and Memory</skos:hasTopConcept>
        <skos:definition>The process of identifying the the source or context at acquisition of information that has been stored in memory.</skos:definition>
        <dc:identifier>trm_4a3fd79d0b19b</dc:identifier>
        <skos:prefLabel>Source monitoring</skos:prefLabel>
        <dc:Date>2009-07-10 14:06:32</dc:Date>
        <dc:Contributor>Agatha Lenartowicz</dc:Contributor>
        <dc:Title>Source monitoring</dc:Title>
    </owl:Class>
    


    <!-- http://www.cognitiveatlas.org/ontology/cogat.owl#CAO_00529 -->

    <owl:Class rdf:about="&cogat;CAO_00529">
        <rdfs:label>Spatial ability</rdfs:label>
        <rdfs:subClassOf rdf:resource="&cogat;CAO_00001"/>
        <skos:hasTopConcept>Perception</skos:hasTopConcept>
        <dc:Contributor>Brenda Gregory</dc:Contributor>
        <skos:prefLabel>Spatial ability</skos:prefLabel>
        <dc:identifier>trm_4a3fd79d0b1a6</dc:identifier>
        <skos:altLabel></skos:altLabel>
        <dc:Title>Spatial ability</dc:Title>
        <dc:Date>2011-05-03 13:54:57</dc:Date>
        <skos:definition>skill in perceiving the visual world, transforming and modifying initial perceptions, and mentally recreating spatial aspects of oneand#39;s visual experience without the relevant stimuli.</skos:definition>
    </owl:Class>
    


    <!-- http://www.cognitiveatlas.org/ontology/cogat.owl#CAO_00530 -->

    <owl:Class rdf:about="&cogat;CAO_00530">
        <rdfs:label>Spatial attention</rdfs:label>
        <rdfs:subClassOf rdf:resource="&cogat;CAO_00567"/>
        <dc:identifier>trm_4a3fd79d0b1b2</dc:identifier>
        <dc:Date>2009-07-10 14:06:32</dc:Date>
        <dc:Contributor>Agatha Lenartowicz</dc:Contributor>
        <skos:altLabel></skos:altLabel>
        <skos:hasTopConcept>Attention</skos:hasTopConcept>
        <skos:definition>The allocation or prioritization of mental resources based on spatial coordinates (with respect to the body, head etc).</skos:definition>
        <skos:prefLabel>Spatial attention</skos:prefLabel>
        <dc:Title>Spatial attention</dc:Title>
    </owl:Class>
    


    <!-- http://www.cognitiveatlas.org/ontology/cogat.owl#CAO_00531 -->

    <owl:Class rdf:about="&cogat;CAO_00531">
        <rdfs:label>Spatial cognition</rdfs:label>
        <rdfs:subClassOf rdf:resource="&cogat;CAO_00001"/>
        <skos:hasTopConcept></skos:hasTopConcept>
        <skos:altLabel></skos:altLabel>
        <dc:identifier>trm_4a3fd79d0b1bd</dc:identifier>
        <dc:Date>2011-04-19 12:12:11</dc:Date>
        <dc:Contributor>Brenda Gregory</dc:Contributor>
        <skos:prefLabel>Spatial cognition</skos:prefLabel>
        <skos:definition>the acquisition, organization, utilization, and revision of knowledge about spatial environments.</skos:definition>
        <dc:Title>Spatial cognition</dc:Title>
    </owl:Class>
    


    <!-- http://www.cognitiveatlas.org/ontology/cogat.owl#CAO_00533 -->

    <owl:Class rdf:about="&cogat;CAO_00533">
        <rdfs:label>Spatial memory</rdfs:label>
        <rdfs:subClassOf rdf:resource="&cogat;CAO_00394"/>
        <rdfs:subClassOf>
            <owl:Restriction>
                <owl:onProperty rdf:resource="&ro;part_of"/>
                <owl:someValuesFrom rdf:resource="&cogat;CAO_00495"/>
            </owl:Restriction>
        </rdfs:subClassOf>
        <skos:definition>the part of memory  responsible for recording information about oneand#39;s environment and its spatial orientation.</skos:definition>
        <dc:Contributor>Russ Poldrack</dc:Contributor>
        <skos:hasTopConcept>Learning and Memory</skos:hasTopConcept>
        <dc:Date>2012-03-28 18:42:28</dc:Date>
        <dc:Title>Spatial memory</dc:Title>
        <skos:prefLabel>Spatial memory</skos:prefLabel>
        <dc:identifier>trm_4a3fd79d0b1d5</dc:identifier>
        <skos:altLabel></skos:altLabel>
    </owl:Class>
    


    <!-- http://www.cognitiveatlas.org/ontology/cogat.owl#CAO_00534 -->

    <owl:Class rdf:about="&cogat;CAO_00534">
        <rdfs:label>Spatial working memory</rdfs:label>
        <rdfs:subClassOf rdf:resource="&cogat;CAO_00587"/>
        <skos:altLabel></skos:altLabel>
        <skos:hasTopConcept>Attention</skos:hasTopConcept>
        <dc:Contributor>Agatha Lenartowicz</dc:Contributor>
        <dc:Title>Spatial working memory</dc:Title>
        <skos:definition>The ability to maintain online information that relates to space. This process has limited capacity and its contents are not stored permanently.</skos:definition>
        <dc:Date>2009-07-10 14:06:32</dc:Date>
        <dc:identifier>trm_4a3fd79d0b1e0</dc:identifier>
        <skos:prefLabel>Spatial working memory</skos:prefLabel>
    </owl:Class>
    


    <!-- http://www.cognitiveatlas.org/ontology/cogat.owl#CAO_00535 -->

    <owl:Class rdf:about="&cogat;CAO_00535">
        <rdfs:label>Speech perception</rdfs:label>
        <rdfs:subClassOf rdf:resource="&cogat;CAO_00001"/>
        <skos:altLabel></skos:altLabel>
        <dc:Contributor>Russ Poldrack</dc:Contributor>
        <skos:hasTopConcept>Language</skos:hasTopConcept>
        <dc:Date>2012-03-28 18:42:51</dc:Date>
        <skos:prefLabel>Speech perception</skos:prefLabel>
        <dc:identifier>trm_4a3fd79d0b1f7</dc:identifier>
        <dc:Title>Speech perception</dc:Title>
        <skos:definition>the process by which the sounds of language are heard, interpreted and understood. </skos:definition>
    </owl:Class>
    


    <!-- http://www.cognitiveatlas.org/ontology/cogat.owl#CAO_00536 -->

    <owl:Class rdf:about="&cogat;CAO_00536">
        <rdfs:label>Speech processing</rdfs:label>
        <rdfs:subClassOf rdf:resource="&cogat;CAO_00535"/>
        <dc:Title>Speech processing</dc:Title>
        <dc:Date>2012-03-28 18:43:33</dc:Date>
        <skos:prefLabel>Speech processing</skos:prefLabel>
        <skos:altLabel></skos:altLabel>
        <skos:definition>the processing of speech signals</skos:definition>
        <skos:hasTopConcept>Language</skos:hasTopConcept>
        <dc:identifier>trm_4a3fd79d0b238</dc:identifier>
        <dc:Contributor>Russ Poldrack</dc:Contributor>
    </owl:Class>
    


    <!-- http://www.cognitiveatlas.org/ontology/cogat.owl#CAO_00537 -->

    <owl:Class rdf:about="&cogat;CAO_00537">
        <rdfs:label>Speech production</rdfs:label>
        <rdfs:subClassOf rdf:resource="&cogat;CAO_00001"/>
        <skos:hasTopConcept>Language</skos:hasTopConcept>
        <dc:Contributor>Natalie Picchetti</dc:Contributor>
        <skos:prefLabel>Speech production</skos:prefLabel>
        <dc:identifier>trm_4a3fd79d0b247</dc:identifier>
        <skos:altLabel></skos:altLabel>
        <skos:definition>is the process by which spoken words are selected to be produced, have their phonetics formulated and then finally are articulated by the motor system in the vocal apparatus. Speech production can be spontaneous such as when a person creates the words of a conversation, reaction such as when they name a picture or read aloud a written word, or a vocal imitation such as in speech repetition.  Speech production is not the same as language production since language can also be produced manually by signs. </skos:definition>
        <dc:Date>2011-04-11 15:26:48</dc:Date>
        <dc:Title>Speech production</dc:Title>
    </owl:Class>
    


    <!-- http://www.cognitiveatlas.org/ontology/cogat.owl#CAO_00538 -->

    <owl:Class rdf:about="&cogat;CAO_00538">
        <rdfs:label>Spreading activation</rdfs:label>
        <rdfs:subClassOf rdf:resource="&cogat;CAO_00001"/>
        <skos:altLabel></skos:altLabel>
        <skos:definition>a method for searching associative networks, neural networks, or semantic networks; the search process is initiated by labeling a set of source nodes (e.g. concepts in a semantic network) with weights or and#34;activationand#34; and then iteratively propagating or and#34;spreadingand#34; that activation out to other nodes linked to the source nodes.</skos:definition>
        <skos:prefLabel>Spreading activation</skos:prefLabel>
        <dc:identifier>trm_4a3fd79d0b26d</dc:identifier>
        <dc:Contributor>Brenda Gregory</dc:Contributor>
        <skos:hasTopConcept></skos:hasTopConcept>
        <dc:Title>Spreading activation</dc:Title>
        <dc:Date>2011-04-28 17:24:55</dc:Date>
    </owl:Class>
    


    <!-- http://www.cognitiveatlas.org/ontology/cogat.owl#CAO_00539 -->

    <owl:Class rdf:about="&cogat;CAO_00539">
        <rdfs:label>Stereopsis</rdfs:label>
        <rdfs:subClassOf rdf:resource="&cogat;CAO_00001"/>
        <skos:hasTopConcept>Perception</skos:hasTopConcept>
        <skos:altLabel></skos:altLabel>
        <dc:identifier>trm_4a3fd79d0b279</dc:identifier>
        <skos:prefLabel>Stereopsis</skos:prefLabel>
        <dc:Title>Stereopsis</dc:Title>
        <dc:Date>2011-08-19 13:54:04</dc:Date>
        <skos:definition>the process in visual perception leading to the sensation of depth from the two slightly different projections of the world onto the retinas of the two eyes.</skos:definition>
        <dc:Contributor>Akram Bakkour</dc:Contributor>
    </owl:Class>
    


    <!-- http://www.cognitiveatlas.org/ontology/cogat.owl#CAO_00540 -->

    <owl:Class rdf:about="&cogat;CAO_00540">
        <rdfs:label>Stereotypes</rdfs:label>
        <rdfs:subClassOf rdf:resource="&cogat;CAO_00001"/>
        <dc:Title>Stereotypes</dc:Title>
        <dc:identifier>trm_4a3fd79d0b285</dc:identifier>
        <dc:Date>2012-03-28 18:44:18</dc:Date>
        <skos:hasTopConcept>Social Function</skos:hasTopConcept>
        <skos:definition>something conforming to a fixed or general pattern; a standardized mental picture that is held in common by members of a group and that represents an oversimplified opinion, prejudiced attitude, or uncritical judgment.</skos:definition>
        <skos:prefLabel>Stereotypes</skos:prefLabel>
        <dc:Contributor>Russ Poldrack</dc:Contributor>
        <skos:altLabel></skos:altLabel>
    </owl:Class>
    


    <!-- http://www.cognitiveatlas.org/ontology/cogat.owl#CAO_00542 -->

    <owl:Class rdf:about="&cogat;CAO_00542">
        <rdfs:label>Strategy</rdfs:label>
        <rdfs:subClassOf rdf:resource="&cogat;CAO_00001"/>
        <dc:Title>Strategy</dc:Title>
        <skos:prefLabel>Strategy</skos:prefLabel>
        <skos:definition>A plan of action designed to achieve a particular goal.</skos:definition>
        <dc:Date>2011-05-18 14:07:17</dc:Date>
        <dc:identifier>trm_4a3fd79d0b29c</dc:identifier>
        <skos:altLabel></skos:altLabel>
        <dc:Contributor>Brenda Gregory</dc:Contributor>
        <skos:hasTopConcept></skos:hasTopConcept>
    </owl:Class>
    


    <!-- http://www.cognitiveatlas.org/ontology/cogat.owl#CAO_00543 -->

    <owl:Class rdf:about="&cogat;CAO_00543">
        <rdfs:label>Stress</rdfs:label>
        <rdfs:subClassOf rdf:resource="&cogat;CAO_00001"/>
        <skos:hasTopConcept>Emotion</skos:hasTopConcept>
        <dc:identifier>trm_4a3fd79d0b2a8</dc:identifier>
        <dc:Date>2012-03-28 18:45:54</dc:Date>
        <dc:Contributor>Russ Poldrack</dc:Contributor>
        <dc:Title>Stress</dc:Title>
        <skos:definition>refers to the consequence of the failure of an organism – human or animal – to respond appropriately to emotional or physical threats, whether actual or imagined. </skos:definition>
        <skos:altLabel></skos:altLabel>
        <skos:prefLabel>Stress</skos:prefLabel>
    </owl:Class>
    


    <!-- http://www.cognitiveatlas.org/ontology/cogat.owl#CAO_00544 -->

    <owl:Class rdf:about="&cogat;CAO_00544">
        <rdfs:label>Sublexical route</rdfs:label>
        <rdfs:subClassOf rdf:resource="&cogat;CAO_00001"/>
        <rdfs:subClassOf>
            <owl:Restriction>
                <owl:onProperty rdf:resource="&ro;part_of"/>
                <owl:someValuesFrom rdf:resource="&cogat;CAO_00479"/>
            </owl:Restriction>
        </rdfs:subClassOf>
        <skos:altLabel></skos:altLabel>
        <skos:hasTopConcept>Language</skos:hasTopConcept>
        <dc:identifier>trm_4a3fd79d0b2b4</dc:identifier>
        <skos:definition>is a theoretical component of Coltheartand#39;s dual-route reading model that refers to using spelling-to-sound correspondences to convert a written word (i.e. orthography) into a spoken word (i.e. phonology).  In other words, it is the route by which letters are linked to their sounds and the sounds are assembled into a whole word pronunciation.  It complements the lexical route where the whole word is recognized and linked to its sound.</skos:definition>
        <dc:Date>2010-05-09 00:33:37</dc:Date>
        <dc:Title>Sublexical route</dc:Title>
        <skos:prefLabel>Sublexical route</skos:prefLabel>
        <dc:Contributor>Joseph Devlin</dc:Contributor>
    </owl:Class>
    


    <!-- http://www.cognitiveatlas.org/ontology/cogat.owl#CAO_00545 -->

    <owl:Class rdf:about="&cogat;CAO_00545">
        <rdfs:label>Subliminal perception</rdfs:label>
        <rdfs:subClassOf rdf:resource="&cogat;CAO_00001"/>
        <skos:hasTopConcept>Perception</skos:hasTopConcept>
        <dc:Date>2011-05-11 14:46:29</dc:Date>
        <dc:Title>Subliminal perception</dc:Title>
        <dc:identifier>trm_4a3fd79d0b2bf</dc:identifier>
        <dc:Contributor>Natalie Picchetti</dc:Contributor>
        <skos:definition>a visual or auditory message that is allegedly perceived psychologically, but not consciously; occurs when a stimulus is too weak to be perceived yet a person is influenced by it. </skos:definition>
        <skos:prefLabel>Subliminal perception</skos:prefLabel>
        <skos:altLabel></skos:altLabel>
    </owl:Class>
    


    <!-- http://www.cognitiveatlas.org/ontology/cogat.owl#CAO_00547 -->

    <owl:Class rdf:about="&cogat;CAO_00547">
        <rdfs:label>Supervisory attentional system</rdfs:label>
        <rdfs:subClassOf rdf:resource="&cogat;CAO_00001"/>
        <dc:identifier>trm_4a3fd79d0b2fa</dc:identifier>
        <skos:hasTopConcept>Executive-Cognitive Control</skos:hasTopConcept>
        <skos:altLabel></skos:altLabel>
        <skos:prefLabel>Supervisory attentional system</skos:prefLabel>
        <skos:definition>a loosely defined collection of brain processes that are responsible for planning, cognitive flexibility, abstract thinking, rule acquisition, initiating appropriate actions and inhibiting inappropriate actions, and selecting relevant sensory information.</skos:definition>
        <dc:Date>2012-03-28 18:48:50</dc:Date>
        <dc:Contributor>Russ Poldrack</dc:Contributor>
        <dc:Title>Supervisory attentional system</dc:Title>
    </owl:Class>
    


    <!-- http://www.cognitiveatlas.org/ontology/cogat.owl#CAO_00548 -->

    <owl:Class rdf:about="&cogat;CAO_00548">
        <rdfs:label>Surprise</rdfs:label>
        <rdfs:subClassOf rdf:resource="&cogat;CAO_00276"/>
        <dc:Date>2011-05-17 10:05:39</dc:Date>
        <dc:Contributor>Brenda Gregory</dc:Contributor>
        <skos:altLabel></skos:altLabel>
        <skos:prefLabel>Surprise</skos:prefLabel>
        <dc:Title>Surprise</dc:Title>
        <dc:identifier>trm_4a3fd79d0b306</dc:identifier>
        <skos:hasTopConcept>Emotion</skos:hasTopConcept>
        <skos:definition>a brief emotional state that is the result of experiencing an unexpected relevant event.</skos:definition>
    </owl:Class>
    


    <!-- http://www.cognitiveatlas.org/ontology/cogat.owl#CAO_00549 -->

    <owl:Class rdf:about="&cogat;CAO_00549">
        <rdfs:label>Sustained attention</rdfs:label>
        <rdfs:subClassOf rdf:resource="&cogat;CAO_00144"/>
        <skos:altLabel></skos:altLabel>
        <dc:Contributor>Brenda Gregory</dc:Contributor>
        <skos:prefLabel>Sustained attention</skos:prefLabel>
        <dc:Date>2011-04-28 12:16:41</dc:Date>
        <skos:definition>the ability to maintain a consistent behavioral response during continuous and repetitive activity.</skos:definition>
        <dc:Title>Sustained attention</dc:Title>
        <skos:hasTopConcept>Attention</skos:hasTopConcept>
        <dc:identifier>trm_4a3fd79d0b311</dc:identifier>
    </owl:Class>
    


    <!-- http://www.cognitiveatlas.org/ontology/cogat.owl#CAO_00550 -->

    <owl:Class rdf:about="&cogat;CAO_00550">
        <rdfs:label>Syntactic parsing</rdfs:label>
        <rdfs:subClassOf rdf:resource="&cogat;CAO_00001"/>
        <dc:identifier>trm_4a3fd79d0b340</dc:identifier>
        <dc:Title>Syntactic parsing</dc:Title>
        <skos:hasTopConcept>Language</skos:hasTopConcept>
        <skos:definition>the way that human beings, rather than computers, analyze a sentence or phrase (in spoken language or text) in terms of grammatical constituents, identifying the parts of speech, syntactic relations, etc.</skos:definition>
        <dc:Date>2011-03-30 11:35:54</dc:Date>
        <skos:altLabel></skos:altLabel>
        <dc:Contributor>Russ Poldrack</dc:Contributor>
        <skos:prefLabel>Syntactic parsing</skos:prefLabel>
    </owl:Class>
    


    <!-- http://www.cognitiveatlas.org/ontology/cogat.owl#CAO_00551 -->

    <owl:Class rdf:about="&cogat;CAO_00551">
        <rdfs:label>Syntactic processing</rdfs:label>
        <rdfs:subClassOf rdf:resource="&cogat;CAO_00001"/>
        <skos:prefLabel>Syntactic processing</skos:prefLabel>
        <dc:identifier>trm_4a3fd79d0b34b</dc:identifier>
        <dc:Contributor>Akram Bakkour</dc:Contributor>
        <skos:altLabel></skos:altLabel>
        <dc:Date>2011-08-19 14:21:47</dc:Date>
        <skos:hasTopConcept>Language</skos:hasTopConcept>
        <skos:definition>processing of the structural and grammatical aspects of language</skos:definition>
        <dc:Title>Syntactic processing</dc:Title>
    </owl:Class>
    


    <!-- http://www.cognitiveatlas.org/ontology/cogat.owl#CAO_00552 -->

    <owl:Class rdf:about="&cogat;CAO_00552">
        <rdfs:label>Syntax</rdfs:label>
        <rdfs:subClassOf rdf:resource="&cogat;CAO_00001"/>
        <skos:definition>the way in which linguistic elements (as words) are put together to form constituents (as phrases or clauses); a connected or orderly system, harmonious arrangement of parts or elements.</skos:definition>
        <skos:altLabel></skos:altLabel>
        <dc:Date>2011-05-04 11:06:08</dc:Date>
        <dc:identifier>trm_4a3fd79d0b357</dc:identifier>
        <skos:hasTopConcept>Language</skos:hasTopConcept>
        <dc:Contributor>Brenda Gregory</dc:Contributor>
        <skos:prefLabel>Syntax</skos:prefLabel>
        <dc:Title>Syntax</dc:Title>
    </owl:Class>
    


    <!-- http://www.cognitiveatlas.org/ontology/cogat.owl#CAO_00553 -->

    <owl:Class rdf:about="&cogat;CAO_00553">
        <rdfs:label>Taste aversion</rdfs:label>
        <rdfs:subClassOf rdf:resource="&cogat;CAO_00001"/>
        <dc:Contributor>Mei-Yen Chen</dc:Contributor>
        <dc:identifier>trm_4a3fd79d0b363</dc:identifier>
        <skos:altLabel></skos:altLabel>
        <skos:definition>occurs when the taste of a certain food is associated with symptoms caused by a toxic, spoiled, or poisonous substance;  generally caused after ingestion of the food causes nausea, sickness, or vomiting. The ability to develop a taste aversion is considered an adaptive trait or survival mechanism that trains the body to avoid poisonous substances (e.g., poisonous berries) before they can cause harm.</skos:definition>
        <dc:Title>Taste aversion</dc:Title>
        <skos:prefLabel>Taste aversion</skos:prefLabel>
        <skos:hasTopConcept>Emotion</skos:hasTopConcept>
        <dc:Date>2011-08-12 13:08:35</dc:Date>
    </owl:Class>
    


    <!-- http://www.cognitiveatlas.org/ontology/cogat.owl#CAO_00554 -->

    <owl:Class rdf:about="&cogat;CAO_00554">
        <rdfs:label>Text comprehension</rdfs:label>
        <rdfs:subClassOf rdf:resource="&cogat;CAO_00373"/>
        <skos:definition>Intentional thinking during which meaning is constructed through interactions between text and reader.</skos:definition>
        <dc:Date>2011-08-12 13:10:02</dc:Date>
        <skos:altLabel></skos:altLabel>
        <dc:Contributor>Mei-Yen Chen</dc:Contributor>
        <dc:Title>Text comprehension</dc:Title>
        <skos:hasTopConcept>Language</skos:hasTopConcept>
        <skos:prefLabel>Text comprehension</skos:prefLabel>
        <dc:identifier>trm_4a3fd79d0b37a</dc:identifier>
    </owl:Class>
    


    <!-- http://www.cognitiveatlas.org/ontology/cogat.owl#CAO_00555 -->

    <owl:Class rdf:about="&cogat;CAO_00555">
        <rdfs:label>Text processing</rdfs:label>
        <rdfs:subClassOf rdf:resource="&cogat;CAO_00001"/>
        <rdfs:subClassOf>
            <owl:Restriction>
                <owl:onProperty rdf:resource="&ro;part_of"/>
                <owl:someValuesFrom rdf:resource="&cogat;CAO_00579"/>
            </owl:Restriction>
        </rdfs:subClassOf>
        <rdfs:subClassOf>
            <owl:Restriction>
                <owl:onProperty rdf:resource="&ro;part_of"/>
                <owl:someValuesFrom rdf:resource="&cogat;CAO_00554"/>
            </owl:Restriction>
        </rdfs:subClassOf>
        <dc:Date>2011-08-12 13:10:15</dc:Date>
        <dc:Title>Text processing</dc:Title>
        <skos:altLabel></skos:altLabel>
        <skos:prefLabel>Text processing</skos:prefLabel>
        <skos:hasTopConcept>Language</skos:hasTopConcept>
        <dc:identifier>trm_4a3fd79d0b386</dc:identifier>
        <skos:definition>The handling of alphabetic characters</skos:definition>
        <dc:Contributor>Mei-Yen Chen</dc:Contributor>
    </owl:Class>
    


    <!-- http://www.cognitiveatlas.org/ontology/cogat.owl#CAO_00556 -->

    <owl:Class rdf:about="&cogat;CAO_00556">
        <rdfs:label>Theory of mind</rdfs:label>
        <rdfs:subClassOf rdf:resource="&cogat;CAO_00001"/>
        <skos:prefLabel>Theory of mind</skos:prefLabel>
        <skos:altLabel></skos:altLabel>
        <skos:definition>the ability for a person to connect emotional states to themselves and others and understand that other people may have different  beliefs, desires, or intentions from oneand#39;s self.  It is intimately connected with the development of a personand#39;s ability to analyze and interpret the intentions of others.</skos:definition>
        <dc:identifier>trm_4a3fd79d0b392</dc:identifier>
        <dc:Title>Theory of mind</dc:Title>
        <dc:Date>2011-08-12 13:08:00</dc:Date>
        <skos:hasTopConcept>Social Function</skos:hasTopConcept>
        <dc:Contributor>Mei-Yen Chen</dc:Contributor>
    </owl:Class>
    


    <!-- http://www.cognitiveatlas.org/ontology/cogat.owl#CAO_00557 -->

    <owl:Class rdf:about="&cogat;CAO_00557">
        <rdfs:label>Thermosensation</rdfs:label>
        <rdfs:subClassOf rdf:resource="&cogat;CAO_00525"/>
        <dc:Date>2011-05-16 15:46:13</dc:Date>
        <skos:definition>the sensory perception of thermal stimuli.</skos:definition>
        <skos:prefLabel>Thermosensation</skos:prefLabel>
        <skos:altLabel></skos:altLabel>
        <skos:hasTopConcept>Perception</skos:hasTopConcept>
        <dc:Contributor>Brenda Gregory</dc:Contributor>
        <dc:identifier>trm_4a3fd79d0b39d</dc:identifier>
        <dc:Title>Thermosensation</dc:Title>
    </owl:Class>
    


    <!-- http://www.cognitiveatlas.org/ontology/cogat.owl#CAO_00558 -->

    <owl:Class rdf:about="&cogat;CAO_00558">
        <rdfs:label>Top down processing</rdfs:label>
        <rdfs:subClassOf rdf:resource="&cogat;CAO_00001"/>
        <dc:Contributor>Brenda Gregory</dc:Contributor>
        <skos:definition>perceptions formed by starting with the larger concept or idea, then working down to the finer details of that concept or idea.</skos:definition>
        <skos:altLabel></skos:altLabel>
        <dc:Title>Top down processing</dc:Title>
        <dc:identifier>trm_4a3fd79d0b3cb</dc:identifier>
        <dc:Date>2011-04-29 16:02:04</dc:Date>
        <skos:prefLabel>Top down processing</skos:prefLabel>
        <skos:hasTopConcept></skos:hasTopConcept>
    </owl:Class>
    


    <!-- http://www.cognitiveatlas.org/ontology/cogat.owl#CAO_00559 -->

    <owl:Class rdf:about="&cogat;CAO_00559">
        <rdfs:label>Traumatic memory</rdfs:label>
        <rdfs:subClassOf rdf:resource="&cogat;CAO_00394"/>
        <skos:altLabel></skos:altLabel>
        <dc:identifier>trm_4a3fd79d0b3ef</dc:identifier>
        <skos:hasTopConcept>Learning and Memory</skos:hasTopConcept>
        <skos:prefLabel>Traumatic memory</skos:prefLabel>
        <dc:Date>2012-03-28 18:52:52</dc:Date>
        <dc:Title>Traumatic memory</dc:Title>
        <dc:Contributor>Russ Poldrack</dc:Contributor>
        <skos:definition>A type of memory results from trauma experience, such as a natural disaster or violent events.</skos:definition>
    </owl:Class>
    


    <!-- http://www.cognitiveatlas.org/ontology/cogat.owl#CAO_00560 -->

    <owl:Class rdf:about="&cogat;CAO_00560">
        <rdfs:label>Uncertainty</rdfs:label>
        <rdfs:subClassOf rdf:resource="&cogat;CAO_00001"/>
        <dc:identifier>trm_4a3fd79d0b3fa</dc:identifier>
        <dc:Title>Uncertainty</dc:Title>
        <dc:Date>2012-03-28 18:56:17</dc:Date>
        <skos:altLabel></skos:altLabel>
        <dc:Contributor>Russ Poldrack</dc:Contributor>
        <skos:prefLabel>Uncertainty</skos:prefLabel>
        <skos:hasTopConcept>Reasoning and Decision Making</skos:hasTopConcept>
        <skos:definition>the lack of knowledge regarding the likelihood of potential outcomes</skos:definition>
    </owl:Class>
    


    <!-- http://www.cognitiveatlas.org/ontology/cogat.owl#CAO_00561 -->

    <owl:Class rdf:about="&cogat;CAO_00561">
        <rdfs:label>Unconscious process</rdfs:label>
        <rdfs:subClassOf rdf:resource="&cogat;CAO_00001"/>
        <rdfs:subClassOf>
            <owl:Restriction>
                <owl:onProperty rdf:resource="&ro;part_of"/>
                <owl:someValuesFrom rdf:resource="&cogat;CAO_00683"/>
            </owl:Restriction>
        </rdfs:subClassOf>
        <dc:Title>Unconscious process</dc:Title>
        <dc:identifier>trm_4a3fd79d0b406</dc:identifier>
        <skos:prefLabel>Unconscious process</skos:prefLabel>
        <skos:altLabel></skos:altLabel>
        <skos:hasTopConcept></skos:hasTopConcept>
        <dc:Contributor>Brenda Gregory</dc:Contributor>
        <dc:Date>2011-05-17 09:59:39</dc:Date>
        <skos:definition>a mental process that you are not directly aware of.</skos:definition>
    </owl:Class>
    


    <!-- http://www.cognitiveatlas.org/ontology/cogat.owl#CAO_00562 -->

    <owl:Class rdf:about="&cogat;CAO_00562">
        <rdfs:label>Utility</rdfs:label>
        <rdfs:subClassOf rdf:resource="&cogat;CAO_00001"/>
        <dc:Title>Utility</dc:Title>
        <dc:Contributor>Russ Poldrack</dc:Contributor>
        <skos:altLabel></skos:altLabel>
        <skos:definition>a measure of value associated with a particular outcome</skos:definition>
        <skos:hasTopConcept>Reasoning and Decision Making</skos:hasTopConcept>
        <dc:identifier>trm_4a3fd79d0b412</dc:identifier>
        <dc:Date>2012-03-28 18:58:04</dc:Date>
        <skos:prefLabel>Utility</skos:prefLabel>
    </owl:Class>
    


    <!-- http://www.cognitiveatlas.org/ontology/cogat.owl#CAO_00563 -->

    <owl:Class rdf:about="&cogat;CAO_00563">
        <rdfs:label>Valence</rdfs:label>
        <rdfs:subClassOf rdf:resource="&cogat;CAO_00562"/>
        <skos:hasTopConcept>Emotion</skos:hasTopConcept>
        <skos:prefLabel>Valence</skos:prefLabel>
        <dc:Contributor>Russ Poldrack</dc:Contributor>
        <skos:altLabel></skos:altLabel>
        <dc:identifier>trm_4a3fd79d0b429</dc:identifier>
        <dc:Title>Valence</dc:Title>
        <skos:definition>the degree of attractiveness an individual, activity, or thing possesses as a behavioral goal.</skos:definition>
        <dc:Date>2012-03-28 18:58:39</dc:Date>
    </owl:Class>
    


    <!-- http://www.cognitiveatlas.org/ontology/cogat.owl#CAO_00564 -->

    <owl:Class rdf:about="&cogat;CAO_00564">
        <rdfs:label>Verbal fluency</rdfs:label>
        <rdfs:subClassOf rdf:resource="&cogat;CAO_00001"/>
        <skos:altLabel></skos:altLabel>
        <skos:prefLabel>Verbal fluency</skos:prefLabel>
        <skos:hasTopConcept>Language</skos:hasTopConcept>
        <dc:Date>2011-08-12 13:21:08</dc:Date>
        <skos:definition>the ability to rapidly access your mental vocabulary while talking or writing.</skos:definition>
        <dc:Title>Verbal fluency</dc:Title>
        <dc:identifier>trm_4a3fd79d0b44c</dc:identifier>
        <dc:Contributor>Mei-Yen Chen</dc:Contributor>
    </owl:Class>
    


    <!-- http://www.cognitiveatlas.org/ontology/cogat.owl#CAO_00565 -->

    <owl:Class rdf:about="&cogat;CAO_00565">
        <rdfs:label>Verbal memory</rdfs:label>
        <rdfs:subClassOf rdf:resource="&cogat;CAO_00394"/>
        <skos:definition>Recall based on spoken words.</skos:definition>
        <dc:Contributor>Brenda Gregory</dc:Contributor>
        <dc:identifier>trm_4a3fd79d0b457</dc:identifier>
        <skos:altLabel></skos:altLabel>
        <skos:prefLabel>Verbal memory</skos:prefLabel>
        <skos:hasTopConcept>Learning and Memory</skos:hasTopConcept>
        <dc:Title>Verbal memory</dc:Title>
        <dc:Date>2011-05-18 14:24:27</dc:Date>
    </owl:Class>
    


    <!-- http://www.cognitiveatlas.org/ontology/cogat.owl#CAO_00567 -->

    <owl:Class rdf:about="&cogat;CAO_00567">
        <rdfs:label>Visual attention</rdfs:label>
        <rdfs:subClassOf rdf:resource="&cogat;CAO_00144"/>
        <skos:hasTopConcept>Attention</skos:hasTopConcept>
        <dc:Contributor>Brenda Gregory</dc:Contributor>
        <skos:altLabel></skos:altLabel>
        <skos:prefLabel>Visual attention</skos:prefLabel>
        <dc:identifier>trm_4a3fd79d0b46f</dc:identifier>
        <skos:definition>two-stage process in which attention is distributed uniformly over the external visual scene and processing of information is performed in parallel, attention is then concentrated to a specific area of the visual scene (i.e. it is focused), and processing is performed in a serial fashion.</skos:definition>
        <dc:Title>Visual attention</dc:Title>
        <dc:Date>2011-04-28 16:13:37</dc:Date>
    </owl:Class>
    


    <!-- http://www.cognitiveatlas.org/ontology/cogat.owl#CAO_00568 -->

    <owl:Class rdf:about="&cogat;CAO_00568">
        <rdfs:label>Visual buffer</rdfs:label>
        <rdfs:subClassOf rdf:resource="&cogat;CAO_00001"/>
        <dc:Date>2012-03-28 19:00:28</dc:Date>
        <dc:Contributor>Russ Poldrack</dc:Contributor>
        <skos:hasTopConcept>Perception</skos:hasTopConcept>
        <dc:Title>Visual buffer</dc:Title>
        <skos:definition>a short-term memory store for visual information</skos:definition>
        <skos:prefLabel>Visual buffer</skos:prefLabel>
        <skos:altLabel></skos:altLabel>
        <dc:identifier>trm_4a3fd79d0b47b</dc:identifier>
    </owl:Class>
    


    <!-- http://www.cognitiveatlas.org/ontology/cogat.owl#CAO_00569 -->

    <owl:Class rdf:about="&cogat;CAO_00569">
        <rdfs:label>Visual imagery</rdfs:label>
        <rdfs:subClassOf rdf:resource="&cogat;CAO_00576"/>
        <skos:altLabel></skos:altLabel>
        <skos:prefLabel>Visual imagery</skos:prefLabel>
        <dc:identifier>trm_4a3fd79d0b487</dc:identifier>
        <dc:Date>2012-03-28 19:00:56</dc:Date>
        <dc:Title>Visual imagery</dc:Title>
        <dc:Contributor>Russ Poldrack</dc:Contributor>
        <skos:definition>an experience that, on most occasions, significantly resembles the experience of perceiving some object, event, or scene, but occurs when the relevant object, event, or scene is not actually present to the senses. </skos:definition>
        <skos:hasTopConcept></skos:hasTopConcept>
    </owl:Class>
    


    <!-- http://www.cognitiveatlas.org/ontology/cogat.owl#CAO_00570 -->

    <owl:Class rdf:about="&cogat;CAO_00570">
        <rdfs:label>Visual masking</rdfs:label>
        <rdfs:subClassOf rdf:resource="&cogat;CAO_00001"/>
        <skos:altLabel></skos:altLabel>
        <dc:identifier>trm_4a3fd79d0b492</dc:identifier>
        <skos:hasTopConcept></skos:hasTopConcept>
        <skos:definition>the reduction or elimination of the visibility of a brief (≤ 50 ms) stimulus, called the “target”, by the presentation of a second brief stimulus, called the “mask”.</skos:definition>
        <dc:Date>2011-05-03 13:57:36</dc:Date>
        <dc:Title>Visual masking</dc:Title>
        <skos:prefLabel>Visual masking</skos:prefLabel>
        <dc:Contributor>Brenda Gregory</dc:Contributor>
    </owl:Class>
    


    <!-- http://www.cognitiveatlas.org/ontology/cogat.owl#CAO_00571 -->

    <owl:Class rdf:about="&cogat;CAO_00571">
        <rdfs:label>Visual memory</rdfs:label>
        <rdfs:subClassOf rdf:resource="&cogat;CAO_00394"/>
        <skos:prefLabel>Visual memory</skos:prefLabel>
        <dc:identifier>trm_4a3fd79d0b49e</dc:identifier>
        <dc:Contributor>Brenda Gregory</dc:Contributor>
        <skos:altLabel></skos:altLabel>
        <skos:hasTopConcept>Learning and Memory</skos:hasTopConcept>
        <dc:Title>Visual memory</dc:Title>
        <dc:Date>2011-04-29 10:56:51</dc:Date>
        <skos:definition>a part of memory  preserving some characteristics of our senses pertaining to visual experience.</skos:definition>
    </owl:Class>
    


    <!-- http://www.cognitiveatlas.org/ontology/cogat.owl#CAO_00572 -->

    <owl:Class rdf:about="&cogat;CAO_00572">
        <rdfs:label>Visual object recognition</rdfs:label>
        <rdfs:subClassOf rdf:resource="&cogat;CAO_00428"/>
        <rdfs:subClassOf>
            <owl:Restriction>
                <owl:onProperty rdf:resource="&ro;part_of"/>
                <owl:someValuesFrom rdf:resource="&cogat;CAO_00573"/>
            </owl:Restriction>
        </rdfs:subClassOf>
        <skos:definition>is the process of identifying an object based on its visual attributes</skos:definition>
        <skos:hasTopConcept>Perception</skos:hasTopConcept>
        <skos:altLabel></skos:altLabel>
        <dc:Date>2010-01-31 14:12:49</dc:Date>
        <dc:Title>Visual object recognition</dc:Title>
        <skos:prefLabel>Visual object recognition</skos:prefLabel>
        <dc:identifier>trm_4a3fd79d0b4a9</dc:identifier>
        <dc:Contributor>Joseph Devlin</dc:Contributor>
    </owl:Class>
    


    <!-- http://www.cognitiveatlas.org/ontology/cogat.owl#CAO_00573 -->

    <owl:Class rdf:about="&cogat;CAO_00573">
        <rdfs:label>Visual perception</rdfs:label>
        <rdfs:subClassOf rdf:resource="&cogat;CAO_00001"/>
        <rdfs:subClassOf>
            <owl:Restriction>
                <owl:onProperty rdf:resource="&ro;part_of"/>
                <owl:someValuesFrom rdf:resource="&cogat;CAO_00150"/>
            </owl:Restriction>
        </rdfs:subClassOf>
        <skos:prefLabel>Visual perception</skos:prefLabel>
        <skos:definition>Ability to interpret information from visible light reaching the eye.</skos:definition>
        <dc:Title>Visual perception</dc:Title>
        <skos:hasTopConcept>Perception</skos:hasTopConcept>
        <dc:identifier>trm_4a3fd79d0b4b5</dc:identifier>
        <dc:Contributor>Agatha Lenartowicz</dc:Contributor>
        <dc:Date>2009-07-10 14:06:33</dc:Date>
        <skos:altLabel></skos:altLabel>
    </owl:Class>
    


    <!-- http://www.cognitiveatlas.org/ontology/cogat.owl#CAO_00574 -->

    <owl:Class rdf:about="&cogat;CAO_00574">
        <rdfs:label>Visual representation</rdfs:label>
        <rdfs:subClassOf rdf:resource="&cogat;CAO_00397"/>
        <dc:Contributor>Russ Poldrack</dc:Contributor>
        <skos:prefLabel>Visual representation</skos:prefLabel>
        <dc:Title>Visual representation</dc:Title>
        <skos:definition>An internal representation of visual information</skos:definition>
        <skos:hasTopConcept>Perception</skos:hasTopConcept>
        <dc:identifier>trm_4a3fd79d0b4c1</dc:identifier>
        <skos:altLabel></skos:altLabel>
        <dc:Date>2012-03-28 19:02:21</dc:Date>
    </owl:Class>
    


    <!-- http://www.cognitiveatlas.org/ontology/cogat.owl#CAO_00575 -->

    <owl:Class rdf:about="&cogat;CAO_00575">
        <rdfs:label>Visual search</rdfs:label>
        <rdfs:subClassOf rdf:resource="&cogat;CAO_00502"/>
        <dc:Title>Visual search</dc:Title>
        <skos:altLabel></skos:altLabel>
        <dc:identifier>trm_4a3fd79d0b4cd</dc:identifier>
        <skos:prefLabel>Visual search</skos:prefLabel>
        <skos:hasTopConcept>Attention</skos:hasTopConcept>
        <skos:definition>a type of perceptual task requiring attention that typically involves an active scan of the visual environment for a particular object or feature (the target) among other objects or features (the distractors).</skos:definition>
        <dc:Date>2011-08-12 13:37:37</dc:Date>
        <dc:Contributor>Mei-Yen Chen</dc:Contributor>
    </owl:Class>
    


    <!-- http://www.cognitiveatlas.org/ontology/cogat.owl#CAO_00576 -->

    <owl:Class rdf:about="&cogat;CAO_00576">
        <rdfs:label>Visual working memory</rdfs:label>
        <rdfs:subClassOf rdf:resource="&cogat;CAO_00587"/>
        <dc:Contributor>Agatha Lenartowicz</dc:Contributor>
        <skos:altLabel></skos:altLabel>
        <skos:prefLabel>Visual working memory</skos:prefLabel>
        <dc:Date>2009-07-10 14:06:33</dc:Date>
        <dc:identifier>trm_4a3fd79d0b4d8</dc:identifier>
        <dc:Title>Visual working memory</dc:Title>
        <skos:definition>The ability to maintain visual information online for a limited time interval (~ 4 sec). This information has a capacity of ~15 items and is not stored permanently.</skos:definition>
        <skos:hasTopConcept>Attention</skos:hasTopConcept>
    </owl:Class>
    


    <!-- http://www.cognitiveatlas.org/ontology/cogat.owl#CAO_00577 -->

    <owl:Class rdf:about="&cogat;CAO_00577">
        <rdfs:label>Visuospatial sketch pad</rdfs:label>
        <rdfs:subClassOf rdf:resource="&cogat;CAO_00001"/>
        <rdfs:subClassOf>
            <owl:Restriction>
                <owl:onProperty rdf:resource="&ro;part_of"/>
                <owl:someValuesFrom rdf:resource="&cogat;CAO_00576"/>
            </owl:Restriction>
        </rdfs:subClassOf>
        <rdfs:subClassOf>
            <owl:Restriction>
                <owl:onProperty rdf:resource="&ro;part_of"/>
                <owl:someValuesFrom rdf:resource="&cogat;CAO_00534"/>
            </owl:Restriction>
        </rdfs:subClassOf>
        <dc:identifier>trm_4a3fd79d0b507</dc:identifier>
        <skos:definition>The cognitive construct and mental process of temporarily storing visual and spatial information for online use in operations of working memory (c.f., Alan Baddeley) . </skos:definition>
        <skos:altLabel></skos:altLabel>
        <dc:Title>Visuospatial sketch pad</dc:Title>
        <skos:hasTopConcept>Executive-Cognitive Control</skos:hasTopConcept>
        <dc:Date>2009-07-10 14:06:33</dc:Date>
        <skos:prefLabel>Visuospatial sketch pad</skos:prefLabel>
        <dc:Contributor>Agatha Lenartowicz</dc:Contributor>
    </owl:Class>
    


    <!-- http://www.cognitiveatlas.org/ontology/cogat.owl#CAO_00578 -->

    <owl:Class rdf:about="&cogat;CAO_00578">
        <rdfs:label>Wisdom</rdfs:label>
        <rdfs:subClassOf rdf:resource="&cogat;CAO_00001"/>
        <skos:altLabel></skos:altLabel>
        <dc:Title>Wisdom</dc:Title>
        <dc:Contributor>Brenda Gregory</dc:Contributor>
        <dc:Date>2011-05-12 15:34:55</dc:Date>
        <skos:prefLabel>Wisdom</skos:prefLabel>
        <dc:identifier>trm_4a3fd79d0b530</dc:identifier>
        <skos:hasTopConcept></skos:hasTopConcept>
        <skos:definition>accumulated philosophic or scientific learning.</skos:definition>
    </owl:Class>
    


    <!-- http://www.cognitiveatlas.org/ontology/cogat.owl#CAO_00579 -->

    <owl:Class rdf:about="&cogat;CAO_00579">
        <rdfs:label>Word comprehension</rdfs:label>
        <rdfs:subClassOf rdf:resource="&cogat;CAO_00001"/>
        <dc:Date>2011-08-12 13:38:26</dc:Date>
        <skos:definition>the ability to understand the meaning of words.</skos:definition>
        <skos:prefLabel>Word comprehension</skos:prefLabel>
        <skos:altLabel></skos:altLabel>
        <dc:Title>Word comprehension</dc:Title>
        <dc:Contributor>Mei-Yen Chen</dc:Contributor>
        <skos:hasTopConcept>Language</skos:hasTopConcept>
        <dc:identifier>trm_4a3fd79d0b548</dc:identifier>
    </owl:Class>
    


    <!-- http://www.cognitiveatlas.org/ontology/cogat.owl#CAO_00581 -->

    <owl:Class rdf:about="&cogat;CAO_00581">
        <rdfs:label>Word generation</rdfs:label>
        <rdfs:subClassOf rdf:resource="&cogat;CAO_00001"/>
        <skos:definition>The cognitive process of producing words on ones own term instead of extracting them from an outside source.  </skos:definition>
        <dc:Contributor>Natalie Picchetti</dc:Contributor>
        <dc:Date>2011-03-01 11:27:36</dc:Date>
        <dc:Title>Word generation</dc:Title>
        <skos:prefLabel>Word generation</skos:prefLabel>
        <skos:altLabel></skos:altLabel>
        <skos:hasTopConcept>Language</skos:hasTopConcept>
        <dc:identifier>trm_4a3fd79d0b55f</dc:identifier>
    </owl:Class>
    


    <!-- http://www.cognitiveatlas.org/ontology/cogat.owl#CAO_00582 -->

    <owl:Class rdf:about="&cogat;CAO_00582">
        <rdfs:label>Word order</rdfs:label>
        <rdfs:subClassOf rdf:resource="&cogat;CAO_00001"/>
        <skos:altLabel></skos:altLabel>
        <skos:hasTopConcept>Language</skos:hasTopConcept>
        <dc:Title>Word order</dc:Title>
        <dc:Contributor>Natalie Picchetti</dc:Contributor>
        <skos:prefLabel>Word order</skos:prefLabel>
        <dc:Date>2011-03-09 10:52:14</dc:Date>
        <dc:identifier>trm_4a3fd79d0b56b</dc:identifier>
        <skos:definition>is the sequence of the syntactic constituents of a language.</skos:definition>
    </owl:Class>
    


    <!-- http://www.cognitiveatlas.org/ontology/cogat.owl#CAO_00583 -->

    <owl:Class rdf:about="&cogat;CAO_00583">
        <rdfs:label>Word production</rdfs:label>
        <rdfs:subClassOf rdf:resource="&cogat;CAO_00001"/>
        <dc:Contributor>Mei-Yen Chen</dc:Contributor>
        <skos:prefLabel>Word production</skos:prefLabel>
        <dc:Title>Word production</dc:Title>
        <dc:Date>2011-08-12 13:56:27</dc:Date>
        <skos:definition>A processing of generating word, such as speaking and spelling.</skos:definition>
        <dc:identifier>trm_4a3fd79d0b578</dc:identifier>
        <skos:altLabel></skos:altLabel>
        <skos:hasTopConcept>Language</skos:hasTopConcept>
    </owl:Class>
    


    <!-- http://www.cognitiveatlas.org/ontology/cogat.owl#CAO_00584 -->

    <owl:Class rdf:about="&cogat;CAO_00584">
        <rdfs:label>Word pronunciation</rdfs:label>
        <rdfs:subClassOf rdf:resource="&cogat;CAO_00001"/>
        <rdfs:subClassOf>
            <owl:Restriction>
                <owl:onProperty rdf:resource="&ro;part_of"/>
                <owl:someValuesFrom rdf:resource="&cogat;CAO_00581"/>
            </owl:Restriction>
        </rdfs:subClassOf>
        <dc:Title>Word pronunciation</dc:Title>
        <skos:prefLabel>Word pronunciation</skos:prefLabel>
        <dc:Date>2011-04-12 12:45:19</dc:Date>
        <skos:hasTopConcept>Language</skos:hasTopConcept>
        <skos:definition>is the act or result of producing the sounds of speech, including articulation, stress, and intonation, often with reference to some standard of correctness or acceptability.</skos:definition>
        <dc:identifier>trm_4a3fd79d0b583</dc:identifier>
        <dc:Contributor>Natalie Picchetti</dc:Contributor>
        <skos:altLabel></skos:altLabel>
    </owl:Class>
    


    <!-- http://www.cognitiveatlas.org/ontology/cogat.owl#CAO_00585 -->

    <owl:Class rdf:about="&cogat;CAO_00585">
        <rdfs:label>Word recognition</rdfs:label>
        <rdfs:subClassOf rdf:resource="&cogat;CAO_00646"/>
        <rdfs:subClassOf>
            <owl:Restriction>
                <owl:onProperty rdf:resource="&ro;part_of"/>
                <owl:someValuesFrom rdf:resource="&cogat;CAO_00479"/>
            </owl:Restriction>
        </rdfs:subClassOf>
        <dc:Date>2011-08-12 13:57:24</dc:Date>
        <skos:prefLabel>Word recognition</skos:prefLabel>
        <dc:Title>Word recognition</dc:Title>
        <skos:hasTopConcept>Language</skos:hasTopConcept>
        <dc:Contributor>Mei-Yen Chen</dc:Contributor>
        <skos:definition>the ability of a reader to recognize written words correctly and virtually effortlessly.</skos:definition>
        <dc:identifier>trm_4a3fd79d0b58f</dc:identifier>
        <skos:altLabel></skos:altLabel>
    </owl:Class>
    


    <!-- http://www.cognitiveatlas.org/ontology/cogat.owl#CAO_00586 -->

    <owl:Class rdf:about="&cogat;CAO_00586">
        <rdfs:label>Word repetition</rdfs:label>
        <rdfs:subClassOf rdf:resource="&cogat;CAO_00001"/>
        <skos:prefLabel>Word repetition</skos:prefLabel>
        <dc:Date>2011-08-12 13:58:32</dc:Date>
        <dc:Contributor>Mei-Yen Chen</dc:Contributor>
        <skos:hasTopConcept>Language</skos:hasTopConcept>
        <skos:definition>is the saying by one individual of the spoken vocalizations(word(s)) made by another individual. This requires the ability in the person making the copy to map the sensory input they hear from the other personand#39;s vocal pronunciation into a similar motor output with their own vocal tract.</skos:definition>
        <skos:altLabel></skos:altLabel>
        <dc:Title>Word repetition</dc:Title>
        <dc:identifier>trm_4a3fd79d0b59b</dc:identifier>
    </owl:Class>
    


    <!-- http://www.cognitiveatlas.org/ontology/cogat.owl#CAO_00587 -->

    <owl:Class rdf:about="&cogat;CAO_00587">
        <rdfs:label>Working memory</rdfs:label>
        <rdfs:subClassOf rdf:resource="&cogat;CAO_00670"/>
        <skos:definition>active maintenance and flexible updating of goal-task relevant information (items, goals, strategies, etc.) in a form that resists interference but has limited capacity. These representations may involve flexible binding of representations, may be characterized by the absence of external support for the internally maintained representations, and are frequently temporary due to ongoing interference </skos:definition>
        <skos:prefLabel>Working memory</skos:prefLabel>
        <skos:hasTopConcept>Executive-Cognitive Control</skos:hasTopConcept>
        <dc:identifier>trm_4a3fd79d0b5a7</dc:identifier>
        <dc:Title>Working memory</dc:Title>
        <skos:altLabel></skos:altLabel>
        <dc:Date>2011-08-09 10:29:18</dc:Date>
        <dc:Contributor>Russ Poldrack</dc:Contributor>
    </owl:Class>
    


    <!-- http://www.cognitiveatlas.org/ontology/cogat.owl#CAO_00588 -->

    <owl:Class rdf:about="&cogat;CAO_00588">
        <rdfs:label>Action initiation</rdfs:label>
        <rdfs:subClassOf rdf:resource="&cogat;CAO_00001"/>
        <dc:Title>Action initiation</dc:Title>
        <skos:altLabel></skos:altLabel>
        <skos:hasTopConcept>Action</skos:hasTopConcept>
        <skos:definition>the facilitation or initiation of an act</skos:definition>
        <dc:Contributor>Russ Poldrack</dc:Contributor>
        <skos:prefLabel>Action initiation</skos:prefLabel>
        <dc:Date>2012-03-28 08:29:57</dc:Date>
        <dc:identifier>trm_4a3fd79d0b5c0</dc:identifier>
    </owl:Class>
    


    <!-- http://www.cognitiveatlas.org/ontology/cogat.owl#CAO_00589 -->

    <owl:Class rdf:about="&cogat;CAO_00589">
        <rdfs:label>Action selection</rdfs:label>
        <rdfs:subClassOf rdf:resource="&cogat;CAO_00253"/>
        <dc:identifier>trm_4a3fd79d0b5cb</dc:identifier>
        <dc:Contributor>Russ Poldrack</dc:Contributor>
        <skos:hasTopConcept>Executive-Cognitive Control</skos:hasTopConcept>
        <skos:prefLabel>Action selection</skos:prefLabel>
        <skos:definition>The selection of one action from a set of possible actions.</skos:definition>
        <skos:altLabel></skos:altLabel>
        <dc:Date>2010-01-10 15:24:38</dc:Date>
        <dc:Title>Action selection</dc:Title>
    </owl:Class>
    


    <!-- http://www.cognitiveatlas.org/ontology/cogat.owl#CAO_00590 -->

    <owl:Class rdf:about="&cogat;CAO_00590">
        <rdfs:label>Attention shift</rdfs:label>
        <rdfs:subClassOf rdf:resource="&cogat;CAO_00001"/>
        <dc:identifier>trm_4a3fd79d0b5d7</dc:identifier>
        <dc:Date>2012-03-28 08:57:29</dc:Date>
        <skos:hasTopConcept>Attention</skos:hasTopConcept>
        <dc:Title>Attention shift</dc:Title>
        <skos:prefLabel>Attention shift</skos:prefLabel>
        <dc:Contributor>Russ Poldrack</dc:Contributor>
        <skos:definition>The change that occurs when information that is currently active in the mind is replaced by other information. The information content is typically sensory in nature.</skos:definition>
        <skos:altLabel></skos:altLabel>
    </owl:Class>
    


    <!-- http://www.cognitiveatlas.org/ontology/cogat.owl#CAO_00591 -->

    <owl:Class rdf:about="&cogat;CAO_00591">
        <rdfs:label>Attention span</rdfs:label>
        <rdfs:subClassOf rdf:resource="&cogat;CAO_00001"/>
        <rdfs:subClassOf>
            <owl:Restriction>
                <owl:onProperty rdf:resource="&ro;part_of"/>
                <owl:someValuesFrom rdf:resource="&cogat;CAO_00144"/>
            </owl:Restriction>
        </rdfs:subClassOf>
        <skos:prefLabel>Attention span</skos:prefLabel>
        <skos:definition>Amount of time or space that an individual can dedicate to particular task or content without becoming distracted.</skos:definition>
        <skos:altLabel></skos:altLabel>
        <skos:hasTopConcept>Attention</skos:hasTopConcept>
        <dc:Date>2009-07-10 14:06:33</dc:Date>
        <dc:identifier>trm_4a3fd79d0b5e3</dc:identifier>
        <dc:Contributor>Agatha Lenartowicz</dc:Contributor>
        <dc:Title>Attention span</dc:Title>
    </owl:Class>
    


    <!-- http://www.cognitiveatlas.org/ontology/cogat.owl#CAO_00592 -->

    <owl:Class rdf:about="&cogat;CAO_00592">
        <rdfs:label>Attentional focusing</rdfs:label>
        <rdfs:subClassOf rdf:resource="&cogat;CAO_00001"/>
        <rdfs:subClassOf>
            <owl:Restriction>
                <owl:onProperty rdf:resource="&ro;part_of"/>
                <owl:someValuesFrom rdf:resource="&cogat;CAO_00144"/>
            </owl:Restriction>
        </rdfs:subClassOf>
        <skos:altLabel></skos:altLabel>
        <dc:Title>Attentional focusing</dc:Title>
        <dc:Contributor>Russ Poldrack</dc:Contributor>
        <dc:Date>2012-03-28 08:58:45</dc:Date>
        <skos:prefLabel>Attentional focusing</skos:prefLabel>
        <dc:identifier>trm_4a3fd79d0b5ef</dc:identifier>
        <skos:definition>The ability to focus attention on cues in the environment that are relevant to the task in hand; can also include suppression of distracting stimuli</skos:definition>
        <skos:hasTopConcept>Attention</skos:hasTopConcept>
    </owl:Class>
    


    <!-- http://www.cognitiveatlas.org/ontology/cogat.owl#CAO_00593 -->

    <owl:Class rdf:about="&cogat;CAO_00593">
        <rdfs:label>Attention shifting</rdfs:label>
        <rdfs:subClassOf rdf:resource="&cogat;CAO_00001"/>
        <skos:definition>The process by which information that is currently relevant in the mind is replaced by other information. This information is typically sensory in nature but may also be semantic.</skos:definition>
        <dc:Contributor>Russ Poldrack</dc:Contributor>
        <dc:Title>Attention shifting</dc:Title>
        <skos:altLabel></skos:altLabel>
        <dc:identifier>trm_4a3fd79d0b5fb</dc:identifier>
        <skos:prefLabel>Attention shifting</skos:prefLabel>
        <skos:hasTopConcept>Attention</skos:hasTopConcept>
        <dc:Date>2012-03-28 08:57:46</dc:Date>
    </owl:Class>
    


    <!-- http://www.cognitiveatlas.org/ontology/cogat.owl#CAO_00594 -->

    <owl:Class rdf:about="&cogat;CAO_00594">
        <rdfs:label>Set shifting</rdfs:label>
        <rdfs:subClassOf rdf:resource="&cogat;CAO_00001"/>
        <dc:identifier>trm_4a3fd79d0b607</dc:identifier>
        <dc:Date>2009-12-21 14:42:51</dc:Date>
        <dc:Contributor>Agatha Lenartowicz</dc:Contributor>
        <skos:prefLabel>Set shifting</skos:prefLabel>
        <skos:altLabel></skos:altLabel>
        <skos:hasTopConcept>Executive-Cognitive Control</skos:hasTopConcept>
        <skos:definition>The process of changing ones behavioral objective.</skos:definition>
        <dc:Title>Set shifting</dc:Title>
    </owl:Class>
    


    <!-- http://www.cognitiveatlas.org/ontology/cogat.owl#CAO_00595 -->

    <owl:Class rdf:about="&cogat;CAO_00595">
        <rdfs:label>Task switching</rdfs:label>
        <rdfs:subClassOf rdf:resource="&cogat;CAO_00673"/>
        <skos:hasTopConcept>Executive-Cognitive Control</skos:hasTopConcept>
        <dc:identifier>trm_4a3fd79d0b613</dc:identifier>
        <skos:prefLabel>Task switching</skos:prefLabel>
        <skos:definition>The process of switching from one task or goal to another, depending on the context or instructions.</skos:definition>
        <dc:Contributor>Glenn Wylie</dc:Contributor>
        <dc:Date>2010-04-23 10:49:18</dc:Date>
        <skos:altLabel></skos:altLabel>
        <dc:Title>Task switching</dc:Title>
    </owl:Class>
    


    <!-- http://www.cognitiveatlas.org/ontology/cogat.owl#CAO_00596 -->

    <owl:Class rdf:about="&cogat;CAO_00596">
        <rdfs:label>Decision</rdfs:label>
        <rdfs:subClassOf rdf:resource="&cogat;CAO_00001"/>
        <skos:definition>The outcome of a process during which a choice is made, usually between several possible options</skos:definition>
        <skos:altLabel></skos:altLabel>
        <dc:Contributor>Tom Schonberg</dc:Contributor>
        <dc:Title>Decision</dc:Title>
        <dc:identifier>trm_4a3fd79d0b61f</dc:identifier>
        <skos:prefLabel>Decision</skos:prefLabel>
        <skos:hasTopConcept>Reasoning and Decision Making</skos:hasTopConcept>
        <dc:Date>2009-07-10 14:06:33</dc:Date>
    </owl:Class>
    


    <!-- http://www.cognitiveatlas.org/ontology/cogat.owl#CAO_00597 -->

    <owl:Class rdf:about="&cogat;CAO_00597">
        <rdfs:label>Framing</rdfs:label>
        <rdfs:subClassOf rdf:resource="&cogat;CAO_00001"/>
        <skos:definition>Framing is a method of biasing opinions- a framing effect occurs when the description of information, such as a speaker presenting an issue, has an emphasis on a subset of potentially relevant considerations and causes individuals to focus on these considerations when constructing their opinions.</skos:definition>
        <skos:altLabel></skos:altLabel>
        <skos:hasTopConcept>Reasoning and Decision Making</skos:hasTopConcept>
        <skos:prefLabel>Framing</skos:prefLabel>
        <dc:Contributor>Naomi Kenner</dc:Contributor>
        <dc:Title>Framing</dc:Title>
        <dc:Date>2009-07-10 14:06:33</dc:Date>
        <dc:identifier>trm_4a3fd79d0b636</dc:identifier>
    </owl:Class>
    


    <!-- http://www.cognitiveatlas.org/ontology/cogat.owl#CAO_00598 -->

    <owl:Class rdf:about="&cogat;CAO_00598">
        <rdfs:label>Risk seeking</rdfs:label>
        <rdfs:subClassOf rdf:resource="&cogat;CAO_00109"/>
        <skos:hasTopConcept>Reasoning and Decision Making</skos:hasTopConcept>
        <skos:altLabel></skos:altLabel>
        <dc:identifier>trm_4a3fd79d0b64e</dc:identifier>
        <dc:Title>Risk seeking</dc:Title>
        <skos:prefLabel>Risk seeking</skos:prefLabel>
        <dc:Contributor>Emily Barkley-Levenson</dc:Contributor>
        <skos:definition>The willingness of an individual to choose an option with a less-than-certain probability of reward over an option with a certain reward of equal or higher expected value. </skos:definition>
        <dc:Date>2009-07-10 14:06:33</dc:Date>
    </owl:Class>
    


    <!-- http://www.cognitiveatlas.org/ontology/cogat.owl#CAO_00599 -->

    <owl:Class rdf:about="&cogat;CAO_00599">
        <rdfs:label>Emotion perception</rdfs:label>
        <rdfs:subClassOf rdf:resource="&cogat;CAO_00001"/>
        <skos:prefLabel>Emotion perception</skos:prefLabel>
        <skos:definition>The process involving understanding feelings with different valences of oneself or of others</skos:definition>
        <dc:Title>Emotion perception</dc:Title>
        <dc:Date>2011-08-14 15:59:25</dc:Date>
        <dc:Contributor>Tyler Davis</dc:Contributor>
        <dc:identifier>trm_4a3fd79d0b65a</dc:identifier>
        <skos:altLabel></skos:altLabel>
        <skos:hasTopConcept>Emotion</skos:hasTopConcept>
    </owl:Class>
    


    <!-- http://www.cognitiveatlas.org/ontology/cogat.owl#CAO_00600 -->

    <owl:Class rdf:about="&cogat;CAO_00600">
        <rdfs:label>Emotion recognition</rdfs:label>
        <rdfs:subClassOf rdf:resource="&cogat;CAO_00001"/>
        <skos:definition>The process of assigning an emotion to one of the discrete categories of emotion available in a particular culture.</skos:definition>
        <dc:identifier>trm_4a3fd79d0b665</dc:identifier>
        <dc:Title>Emotion recognition</dc:Title>
        <skos:prefLabel>Emotion recognition</skos:prefLabel>
        <dc:Date>2012-03-28 10:54:55</dc:Date>
        <skos:hasTopConcept>Emotion</skos:hasTopConcept>
        <dc:Contributor>Russ Poldrack</dc:Contributor>
        <skos:altLabel></skos:altLabel>
    </owl:Class>
    


    <!-- http://www.cognitiveatlas.org/ontology/cogat.owl#CAO_00601 -->

    <owl:Class rdf:about="&cogat;CAO_00601">
        <rdfs:label>Emotional bonding</rdfs:label>
        <rdfs:subClassOf rdf:resource="&cogat;CAO_00001"/>
        <dc:Contributor>Russ Poldrack</dc:Contributor>
        <skos:prefLabel>Emotional bonding</skos:prefLabel>
        <skos:hasTopConcept>Social Function</skos:hasTopConcept>
        <dc:Date>2012-03-28 10:55:11</dc:Date>
        <dc:Title>Emotional bonding</dc:Title>
        <skos:altLabel></skos:altLabel>
        <dc:identifier>trm_4a3fd79d0b671</dc:identifier>
        <skos:definition>A process of bringing people together based on mutually shared emotions. </skos:definition>
    </owl:Class>
    


    <!-- http://www.cognitiveatlas.org/ontology/cogat.owl#CAO_00602 -->

    <owl:Class rdf:about="&cogat;CAO_00602">
        <rdfs:label>Empathy</rdfs:label>
        <rdfs:subClassOf rdf:resource="&cogat;CAO_00001"/>
        <skos:altLabel></skos:altLabel>
        <skos:definition>The act of understanding, being aware of, being sensitive to, and or experiencing the feelings, thoughts, and experience of another. </skos:definition>
        <skos:hasTopConcept>Emotion</skos:hasTopConcept>
        <dc:Contributor>Tyler Davis</dc:Contributor>
        <dc:Title>Empathy</dc:Title>
        <dc:Date>2011-08-14 16:10:33</dc:Date>
        <dc:identifier>trm_4a3fd79d0b67d</dc:identifier>
        <skos:prefLabel>Empathy</skos:prefLabel>
    </owl:Class>
    


    <!-- http://www.cognitiveatlas.org/ontology/cogat.owl#CAO_00603 -->

    <owl:Class rdf:about="&cogat;CAO_00603">
        <rdfs:label>Fear</rdfs:label>
        <rdfs:subClassOf rdf:resource="&cogat;CAO_00001"/>
        <dc:identifier>trm_4a3fd79d0b689</dc:identifier>
        <skos:hasTopConcept>Emotion</skos:hasTopConcept>
        <dc:Date>2012-03-28 11:57:19</dc:Date>
        <skos:altLabel></skos:altLabel>
        <dc:Contributor>Russ Poldrack</dc:Contributor>
        <skos:definition>A state of high negative emotional arousal triggered by an impending threat (real or imaginary) and generally associated with the flight or fight response.</skos:definition>
        <dc:Title>Fear</dc:Title>
        <skos:prefLabel>Fear</skos:prefLabel>
    </owl:Class>
    


    <!-- http://www.cognitiveatlas.org/ontology/cogat.owl#CAO_00604 -->

    <owl:Class rdf:about="&cogat;CAO_00604">
        <rdfs:label>Frustration</rdfs:label>
        <rdfs:subClassOf rdf:resource="&cogat;CAO_00001"/>
        <dc:Contributor>Russ Poldrack</dc:Contributor>
        <skos:altLabel></skos:altLabel>
        <skos:hasTopConcept>Emotion</skos:hasTopConcept>
        <dc:identifier>trm_4a3fd79d0b695</dc:identifier>
        <dc:Date>2012-03-28 12:00:18</dc:Date>
        <skos:prefLabel>Frustration</skos:prefLabel>
        <dc:Title>Frustration</dc:Title>
        <skos:definition>a deep chronic sense or state of insecurity and dissatisfaction arising from unresolved problems or unfulfilled needs.</skos:definition>
    </owl:Class>
    


    <!-- http://www.cognitiveatlas.org/ontology/cogat.owl#CAO_00605 -->

    <owl:Class rdf:about="&cogat;CAO_00605">
        <rdfs:label>Grief</rdfs:label>
        <rdfs:subClassOf rdf:resource="&cogat;CAO_00001"/>
        <dc:identifier>trm_4a3fd79d0b6a1</dc:identifier>
        <dc:Title>Grief</dc:Title>
        <dc:Contributor>Brenda Gregory</dc:Contributor>
        <skos:prefLabel>Grief</skos:prefLabel>
        <skos:definition>deep and poignant distress caused by or as if by bereavement.</skos:definition>
        <dc:Date>2011-05-11 16:20:10</dc:Date>
        <skos:altLabel></skos:altLabel>
        <skos:hasTopConcept>Emotion</skos:hasTopConcept>
    </owl:Class>
    


    <!-- http://www.cognitiveatlas.org/ontology/cogat.owl#CAO_00606 -->

    <owl:Class rdf:about="&cogat;CAO_00606">
        <rdfs:label>Happiness</rdfs:label>
        <rdfs:subClassOf rdf:resource="&cogat;CAO_00001"/>
        <skos:hasTopConcept>Emotion</skos:hasTopConcept>
        <skos:prefLabel>Happiness</skos:prefLabel>
        <dc:identifier>trm_4a3fd79d0b6ad</dc:identifier>
        <skos:definition>a state of mind or feeling characterized by contentment, love, satisfaction, pleasure, or joy.</skos:definition>
        <skos:altLabel></skos:altLabel>
        <dc:Title>Happiness</dc:Title>
        <dc:Contributor>Russ Poldrack</dc:Contributor>
        <dc:Date>2012-03-28 12:51:32</dc:Date>
    </owl:Class>
    


    <!-- http://www.cognitiveatlas.org/ontology/cogat.owl#CAO_00607 -->

    <owl:Class rdf:about="&cogat;CAO_00607">
        <rdfs:label>Comprehension</rdfs:label>
        <rdfs:subClassOf rdf:resource="&cogat;CAO_00001"/>
        <dc:Title>Comprehension</dc:Title>
        <skos:prefLabel>Comprehension</skos:prefLabel>
        <skos:hasTopConcept>Language</skos:hasTopConcept>
        <dc:Contributor>Russ Poldrack</dc:Contributor>
        <skos:definition>the act or capacity of understanding linguistic information</skos:definition>
        <dc:Date>2012-03-28 09:39:56</dc:Date>
        <dc:identifier>trm_4a3fd79d0b6b9</dc:identifier>
        <skos:altLabel></skos:altLabel>
    </owl:Class>
    


    <!-- http://www.cognitiveatlas.org/ontology/cogat.owl#CAO_00608 -->

    <owl:Class rdf:about="&cogat;CAO_00608">
        <rdfs:label>Discourse</rdfs:label>
        <rdfs:subClassOf rdf:resource="&cogat;CAO_00001"/>
        <skos:hasTopConcept>Language</skos:hasTopConcept>
        <skos:definition>the capacity of orderly thought or procedure, verbal interchange of ideas; formal and orderly and usually extended expression of thought on a subject, connected speech or writing, linguistic unit larger than a sentence.</skos:definition>
        <dc:Title>Discourse</dc:Title>
        <dc:identifier>trm_4a3fd79d0b6c5</dc:identifier>
        <dc:Contributor>Russ Poldrack</dc:Contributor>
        <skos:prefLabel>Discourse</skos:prefLabel>
        <dc:Date>2012-03-28 09:49:41</dc:Date>
        <skos:altLabel></skos:altLabel>
    </owl:Class>
    


    <!-- http://www.cognitiveatlas.org/ontology/cogat.owl#CAO_00609 -->

    <owl:Class rdf:about="&cogat;CAO_00609">
        <rdfs:label>Discourse comprehension</rdfs:label>
        <rdfs:subClassOf rdf:resource="&cogat;CAO_00607"/>
        <dc:Contributor>Russ Poldrack</dc:Contributor>
        <skos:altLabel></skos:altLabel>
        <dc:identifier>trm_4a3fd79d0b6d1</dc:identifier>
        <skos:definition>Discourse comprehension is the act of interpreting a written or spoken message by integrating the incoming information into the memory or knowledge structures of the interpreter.</skos:definition>
        <dc:Date>2012-03-28 09:49:51</dc:Date>
        <dc:Title>Discourse comprehension</dc:Title>
        <skos:hasTopConcept>Language</skos:hasTopConcept>
        <skos:prefLabel>Discourse comprehension</skos:prefLabel>
    </owl:Class>
    


    <!-- http://www.cognitiveatlas.org/ontology/cogat.owl#CAO_00610 -->

    <owl:Class rdf:about="&cogat;CAO_00610">
        <rdfs:label>Discourse knowledge</rdfs:label>
        <rdfs:subClassOf rdf:resource="&cogat;CAO_00371"/>
        <skos:hasTopConcept>Language</skos:hasTopConcept>
        <dc:Date>2012-03-28 09:50:22</dc:Date>
        <dc:Contributor>Russ Poldrack</dc:Contributor>
        <skos:altLabel></skos:altLabel>
        <dc:identifier>trm_4a3fd79d0b6dd</dc:identifier>
        <skos:definition>knowledge regarding discourse </skos:definition>
        <dc:Title>Discourse knowledge</dc:Title>
        <skos:prefLabel>Discourse knowledge</skos:prefLabel>
    </owl:Class>
    


    <!-- http://www.cognitiveatlas.org/ontology/cogat.owl#CAO_00611 -->

    <owl:Class rdf:about="&cogat;CAO_00611">
        <rdfs:label>Discourse planning</rdfs:label>
        <rdfs:subClassOf rdf:resource="&cogat;CAO_00452"/>
        <skos:definition>the formulation of structures, patterns, mental representations, and processes that constitute the written and spoken unit of connected speech or writing longer than a sentence. </skos:definition>
        <dc:Date>2011-04-07 11:16:27</dc:Date>
        <skos:prefLabel>Discourse planning</skos:prefLabel>
        <skos:altLabel></skos:altLabel>
        <dc:Title>Discourse planning</dc:Title>
        <skos:hasTopConcept>Language</skos:hasTopConcept>
        <dc:identifier>trm_4a3fd79d0b6e9</dc:identifier>
        <dc:Contributor>Natalie Picchetti</dc:Contributor>
    </owl:Class>
    


    <!-- http://www.cognitiveatlas.org/ontology/cogat.owl#CAO_00612 -->

    <owl:Class rdf:about="&cogat;CAO_00612">
        <rdfs:label>Discourse processing</rdfs:label>
        <rdfs:subClassOf rdf:resource="&cogat;CAO_00001"/>
        <dc:identifier>trm_4a3fd79d0b6f5</dc:identifier>
        <skos:altLabel></skos:altLabel>
        <dc:Date>2011-04-07 11:30:15</dc:Date>
        <skos:prefLabel>Discourse processing</skos:prefLabel>
        <dc:Contributor>Natalie Picchetti</dc:Contributor>
        <dc:Title>Discourse processing</dc:Title>
        <skos:hasTopConcept>Language</skos:hasTopConcept>
        <skos:definition>is the cognitive process that investigates the structures, patterns, mental representations, and processes that underlie the written and spoken unit of connected speech or writing longer than a sentence.  </skos:definition>
    </owl:Class>
    


    <!-- http://www.cognitiveatlas.org/ontology/cogat.owl#CAO_00613 -->

    <owl:Class rdf:about="&cogat;CAO_00613">
        <rdfs:label>Discourse production</rdfs:label>
        <rdfs:subClassOf rdf:resource="&cogat;CAO_00001"/>
        <dc:Contributor>Natalie Picchetti</dc:Contributor>
        <dc:identifier>trm_4a3fd79d0b701</dc:identifier>
        <skos:definition>the formation of a spoken unit of connected speech or writing longer than a sentence. </skos:definition>
        <dc:Date>2011-04-07 11:18:02</dc:Date>
        <skos:altLabel></skos:altLabel>
        <skos:hasTopConcept>Language</skos:hasTopConcept>
        <skos:prefLabel>Discourse production</skos:prefLabel>
        <dc:Title>Discourse production</dc:Title>
    </owl:Class>
    


    <!-- http://www.cognitiveatlas.org/ontology/cogat.owl#CAO_00614 -->

    <owl:Class rdf:about="&cogat;CAO_00614">
        <rdfs:label>Grammatical encoding</rdfs:label>
        <rdfs:subClassOf rdf:resource="&cogat;CAO_00001"/>
        <skos:prefLabel>Grammatical encoding</skos:prefLabel>
        <skos:definition>the selection of semantically appropriate lexical items and the generation of a syntactic frame or surface form.  </skos:definition>
        <skos:hasTopConcept>Language</skos:hasTopConcept>
        <dc:identifier>trm_4a3fd79d0b756</dc:identifier>
        <skos:altLabel></skos:altLabel>
        <dc:Date>2011-04-11 14:23:28</dc:Date>
        <dc:Contributor>Natalie Picchetti</dc:Contributor>
        <dc:Title>Grammatical encoding</dc:Title>
    </owl:Class>
    


    <!-- http://www.cognitiveatlas.org/ontology/cogat.owl#CAO_00615 -->

    <owl:Class rdf:about="&cogat;CAO_00615">
        <rdfs:label>Grapheme</rdfs:label>
        <rdfs:subClassOf rdf:resource="&cogat;CAO_00001"/>
        <dc:Date>2012-03-28 12:01:59</dc:Date>
        <skos:hasTopConcept>Language</skos:hasTopConcept>
        <dc:Title>Grapheme</dc:Title>
        <dc:identifier>trm_4a3fd79d0b76e</dc:identifier>
        <skos:altLabel></skos:altLabel>
        <skos:definition>a unit (as a letter or digraph) of a writing system; the set of units of a writing system (as letters and letter combinations) that represent a phoneme.</skos:definition>
        <skos:prefLabel>Grapheme</skos:prefLabel>
        <dc:Contributor>Russ Poldrack</dc:Contributor>
    </owl:Class>
    


    <!-- http://www.cognitiveatlas.org/ontology/cogat.owl#CAO_00616 -->

    <owl:Class rdf:about="&cogat;CAO_00616">
        <rdfs:label>Graphemic buffer</rdfs:label>
        <rdfs:subClassOf rdf:resource="&cogat;CAO_00001"/>
        <skos:definition>a component dedicated to the temporary storage of abstract orthographic representations prior to their format-specific expression in spelling and-or reading.</skos:definition>
        <skos:hasTopConcept>Language</skos:hasTopConcept>
        <skos:prefLabel>Graphemic buffer</skos:prefLabel>
        <dc:Contributor>Russ Poldrack</dc:Contributor>
        <skos:altLabel></skos:altLabel>
        <dc:Title>Graphemic buffer</dc:Title>
        <dc:Date>2012-03-28 12:02:09</dc:Date>
        <dc:identifier>trm_4a3fd79d0b779</dc:identifier>
    </owl:Class>
    


    <!-- http://www.cognitiveatlas.org/ontology/cogat.owl#CAO_00617 -->

    <owl:Class rdf:about="&cogat;CAO_00617">
        <rdfs:label>Illocutionary force</rdfs:label>
        <rdfs:subClassOf rdf:resource="&cogat;CAO_00001"/>
        <dc:Title>Illocutionary force</dc:Title>
        <dc:identifier>trm_4a3fd79d0b7b5</dc:identifier>
        <skos:prefLabel>Illocutionary force</skos:prefLabel>
        <dc:Date>2012-03-28 14:30:10</dc:Date>
        <dc:Contributor>Russ Poldrack</dc:Contributor>
        <skos:altLabel></skos:altLabel>
        <skos:definition>a speakerand#39;s intention in delivering an utterance.</skos:definition>
        <skos:hasTopConcept>Language</skos:hasTopConcept>
    </owl:Class>
    


    <!-- http://www.cognitiveatlas.org/ontology/cogat.owl#CAO_00618 -->

    <owl:Class rdf:about="&cogat;CAO_00618">
        <rdfs:label>Language acquisition</rdfs:label>
        <rdfs:subClassOf rdf:resource="&cogat;CAO_00001"/>
        <skos:definition>the process by which humans acquire the capacity to perceive, produce and use words to understand and communicate.</skos:definition>
        <dc:identifier>trm_4a3fd79d0b7f4</dc:identifier>
        <dc:Title>Language acquisition</dc:Title>
        <skos:prefLabel>Language acquisition</skos:prefLabel>
        <dc:Contributor>Brenda Gregory</dc:Contributor>
        <skos:altLabel></skos:altLabel>
        <skos:hasTopConcept>Language</skos:hasTopConcept>
        <dc:Date>2011-04-19 13:50:53</dc:Date>
    </owl:Class>
    


    <!-- http://www.cognitiveatlas.org/ontology/cogat.owl#CAO_00619 -->

    <owl:Class rdf:about="&cogat;CAO_00619">
        <rdfs:label>Language processing</rdfs:label>
        <rdfs:subClassOf rdf:resource="&cogat;CAO_00001"/>
        <skos:hasTopConcept>Language</skos:hasTopConcept>
        <skos:altLabel></skos:altLabel>
        <dc:Date>2011-05-18 09:52:02</dc:Date>
        <dc:identifier>trm_4a3fd79d0b802</dc:identifier>
        <skos:prefLabel>Language processing</skos:prefLabel>
        <dc:Title>Language processing</dc:Title>
        <skos:definition>the way human beings process speech or writing and understand it as language.</skos:definition>
        <dc:Contributor>Brenda Gregory</dc:Contributor>
    </owl:Class>
    


    <!-- http://www.cognitiveatlas.org/ontology/cogat.owl#CAO_00620 -->

    <owl:Class rdf:about="&cogat;CAO_00620">
        <rdfs:label>Lexical access</rdfs:label>
        <rdfs:subClassOf rdf:resource="&cogat;CAO_00001"/>
        <skos:prefLabel>Lexical access</skos:prefLabel>
        <skos:hasTopConcept>Language</skos:hasTopConcept>
        <dc:Contributor>Brenda Gregory</dc:Contributor>
        <dc:Date>2011-04-19 12:19:05</dc:Date>
        <skos:definition>the process by which contact is made with the lexicon on the basis of an initial acoustic-phonetic or phonological representation of some portion of the speech input, the result of lexical success is a cohort of potential word candidates which are compatible with this initial analysis.</skos:definition>
        <dc:Title>Lexical access</dc:Title>
        <dc:identifier>trm_4a3fd79d0b80f</dc:identifier>
        <skos:altLabel></skos:altLabel>
    </owl:Class>
    


    <!-- http://www.cognitiveatlas.org/ontology/cogat.owl#CAO_00621 -->

    <owl:Class rdf:about="&cogat;CAO_00621">
        <rdfs:label>Lexical ambiguity</rdfs:label>
        <rdfs:subClassOf rdf:resource="&cogat;CAO_00001"/>
        <dc:Contributor>Brenda Gregory</dc:Contributor>
        <dc:Date>2011-05-16 11:10:04</dc:Date>
        <dc:Title>Lexical ambiguity</dc:Title>
        <skos:prefLabel>Lexical ambiguity</skos:prefLabel>
        <skos:altLabel></skos:altLabel>
        <dc:identifier>trm_4a3fd79d0b81b</dc:identifier>
        <skos:hasTopConcept>Language</skos:hasTopConcept>
        <skos:definition>the presence of two or more possible meanings within a single word.</skos:definition>
    </owl:Class>
    


    <!-- http://www.cognitiveatlas.org/ontology/cogat.owl#CAO_00622 -->

    <owl:Class rdf:about="&cogat;CAO_00622">
        <rdfs:label>Lexical processing</rdfs:label>
        <rdfs:subClassOf rdf:resource="&cogat;CAO_00001"/>
        <dc:Title>Lexical processing</dc:Title>
        <skos:prefLabel>Lexical processing</skos:prefLabel>
        <skos:altLabel></skos:altLabel>
        <dc:identifier>trm_4a3fd79d0b826</dc:identifier>
        <dc:Contributor>Russ Poldrack</dc:Contributor>
        <skos:definition>A general term referring to the processing of single words, typically in the context of visual or auditory word recognition.</skos:definition>
        <dc:Date>2012-03-28 17:15:43</dc:Date>
        <skos:hasTopConcept>Language</skos:hasTopConcept>
    </owl:Class>
    


    <!-- http://www.cognitiveatlas.org/ontology/cogat.owl#CAO_00623 -->

    <owl:Class rdf:about="&cogat;CAO_00623">
        <rdfs:label>Morphological processing</rdfs:label>
        <rdfs:subClassOf rdf:resource="&cogat;CAO_00001"/>
        <dc:Contributor>Natalie Picchetti</dc:Contributor>
        <skos:prefLabel>Morphological processing</skos:prefLabel>
        <skos:altLabel></skos:altLabel>
        <skos:hasTopConcept>Language</skos:hasTopConcept>
        <skos:definition>is how the brain registers the patterns of word formation in a particular language, including inflection, derivation, and composition. </skos:definition>
        <dc:Date>2011-04-12 11:56:07</dc:Date>
        <dc:identifier>trm_4a3fd79d0b832</dc:identifier>
        <dc:Title>Morphological processing</dc:Title>
    </owl:Class>
    


    <!-- http://www.cognitiveatlas.org/ontology/cogat.owl#CAO_00624 -->

    <owl:Class rdf:about="&cogat;CAO_00624">
        <rdfs:label>Morphology</rdfs:label>
        <rdfs:subClassOf rdf:resource="&cogat;CAO_00001"/>
        <skos:altLabel></skos:altLabel>
        <skos:prefLabel>Morphology</skos:prefLabel>
        <dc:Contributor>Russ Poldrack</dc:Contributor>
        <dc:Date>2012-03-28 17:37:07</dc:Date>
        <dc:Title>Morphology</dc:Title>
        <dc:identifier>trm_4a3fd79d0b83e</dc:identifier>
        <skos:hasTopConcept>Language</skos:hasTopConcept>
        <skos:definition>the structure and content of word forms</skos:definition>
    </owl:Class>
    


    <!-- http://www.cognitiveatlas.org/ontology/cogat.owl#CAO_00625 -->

    <owl:Class rdf:about="&cogat;CAO_00625">
        <rdfs:label>Orthography</rdfs:label>
        <rdfs:subClassOf rdf:resource="&cogat;CAO_00001"/>
        <dc:Date>2012-03-28 17:53:27</dc:Date>
        <skos:hasTopConcept>Language</skos:hasTopConcept>
        <skos:prefLabel>Orthography</skos:prefLabel>
        <dc:Title>Orthography</dc:Title>
        <skos:altLabel></skos:altLabel>
        <dc:Contributor>Russ Poldrack</dc:Contributor>
        <dc:identifier>trm_4a3fd79d0b84a</dc:identifier>
        <skos:definition>the representation of the sounds of a language by written or printed symbols; a part of language study that deals with letters and spelling. </skos:definition>
    </owl:Class>
    


    <!-- http://www.cognitiveatlas.org/ontology/cogat.owl#CAO_00626 -->

    <owl:Class rdf:about="&cogat;CAO_00626">
        <rdfs:label>Phonetics</rdfs:label>
        <rdfs:subClassOf rdf:resource="&cogat;CAO_00001"/>
        <skos:prefLabel>Phonetics</skos:prefLabel>
        <dc:Title>Phonetics</dc:Title>
        <skos:altLabel></skos:altLabel>
        <skos:hasTopConcept>Language</skos:hasTopConcept>
        <dc:Date>2011-04-28 17:22:02</dc:Date>
        <dc:identifier>trm_4a3fd79d0b862</dc:identifier>
        <dc:Contributor>Brenda Gregory</dc:Contributor>
        <skos:definition>the system of speech sounds of a language or group of languages; the study and systematic classification of the sounds made in spoken utterance.</skos:definition>
    </owl:Class>
    


    <!-- http://www.cognitiveatlas.org/ontology/cogat.owl#CAO_00627 -->

    <owl:Class rdf:about="&cogat;CAO_00627">
        <rdfs:label>Semantic processing</rdfs:label>
        <rdfs:subClassOf rdf:resource="&cogat;CAO_00001"/>
        <skos:hasTopConcept>Language</skos:hasTopConcept>
        <dc:Contributor>Russ Poldrack</dc:Contributor>
        <dc:Date>2012-03-28 18:32:48</dc:Date>
        <dc:Title>Semantic processing</dc:Title>
        <skos:definition>refers to the cognitive processing of the meanings of a stimulus </skos:definition>
        <skos:prefLabel>Semantic processing</skos:prefLabel>
        <dc:identifier>trm_4a3fd79d0b87a</dc:identifier>
        <skos:altLabel></skos:altLabel>
    </owl:Class>
    


    <!-- http://www.cognitiveatlas.org/ontology/cogat.owl#CAO_00628 -->

    <owl:Class rdf:about="&cogat;CAO_00628">
        <rdfs:label>Sentence comprehension</rdfs:label>
        <rdfs:subClassOf rdf:resource="&cogat;CAO_00607"/>
        <rdfs:subClassOf>
            <owl:Restriction>
                <owl:onProperty rdf:resource="&ro;part_of"/>
                <owl:someValuesFrom rdf:resource="&cogat;CAO_00372"/>
            </owl:Restriction>
        </rdfs:subClassOf>
        <dc:Contributor>Natalie Picchetti</dc:Contributor>
        <skos:prefLabel>Sentence comprehension</skos:prefLabel>
        <dc:Title>Sentence comprehension</dc:Title>
        <skos:definition>takes place whenever a reader or listener processes a language utterance, either in isolation or in the context of a conversation or a text.</skos:definition>
        <skos:altLabel></skos:altLabel>
        <dc:identifier>trm_4a3fd79d0b892</dc:identifier>
        <dc:Date>2011-04-12 11:54:01</dc:Date>
        <skos:hasTopConcept>Language</skos:hasTopConcept>
    </owl:Class>
    


    <!-- http://www.cognitiveatlas.org/ontology/cogat.owl#CAO_00629 -->

    <owl:Class rdf:about="&cogat;CAO_00629">
        <rdfs:label>Sentence processing</rdfs:label>
        <rdfs:subClassOf rdf:resource="&cogat;CAO_00001"/>
        <dc:identifier>trm_4a3fd79d0b89e</dc:identifier>
        <skos:hasTopConcept>Language</skos:hasTopConcept>
        <skos:prefLabel>Sentence processing</skos:prefLabel>
        <dc:Contributor>Natalie Picchetti</dc:Contributor>
        <dc:Title>Sentence processing</dc:Title>
        <skos:definition>takes place whenever a reader or listener cognitively processes a language utterance, either in isolation or in the context of a conversation or a text. </skos:definition>
        <skos:altLabel></skos:altLabel>
        <dc:Date>2011-04-11 15:23:00</dc:Date>
    </owl:Class>
    


    <!-- http://www.cognitiveatlas.org/ontology/cogat.owl#CAO_00630 -->

    <owl:Class rdf:about="&cogat;CAO_00630">
        <rdfs:label>Sentence production</rdfs:label>
        <rdfs:subClassOf rdf:resource="&cogat;CAO_00001"/>
        <dc:Contributor>Russ Poldrack</dc:Contributor>
        <skos:altLabel></skos:altLabel>
        <skos:hasTopConcept>Language</skos:hasTopConcept>
        <dc:Date>2012-03-28 18:35:22</dc:Date>
        <skos:prefLabel>Sentence production</skos:prefLabel>
        <dc:Title>Sentence production</dc:Title>
        <skos:definition>The creation and-or utterance of a sentence</skos:definition>
        <dc:identifier>trm_4a3fd79d0b8aa</dc:identifier>
    </owl:Class>
    


    <!-- http://www.cognitiveatlas.org/ontology/cogat.owl#CAO_00631 -->

    <owl:Class rdf:about="&cogat;CAO_00631">
        <rdfs:label>Active recall</rdfs:label>
        <rdfs:subClassOf rdf:resource="&cogat;CAO_00001"/>
        <skos:prefLabel>Active recall</skos:prefLabel>
        <dc:Contributor>Brenda Gregory</dc:Contributor>
        <skos:definition>a principle of efficient learning, which claims the need to actively stimulate memory during the learning process.</skos:definition>
        <dc:identifier>trm_4a3fd79d0b8b5</dc:identifier>
        <dc:Title>Active recall</dc:Title>
        <skos:hasTopConcept>Learning and Memory</skos:hasTopConcept>
        <dc:Date>2011-05-16 15:03:14</dc:Date>
        <skos:altLabel></skos:altLabel>
    </owl:Class>
    


    <!-- http://www.cognitiveatlas.org/ontology/cogat.owl#CAO_00632 -->

    <owl:Class rdf:about="&cogat;CAO_00632">
        <rdfs:label>Active retrieval</rdfs:label>
        <rdfs:subClassOf rdf:resource="&cogat;CAO_00001"/>
        <rdfs:subClassOf>
            <owl:Restriction>
                <owl:onProperty rdf:resource="&ro;part_of"/>
                <owl:someValuesFrom rdf:resource="&cogat;CAO_00296"/>
            </owl:Restriction>
        </rdfs:subClassOf>
        <dc:Contributor>Corey White</dc:Contributor>
        <skos:hasTopConcept>Learning and Memory</skos:hasTopConcept>
        <dc:identifier>trm_4a3fd79d0b8c1</dc:identifier>
        <dc:Date>2011-08-11 08:29:15</dc:Date>
        <skos:definition>Effortful (volitional) attempt to consciously recollect a memory; often required when retrieval cannot be automatically driven by stimuli. </skos:definition>
        <dc:Title>Active retrieval</dc:Title>
        <skos:prefLabel>Active retrieval</skos:prefLabel>
        <skos:altLabel></skos:altLabel>
    </owl:Class>
    


    <!-- http://www.cognitiveatlas.org/ontology/cogat.owl#CAO_00633 -->

    <owl:Class rdf:about="&cogat;CAO_00633">
        <rdfs:label>Consolidation</rdfs:label>
        <rdfs:subClassOf rdf:resource="&cogat;CAO_00001"/>
        <rdfs:subClassOf>
            <owl:Restriction>
                <owl:onProperty rdf:resource="&ro;part_of"/>
                <owl:someValuesFrom rdf:resource="&cogat;CAO_00647"/>
            </owl:Restriction>
        </rdfs:subClassOf>
        <skos:prefLabel>Consolidation</skos:prefLabel>
        <dc:identifier>trm_4a3fd79d0b8cd</dc:identifier>
        <dc:Title>Consolidation</dc:Title>
        <dc:Contributor>Russ Poldrack</dc:Contributor>
        <skos:definition>the process by which a representation becomes stabilized</skos:definition>
        <skos:hasTopConcept></skos:hasTopConcept>
        <skos:altLabel></skos:altLabel>
        <dc:Date>2012-03-28 17:33:36</dc:Date>
    </owl:Class>
    


    <!-- http://www.cognitiveatlas.org/ontology/cogat.owl#CAO_00634 -->

    <owl:Class rdf:about="&cogat;CAO_00634">
        <rdfs:label>Elaborative rehearsal</rdfs:label>
        <rdfs:subClassOf rdf:resource="&cogat;CAO_00001"/>
        <skos:prefLabel>Elaborative rehearsal</skos:prefLabel>
        <skos:definition>a type of rehearsal proposed by Craik and Lockhart (1972) in their Levels of Processing model of memory. Elaborative rehearsal involves deep semantic processing of a to-be-remembered item resulting in the production of durable memories.</skos:definition>
        <dc:Contributor>Brenda Gregory</dc:Contributor>
        <skos:hasTopConcept>Learning and Memory</skos:hasTopConcept>
        <dc:identifier>trm_4a3fd79d0b8d9</dc:identifier>
        <dc:Date>2011-05-03 13:53:58</dc:Date>
        <skos:altLabel></skos:altLabel>
        <dc:Title>Elaborative rehearsal</dc:Title>
    </owl:Class>
    


    <!-- http://www.cognitiveatlas.org/ontology/cogat.owl#CAO_00635 -->

    <owl:Class rdf:about="&cogat;CAO_00635">
        <rdfs:label>Encoding</rdfs:label>
        <rdfs:subClassOf rdf:resource="&cogat;CAO_00001"/>
        <skos:altLabel></skos:altLabel>
        <dc:Date>2011-08-14 16:11:23</dc:Date>
        <skos:prefLabel>Encoding</skos:prefLabel>
        <dc:Title>Encoding</dc:Title>
        <dc:Contributor>Tyler Davis</dc:Contributor>
        <skos:hasTopConcept>Learning and Memory</skos:hasTopConcept>
        <dc:identifier>trm_4a3fd79d0b8e5</dc:identifier>
        <skos:definition>The process of creating a new memory trace.</skos:definition>
    </owl:Class>
    


    <!-- http://www.cognitiveatlas.org/ontology/cogat.owl#CAO_00636 -->

    <owl:Class rdf:about="&cogat;CAO_00636">
        <rdfs:label>Episodic buffer</rdfs:label>
        <rdfs:subClassOf rdf:resource="&cogat;CAO_00001"/>
        <dc:Date>2012-03-28 10:58:37</dc:Date>
        <dc:Title>Episodic buffer</dc:Title>
        <skos:prefLabel>Episodic buffer</skos:prefLabel>
        <skos:altLabel></skos:altLabel>
        <skos:hasTopConcept>Learning and Memory</skos:hasTopConcept>
        <dc:identifier>trm_4a3fd79d0b8f0</dc:identifier>
        <dc:Contributor>Russ Poldrack</dc:Contributor>
        <skos:definition>A theoretical construct that is part of Alan Baddeleyand#39;s working memory model and the object of which is to integrate information across sensory domains and communicate with long term memory in the service of working memory. </skos:definition>
    </owl:Class>
    


    <!-- http://www.cognitiveatlas.org/ontology/cogat.owl#CAO_00637 -->

    <owl:Class rdf:about="&cogat;CAO_00637">
        <rdfs:label>Familiarity</rdfs:label>
        <rdfs:subClassOf rdf:resource="&cogat;CAO_00001"/>
        <skos:definition>A quality of memory that is associated with a feeling of knowing that an event has previously occurred, but often not including enough contextual or episodic details sufficient for claiming actual remembering of the event.</skos:definition>
        <dc:identifier>trm_4a3fd79d0b8fc</dc:identifier>
        <dc:Contributor>Tyler Davis</dc:Contributor>
        <skos:prefLabel>Familiarity</skos:prefLabel>
        <skos:altLabel></skos:altLabel>
        <dc:Date>2011-08-14 16:54:36</dc:Date>
        <dc:Title>Familiarity</dc:Title>
        <skos:hasTopConcept>Learning and Memory</skos:hasTopConcept>
    </owl:Class>
    


    <!-- http://www.cognitiveatlas.org/ontology/cogat.owl#CAO_00638 -->

    <owl:Class rdf:about="&cogat;CAO_00638">
        <rdfs:label>Forgetting</rdfs:label>
        <rdfs:subClassOf rdf:resource="&cogat;CAO_00001"/>
        <dc:Date>2012-03-28 11:59:56</dc:Date>
        <dc:identifier>trm_4a3fd79d0b908</dc:identifier>
        <skos:altLabel></skos:altLabel>
        <skos:definition>The loss of or inability to retrieve a memory.</skos:definition>
        <skos:prefLabel>Forgetting</skos:prefLabel>
        <skos:hasTopConcept>Learning and Memory</skos:hasTopConcept>
        <dc:Contributor>Russ Poldrack</dc:Contributor>
        <dc:Title>Forgetting</dc:Title>
    </owl:Class>
    


    <!-- http://www.cognitiveatlas.org/ontology/cogat.owl#CAO_00639 -->

    <owl:Class rdf:about="&cogat;CAO_00639">
        <rdfs:label>Memory acquisition</rdfs:label>
        <rdfs:subClassOf rdf:resource="&cogat;CAO_00001"/>
        <skos:altLabel></skos:altLabel>
        <skos:definition>is the process of storage and retrieval of new information in memory. </skos:definition>
        <dc:Contributor>Natalie Picchetti</dc:Contributor>
        <dc:identifier>trm_4a3fd79d0b914</dc:identifier>
        <dc:Date>2011-04-12 11:13:11</dc:Date>
        <skos:prefLabel>Memory acquisition</skos:prefLabel>
        <skos:hasTopConcept>Learning and Memory</skos:hasTopConcept>
        <dc:Title>Memory acquisition</dc:Title>
    </owl:Class>
    


    <!-- http://www.cognitiveatlas.org/ontology/cogat.owl#CAO_00640 -->

    <owl:Class rdf:about="&cogat;CAO_00640">
        <rdfs:label>Memory consolidation</rdfs:label>
        <rdfs:subClassOf rdf:resource="&cogat;CAO_00633"/>
        <dc:Title>Memory consolidation</dc:Title>
        <dc:Contributor>Russ Poldrack</dc:Contributor>
        <skos:prefLabel>Memory consolidation</skos:prefLabel>
        <skos:definition>a category of processes that stabilize a memory trace after the initial acquisition. </skos:definition>
        <skos:hasTopConcept></skos:hasTopConcept>
        <skos:altLabel></skos:altLabel>
        <dc:identifier>trm_4a3fd79d0b920</dc:identifier>
        <dc:Date>2012-03-28 17:34:05</dc:Date>
    </owl:Class>
    


    <!-- http://www.cognitiveatlas.org/ontology/cogat.owl#CAO_00641 -->

    <owl:Class rdf:about="&cogat;CAO_00641">
        <rdfs:label>Memory decay</rdfs:label>
        <rdfs:subClassOf rdf:resource="&cogat;CAO_00001"/>
        <skos:altLabel></skos:altLabel>
        <dc:Title>Memory decay</dc:Title>
        <dc:Contributor>Brenda Gregory</dc:Contributor>
        <dc:identifier>trm_4a3fd79d0b92c</dc:identifier>
        <skos:definition>the loss of memory over time.</skos:definition>
        <skos:hasTopConcept></skos:hasTopConcept>
        <dc:Date>2011-05-17 09:57:43</dc:Date>
        <skos:prefLabel>Memory decay</skos:prefLabel>
    </owl:Class>
    


    <!-- http://www.cognitiveatlas.org/ontology/cogat.owl#CAO_00642 -->

    <owl:Class rdf:about="&cogat;CAO_00642">
        <rdfs:label>Memory storage</rdfs:label>
        <rdfs:subClassOf rdf:resource="&cogat;CAO_00001"/>
        <rdfs:subClassOf>
            <owl:Restriction>
                <owl:onProperty rdf:resource="&ro;part_of"/>
                <owl:someValuesFrom rdf:resource="&cogat;CAO_00489"/>
            </owl:Restriction>
        </rdfs:subClassOf>
        <dc:Title>Memory storage</dc:Title>
        <skos:definition>The representation of information in the brain in a form that enables potential retrieval at a later time.</skos:definition>
        <dc:Contributor>Tal Yarkoni</dc:Contributor>
        <skos:hasTopConcept>Learning and Memory</skos:hasTopConcept>
        <dc:identifier>trm_4a3fd79d0b938</dc:identifier>
        <dc:Date>2010-04-27 07:32:05</dc:Date>
        <skos:altLabel></skos:altLabel>
        <skos:prefLabel>Memory storage</skos:prefLabel>
    </owl:Class>
    


    <!-- http://www.cognitiveatlas.org/ontology/cogat.owl#CAO_00643 -->

    <owl:Class rdf:about="&cogat;CAO_00643">
        <rdfs:label>Memory trace</rdfs:label>
        <rdfs:subClassOf rdf:resource="&cogat;CAO_00001"/>
        <rdfs:subClassOf>
            <owl:Restriction>
                <owl:onProperty rdf:resource="&ro;part_of"/>
                <owl:someValuesFrom rdf:resource="&cogat;CAO_00667"/>
            </owl:Restriction>
        </rdfs:subClassOf>
        <dc:Title>Memory trace</dc:Title>
        <dc:Contributor>Tal Yarkoni</dc:Contributor>
        <dc:identifier>trm_4a3fd79d0b943</dc:identifier>
        <skos:prefLabel>Memory trace</skos:prefLabel>
        <skos:definition>A residual, and often decayed, neural representation of previous knowledge or experience.</skos:definition>
        <skos:altLabel></skos:altLabel>
        <dc:Date>2010-04-27 07:39:30</dc:Date>
        <skos:hasTopConcept></skos:hasTopConcept>
    </owl:Class>
    


    <!-- http://www.cognitiveatlas.org/ontology/cogat.owl#CAO_00644 -->

    <owl:Class rdf:about="&cogat;CAO_00644">
        <rdfs:label>Metamemory</rdfs:label>
        <rdfs:subClassOf rdf:resource="&cogat;CAO_00399"/>
        <dc:Title>Metamemory</dc:Title>
        <skos:prefLabel>Metamemory</skos:prefLabel>
        <skos:altLabel></skos:altLabel>
        <dc:Date>2012-02-23 08:51:52</dc:Date>
        <dc:identifier>trm_4a3fd79d0b94f</dc:identifier>
        <skos:definition>subjective awareness of and knowledge about memory, and strategies for its effective access and application; includes: awareness of memory contents, different and appropriate memory strategies for particular tasks, and how to use a given memory strategy most effectively.</skos:definition>
        <dc:Contributor>Michael Sharman</dc:Contributor>
        <skos:hasTopConcept>Executive-Cognitive Control</skos:hasTopConcept>
    </owl:Class>
    


    <!-- http://www.cognitiveatlas.org/ontology/cogat.owl#CAO_00645 -->

    <owl:Class rdf:about="&cogat;CAO_00645">
        <rdfs:label>Recall</rdfs:label>
        <rdfs:subClassOf rdf:resource="&cogat;CAO_00648"/>
        <skos:altLabel></skos:altLabel>
        <skos:definition>The process of retrieving previously stored information, done without the aid of external cues.</skos:definition>
        <dc:Title>Recall</dc:Title>
        <dc:Contributor>Agatha Lenartowicz</dc:Contributor>
        <skos:hasTopConcept>Learning and Memory</skos:hasTopConcept>
        <dc:identifier>trm_4a3fd79d0b95b</dc:identifier>
        <dc:Date>2009-07-10 14:06:33</dc:Date>
        <skos:prefLabel>Recall</skos:prefLabel>
    </owl:Class>
    


    <!-- http://www.cognitiveatlas.org/ontology/cogat.owl#CAO_00646 -->

    <owl:Class rdf:about="&cogat;CAO_00646">
        <rdfs:label>Recognition</rdfs:label>
        <rdfs:subClassOf rdf:resource="&cogat;CAO_00648"/>
        <skos:definition>the identification of an object, either via its identity or via some feature (such as whether it was previously encountered)</skos:definition>
        <dc:Contributor>Russ Poldrack</dc:Contributor>
        <skos:hasTopConcept>Learning and Memory</skos:hasTopConcept>
        <skos:altLabel></skos:altLabel>
        <dc:Date>2012-03-28 18:16:19</dc:Date>
        <skos:prefLabel>Recognition</skos:prefLabel>
        <dc:identifier>trm_4a3fd79d0b967</dc:identifier>
        <dc:Title>Recognition</dc:Title>
    </owl:Class>
    


    <!-- http://www.cognitiveatlas.org/ontology/cogat.owl#CAO_00647 -->

    <owl:Class rdf:about="&cogat;CAO_00647">
        <rdfs:label>Reconsolidation</rdfs:label>
        <rdfs:subClassOf rdf:resource="&cogat;CAO_00640"/>
        <skos:prefLabel>Reconsolidation</skos:prefLabel>
        <dc:identifier>trm_4a3fd79d0b972</dc:identifier>
        <dc:Contributor>Brenda Gregory</dc:Contributor>
        <skos:altLabel></skos:altLabel>
        <dc:Date>2011-04-28 17:26:42</dc:Date>
        <skos:hasTopConcept>Learning and Memory</skos:hasTopConcept>
        <dc:Title>Reconsolidation</dc:Title>
        <skos:definition>the process of previously consolidated memories being recalled and actively consolidated, it is a distinct process that serves to maintain, strengthen and modify memories that are already stored in the long-term memory.</skos:definition>
    </owl:Class>
    


    <!-- http://www.cognitiveatlas.org/ontology/cogat.owl#CAO_00648 -->

    <owl:Class rdf:about="&cogat;CAO_00648">
        <rdfs:label>Remembering</rdfs:label>
        <rdfs:subClassOf rdf:resource="&cogat;CAO_00001"/>
        <rdfs:subClassOf>
            <owl:Restriction>
                <owl:onProperty rdf:resource="&ro;part_of"/>
                <owl:someValuesFrom rdf:resource="&cogat;CAO_00394"/>
            </owl:Restriction>
        </rdfs:subClassOf>
        <skos:prefLabel>Remembering</skos:prefLabel>
        <dc:Title>Remembering</dc:Title>
        <dc:Contributor>Akram Bakkour</dc:Contributor>
        <skos:definition>the process of consciously reviving or bringing to awareness previous events, experiences, or information. Remembering also involves the process of retaining such material, which is essential to learning. Remembering is distinct from knowing.</skos:definition>
        <dc:Date>2011-08-12 09:20:33</dc:Date>
        <skos:hasTopConcept>Learning and Memory</skos:hasTopConcept>
        <skos:altLabel></skos:altLabel>
        <dc:identifier>trm_4a3fd79d0b97e</dc:identifier>
    </owl:Class>
    


    <!-- http://www.cognitiveatlas.org/ontology/cogat.owl#CAO_00649 -->

    <owl:Class rdf:about="&cogat;CAO_00649">
        <rdfs:label>Acuity</rdfs:label>
        <rdfs:subClassOf rdf:resource="&cogat;CAO_00001"/>
        <dc:identifier>trm_4a3fd79d0b98a</dc:identifier>
        <dc:Contributor>Russ Poldrack</dc:Contributor>
        <dc:Date>2012-03-28 08:43:14</dc:Date>
        <skos:prefLabel>Acuity</skos:prefLabel>
        <dc:Title>Acuity</dc:Title>
        <skos:altLabel></skos:altLabel>
        <skos:definition>accuracy of perception. </skos:definition>
        <skos:hasTopConcept>Perception</skos:hasTopConcept>
    </owl:Class>
    


    <!-- http://www.cognitiveatlas.org/ontology/cogat.owl#CAO_00650 -->

    <owl:Class rdf:about="&cogat;CAO_00650">
        <rdfs:label>Echolocation</rdfs:label>
        <rdfs:subClassOf rdf:resource="&cogat;CAO_00001"/>
        <dc:Date>2012-03-28 10:52:35</dc:Date>
        <skos:definition>the general method of locating objects by determining the time for an echo to return and the direction from which it returns, used by some animals</skos:definition>
        <skos:altLabel></skos:altLabel>
        <dc:identifier>trm_4a3fd79d0b996</dc:identifier>
        <dc:Contributor>Russ Poldrack</dc:Contributor>
        <dc:Title>Echolocation</dc:Title>
        <skos:hasTopConcept>Perception</skos:hasTopConcept>
        <skos:prefLabel>Echolocation</skos:prefLabel>
    </owl:Class>
    


    <!-- http://www.cognitiveatlas.org/ontology/cogat.owl#CAO_00651 -->

    <owl:Class rdf:about="&cogat;CAO_00651">
        <rdfs:label>Edge detection</rdfs:label>
        <rdfs:subClassOf rdf:resource="&cogat;CAO_00001"/>
        <skos:definition>a fundamental tool in image processing and computer vision, particularly in the areas of feature detection and feature extraction, which aim at identifying points in a digital image at which the image brightness changes sharply or more formally has discontinuities.</skos:definition>
        <skos:prefLabel>Edge detection</skos:prefLabel>
        <dc:Contributor>Russ Poldrack</dc:Contributor>
        <skos:altLabel></skos:altLabel>
        <dc:Date>2012-03-28 10:53:12</dc:Date>
        <skos:hasTopConcept>Perception</skos:hasTopConcept>
        <dc:Title>Edge detection</dc:Title>
        <dc:identifier>trm_4a3fd79d0b9a1</dc:identifier>
    </owl:Class>
    


    <!-- http://www.cognitiveatlas.org/ontology/cogat.owl#CAO_00652 -->

    <owl:Class rdf:about="&cogat;CAO_00652">
        <rdfs:label>Feature detection</rdfs:label>
        <rdfs:subClassOf rdf:resource="&cogat;CAO_00001"/>
        <skos:definition>a process of recognizing specific aspects of a stimulus, such as lines, edges, angle, or movement. </skos:definition>
        <dc:identifier>trm_4a3fd79d0b9ad</dc:identifier>
        <dc:Date>2011-08-14 16:58:37</dc:Date>
        <skos:altLabel></skos:altLabel>
        <dc:Title>Feature detection</dc:Title>
        <skos:hasTopConcept>Perception</skos:hasTopConcept>
        <skos:prefLabel>Feature detection</skos:prefLabel>
        <dc:Contributor>Tyler Davis</dc:Contributor>
    </owl:Class>
    


    <!-- http://www.cognitiveatlas.org/ontology/cogat.owl#CAO_00653 -->

    <owl:Class rdf:about="&cogat;CAO_00653">
        <rdfs:label>Figure ground</rdfs:label>
        <rdfs:subClassOf rdf:resource="&cogat;CAO_00001"/>
        <dc:identifier>trm_4a3fd79d0b9b9</dc:identifier>
        <skos:hasTopConcept>Perception</skos:hasTopConcept>
        <skos:definition>Segmentation of a visual space into objects and background.</skos:definition>
        <dc:Title>Figure ground</dc:Title>
        <skos:altLabel></skos:altLabel>
        <skos:prefLabel>Figure ground</skos:prefLabel>
        <dc:Date>2012-03-28 11:57:49</dc:Date>
        <dc:Contributor>Russ Poldrack</dc:Contributor>
    </owl:Class>
    


    <!-- http://www.cognitiveatlas.org/ontology/cogat.owl#CAO_00655 -->

    <owl:Class rdf:about="&cogat;CAO_00655">
        <rdfs:label>Figure ground reversal</rdfs:label>
        <rdfs:subClassOf rdf:resource="&cogat;CAO_00001"/>
        <dc:Date>2011-08-14 17:11:06</dc:Date>
        <dc:Contributor>Tyler Davis</dc:Contributor>
        <dc:identifier>trm_4a3fd79d0b9d1</dc:identifier>
        <skos:prefLabel>Figure ground reversal</skos:prefLabel>
        <dc:Title>Figure ground reversal</dc:Title>
        <skos:altLabel></skos:altLabel>
        <skos:definition>Occurs in certain visual illusions (e.g., Vases and Faces or and#34;Rubinand#39;s Vaseand#34;) in which there are multiple valid figure-ground segmentations that can be selected depending on an observerand#39;s interpretation.</skos:definition>
        <skos:hasTopConcept>Perception</skos:hasTopConcept>
    </owl:Class>
    


    <!-- http://www.cognitiveatlas.org/ontology/cogat.owl#CAO_00656 -->

    <owl:Class rdf:about="&cogat;CAO_00656">
        <rdfs:label>Figure ground segregation</rdfs:label>
        <rdfs:subClassOf rdf:resource="&cogat;CAO_00001"/>
        <skos:definition>Discriminating objects from their surroundings by the visual system.</skos:definition>
        <skos:prefLabel>Figure ground segregation</skos:prefLabel>
        <dc:Contributor>Brenda Gregory</dc:Contributor>
        <skos:altLabel></skos:altLabel>
        <dc:Date>2011-04-19 13:55:00</dc:Date>
        <skos:hasTopConcept>Perception</skos:hasTopConcept>
        <dc:Title>Figure ground segregation</dc:Title>
        <dc:identifier>trm_4a3fd79d0b9dd</dc:identifier>
    </owl:Class>
    


    <!-- http://www.cognitiveatlas.org/ontology/cogat.owl#CAO_00657 -->

    <owl:Class rdf:about="&cogat;CAO_00657">
        <rdfs:label>Gustation</rdfs:label>
        <rdfs:subClassOf rdf:resource="&cogat;CAO_00001"/>
        <skos:altLabel></skos:altLabel>
        <skos:hasTopConcept>Perception</skos:hasTopConcept>
        <dc:Date>2009-12-21 14:36:45</dc:Date>
        <dc:Title>Gustation</dc:Title>
        <dc:Contributor>Agatha Lenartowicz</dc:Contributor>
        <skos:definition>Form of chemoreception that facilitates taste perception.</skos:definition>
        <skos:prefLabel>Gustation</skos:prefLabel>
        <dc:identifier>trm_4a3fd79d0b9e9</dc:identifier>
    </owl:Class>
    


    <!-- http://www.cognitiveatlas.org/ontology/cogat.owl#CAO_00659 -->

    <owl:Class rdf:about="&cogat;CAO_00659">
        <rdfs:label>Memory retrieval</rdfs:label>
        <rdfs:subClassOf rdf:resource="&cogat;CAO_00490"/>
        <rdfs:subClassOf>
            <owl:Restriction>
                <owl:onProperty rdf:resource="&ro;part_of"/>
                <owl:someValuesFrom rdf:resource="&cogat;CAO_00648"/>
            </owl:Restriction>
        </rdfs:subClassOf>
        <rdfs:subClassOf>
            <owl:Restriction>
                <owl:onProperty rdf:resource="&ro;part_of"/>
                <owl:someValuesFrom rdf:resource="&cogat;CAO_00645"/>
            </owl:Restriction>
        </rdfs:subClassOf>
        <rdfs:subClassOf>
            <owl:Restriction>
                <owl:onProperty rdf:resource="&ro;part_of"/>
                <owl:someValuesFrom rdf:resource="&cogat;CAO_00646"/>
            </owl:Restriction>
        </rdfs:subClassOf>
        <skos:definition>the process of accessing a stored memory</skos:definition>
        <skos:altLabel></skos:altLabel>
        <dc:Contributor>Russ Poldrack</dc:Contributor>
        <skos:hasTopConcept>Learning and Memory</skos:hasTopConcept>
        <skos:prefLabel>Memory retrieval</skos:prefLabel>
        <dc:Title>Memory retrieval</dc:Title>
        <dc:Date>2012-03-28 17:34:48</dc:Date>
        <dc:identifier>trm_4a3fd79d0ba01</dc:identifier>
    </owl:Class>
    


    <!-- http://www.cognitiveatlas.org/ontology/cogat.owl#CAO_00660 -->

    <owl:Class rdf:about="&cogat;CAO_00660">
        <rdfs:label>Active maintenance</rdfs:label>
        <rdfs:subClassOf rdf:resource="&cogat;CAO_00001"/>
        <rdfs:subClassOf>
            <owl:Restriction>
                <owl:onProperty rdf:resource="&ro;part_of"/>
                <owl:someValuesFrom rdf:resource="&cogat;CAO_00587"/>
            </owl:Restriction>
        </rdfs:subClassOf>
        <skos:definition>The maintenance of information in working memory through active (volitional) rather than passive means</skos:definition>
        <dc:Title>Active maintenance</dc:Title>
        <skos:hasTopConcept>Executive-Cognitive Control</skos:hasTopConcept>
        <dc:identifier>trm_4a3fd79d0ba0d</dc:identifier>
        <skos:altLabel></skos:altLabel>
        <dc:Contributor>Russ Poldrack</dc:Contributor>
        <skos:prefLabel>Active maintenance</skos:prefLabel>
        <dc:Date>2010-07-14 11:39:19</dc:Date>
    </owl:Class>
    


    <!-- http://www.cognitiveatlas.org/ontology/cogat.owl#CAO_00661 -->

    <owl:Class rdf:about="&cogat;CAO_00661">
        <rdfs:label>Articulatory loop</rdfs:label>
        <rdfs:subClassOf rdf:resource="&cogat;CAO_00667"/>
        <rdfs:subClassOf>
            <owl:Restriction>
                <owl:onProperty rdf:resource="&ro;part_of"/>
                <owl:someValuesFrom rdf:resource="&cogat;CAO_00587"/>
            </owl:Restriction>
        </rdfs:subClassOf>
        <dc:Title>Articulatory loop</dc:Title>
        <dc:Contributor>Russ Poldrack</dc:Contributor>
        <skos:definition>(also referred to as the ‘phonological loop’), is one of the subsystems postulated in Alan Baddeley’s multicomponent model of WORKING MEMORY, specialized for the temporary storage of verbal information.  It consists of a phonological store and an articulatory rehearsal process. The phonological store can hold speech-based information, subject to a rapid decay. The articulatory rehearsal process can refresh the decaying representation by reading it off and feeding it back to the store. It also serves to convert visually presented information (such as written words) into phonological codes and register them into the phonological store. </skos:definition>
        <skos:hasTopConcept>Learning and Memory</skos:hasTopConcept>
        <skos:altLabel></skos:altLabel>
        <dc:Date>2012-03-28 08:55:18</dc:Date>
        <dc:identifier>trm_4a3fd79d0ba19</dc:identifier>
        <skos:prefLabel>Articulatory loop</skos:prefLabel>
    </owl:Class>
    


    <!-- http://www.cognitiveatlas.org/ontology/cogat.owl#CAO_00662 -->

    <owl:Class rdf:about="&cogat;CAO_00662">
        <rdfs:label>Central executive</rdfs:label>
        <rdfs:subClassOf rdf:resource="&cogat;CAO_00001"/>
        <rdfs:subClassOf>
            <owl:Restriction>
                <owl:onProperty rdf:resource="&ro;part_of"/>
                <owl:someValuesFrom rdf:resource="&cogat;CAO_00292"/>
            </owl:Restriction>
        </rdfs:subClassOf>
        <dc:Date>2009-07-10 14:06:33</dc:Date>
        <skos:hasTopConcept>Executive-Cognitive Control</skos:hasTopConcept>
        <dc:identifier>trm_4a3fd79d0ba25</dc:identifier>
        <dc:Contributor>Agatha Lenartowicz</dc:Contributor>
        <skos:definition>The core mental process of working memory that allows for information that is stored in short-term memory to be actively manipulated (e.g., mental arithmetic). The term and#39;central executiveand#39; is typically associated with psychologist Alan Baddeleyand#39;s and#34;Model of Working Memoryand#34;.</skos:definition>
        <skos:prefLabel>Central executive</skos:prefLabel>
        <dc:Title>Central executive</dc:Title>
        <skos:altLabel></skos:altLabel>
    </owl:Class>
    


    <!-- http://www.cognitiveatlas.org/ontology/cogat.owl#CAO_00663 -->

    <owl:Class rdf:about="&cogat;CAO_00663">
        <rdfs:label>Maintenance</rdfs:label>
        <rdfs:subClassOf rdf:resource="&cogat;CAO_00001"/>
        <skos:hasTopConcept>Executive-Cognitive Control</skos:hasTopConcept>
        <dc:Date>2009-07-10 14:06:33</dc:Date>
        <skos:altLabel></skos:altLabel>
        <dc:identifier>trm_4a3fd79d0ba30</dc:identifier>
        <skos:definition>The process of keeping information in active and immediately accessible state.</skos:definition>
        <dc:Contributor>Agatha Lenartowicz</dc:Contributor>
        <skos:prefLabel>Maintenance</skos:prefLabel>
        <dc:Title>Maintenance</dc:Title>
    </owl:Class>
    


    <!-- http://www.cognitiveatlas.org/ontology/cogat.owl#CAO_00664 -->

    <owl:Class rdf:about="&cogat;CAO_00664">
        <rdfs:label>Manipulation</rdfs:label>
        <rdfs:subClassOf rdf:resource="&cogat;CAO_00001"/>
        <dc:Title>Manipulation</dc:Title>
        <dc:Contributor>Russ Poldrack</dc:Contributor>
        <skos:prefLabel>Manipulation</skos:prefLabel>
        <dc:Date>2012-03-28 17:30:27</dc:Date>
        <skos:hasTopConcept>Executive-Cognitive Control</skos:hasTopConcept>
        <dc:identifier>trm_4a3fd79d0ba3c</dc:identifier>
        <skos:altLabel></skos:altLabel>
        <skos:definition>performance of operations upon information held in working memory</skos:definition>
    </owl:Class>
    


    <!-- http://www.cognitiveatlas.org/ontology/cogat.owl#CAO_00665 -->

    <owl:Class rdf:about="&cogat;CAO_00665">
        <rdfs:label>Phonological loop</rdfs:label>
        <rdfs:subClassOf rdf:resource="&cogat;CAO_00667"/>
        <rdfs:subClassOf>
            <owl:Restriction>
                <owl:onProperty rdf:resource="&ro;part_of"/>
                <owl:someValuesFrom rdf:resource="&cogat;CAO_00171"/>
            </owl:Restriction>
        </rdfs:subClassOf>
        <skos:prefLabel>Phonological loop</skos:prefLabel>
        <skos:altLabel></skos:altLabel>
        <dc:identifier>trm_4a3fd79d0ba48</dc:identifier>
        <dc:Date>2012-03-28 17:58:07</dc:Date>
        <skos:hasTopConcept>Learning and Memory</skos:hasTopConcept>
        <skos:definition>deals with sound or phonological information and consists of two parts: a short-term phonological store with auditory  memory traces that are subject to rapid decay and an articulatory rehearsal component that can revive the memory traces. </skos:definition>
        <dc:Title>Phonological loop</dc:Title>
        <dc:Contributor>Russ Poldrack</dc:Contributor>
    </owl:Class>
    


    <!-- http://www.cognitiveatlas.org/ontology/cogat.owl#CAO_00666 -->

    <owl:Class rdf:about="&cogat;CAO_00666">
        <rdfs:label>Rehearsal</rdfs:label>
        <rdfs:subClassOf rdf:resource="&cogat;CAO_00001"/>
        <rdfs:subClassOf>
            <owl:Restriction>
                <owl:onProperty rdf:resource="&ro;part_of"/>
                <owl:someValuesFrom rdf:resource="&cogat;CAO_00517"/>
            </owl:Restriction>
        </rdfs:subClassOf>
        <skos:definition>The repetition of information in an attempt to maintain it longer in memory.</skos:definition>
        <skos:hasTopConcept>Learning and Memory</skos:hasTopConcept>
        <dc:Contributor>Russ Poldrack</dc:Contributor>
        <dc:Date>2012-03-28 18:16:47</dc:Date>
        <dc:identifier>trm_4a3fd79d0ba54</dc:identifier>
        <skos:prefLabel>Rehearsal</skos:prefLabel>
        <skos:altLabel></skos:altLabel>
        <dc:Title>Rehearsal</dc:Title>
    </owl:Class>
    


    <!-- http://www.cognitiveatlas.org/ontology/cogat.owl#CAO_00667 -->

    <owl:Class rdf:about="&cogat;CAO_00667">
        <rdfs:label>Rehearsal loop</rdfs:label>
        <rdfs:subClassOf rdf:resource="&cogat;CAO_00001"/>
        <rdfs:subClassOf>
            <owl:Restriction>
                <owl:onProperty rdf:resource="&ro;part_of"/>
                <owl:someValuesFrom rdf:resource="&cogat;CAO_00587"/>
            </owl:Restriction>
        </rdfs:subClassOf>
        <rdfs:subClassOf>
            <owl:Restriction>
                <owl:onProperty rdf:resource="&ro;part_of"/>
                <owl:someValuesFrom rdf:resource="&cogat;CAO_00451"/>
            </owl:Restriction>
        </rdfs:subClassOf>
        <skos:altLabel></skos:altLabel>
        <skos:definition>or phonological loop, also called the phonetic loop or the articulatory loop, is the part of working memory that rehearses verbal information. It consists of two parts: a short-term phonological store with auditory memory traces that are subject to rapid decay and an articulatory rehearsal component that can revive the memory traces.The first component is a phonological memory store which can hold traces of acoustic or speech based material. Material in this short term store lasts about two seconds unless it is maintained through the use of the second subcomponent, articulatory subvocal rehearsal. Prevention of articulatory rehearsal results in very rapid forgetting (a process known as decay). </skos:definition>
        <skos:prefLabel>Rehearsal loop</skos:prefLabel>
        <dc:Title>Rehearsal loop</dc:Title>
        <dc:Contributor>Natalie Picchetti</dc:Contributor>
        <dc:Date>2011-04-12 09:52:37</dc:Date>
        <dc:identifier>trm_4a3fd79d0ba60</dc:identifier>
        <skos:hasTopConcept>Learning and Memory</skos:hasTopConcept>
    </owl:Class>
    


    <!-- http://www.cognitiveatlas.org/ontology/cogat.owl#CAO_00668 -->

    <owl:Class rdf:about="&cogat;CAO_00668">
        <rdfs:label>Working memory retrieval</rdfs:label>
        <rdfs:subClassOf rdf:resource="&cogat;CAO_00001"/>
        <rdfs:subClassOf>
            <owl:Restriction>
                <owl:onProperty rdf:resource="&ro;part_of"/>
                <owl:someValuesFrom rdf:resource="&cogat;CAO_00587"/>
            </owl:Restriction>
        </rdfs:subClassOf>
        <skos:altLabel></skos:altLabel>
        <skos:definition>The process of accessing information that is maintained in working memory; the sub-process by which the contents of working memory are accessed.</skos:definition>
        <dc:identifier>trm_4a3fd79d0ba6c</dc:identifier>
        <skos:hasTopConcept>Executive-Cognitive Control</skos:hasTopConcept>
        <dc:Contributor>Agatha Lenartowicz</dc:Contributor>
        <dc:Date>2009-07-10 14:06:33</dc:Date>
        <dc:Title>Working memory retrieval</dc:Title>
        <skos:prefLabel>Working memory retrieval</skos:prefLabel>
    </owl:Class>
    


    <!-- http://www.cognitiveatlas.org/ontology/cogat.owl#CAO_00669 -->

    <owl:Class rdf:about="&cogat;CAO_00669">
        <rdfs:label>Working memory storage</rdfs:label>
        <rdfs:subClassOf rdf:resource="&cogat;CAO_00001"/>
        <rdfs:subClassOf>
            <owl:Restriction>
                <owl:onProperty rdf:resource="&ro;part_of"/>
                <owl:someValuesFrom rdf:resource="&cogat;CAO_00587"/>
            </owl:Restriction>
        </rdfs:subClassOf>
        <dc:Date>2009-07-10 14:06:33</dc:Date>
        <skos:altLabel></skos:altLabel>
        <dc:Contributor>Agatha Lenartowicz</dc:Contributor>
        <dc:Title>Working memory storage</dc:Title>
        <skos:hasTopConcept>Executive-Cognitive Control</skos:hasTopConcept>
        <dc:identifier>trm_4a3fd79d0ba77</dc:identifier>
        <skos:definition>The maintenance of information of working memory; a sub-component of working memory that allows for contents of working memory to be retained.</skos:definition>
        <skos:prefLabel>Working memory storage</skos:prefLabel>
    </owl:Class>
    


    <!-- http://www.cognitiveatlas.org/ontology/cogat.owl#CAO_00670 -->

    <owl:Class rdf:about="&cogat;CAO_00670">
        <rdfs:label>Cognitive control</rdfs:label>
        <rdfs:subClassOf rdf:resource="&cogat;CAO_00001"/>
        <dc:Contributor>Russ Poldrack</dc:Contributor>
        <skos:altLabel>executive control</skos:altLabel>
        <dc:identifier>trm_4aae62e4ad209</dc:identifier>
        <dc:Title>Cognitive control</dc:Title>
        <skos:hasTopConcept>Executive-Cognitive Control</skos:hasTopConcept>
        <skos:definition>The top-down modulation of cognitive processes based on higher-order representations such as goals or plans.</skos:definition>
        <dc:Date>2010-01-10 15:30:42</dc:Date>
        <skos:prefLabel>Cognitive control</skos:prefLabel>
    </owl:Class>
    


    <!-- http://www.cognitiveatlas.org/ontology/cogat.owl#CAO_00671 -->

    <owl:Class rdf:about="&cogat;CAO_00671">
        <rdfs:label>Echoic memory</rdfs:label>
        <rdfs:subClassOf rdf:resource="&cogat;CAO_00163"/>
        <dc:Contributor>Brenda Gregory</dc:Contributor>
        <dc:identifier>trm_4b185801de7a1</dc:identifier>
        <skos:altLabel></skos:altLabel>
        <skos:definition>refers to the phenomenon in which there is a brief mental echo that continues to sound after an auditory stimulus has been heard.</skos:definition>
        <dc:Title>Echoic memory</dc:Title>
        <skos:hasTopConcept>Learning and Memory</skos:hasTopConcept>
        <skos:prefLabel>Echoic memory</skos:prefLabel>
        <dc:Date>2011-05-12 15:21:16</dc:Date>
    </owl:Class>
    


    <!-- http://www.cognitiveatlas.org/ontology/cogat.owl#CAO_00673 -->

    <owl:Class rdf:about="&cogat;CAO_00673">
        <rdfs:label>Task set reconfiguration</rdfs:label>
        <rdfs:subClassOf rdf:resource="&cogat;CAO_00001"/>
        <skos:altLabel></skos:altLabel>
        <skos:definition>A change in the task set based on some internal or external cue</skos:definition>
        <skos:prefLabel>Task set reconfiguration</skos:prefLabel>
        <skos:hasTopConcept>Executive-Cognitive Control</skos:hasTopConcept>
        <dc:Title>Task set reconfiguration</dc:Title>
        <dc:Contributor>Mei-Yen Chen</dc:Contributor>
        <dc:Date>2011-08-12 13:09:24</dc:Date>
        <dc:identifier>trm_4b45f56827e93</dc:identifier>
    </owl:Class>
    


    <!-- http://www.cognitiveatlas.org/ontology/cogat.owl#CAO_00674 -->

    <owl:Class rdf:about="&cogat;CAO_00674">
        <rdfs:label>Reward</rdfs:label>
        <rdfs:subClassOf rdf:resource="&cogat;CAO_00001"/>
        <rdfs:subClassOf>
            <owl:Restriction>
                <owl:onProperty rdf:resource="&ro;part_of"/>
                <owl:someValuesFrom rdf:resource="&cogat;CAO_00377"/>
            </owl:Restriction>
        </rdfs:subClassOf>
        <dc:Title>Reward</dc:Title>
        <skos:prefLabel>Reward</skos:prefLabel>
        <skos:hasTopConcept>Learning and Memory</skos:hasTopConcept>
        <dc:Date>2011-08-12 11:58:40</dc:Date>
        <skos:altLabel>reinforcement</skos:altLabel>
        <dc:identifier>trm_4b6525253c63f</dc:identifier>
        <skos:definition>A positive return for performance of a specific behavior.</skos:definition>
        <dc:Contributor>Akram Bakkour</dc:Contributor>
    </owl:Class>
    


    <!-- http://www.cognitiveatlas.org/ontology/cogat.owl#CAO_00675 -->

    <owl:Class rdf:about="&cogat;CAO_00675">
        <rdfs:label>Pain</rdfs:label>
        <rdfs:subClassOf rdf:resource="&cogat;CAO_00525"/>
        <dc:identifier>trm_4b65259eeee34</dc:identifier>
        <skos:prefLabel>Pain</skos:prefLabel>
        <skos:hasTopConcept>Emotion</skos:hasTopConcept>
        <dc:Contributor>Russ Poldrack</dc:Contributor>
        <dc:Title>Pain</dc:Title>
        <dc:Date>2012-03-28 17:53:40</dc:Date>
        <skos:altLabel></skos:altLabel>
        <skos:definition>An unpleasant sensory and emotional experience associated with actual or potential tissue damage.</skos:definition>
    </owl:Class>
    


    <!-- http://www.cognitiveatlas.org/ontology/cogat.owl#CAO_00676 -->

    <owl:Class rdf:about="&cogat;CAO_00676">
        <rdfs:label>Joint attention</rdfs:label>
        <rdfs:subClassOf rdf:resource="&cogat;CAO_00001"/>
        <skos:altLabel></skos:altLabel>
        <dc:Contributor>Russ Poldrack</dc:Contributor>
        <dc:Date>2012-03-28 17:11:43</dc:Date>
        <skos:definition>the process of alerting one person to a stimulus through nonverbal cues such as finger pointing or gazing. It is one of the first signs of the development of a theory of mind in babies and serves as an important step to later language and social development.</skos:definition>
        <dc:Title>Joint attention</dc:Title>
        <skos:hasTopConcept>Attention</skos:hasTopConcept>
        <dc:identifier>trm_4b75ed06c917d</dc:identifier>
        <skos:prefLabel>Joint attention</skos:prefLabel>
    </owl:Class>
    


    <!-- http://www.cognitiveatlas.org/ontology/cogat.owl#CAO_00677 -->

    <owl:Class rdf:about="&cogat;CAO_00677">
        <rdfs:label>Behavioral inhibition (cognitive)</rdfs:label>
        <rdfs:subClassOf rdf:resource="&cogat;CAO_00001"/>
        <rdfs:subClassOf>
            <owl:Restriction>
                <owl:onProperty rdf:resource="&ro;part_of"/>
                <owl:someValuesFrom rdf:resource="&cogat;CAO_00292"/>
            </owl:Restriction>
        </rdfs:subClassOf>
        <dc:identifier>trm_4b7c270940f9d</dc:identifier>
        <skos:altLabel>behavioral inhibition</skos:altLabel>
        <dc:Date>2010-02-17 09:27:37</dc:Date>
        <skos:hasTopConcept>Executive-Cognitive Control</skos:hasTopConcept>
        <skos:definition>Often used as a synonym of and#34;response inhibitionand#34; to describe the inhibition of actions. </skos:definition>
        <dc:Title>Behavioral inhibition (cognitive)</dc:Title>
        <dc:Contributor>System Administrator</dc:Contributor>
        <skos:prefLabel>Behavioral inhibition (cognitive)</skos:prefLabel>
    </owl:Class>
    


    <!-- http://www.cognitiveatlas.org/ontology/cogat.owl#CAO_00678 -->

    <owl:Class rdf:about="&cogat;CAO_00678">
        <rdfs:label>Behavioral inhibition (temperament)</rdfs:label>
        <rdfs:subClassOf rdf:resource="&cogat;CAO_00001"/>
        <skos:hasTopConcept></skos:hasTopConcept>
        <skos:definition>A temperamental characteristic described by shyness and social anxiety.</skos:definition>
        <dc:Contributor>Russ Poldrack</dc:Contributor>
        <dc:Title>Behavioral inhibition (temperament)</dc:Title>
        <dc:identifier>trm_4b7c27094a093</dc:identifier>
        <skos:altLabel>behavioral inhibition</skos:altLabel>
        <skos:prefLabel>Behavioral inhibition (temperament)</skos:prefLabel>
        <dc:Date>2010-02-17 09:27:37</dc:Date>
    </owl:Class>
    


    <!-- http://www.cognitiveatlas.org/ontology/cogat.owl#CAO_00679 -->

    <owl:Class rdf:about="&cogat;CAO_00679">
        <rdfs:label>Central coherence</rdfs:label>
        <rdfs:subClassOf rdf:resource="&cogat;CAO_00001"/>
        <dc:Contributor>Deanna Lau</dc:Contributor>
        <skos:prefLabel>Central coherence</skos:prefLabel>
        <dc:Title>Central coherence</dc:Title>
        <dc:identifier>trm_4b82c75498408</dc:identifier>
        <skos:definition>A personand#39;s ability to understand things in context</skos:definition>
        <skos:hasTopConcept></skos:hasTopConcept>
        <dc:Date>2010-02-22 10:05:08</dc:Date>
        <skos:altLabel></skos:altLabel>
    </owl:Class>
    


    <!-- http://www.cognitiveatlas.org/ontology/cogat.owl#CAO_00680 -->

    <owl:Class rdf:about="&cogat;CAO_00680">
        <rdfs:label>Interference resolution</rdfs:label>
        <rdfs:subClassOf rdf:resource="&cogat;CAO_00001"/>
        <rdfs:subClassOf>
            <owl:Restriction>
                <owl:onProperty rdf:resource="&ro;part_of"/>
                <owl:someValuesFrom rdf:resource="&cogat;CAO_00587"/>
            </owl:Restriction>
        </rdfs:subClassOf>
        <skos:prefLabel>Interference resolution</skos:prefLabel>
        <skos:definition>The process of selecting information with regard to its relevance to an ongoing task.</skos:definition>
        <skos:hasTopConcept>Executive-Cognitive Control</skos:hasTopConcept>
        <dc:Date>2012-03-28 17:09:38</dc:Date>
        <dc:Contributor>Russ Poldrack</dc:Contributor>
        <dc:identifier>trm_4c3e04d656f06</dc:identifier>
        <skos:altLabel></skos:altLabel>
        <dc:Title>Interference resolution</dc:Title>
    </owl:Class>
    


    <!-- http://www.cognitiveatlas.org/ontology/cogat.owl#CAO_00681 -->

    <owl:Class rdf:about="&cogat;CAO_00681">
        <rdfs:label>Updating</rdfs:label>
        <rdfs:subClassOf rdf:resource="&cogat;CAO_00001"/>
        <rdfs:subClassOf>
            <owl:Restriction>
                <owl:onProperty rdf:resource="&ro;part_of"/>
                <owl:someValuesFrom rdf:resource="&cogat;CAO_00587"/>
            </owl:Restriction>
        </rdfs:subClassOf>
        <skos:prefLabel>Updating</skos:prefLabel>
        <skos:definition>The revision or refreshing of information that is maintained in working memory</skos:definition>
        <dc:Title>Updating</dc:Title>
        <dc:identifier>trm_4c3e05903e4bb</dc:identifier>
        <skos:hasTopConcept>Executive-Cognitive Control</skos:hasTopConcept>
        <dc:Contributor>Russ Poldrack</dc:Contributor>
        <dc:Date>2012-03-28 18:57:32</dc:Date>
        <skos:altLabel></skos:altLabel>
    </owl:Class>
    


    <!-- http://www.cognitiveatlas.org/ontology/cogat.owl#CAO_00682 -->

    <owl:Class rdf:about="&cogat;CAO_00682">
        <rdfs:label>Task set</rdfs:label>
        <rdfs:subClassOf rdf:resource="&cogat;CAO_00001"/>
        <skos:hasTopConcept>Executive-Cognitive Control</skos:hasTopConcept>
        <dc:Title>Task set</dc:Title>
        <skos:prefLabel>Task set</skos:prefLabel>
        <skos:altLabel></skos:altLabel>
        <dc:Contributor>Mei-Yen Chen</dc:Contributor>
        <dc:identifier>trm_4c3e0646a2408</dc:identifier>
        <skos:definition>The set of rules and-or stimulus-response mappings that define how a task should be performed.</skos:definition>
        <dc:Date>2011-08-12 13:09:15</dc:Date>
    </owl:Class>
    


    <!-- http://www.cognitiveatlas.org/ontology/cogat.owl#CAO_00683 -->

    <owl:Class rdf:about="&cogat;CAO_00683">
        <rdfs:label>Subconscious</rdfs:label>
        <rdfs:subClassOf rdf:resource="&cogat;CAO_00001"/>
        <dc:Contributor>Peter Walla</dc:Contributor>
        <dc:Title>Subconscious</dc:Title>
        <dc:identifier>trm_4d21e9a7dd8ca</dc:identifier>
        <dc:Date>2011-01-03 07:23:26</dc:Date>
        <skos:definition>Subconscious is any neural activity which has the potential to be conscious, but at the moment is processed below the level of consciousness.  In contrast to unconscious information processing, subconscious processing contains meaning (semantic information).  Intuition is a good example for subconscious information processing. In other words, intuition means thinking below the level of consciousness whereby only the output enters the stream of consciousness.  from Peter Walla</skos:definition>
        <skos:prefLabel>Subconscious</skos:prefLabel>
        <skos:altLabel></skos:altLabel>
        <skos:hasTopConcept></skos:hasTopConcept>
    </owl:Class>
    


    <!-- http://www.cognitiveatlas.org/ontology/cogat.owl#CAO_00684 -->

    <owl:Class rdf:about="&cogat;CAO_00684">
        <rdfs:label>Semantic information</rdfs:label>
        <rdfs:subClassOf rdf:resource="&cogat;CAO_00001"/>
        <skos:hasTopConcept></skos:hasTopConcept>
        <dc:Title>Semantic information</dc:Title>
        <skos:altLabel>semantic knowledge</skos:altLabel>
        <skos:definition>information that is not tied to any specific object, event, domain, or application. It includes general factual information about the world (as in an encyclopedia) and oneself.</skos:definition>
        <dc:Date>2011-08-12 14:10:20</dc:Date>
        <dc:Contributor>Akram Bakkour</dc:Contributor>
        <skos:prefLabel>Semantic information</skos:prefLabel>
        <dc:identifier>trm_4d2201d530697</dc:identifier>
    </owl:Class>
    


    <!-- http://www.cognitiveatlas.org/ontology/cogat.owl#CAO_00685 -->

    <owl:Class rdf:about="&cogat;CAO_00685">
        <rdfs:label>Paraphasia</rdfs:label>
        <rdfs:subClassOf rdf:resource="&cogat;CAO_00001"/>
        <skos:hasTopConcept>Language</skos:hasTopConcept>
        <skos:altLabel></skos:altLabel>
        <skos:definition>generally refers to errors in naming. Collectively, this term is applied to any unintended error of word or sound choice. </skos:definition>
        <dc:Date>2011-04-11 14:24:31</dc:Date>
        <dc:Contributor>Natalie Picchetti</dc:Contributor>
        <dc:Title>Paraphasia</dc:Title>
        <dc:identifier>trm_4d7fa1a3e2a10</dc:identifier>
        <skos:prefLabel>Paraphasia</skos:prefLabel>
    </owl:Class>
    


    <!-- http://www.cognitiveatlas.org/ontology/cogat.owl#CAO_00686 -->

    <owl:Class rdf:about="&cogat;CAO_00686">
        <rdfs:label>Phonemic paraphasia</rdfs:label>
        <rdfs:subClassOf rdf:resource="&cogat;CAO_00001"/>
        <skos:altLabel></skos:altLabel>
        <skos:prefLabel>Phonemic paraphasia</skos:prefLabel>
        <dc:Date>2011-04-11 14:24:12</dc:Date>
        <dc:identifier>trm_4d7fa1ee2f870</dc:identifier>
        <dc:Contributor>Natalie Picchetti</dc:Contributor>
        <dc:Title>Phonemic paraphasia</dc:Title>
        <skos:definition>is the production of unintended sounds or syllables in the utterance of partially recognizable word, e.g., ‘paker’ for ‘paper.’ </skos:definition>
        <skos:hasTopConcept>Language</skos:hasTopConcept>
    </owl:Class>
    


    <!-- http://www.cognitiveatlas.org/ontology/cogat.owl#CAO_00687 -->

    <owl:Class rdf:about="&cogat;CAO_00687">
        <rdfs:label>Neologism</rdfs:label>
        <rdfs:subClassOf rdf:resource="&cogat;CAO_00001"/>
        <dc:Contributor>Natalie Picchetti</dc:Contributor>
        <dc:Date>2011-04-11 13:28:35</dc:Date>
        <skos:altLabel></skos:altLabel>
        <skos:definition>is the production of nonsense word or words, usually without recognition of errors, e.g., ‘table’ becomes ‘tilto.’  </skos:definition>
        <dc:Title>Neologism</dc:Title>
        <skos:prefLabel>Neologism</skos:prefLabel>
        <dc:identifier>trm_4d7fa2df05f23</dc:identifier>
        <skos:hasTopConcept>Language</skos:hasTopConcept>
    </owl:Class>
    


    <!-- http://www.cognitiveatlas.org/ontology/cogat.owl#CAO_00688 -->

    <owl:Class rdf:about="&cogat;CAO_00688">
        <rdfs:label>Metacomprehension</rdfs:label>
        <rdfs:subClassOf rdf:resource="&cogat;CAO_00001"/>
        <skos:definition>refers to the learnersand#39; ability to monitor the degree to which they understand information being communicated to them, to recognize failures to comprehend, and to employ repair strategies when failures are identified. </skos:definition>
        <dc:Title>Metacomprehension</dc:Title>
        <skos:hasTopConcept></skos:hasTopConcept>
        <dc:Contributor>Natalie Picchetti</dc:Contributor>
        <skos:prefLabel>Metacomprehension</skos:prefLabel>
        <dc:identifier>trm_4d7fc763cf777</dc:identifier>
        <dc:Date>2011-04-07 11:08:06</dc:Date>
        <skos:altLabel></skos:altLabel>
    </owl:Class>
    


    <!-- http://www.cognitiveatlas.org/ontology/cogat.owl#CAO_00690 -->

    <owl:Class rdf:about="&cogat;CAO_00690">
        <rdfs:label>Conceptual metaphor</rdfs:label>
        <rdfs:subClassOf rdf:resource="&cogat;CAO_00001"/>
        <dc:Date>2011-04-01 12:33:23</dc:Date>
        <dc:Contributor>Natalie Picchetti</dc:Contributor>
        <skos:definition>In cognitive linguistics, metaphor is defined as understanding one conceptual domain in terms of another conceptual domain; for example, using one personand#39;s life experience to understand a different personand#39;s experience. A conceptual domain can be any coherent organization of experience.  </skos:definition>
        <skos:hasTopConcept></skos:hasTopConcept>
        <dc:identifier>trm_4d920c905d465</dc:identifier>
        <dc:Title>Conceptual metaphor</dc:Title>
        <skos:altLabel></skos:altLabel>
        <skos:prefLabel>Conceptual metaphor</skos:prefLabel>
    </owl:Class>
    


    <!-- http://www.cognitiveatlas.org/ontology/cogat.owl#CAO_00691 -->

    <owl:Class rdf:about="&cogat;CAO_00691">
        <rdfs:label>Body representation</rdfs:label>
        <rdfs:subClassOf rdf:resource="&cogat;CAO_00001"/>
        <dc:Date>2012-03-28 09:30:15</dc:Date>
        <dc:Contributor>Russ Poldrack</dc:Contributor>
        <skos:altLabel></skos:altLabel>
        <skos:prefLabel>Body representation</skos:prefLabel>
        <dc:Title>Body representation</dc:Title>
        <skos:hasTopConcept></skos:hasTopConcept>
        <dc:identifier>trm_4e5505361f160</dc:identifier>
        <skos:definition>A mental representation of oneand#39;s own body</skos:definition>
    </owl:Class>
    


    <!-- http://www.cognitiveatlas.org/ontology/cogat.owl#CAO_00692 -->

    <owl:Class rdf:about="&cogat;CAO_00692">
        <rdfs:label>Reward task ()</rdfs:label>
        <rdfs:subClassOf rdf:resource="&cogat;CAO_00001"/>
        <dc:Contributor>Brenda Gregory</dc:Contributor>
        <dc:identifier>trm_4dfa343f8a815</dc:identifier>
        <skos:definition>Subjects perform a task in which correct performance is associated with reward, often monetary reward.</skos:definition>
        <skos:prefLabel>Reward task ()</skos:prefLabel>
        <dc:Title>Reward task ()</dc:Title>
        <dc:Date>2011-06-16 09:50:07</dc:Date>
        <skos:altLabel>Reward Task</skos:altLabel>
        <skos:hasTopConcept></skos:hasTopConcept>
    </owl:Class>
    


    <!-- http://www.cognitiveatlas.org/ontology/cogat.owl#CAO_00693 -->

    <owl:Class rdf:about="&cogat;CAO_00693">
        <rdfs:label>Reward task (reward response)</rdfs:label>
        <rdfs:subClassOf rdf:resource="&cogat;CAO_00001"/>
        <skos:altLabel>Reward Task</skos:altLabel>
        <dc:Date>2011-06-16 09:50:07</dc:Date>
        <skos:hasTopConcept></skos:hasTopConcept>
        <skos:prefLabel>Reward task (reward response)</skos:prefLabel>
        <dc:Title>Reward task (reward response)</dc:Title>
        <dc:Contributor>Carinna Torgerson</dc:Contributor>
        <dc:identifier>trm_4dfa343fa1a36</dc:identifier>
        <skos:definition>Subjects are given an option of an action that dispenses rewards and the extent to which they select this action is measured.</skos:definition>
    </owl:Class>
    


    <!-- http://www.cognitiveatlas.org/ontology/cogat.owl#CAO_00694 -->

    <owl:Class rdf:about="&cogat;CAO_00694">
        <rdfs:label>Multisensory integration</rdfs:label>
        <rdfs:subClassOf rdf:resource="&cogat;CAO_00001"/>
        <skos:prefLabel>Multisensory integration</skos:prefLabel>
        <dc:Date>2012-03-28 17:45:26</dc:Date>
        <skos:hasTopConcept>Perception</skos:hasTopConcept>
        <skos:altLabel></skos:altLabel>
        <dc:identifier>trm_4e31ced566649</dc:identifier>
        <dc:Contributor>Russ Poldrack</dc:Contributor>
        <skos:definition>The process by which unisensory signals are combined to form a new product. It is operationally defined as a multisensory response (neural or behavioral) that is significantly different from the responses evoked by the modality-specific component stimuli</skos:definition>
        <dc:Title>Multisensory integration</dc:Title>
    </owl:Class>
    


    <!-- http://www.cognitiveatlas.org/ontology/cogat.owl#CAO_00695 -->

    <owl:Class rdf:about="&cogat;CAO_00695">
        <rdfs:label>Crossmodal</rdfs:label>
        <rdfs:subClassOf rdf:resource="&cogat;CAO_00001"/>
        <dc:Title>Crossmodal</dc:Title>
        <dc:Contributor>Scott Love</dc:Contributor>
        <dc:identifier>trm_4e31d2241319f</dc:identifier>
        <skos:altLabel>cross-modal</skos:altLabel>
        <skos:prefLabel>Crossmodal</skos:prefLabel>
        <skos:hasTopConcept></skos:hasTopConcept>
        <skos:definition>Describes a complex of two or more modality-specific [unimodal] stimuli from different sensory modalities (from, Stein BE et al., (2009) Experimental brain research 198: 113-26. doi:10.1007-s00221-009-1880-8)</skos:definition>
        <dc:Date>2011-08-04 21:26:13</dc:Date>
    </owl:Class>
    


    <!-- http://www.cognitiveatlas.org/ontology/cogat.owl#CAO_00696 -->

    <owl:Class rdf:about="&cogat;CAO_00696">
        <rdfs:label>Unisensory</rdfs:label>
        <rdfs:subClassOf rdf:resource="&cogat;CAO_00001"/>
        <dc:Date>2012-03-28 18:57:06</dc:Date>
        <dc:Contributor>Russ Poldrack</dc:Contributor>
        <dc:Title>Unisensory</dc:Title>
        <skos:prefLabel>Unisensory</skos:prefLabel>
        <dc:identifier>trm_4e31d365bc7e2</dc:identifier>
        <skos:definition>Describes any sensory process associated with a single sensory modality </skos:definition>
        <skos:hasTopConcept>Perception</skos:hasTopConcept>
        <skos:altLabel></skos:altLabel>
    </owl:Class>
    


    <!-- http://www.cognitiveatlas.org/ontology/cogat.owl#CAO_00697 -->

    <owl:Class rdf:about="&cogat;CAO_00697">
        <rdfs:label>Multisensory</rdfs:label>
        <rdfs:subClassOf rdf:resource="&cogat;CAO_00001"/>
        <skos:hasTopConcept>Perception</skos:hasTopConcept>
        <skos:prefLabel>Multisensory</skos:prefLabel>
        <dc:Title>Multisensory</dc:Title>
        <dc:identifier>trm_4e31d3ba7d25b</dc:identifier>
        <skos:altLabel></skos:altLabel>
        <dc:Date>2012-03-28 17:43:06</dc:Date>
        <skos:definition>a process associated with multiple sensory modalities </skos:definition>
        <dc:Contributor>Russ Poldrack</dc:Contributor>
    </owl:Class>
    


    <!-- http://www.cognitiveatlas.org/ontology/cogat.owl#CAO_00700 -->

    <owl:Class rdf:about="&cogat;CAO_00700">
        <rdfs:label>Synchrony perception</rdfs:label>
        <rdfs:subClassOf rdf:resource="&cogat;CAO_00437"/>
        <skos:hasTopConcept>Perception</skos:hasTopConcept>
        <dc:Contributor>Russ Poldrack</dc:Contributor>
        <skos:prefLabel>Synchrony perception</skos:prefLabel>
        <skos:definition>the process of perceiving whether or not the crossmodal cues (e.g., audio and visual) to an event (e.g., audiovisual speech) are in temporal synchrony with each other.</skos:definition>
        <dc:identifier>trm_4e31e6dca01ca</dc:identifier>
        <dc:Title>Synchrony perception</dc:Title>
        <dc:Date>2012-03-28 18:49:30</dc:Date>
        <skos:altLabel></skos:altLabel>
    </owl:Class>
    


    <!-- http://www.cognitiveatlas.org/ontology/cogat.owl#CAO_00701 -->

    <owl:Class rdf:about="&cogat;CAO_00701">
        <rdfs:label>Tactile working memory</rdfs:label>
        <rdfs:subClassOf rdf:resource="&cogat;CAO_00587"/>
        <dc:identifier>trm_4e416f1373936</dc:identifier>
        <dc:Title>Tactile working memory</dc:Title>
        <dc:Contributor>Mei-Yen Chen</dc:Contributor>
        <skos:definition>working memory for tactile information</skos:definition>
        <dc:Date>2011-08-12 13:08:59</dc:Date>
        <skos:hasTopConcept>Learning and Memory</skos:hasTopConcept>
        <skos:prefLabel>Tactile working memory</skos:prefLabel>
        <skos:altLabel></skos:altLabel>
    </owl:Class>
    


    <!-- http://www.cognitiveatlas.org/ontology/cogat.owl#CAO_00702 -->

    <owl:Class rdf:about="&cogat;CAO_00702">
        <rdfs:label>Interoceptive representation</rdfs:label>
        <rdfs:subClassOf rdf:resource="&cogat;CAO_00691"/>
        <dc:Title>Interoceptive representation</dc:Title>
        <dc:identifier>trm_4e5506161998c</dc:identifier>
        <skos:prefLabel>Interoceptive representation</skos:prefLabel>
        <skos:definition>A representation of the internal state of the body</skos:definition>
        <skos:altLabel></skos:altLabel>
        <dc:Contributor>Russ Poldrack</dc:Contributor>
        <dc:Date>2011-08-24 07:09:26</dc:Date>
        <skos:hasTopConcept></skos:hasTopConcept>
    </owl:Class>
    


    <!-- http://www.cognitiveatlas.org/ontology/cogat.owl#CAO_00703 -->

    <owl:Class rdf:about="&cogat;CAO_00703">
        <rdfs:label>Sense of ownership</rdfs:label>
        <rdfs:subClassOf rdf:resource="&cogat;CAO_00691"/>
        <skos:hasTopConcept></skos:hasTopConcept>
        <skos:prefLabel>Sense of ownership</skos:prefLabel>
        <dc:Contributor>Birgit Nierula</dc:Contributor>
        <dc:identifier>trm_4e5badf095692</dc:identifier>
        <skos:definition>The feeling that something is part of one self.</skos:definition>
        <skos:altLabel></skos:altLabel>
        <dc:Title>Sense of ownership</dc:Title>
        <dc:Date>2011-09-01 08:50:43</dc:Date>
    </owl:Class>
    


    <!-- http://www.ifomis.org/bfo/1.1/span#Process -->

    <owl:Class rdf:about="&span;Process"/>
    


    <!-- http://www.w3.org/2004/02/skos/core#Concept -->

    <owl:Class rdf:about="&skos;Concept"/>
</rdf:RDF>



<!-- Generated by the OWL API (version 3.2.3.1824) http://owlapi.sourceforge.net -->

